@prefix dct: <http://purl.org/dc/terms/> .
@prefix dpv: <https://w3id.org/dpv#> .
@prefix owl: <http://www.w3.org/2002/07/owl#> .
@prefix rdfs: <http://www.w3.org/2000/01/rdf-schema#> .
@prefix schema: <https://schema.org/> .
@prefix skos: <http://www.w3.org/2004/02/skos/core#> .
@prefix sw: <http://www.w3.org/2003/06/sw-vocab-status/ns#> .
@prefix tech: <https://w3id.org/dpv/tech#> .
@prefix vann: <http://purl.org/vocab/vann/> .
@prefix xsd: <http://www.w3.org/2001/XMLSchema#> .

tech:Application a rdfs:Class,
        owl:Class,
        dpv:Technology ;
    dct:contributor "Harshvardhan J. Pandit" ;
    dct:created "2022-06-15"^^xsd:date ;
    rdfs:isDefinedBy tech: ;
    rdfs:subClassOf tech:OperationalTechnology ;
    sw:term_status "accepted"@en ;
    skos:definition "A computing or digital program"@en ;
    skos:prefLabel "Application"@en .

tech:OperationDevice a rdfs:Class,
        owl:Class,
        dpv:Technology ;
    dct:contributor "Harshvardhan J. Pandit" ;
    dct:created "2022-06-15"^^xsd:date ;
    rdfs:isDefinedBy tech: ;
    rdfs:subClassOf tech:OperationalTechnology ;
    sw:term_status "accepted"@en ;
    skos:definition "Technology that acts as an equipment or mechanism for operations"@en ;
    skos:prefLabel "Operation Device"@en .

tech:OperationEnvironment a rdfs:Class,
        owl:Class,
        dpv:Technology ;
    dct:contributor "Harshvardhan J. Pandit" ;
    dct:created "2022-06-15"^^xsd:date ;
    rdfs:isDefinedBy tech: ;
    rdfs:subClassOf tech:OperationalTechnology ;
    sw:term_status "accepted"@en ;
    skos:definition "Technology that provides an environment for operations to be executed"@en ;
    skos:prefLabel "Operation Environment"@en .

tech:OperationManagement a rdfs:Class,
        owl:Class,
        dpv:Technology ;
    dct:contributor "Harshvardhan J. Pandit" ;
    dct:created "2022-06-15"^^xsd:date ;
    rdfs:isDefinedBy tech: ;
    rdfs:subClassOf tech:OperationalTechnology ;
    sw:term_status "accepted"@en ;
    skos:definition "Technology that manages operations"@en ;
    skos:prefLabel "Operation Management"@en .

<https://w3id.org/dpv/tech> a owl:Ontology ;
    dct:conformsTo <http://www.w3.org/2002/07/owl>,
        "http://www.w3.org/2000/01/rdf-schema",
        "http://www.w3.org/2004/02/skos/core" ;
    dct:contributor "Harshvardhan J. Pandit" ;
    dct:created "2022-06-15"@en ;
    dct:creator "Georg P Krog"@en,
        "Harshvardhan J. Pandit"@en,
        "Julian Flake"@en,
        "Paul Ryan"@en ;
    dct:description "Extension to the Data Privacy Vocabulary (DPV) providing concepts for representing information about technologies and its provision"@en ;
    dct:hasVersion <https://w3id.org/dpv/tech> ;
    dct:identifier "https://w3id.org/dpv/tech" ;
    dct:license <https://www.w3.org/copyright/document-license-2023/> ;
    dct:modified "2024-01-01"@en ;
    dct:title "Technology Concepts"@en ;
    vann:preferredNamespacePrefix "tech" ;
    vann:preferredNamespaceUri "https://w3id.org/dpv/tech#" ;
    schema:version "0.8.2" .

tech:OperationalTechnology rdfs:superClassOf tech:Application,
        tech:OperationDevice,
        tech:OperationEnvironment,
        tech:OperationManagement .

