@prefix dct: <http://purl.org/dc/terms/> .
@prefix dpv: <https://w3id.org/dpv#> .
@prefix owl: <http://www.w3.org/2002/07/owl#> .
@prefix rdf: <http://www.w3.org/1999/02/22-rdf-syntax-ns#> .
@prefix rdfs: <http://www.w3.org/2000/01/rdf-schema#> .
@prefix risk: <https://w3id.org/dpv/risk#> .
@prefix schema: <https://schema.org/> .
@prefix skos: <http://www.w3.org/2004/02/skos/core#> .
@prefix sw: <http://www.w3.org/2003/06/sw-vocab-status/ns#> .
@prefix vann: <http://purl.org/vocab/vann/> .
@prefix xsd: <http://www.w3.org/2001/XMLSchema#> .

risk:3LikelihoodLevels a rdfs:Class,
        skos:Concept,
        dpv:Likelihood ;
    dct:contributor "Harshvardhan J. Pandit" ;
    dct:created "2022-08-18"^^xsd:date ;
    rdfs:isDefinedBy risk: ;
    sw:term_status "accepted"@en ;
    skos:broader dpv:Likelihood ;
    skos:definition "Scale with 3 Likelihood Levels from High to Low"@en ;
    skos:inScheme risk:risk-levels-classes ;
    skos:narrower risk:HighLikelihood,
        risk:LowLikelihood,
        risk:ModerateLikelihood ;
    skos:prefLabel "3 Likelihood Levels"@en .

risk:3RiskLevels a rdfs:Class,
        skos:Concept,
        dpv:RiskLevel ;
    dct:contributor "Harshvardhan J. Pandit" ;
    dct:created "2022-08-18"^^xsd:date ;
    rdfs:isDefinedBy risk: ;
    sw:term_status "accepted"@en ;
    skos:broader dpv:RiskLevel ;
    skos:definition "Scale with 3 Risk Levels from High to Low"@en ;
    skos:inScheme risk:risk-levels-classes ;
    skos:narrower risk:HighRisk,
        risk:LowRisk,
        risk:ModerateRisk ;
    skos:prefLabel "3 Risk Levels"@en .

risk:3SeverityLevels a rdfs:Class,
        skos:Concept,
        dpv:Severity ;
    dct:contributor "Harshvardhan J. Pandit" ;
    dct:created "2022-08-18"^^xsd:date ;
    rdfs:isDefinedBy risk: ;
    sw:term_status "accepted"@en ;
    skos:broader dpv:Severity ;
    skos:definition "Scale with 3 Severity Levels from High to Low"@en ;
    skos:inScheme risk:risk-levels-classes ;
    skos:narrower risk:HighSeverity,
        risk:LowSeverity,
        risk:ModerateSeverity ;
    skos:prefLabel "3 Severity Levels"@en .

risk:5LikelihoodLevels a rdfs:Class,
        skos:Concept,
        dpv:Likelihood ;
    dct:contributor "Harshvardhan J. Pandit" ;
    dct:created "2022-08-18"^^xsd:date ;
    rdfs:isDefinedBy risk: ;
    sw:term_status "accepted"@en ;
    skos:broader dpv:Likelihood ;
    skos:definition "Scale with 5 Likelihood Levels from Very High to Very Low"@en ;
    skos:inScheme risk:risk-levels-classes ;
    skos:narrower risk:HighLikelihood,
        risk:LowLikelihood,
        risk:ModerateLikelihood,
        risk:VeryHighLikelihood,
        risk:VeryLowLikelihood ;
    skos:prefLabel "5 Likelihood Levels"@en .

risk:5RiskLevels a rdfs:Class,
        skos:Concept,
        dpv:RiskLevel ;
    dct:contributor "Harshvardhan J. Pandit" ;
    dct:created "2022-08-18"^^xsd:date ;
    rdfs:isDefinedBy risk: ;
    sw:term_status "accepted"@en ;
    skos:broader dpv:RiskLevel ;
    skos:definition "Scale with 5 Risk Levels from Very High to Very Low"@en ;
    skos:inScheme risk:risk-levels-classes ;
    skos:narrower risk:HighRisk,
        risk:LowRisk,
        risk:ModerateRisk,
        risk:VeryHighRisk,
        risk:VeryLowRisk ;
    skos:prefLabel "5 Risk Levels"@en .

risk:5SeverityLevels a rdfs:Class,
        skos:Concept,
        dpv:Severity ;
    dct:contributor "Harshvardhan J. Pandit" ;
    dct:created "2022-08-18"^^xsd:date ;
    rdfs:isDefinedBy risk: ;
    sw:term_status "accepted"@en ;
    skos:broader dpv:Severity ;
    skos:definition "Scale with 5 Severity Levels from Very High to Very Low"@en ;
    skos:inScheme risk:risk-levels-classes ;
    skos:narrower risk:HighSeverity,
        risk:LowSeverity,
        risk:ModerateSeverity,
        risk:VeryHighSeverity,
        risk:VeryLowSeverity ;
    skos:prefLabel "5 Severity Levels"@en .

risk:7LikelihoodLevels a rdfs:Class,
        skos:Concept,
        dpv:Likelihood ;
    dct:contributor "Harshvardhan J. Pandit" ;
    dct:created "2022-08-18"^^xsd:date ;
    rdfs:isDefinedBy risk: ;
    sw:term_status "accepted"@en ;
    skos:broader dpv:Likelihood ;
    skos:definition "Scale with 7 Likelihood Levels from Extremely High to Extremely Low"@en ;
    skos:inScheme risk:risk-levels-classes ;
    skos:narrower risk:ExtremelyHighLikelihood,
        risk:ExtremelyLowLikelihood,
        risk:HighLikelihood,
        risk:LowLikelihood,
        risk:ModerateLikelihood,
        risk:VeryHighLikelihood,
        risk:VeryLowLikelihood ;
    skos:prefLabel "7 Likelihood Levels"@en .

risk:7RiskLevels a rdfs:Class,
        skos:Concept,
        dpv:RiskLevel ;
    dct:contributor "Harshvardhan J. Pandit" ;
    dct:created "2022-08-18"^^xsd:date ;
    rdfs:isDefinedBy risk: ;
    sw:term_status "accepted"@en ;
    skos:broader dpv:RiskLevel ;
    skos:definition "Scale with 7 Risk Levels from Extremely High to Extremely Low"@en ;
    skos:inScheme risk:risk-levels-classes ;
    skos:narrower risk:ExtremelyHighRisk,
        risk:ExtremelyLowRisk,
        risk:HighRisk,
        risk:LowRisk,
        risk:ModerateRisk,
        risk:VeryHighRisk,
        risk:VeryLowRisk ;
    skos:prefLabel "7 Risk Levels"@en .

risk:7SeverityLevels a rdfs:Class,
        skos:Concept,
        dpv:Severity ;
    dct:contributor "Harshvardhan J. Pandit" ;
    dct:created "2022-08-18"^^xsd:date ;
    rdfs:isDefinedBy risk: ;
    sw:term_status "accepted"@en ;
    skos:broader dpv:Severity ;
    skos:definition "Scale with 7 Severity Levels from Extremely High to Extremely Low"@en ;
    skos:inScheme risk:risk-levels-classes ;
    skos:narrower risk:ExtremelyHighSeverity,
        risk:ExtremelyLowSeverity,
        risk:HighSeverity,
        risk:LowSeverity,
        risk:ModerateSeverity,
        risk:VeryHighSeverity,
        risk:VeryLowSeverity ;
    skos:prefLabel "7 Severity Levels"@en .

risk:ACSC-ISM a rdfs:Class,
        skos:Concept,
        risk:RiskManagement ;
    dct:contributor "Harshvardhan J. Pandit" ;
    dct:created "2022-08-18"^^xsd:date ;
    dct:source "(ENISA Compendium of Risk Management Frameworks with Potential Interoperability,https://www.enisa.europa.eu/publications/compendium-of-risk-management-frameworks)"@en ;
    rdfs:isDefinedBy risk: ;
    sw:term_status "accepted"@en ;
    skos:broader risk:RiskManagement ;
    skos:definition "The Australian Cyber Security Centre (ACSC) published the Australian Government Information Security Manual (ISM) which adopts the use of a risk management framework that draws from NIST 800-37, and includes six steps: define the system, select security controls, implement security controls, assess security controls, authorise the system and monitor the system"@en ;
    skos:inScheme risk:risk-methodology-classes ;
    skos:prefLabel "ACSC-ISM"@en .

risk:ALARA a rdfs:Class,
        skos:Concept,
        risk:RiskAnalysis ;
    dct:contributor "Harshvardhan J. Pandit" ;
    dct:created "2022-08-18"^^xsd:date ;
    dct:source "(IEC 31010:2019,https://www.iso.org/standard/72140.html)"@en ;
    rdfs:isDefinedBy risk: ;
    sw:term_status "accepted"@en ;
    skos:broader risk:QualitativeRiskAnalysis,
        risk:QuantitativeRiskAnalysis ;
    skos:definition "As Low as Resonably Achievable (ALARP) - A criteria for deciding significance of risk and means of evaluating tolerability of risk"@en ;
    skos:inScheme risk:risk-assessment-classes ;
    skos:prefLabel "ALARA"@en .

risk:ALARP a rdfs:Class,
        skos:Concept,
        risk:RiskAnalysis ;
    dct:contributor "Harshvardhan J. Pandit" ;
    dct:created "2022-08-18"^^xsd:date ;
    dct:source "(IEC 31010:2019,https://www.iso.org/standard/72140.html)"@en ;
    rdfs:isDefinedBy risk: ;
    sw:term_status "accepted"@en ;
    skos:broader risk:QualitativeRiskAnalysis,
        risk:QuantitativeRiskAnalysis ;
    skos:definition "As Low as Resonably Possible (ALARP) - A criteria for deciding significance of risk and means of evaluating tolerability of risk"@en ;
    skos:inScheme risk:risk-assessment-classes ;
    skos:prefLabel "ALARP"@en .

risk:ANSI-ISA-62443-3-2-2020 a rdfs:Class,
        skos:Concept,
        risk:RiskManagement ;
    dct:contributor "Harshvardhan J. Pandit" ;
    dct:created "2022-08-18"^^xsd:date ;
    dct:source "(ENISA Compendium of Risk Management Frameworks with Potential Interoperability,https://www.enisa.europa.eu/publications/compendium-of-risk-management-frameworks)"@en ;
    rdfs:isDefinedBy risk: ;
    sw:term_status "accepted"@en ;
    skos:broader risk:RiskManagement ;
    skos:definition "ANSI/ISA-62443-3-2-2020 standard, entitled ‘Security for industrial automation and control systems, Part 3-2: Security risk assessment for system design’, from the International Society of Automation (ISA), dedicates an entire part to the assessment of security risk for system design targeting Security and IT professionals"@en ;
    skos:inScheme risk:risk-methodology-classes ;
    skos:prefLabel "ANSI/ISA-62443-3‑2-2020"@en .

risk:AbusiveContentUtilisation a rdfs:Class,
        skos:Concept,
        dpv:Impact ;
    dct:contributor "Harshvardhan J. Pandit" ;
    dct:created "2022-08-17"^^xsd:date ;
    dct:source "(ENISA Reference Incident Classification Taxonomy 2018,https://www.enisa.europa.eu/publications/reference-incident-classification-taxonomy/)"@en ;
    rdfs:isDefinedBy risk: ;
    sw:term_status "accepted"@en ;
    skos:broader dpv:Harm ;
    skos:inScheme risk:risk-consequences-classes ;
    skos:prefLabel "Abusive Content Utilisation"@en .

risk:AttackonPrivateLife a rdfs:Class,
        skos:Concept,
        dpv:Impact ;
    dct:contributor "Harshvardhan J. Pandit" ;
    dct:created "2022-08-17"^^xsd:date ;
    dct:source "(ISO/IEC 27005:2018,https://www.iso.org/standard/75281.html)"@en ;
    rdfs:isDefinedBy risk: ;
    sw:term_status "accepted"@en ;
    skos:broader dpv:Harm ;
    skos:inScheme risk:risk-consequences-classes ;
    skos:prefLabel "Attack on Private Life"@en .

risk:AuthorisationFailure a rdfs:Class,
        skos:Concept,
        dpv:Consequence ;
    dct:contributor "Harshvardhan J. Pandit" ;
    dct:created "2022-08-17"^^xsd:date ;
    dct:source "(ENISa Trust Services Security Incidents 2021,https://www.enisa.europa.eu/publications/trust-services-security-incidents-2021)"@en ;
    rdfs:isDefinedBy risk: ;
    sw:term_status "accepted"@en ;
    skos:broader dpv:Detriment ;
    skos:inScheme risk:risk-consequences-classes ;
    skos:prefLabel "Authorisation Failure"@en .

risk:AvoidSource a rdfs:Class,
        skos:Concept,
        dpv:RiskMitigationMeasure ;
    dct:contributor "Harshvardhan J. Pandit" ;
    dct:created "2022-08-21"^^xsd:date ;
    rdfs:isDefinedBy risk: ;
    sw:term_status "accepted"@en ;
    skos:broader risk:ControlRiskSource ;
    skos:definition "Risk Control that avoids the risk source"@en ;
    skos:inScheme risk:risk-controls-classes ;
    skos:prefLabel "Avoid Source"@en .

risk:BSI-200-2 a rdfs:Class,
        skos:Concept,
        risk:RiskManagement ;
    dct:contributor "Harshvardhan J. Pandit" ;
    dct:created "2022-08-18"^^xsd:date ;
    dct:source "(ENISA Compendium of Risk Management Frameworks with Potential Interoperability,https://www.enisa.europa.eu/publications/compendium-of-risk-management-frameworks)"@en ;
    rdfs:isDefinedBy risk: ;
    sw:term_status "accepted"@en ;
    skos:broader risk:RiskManagement ;
    skos:definition "The BSI-Standard 200-2 (‘IT-Grundschutz Methodology’) provides a methodology for the management of information security which can be adapted to the requirements of organisations of various types and sizes"@en ;
    skos:inScheme risk:risk-methodology-classes ;
    skos:prefLabel "BSI Standard 200-2"@en .

risk:BayesianAnalysis a rdfs:Class,
        skos:Concept,
        risk:RiskAnalysis ;
    dct:contributor "Harshvardhan J. Pandit" ;
    dct:created "2022-08-18"^^xsd:date ;
    dct:source "(IEC 31010:2019,https://www.iso.org/standard/72140.html)"@en ;
    rdfs:isDefinedBy risk: ;
    sw:term_status "accepted"@en ;
    skos:broader risk:QuantitativeRiskAnalysis ;
    skos:definition "A means of making inference about model parameters using Bayes' theorem which has the capability of incorporating empirical data into prior judgements about probabilities"@en ;
    skos:inScheme risk:risk-assessment-classes ;
    skos:prefLabel "Bayesian Analysis"@en .

risk:BayesianNetworks a rdfs:Class,
        skos:Concept,
        risk:RiskAnalysis ;
    dct:contributor "Harshvardhan J. Pandit" ;
    dct:created "2022-08-18"^^xsd:date ;
    dct:source "(IEC 31010:2019,https://www.iso.org/standard/72140.html)"@en ;
    rdfs:isDefinedBy risk: ;
    sw:term_status "accepted"@en ;
    skos:broader risk:QuantitativeRiskAnalysis ;
    skos:definition "A graphical model of variables and their cause-effect relationships expressed using probabilities"@en ;
    skos:inScheme risk:risk-assessment-classes ;
    skos:prefLabel "Bayesian Networks"@en .

risk:Blackmail a rdfs:Class,
        skos:Concept,
        dpv:Impact ;
    dct:contributor "Harshvardhan J. Pandit" ;
    dct:created "2022-08-17"^^xsd:date ;
    dct:source "(ISO/IEC 27005:2018,https://www.iso.org/standard/75281.html)"@en ;
    rdfs:isDefinedBy risk: ;
    sw:term_status "accepted"@en ;
    skos:broader dpv:Harm ;
    skos:inScheme risk:risk-consequences-classes ;
    skos:prefLabel "Blackmail"@en .

risk:BowTie a rdfs:Class,
        skos:Concept,
        risk:RiskAnalysis ;
    dct:contributor "Harshvardhan J. Pandit" ;
    dct:created "2022-08-18"^^xsd:date ;
    dct:source "(IEC 31010:2019,https://www.iso.org/standard/72140.html)"@en ;
    rdfs:isDefinedBy risk: ;
    sw:term_status "accepted"@en ;
    skos:broader risk:QualitativeRiskAnalysis,
        risk:QuantitativeRiskAnalysis ;
    skos:definition "A diagrammatic way of describing the pathways from sources of risk to outcomes, and of reviewing controls"@en ;
    skos:inScheme risk:risk-assessment-classes ;
    skos:prefLabel "Bow Tie Analysis"@en .

risk:Brainstorming a rdfs:Class,
        skos:Concept,
        risk:RiskAnalysis ;
    dct:contributor "Harshvardhan J. Pandit" ;
    dct:created "2022-08-18"^^xsd:date ;
    dct:source "(IEC 31010:2019,https://www.iso.org/standard/72140.html)"@en ;
    rdfs:isDefinedBy risk: ;
    sw:term_status "accepted"@en ;
    skos:broader risk:QualitativeRiskAnalysis ;
    skos:definition "Technique used in workshops to encourage imaginative thinking"@en ;
    skos:inScheme risk:risk-assessment-classes ;
    skos:prefLabel "Brainstorming"@en .

risk:BruteForceAuthorisations a rdfs:Class,
        skos:Concept,
        dpv:Consequence ;
    dct:contributor "Harshvardhan J. Pandit" ;
    dct:created "2022-08-17"^^xsd:date ;
    dct:source "(ENISA Reference Incident Classification Taxonomy 2018,https://www.enisa.europa.eu/publications/reference-incident-classification-taxonomy/)"@en ;
    rdfs:isDefinedBy risk: ;
    sw:term_status "accepted"@en ;
    skos:broader dpv:Detriment ;
    skos:inScheme risk:risk-consequences-classes ;
    skos:prefLabel "Brute Force Authorisations"@en .

risk:BusinessImpact a rdfs:Class,
        skos:Concept,
        dpv:Impact ;
    dct:contributor "Harshvardhan J. Pandit" ;
    dct:created "2022-08-17"^^xsd:date ;
    dct:source "(ENISA Methodology for Sectoral Cybersecurity Assessments,https://www.enisa.europa.eu/publications/methodology-for-a-sectoral-cybersecurity-assessment)"@en ;
    rdfs:isDefinedBy risk: ;
    sw:term_status "accepted"@en ;
    skos:broader dpv:Impact ;
    skos:inScheme risk:risk-consequences-classes ;
    skos:prefLabel "Business impact"@en .

risk:BusinessImpactAnalysis a rdfs:Class,
        skos:Concept,
        risk:RiskAnalysis ;
    dct:contributor "Harshvardhan J. Pandit" ;
    dct:created "2022-08-18"^^xsd:date ;
    dct:source "(IEC 31010:2019,https://www.iso.org/standard/72140.html)"@en ;
    rdfs:isDefinedBy risk: ;
    sw:term_status "accepted"@en ;
    skos:broader risk:QualitativeRiskAnalysis,
        risk:QuantitativeRiskAnalysis ;
    skos:definition "A process that analyses the consequences of a disruptive incident on the organization which determines the recovery priorities of an organization's products and services and, thereby, the priorities of the activities and resources which deliver them"@en ;
    skos:inScheme risk:risk-assessment-classes ;
    skos:prefLabel "Business Impact Analysis"@en .

risk:BusinessPerformanceImpairment a rdfs:Class,
        skos:Concept,
        dpv:Consequence ;
    dct:contributor "Harshvardhan J. Pandit" ;
    dct:created "2022-08-17"^^xsd:date ;
    dct:source "(ISO/IEC 27005:2018,https://www.iso.org/standard/75281.html)"@en ;
    rdfs:isDefinedBy risk: ;
    sw:term_status "accepted"@en ;
    skos:broader dpv:Detriment ;
    skos:inScheme risk:risk-consequences-classes ;
    skos:prefLabel "Business Performance Impairment"@en .

risk:Businessdisruption a rdfs:Class,
        skos:Concept,
        dpv:Consequence ;
    dct:contributor "Harshvardhan J. Pandit" ;
    dct:created "2022-08-17"^^xsd:date ;
    dct:source "(ISO/IEC 27005:2018,https://www.iso.org/standard/75281.html)"@en ;
    rdfs:isDefinedBy risk: ;
    sw:term_status "accepted"@en ;
    skos:broader dpv:Detriment ;
    skos:inScheme risk:risk-consequences-classes ;
    skos:prefLabel "Business disruption"@en .

risk:CCRACII a rdfs:Class,
        skos:Concept,
        risk:RiskManagement ;
    dct:contributor "Harshvardhan J. Pandit" ;
    dct:created "2022-08-18"^^xsd:date ;
    dct:source "(ENISA Compendium of Risk Management Frameworks with Potential Interoperability,https://www.enisa.europa.eu/publications/compendium-of-risk-management-frameworks)"@en ;
    rdfs:isDefinedBy risk: ;
    sw:term_status "accepted"@en ;
    skos:broader risk:RiskManagement ;
    skos:definition "The Guide to Conducting Cybersecurity Risk Assessment for Critical Information Infrastructure (CCRACII) defines commonly used terms such as threat event, vulnerability, likelihood, impact and risk, roles, and responsibilities, in addition to a range for risk levels, ranging from low to very high with different level of risk toleranc"@en ;
    skos:inScheme risk:risk-methodology-classes ;
    skos:prefLabel "CCRACII"@en .

risk:CORAS a rdfs:Class,
        skos:Concept,
        risk:RiskManagement ;
    dct:contributor "Harshvardhan J. Pandit" ;
    dct:created "2022-08-18"^^xsd:date ;
    dct:source "(ENISA Compendium of Risk Management Frameworks with Potential Interoperability,https://www.enisa.europa.eu/publications/compendium-of-risk-management-frameworks)"@en ;
    rdfs:isDefinedBy risk: ;
    sw:term_status "accepted"@en ;
    skos:broader risk:RiskManagement ;
    skos:definition "The CORAS method was developed and is supported by SourceForge. It is a method for conducting the analysis and management of security risk. It provides a customised language for modelling threats and risks as well as detailed guidelines explaining how the language should be used to capture and model relevant information during the various stages of the security analysis"@en ;
    skos:inScheme risk:risk-methodology-classes ;
    skos:prefLabel "CORAS"@en .

risk:CRAMM a rdfs:Class,
        skos:Concept,
        risk:RiskManagement ;
    dct:contributor "Harshvardhan J. Pandit" ;
    dct:created "2022-08-18"^^xsd:date ;
    dct:source "(ENISA Risk Management Standards,https://www.enisa.europa.eu/publications/risk-management-standards)"@en ;
    rdfs:isDefinedBy risk: ;
    sw:term_status "accepted"@en ;
    skos:broader risk:RiskManagement ;
    skos:definition "CCTA Risk Assessment and Management Methodology (CRAMM) is a method that an analyst or group of analysts may use to evaluate the security and risk level of an organisation by analysing and combining the diverse knowledge distributed in the local corporate environment"@en ;
    skos:inScheme risk:risk-methodology-classes ;
    skos:prefLabel "CRAMM"@en .

risk:CVaR a rdfs:Class,
        skos:Concept,
        risk:RiskAnalysis ;
    dct:contributor "Harshvardhan J. Pandit" ;
    dct:created "2022-08-18"^^xsd:date ;
    dct:source "(IEC 31010:2019,https://www.iso.org/standard/72140.html)"@en ;
    rdfs:isDefinedBy risk: ;
    sw:term_status "accepted"@en ;
    skos:broader risk:QuantitativeRiskAnalysis ;
    skos:definition "A measure of the expected loss from a financial portfolio in the worst a % of cases. Also called expected shortfall (ES)"@en ;
    skos:inScheme risk:risk-assessment-classes ;
    skos:prefLabel "Conditional Value at Risk (CVaR)"@en .

risk:CausalMapping a rdfs:Class,
        skos:Concept,
        risk:RiskAnalysis ;
    dct:contributor "Harshvardhan J. Pandit" ;
    dct:created "2022-08-18"^^xsd:date ;
    dct:source "(IEC 31010:2019,https://www.iso.org/standard/72140.html)"@en ;
    rdfs:isDefinedBy risk: ;
    sw:term_status "accepted"@en ;
    skos:broader risk:QualitativeRiskAnalysis ;
    skos:definition "A network diagram representing events, causes and effects and their relationships."@en ;
    skos:inScheme risk:risk-assessment-classes ;
    skos:prefLabel "Causal Mapping"@en .

risk:CauseConsequenceAnalysis a rdfs:Class,
        skos:Concept,
        risk:RiskAnalysis ;
    dct:contributor "Harshvardhan J. Pandit" ;
    dct:created "2022-08-18"^^xsd:date ;
    dct:source "(IEC 31010:2019,https://www.iso.org/standard/72140.html)"@en ;
    rdfs:isDefinedBy risk: ;
    sw:term_status "accepted"@en ;
    skos:broader risk:QuantitativeRiskAnalysis ;
    skos:definition "A combination of fault and event tree analysis that allows inclusion of time delays. Both causes and consequences of an initiating event are considered."@en ;
    skos:inScheme risk:risk-assessment-classes ;
    skos:prefLabel "Cause-Consequence Analysis"@en .

risk:ChangeConsequence a rdfs:Class,
        skos:Concept,
        dpv:RiskMitigationMeasure ;
    dct:contributor "Harshvardhan J. Pandit" ;
    dct:created "2022-08-25"^^xsd:date ;
    rdfs:isDefinedBy risk: ;
    sw:term_status "accepted"@en ;
    skos:broader risk:ControlConsequence ;
    skos:definition "Risk Control that changes Consequence"@en ;
    skos:inScheme risk:risk-controls-classes ;
    skos:prefLabel "Change Consequence"@en .

risk:ChangeImpact a rdfs:Class,
        skos:Concept,
        dpv:RiskMitigationMeasure ;
    dct:contributor "Harshvardhan J. Pandit" ;
    dct:created "2022-08-26"^^xsd:date ;
    dct:modified "2023-07-31"^^xsd:date ;
    rdfs:isDefinedBy risk: ;
    sw:term_status "accepted"@en ;
    skos:broader risk:ControlImpact ;
    skos:definition "Risk Control that changes Impact"@en ;
    skos:inScheme risk:risk-controls-classes ;
    skos:prefLabel "Change Impact"@en .

risk:Checklists a rdfs:Class,
        skos:Concept,
        risk:RiskAnalysis ;
    dct:contributor "Harshvardhan J. Pandit" ;
    dct:created "2022-08-18"^^xsd:date ;
    dct:source "(IEC 31010:2019,https://www.iso.org/standard/72140.html)"@en ;
    rdfs:isDefinedBy risk: ;
    sw:term_status "accepted"@en ;
    skos:broader risk:QualitativeRiskAnalysis ;
    skos:definition "A checklist based on experience or on concepts and models that can be used to help identify risks or controls."@en ;
    skos:inScheme risk:risk-assessment-classes ;
    skos:prefLabel "Checklists"@en .

risk:ChildViolence a rdfs:Class,
        skos:Concept,
        dpv:Impact ;
    dct:contributor "Harshvardhan J. Pandit" ;
    dct:created "2022-08-17"^^xsd:date ;
    dct:source "(ENISA Reference Incident Classification Taxonomy 2018,https://www.enisa.europa.eu/publications/reference-incident-classification-taxonomy/)"@en ;
    rdfs:isDefinedBy risk: ;
    sw:term_status "accepted"@en ;
    skos:broader dpv:Harm ;
    skos:inScheme risk:risk-consequences-classes ;
    skos:prefLabel "Child Violence"@en .

risk:Cindynic a rdfs:Class,
        skos:Concept,
        risk:RiskAnalysis ;
    dct:contributor "Harshvardhan J. Pandit" ;
    dct:created "2022-08-18"^^xsd:date ;
    dct:source "(IEC 31010:2019,https://www.iso.org/standard/72140.html)"@en ;
    rdfs:isDefinedBy risk: ;
    sw:term_status "accepted"@en ;
    skos:broader risk:QualitativeRiskAnalysis ;
    skos:definition "Considers goals, values, rules, data and models of stakeholders and identifies inconsistencies, ambiguities, omissions and ignorance. These form systemic sources and drivers of risk."@en ;
    skos:inScheme risk:risk-assessment-classes ;
    skos:prefLabel "Cindynic Approach"@en .

risk:CitizensImpact a rdfs:Class,
        skos:Concept,
        dpv:Impact ;
    dct:contributor "Harshvardhan J. Pandit" ;
    dct:created "2022-08-17"^^xsd:date ;
    dct:source "(ENISA Methodology for Sectoral Cybersecurity Assessments,https://www.enisa.europa.eu/publications/methodology-for-a-sectoral-cybersecurity-assessment)"@en ;
    rdfs:isDefinedBy risk: ;
    sw:term_status "accepted"@en ;
    skos:broader dpv:Impact ;
    skos:inScheme risk:risk-consequences-classes ;
    skos:prefLabel "Citizens impact"@en .

risk:Classifications a rdfs:Class,
        skos:Concept,
        risk:RiskAnalysis ;
    dct:contributor "Harshvardhan J. Pandit" ;
    dct:created "2022-08-18"^^xsd:date ;
    dct:source "(IEC 31010:2019,https://www.iso.org/standard/72140.html)"@en ;
    rdfs:isDefinedBy risk: ;
    sw:term_status "accepted"@en ;
    skos:broader risk:QualitativeRiskAnalysis ;
    skos:definition "A classification list based on experience or on concepts and models that can be used to help identify risks or controls."@en ;
    skos:inScheme risk:risk-assessment-classes ;
    skos:prefLabel "Classifications"@en .

risk:Coercion a rdfs:Class,
        skos:Concept,
        dpv:Impact ;
    dct:contributor "Harshvardhan J. Pandit" ;
    dct:created "2022-08-17"^^xsd:date ;
    dct:source "(ENISA Threat Taxonomy 2016,https://www.enisa.europa.eu/topics/threat-risk-management/threats-and-trends/enisa-threat-landscape/threat-taxonomy/view)"@en ;
    rdfs:isDefinedBy risk: ;
    sw:term_status "accepted"@en ;
    skos:broader dpv:Harm ;
    skos:inScheme risk:risk-consequences-classes ;
    skos:prefLabel "Coercion"@en .

risk:ComplianceImpact a rdfs:Class,
        skos:Concept,
        dpv:Impact ;
    dct:contributor "Harshvardhan J. Pandit" ;
    dct:created "2022-08-17"^^xsd:date ;
    dct:source "(ENISA Methodology for Sectoral Cybersecurity Assessments,https://www.enisa.europa.eu/publications/methodology-for-a-sectoral-cybersecurity-assessment)"@en ;
    rdfs:isDefinedBy risk: ;
    sw:term_status "accepted"@en ;
    skos:broader dpv:Impact ;
    skos:inScheme risk:risk-consequences-classes ;
    skos:prefLabel "Compliance impact"@en .

risk:CompromiseAccount a rdfs:Class,
        skos:Concept,
        dpv:Impact ;
    dct:contributor "Harshvardhan J. Pandit" ;
    dct:created "2022-08-17"^^xsd:date ;
    dct:source "(ENISA Reference Incident Classification Taxonomy 2018,https://www.enisa.europa.eu/publications/reference-incident-classification-taxonomy/)"@en ;
    rdfs:isDefinedBy risk: ;
    sw:term_status "accepted"@en ;
    skos:broader dpv:Harm ;
    skos:inScheme risk:risk-consequences-classes ;
    skos:prefLabel "Compromise Account"@en .

risk:CompromiseAccountCredentials a rdfs:Class,
        skos:Concept,
        dpv:Impact ;
    dct:contributor "Harshvardhan J. Pandit" ;
    dct:created "2022-08-17"^^xsd:date ;
    dct:source "(ENISA Reference Incident Classification Taxonomy 2018,https://www.enisa.europa.eu/publications/reference-incident-classification-taxonomy/)"@en ;
    rdfs:isDefinedBy risk: ;
    sw:term_status "accepted"@en ;
    skos:broader dpv:Harm ;
    skos:inScheme risk:risk-consequences-classes ;
    skos:prefLabel "Compromise Account Credentials"@en .

risk:CompromiseAccountSecurity a rdfs:Class,
        skos:Concept,
        dpv:Impact ;
    dct:contributor "Harshvardhan J. Pandit" ;
    dct:created "2022-08-17"^^xsd:date ;
    dct:source "(ENISA Reference Incident Classification Taxonomy 2018,https://www.enisa.europa.eu/publications/reference-incident-classification-taxonomy/)"@en ;
    rdfs:isDefinedBy risk: ;
    sw:term_status "accepted"@en ;
    skos:broader dpv:NonMaterialDamage ;
    skos:inScheme risk:risk-consequences-classes ;
    skos:prefLabel "Compromise Account Security"@en .

risk:ConfidentialityBreach a rdfs:Class,
        skos:Concept,
        dpv:Consequence ;
    dct:contributor "Harshvardhan J. Pandit" ;
    dct:created "2022-08-17"^^xsd:date ;
    dct:source "(ISO/IEC 27005:2018,https://www.iso.org/standard/75281.html)"@en ;
    rdfs:isDefinedBy risk: ;
    sw:term_status "accepted"@en ;
    skos:broader dpv:Detriment ;
    skos:inScheme risk:risk-consequences-classes ;
    skos:prefLabel "Confidentiality Breach"@en .

risk:ConsequenceForDataSubject a rdfs:Class,
        skos:Concept,
        dpv:Consequence ;
    dct:contributor "Harshvardhan J. Pandit, Georg P Krog" ;
    dct:created "2022-10-22"^^xsd:date ;
    rdfs:isDefinedBy risk: ;
    sw:term_status "accepted"@en ;
    skos:broader dpv:Consequence ;
    skos:inScheme risk:risk-consequences-classes ;
    skos:prefLabel "Consequence for Data Subject"@en .

risk:ConsequenceOnDataSecurity a rdfs:Class,
        skos:Concept,
        dpv:Consequence ;
    dct:contributor "Harshvardhan J. Pandit, Georg P Krog" ;
    dct:created "2022-10-22"^^xsd:date ;
    rdfs:isDefinedBy risk: ;
    sw:term_status "accepted"@en ;
    skos:broader dpv:Consequence ;
    skos:inScheme risk:risk-consequences-classes ;
    skos:prefLabel "Consequence on Data Security"@en .

risk:ControlConsequence a rdfs:Class,
        skos:Concept,
        dpv:RiskMitigationMeasure ;
    dct:contributor "Harshvardhan J. Pandit" ;
    dct:created "2022-08-24"^^xsd:date ;
    rdfs:isDefinedBy risk: ;
    sw:term_status "accepted"@en ;
    skos:broader dpv:RiskMitigationMeasure ;
    skos:definition "Risk Mitigation Measure that controls the Consequences"@en ;
    skos:inScheme risk:risk-controls-classes ;
    skos:narrower risk:ChangeConsequence,
        risk:ControlImpact,
        risk:RemoveConsequence ;
    skos:prefLabel "Control Consequence"@en .

risk:ControlImpact a rdfs:Class,
        skos:Concept,
        dpv:RiskMitigationMeasure ;
    dct:contributor "Harshvardhan J. Pandit" ;
    dct:created "2022-08-24"^^xsd:date ;
    dct:modified "2023-07-31"^^xsd:date ;
    rdfs:isDefinedBy risk: ;
    sw:term_status "accepted"@en ;
    skos:broader risk:ControlConsequence ;
    skos:definition "Risk Mitigation Measure that controls Impacts"@en ;
    skos:inScheme risk:risk-controls-classes ;
    skos:narrower risk:ChangeImpact,
        risk:RemoveImpact ;
    skos:prefLabel "Control Impact"@en .

risk:ControlMonitors a rdfs:Class,
        skos:Concept,
        dpv:RiskMitigationMeasure ;
    dct:contributor "Harshvardhan J. Pandit" ;
    dct:created "2022-08-30"^^xsd:date ;
    rdfs:isDefinedBy risk: ;
    sw:term_status "accepted"@en ;
    skos:broader dpv:RiskMitigationMeasure ;
    skos:definition "Risk Mitigation Measure that uses controls to monitor events"@en ;
    skos:inScheme risk:risk-controls-classes ;
    skos:narrower risk:MonitorConsequence,
        risk:MonitorImpact,
        risk:MonitorRisk,
        risk:MonitorRiskControl,
        risk:MonitorRiskSource,
        risk:MonitorVulnerabilities ;
    skos:prefLabel "Control Monitors"@en ;
    skos:scopeNote "Monitoring can be associated with characteristics such as assessing or detecting whether something is active, operational, performant, effective, has potential to materialise, is materialising, or has already materialised."@en .

risk:ControlRiskSource a rdfs:Class,
        skos:Concept,
        dpv:RiskMitigationMeasure ;
    dct:contributor "Harshvardhan J. Pandit" ;
    dct:created "2022-08-18"^^xsd:date ;
    rdfs:isDefinedBy risk: ;
    sw:term_status "accepted"@en ;
    skos:broader dpv:RiskMitigationMeasure ;
    skos:definition "Risk Mitigation Measure that controls the Risk Source"@en ;
    skos:inScheme risk:risk-controls-classes ;
    skos:narrower risk:AvoidSource,
        risk:HaltSource,
        risk:RemoveSource ;
    skos:prefLabel "Control Risk Source"@en .

risk:CopyrightViolation a rdfs:Class,
        skos:Concept,
        dpv:Impact ;
    dct:contributor "Harshvardhan J. Pandit" ;
    dct:created "2022-08-17"^^xsd:date ;
    dct:source "(ENISA Reference Incident Classification Taxonomy 2018,https://www.enisa.europa.eu/publications/reference-incident-classification-taxonomy/)"@en ;
    rdfs:isDefinedBy risk: ;
    sw:term_status "accepted"@en ;
    skos:broader dpv:NonMaterialDamage ;
    skos:inScheme risk:risk-consequences-classes ;
    skos:prefLabel "Copyright Violation"@en .

risk:CorruptionData a rdfs:Class,
        skos:Concept,
        dpv:Consequence ;
    dct:contributor "Harshvardhan J. Pandit" ;
    dct:created "2022-08-17"^^xsd:date ;
    dct:source "(ISO/IEC 27005:2018,https://www.iso.org/standard/75281.html)"@en ;
    rdfs:isDefinedBy risk: ;
    sw:term_status "accepted"@en ;
    skos:broader dpv:Damage ;
    skos:inScheme risk:risk-consequences-classes ;
    skos:prefLabel "Corruption of Data"@en .

risk:CostAcquisition a rdfs:Class,
        skos:Concept,
        dpv:Consequence ;
    dct:contributor "Harshvardhan J. Pandit" ;
    dct:created "2022-08-17"^^xsd:date ;
    dct:source "(ISO/IEC 27005:2018,https://www.iso.org/standard/75281.html)"@en ;
    rdfs:isDefinedBy risk: ;
    sw:term_status "accepted"@en ;
    skos:broader dpv:Detriment ;
    skos:inScheme risk:risk-consequences-classes ;
    skos:prefLabel "Cost of Acquisition"@en .

risk:CostBackup a rdfs:Class,
        skos:Concept,
        dpv:Consequence ;
    dct:contributor "Harshvardhan J. Pandit" ;
    dct:created "2022-08-17"^^xsd:date ;
    dct:source "(ISO/IEC 27005:2018,https://www.iso.org/standard/75281.html)"@en ;
    rdfs:isDefinedBy risk: ;
    sw:term_status "accepted"@en ;
    skos:broader dpv:Detriment ;
    skos:inScheme risk:risk-consequences-classes ;
    skos:prefLabel "Cost of Backup"@en .

risk:CostBenefitAnalysis a rdfs:Class,
        skos:Concept,
        risk:RiskAnalysis ;
    dct:contributor "Harshvardhan J. Pandit" ;
    dct:created "2022-08-18"^^xsd:date ;
    dct:source "(IEC 31010:2019,https://www.iso.org/standard/72140.html)"@en ;
    rdfs:isDefinedBy risk: ;
    sw:term_status "accepted"@en ;
    skos:broader risk:QuantitativeRiskAnalysis ;
    skos:definition "Uses money as a scale for estimating positive and negative, tangible and intangible, consequences of different options."@en ;
    skos:inScheme risk:risk-assessment-classes ;
    skos:prefLabel "Cost/benefit Analysis"@en .

risk:CostConfiguration a rdfs:Class,
        skos:Concept,
        dpv:Consequence ;
    dct:contributor "Harshvardhan J. Pandit" ;
    dct:created "2022-08-17"^^xsd:date ;
    dct:source "(ISO/IEC 27005:2018,https://www.iso.org/standard/75281.html)"@en ;
    rdfs:isDefinedBy risk: ;
    sw:term_status "accepted"@en ;
    skos:broader dpv:Detriment ;
    skos:inScheme risk:risk-consequences-classes ;
    skos:prefLabel "Cost of Configuration"@en .

risk:CostInstallation a rdfs:Class,
        skos:Concept,
        dpv:Consequence ;
    dct:contributor "Harshvardhan J. Pandit" ;
    dct:created "2022-08-17"^^xsd:date ;
    dct:source "(ISO/IEC 27005:2018,https://www.iso.org/standard/75281.html)"@en ;
    rdfs:isDefinedBy risk: ;
    sw:term_status "accepted"@en ;
    skos:broader dpv:Detriment ;
    skos:inScheme risk:risk-consequences-classes ;
    skos:prefLabel "Cost of Installation"@en .

risk:CostJudicialPenalties a rdfs:Class,
        skos:Concept,
        dpv:Consequence ;
    dct:contributor "Harshvardhan J. Pandit" ;
    dct:created "2022-08-17"^^xsd:date ;
    dct:source "(ISO/IEC 27005:2018,https://www.iso.org/standard/75281.html)"@en ;
    rdfs:isDefinedBy risk: ;
    sw:term_status "accepted"@en ;
    skos:broader dpv:Detriment ;
    skos:inScheme risk:risk-consequences-classes ;
    skos:prefLabel "Cost of Judicial Penalties"@en .

risk:CostJudicialProceedings a rdfs:Class,
        skos:Concept,
        dpv:Consequence ;
    dct:contributor "Harshvardhan J. Pandit" ;
    dct:created "2022-08-17"^^xsd:date ;
    dct:source "(ISO/IEC 27005:2018,https://www.iso.org/standard/75281.html)"@en ;
    rdfs:isDefinedBy risk: ;
    sw:term_status "accepted"@en ;
    skos:broader dpv:Detriment ;
    skos:inScheme risk:risk-consequences-classes ;
    skos:prefLabel "Cost of Judicial Proceedings"@en .

risk:CostOperationInterruption a rdfs:Class,
        skos:Concept,
        dpv:Consequence ;
    dct:contributor "Harshvardhan J. Pandit" ;
    dct:created "2022-08-17"^^xsd:date ;
    dct:source "(ISO/IEC 27005:2018,https://www.iso.org/standard/75281.html)"@en ;
    rdfs:isDefinedBy risk: ;
    sw:term_status "accepted"@en ;
    skos:broader dpv:Detriment ;
    skos:inScheme risk:risk-consequences-classes ;
    skos:prefLabel "Cost of Operation Interruption"@en .

risk:CostSuspendedOperations a rdfs:Class,
        skos:Concept,
        dpv:Consequence ;
    dct:contributor "Harshvardhan J. Pandit" ;
    dct:created "2022-08-17"^^xsd:date ;
    dct:source "(ISO/IEC 27005:2018,https://www.iso.org/standard/75281.html)"@en ;
    rdfs:isDefinedBy risk: ;
    sw:term_status "accepted"@en ;
    skos:broader dpv:Detriment ;
    skos:inScheme risk:risk-consequences-classes ;
    skos:prefLabel "Cost of Suspended Operations"@en .

risk:CrossImpactAnalysis a rdfs:Class,
        skos:Concept,
        risk:RiskAnalysis ;
    dct:contributor "Harshvardhan J. Pandit" ;
    dct:created "2022-08-18"^^xsd:date ;
    dct:source "(IEC 31010:2019,https://www.iso.org/standard/72140.html)"@en ;
    rdfs:isDefinedBy risk: ;
    sw:term_status "accepted"@en ;
    skos:broader risk:QuantitativeRiskAnalysis ;
    skos:definition "Evaluates changes in the probability of the occurrence of a given set of events consequent on the actual occurrence of one of them."@en ;
    skos:inScheme risk:risk-assessment-classes ;
    skos:prefLabel "Cross Impact Analysis"@en .

risk:Cryptojacking a rdfs:Class,
        skos:Concept,
        dpv:Consequence ;
    dct:contributor "Harshvardhan J. Pandit" ;
    dct:created "2022-08-17"^^xsd:date ;
    dct:source "(ENISA Threat Landscape 2021,https://www.enisa.europa.eu/publications/enisa-threat-landscape-2021)"@en ;
    rdfs:isDefinedBy risk: ;
    sw:term_status "accepted"@en ;
    skos:broader dpv:Detriment ;
    skos:definition "Cryptojacking or hidden cryptomining is a type of cybercrime where a criminal secretly uses a victim’s computing power to generate cryptocurrency"@en ;
    skos:inScheme risk:risk-consequences-classes ;
    skos:prefLabel "Cryptojacking"@en .

risk:CyberSpying a rdfs:Class,
        skos:Concept,
        dpv:Impact ;
    dct:contributor "Harshvardhan J. Pandit" ;
    dct:created "2022-08-17"^^xsd:date ;
    dct:source "(ISO/IEC 27005:2018,https://www.iso.org/standard/75281.html)"@en ;
    rdfs:isDefinedBy risk: ;
    sw:term_status "accepted"@en ;
    skos:broader dpv:NonMaterialDamage ;
    skos:inScheme risk:risk-consequences-classes ;
    skos:prefLabel "Cyber Spying"@en .

risk:CyberStalking a rdfs:Class,
        skos:Concept,
        dpv:Impact ;
    dct:contributor "Harshvardhan J. Pandit" ;
    dct:created "2022-08-17"^^xsd:date ;
    dct:source "(ISO/IEC 27005:2018,https://www.iso.org/standard/75281.html)"@en ;
    rdfs:isDefinedBy risk: ;
    sw:term_status "accepted"@en ;
    skos:broader dpv:NonMaterialDamage ;
    skos:inScheme risk:risk-consequences-classes ;
    skos:prefLabel "Cyber Stalking"@en .

risk:DPIA a rdfs:Class,
        skos:Concept,
        risk:RiskAnalysis ;
    dct:contributor "Harshvardhan J. Pandit" ;
    dct:created "2022-08-18"^^xsd:date ;
    dct:source "(IEC 31010:2019,https://www.iso.org/standard/72140.html)"@en ;
    rdfs:isDefinedBy risk: ;
    sw:term_status "accepted"@en ;
    skos:broader risk:QualitativeRiskAnalysis ;
    skos:definition "Analyses how incidents and events could affect the protection of data and its effects on persons and identifies and quantifies the capabilities that would be needed to manage it."@en ;
    skos:inScheme risk:risk-assessment-classes ;
    skos:prefLabel "Data Protection Impact Assessment (DPIA)"@en .

risk:DamageByThirdParty a rdfs:Class,
        skos:Concept,
        dpv:Consequence ;
    dct:contributor "Harshvardhan J. Pandit" ;
    dct:created "2022-08-17"^^xsd:date ;
    dct:source "(ENISA Threat Taxonomy 2016,https://www.enisa.europa.eu/topics/threat-risk-management/threats-and-trends/enisa-threat-landscape/threat-taxonomy/view)"@en ;
    rdfs:isDefinedBy risk: ;
    sw:term_status "accepted"@en ;
    skos:broader dpv:Damage ;
    skos:inScheme risk:risk-consequences-classes ;
    skos:prefLabel "Damage by Third Party"@en .

risk:DangertoCustomers a rdfs:Class,
        skos:Concept,
        dpv:Impact ;
    dct:contributor "Harshvardhan J. Pandit" ;
    dct:created "2022-08-17"^^xsd:date ;
    dct:source "(ISO/IEC 27005:2018,https://www.iso.org/standard/75281.html)"@en ;
    rdfs:isDefinedBy risk: ;
    sw:term_status "accepted"@en ;
    skos:broader dpv:Harm ;
    skos:inScheme risk:risk-consequences-classes ;
    skos:prefLabel "Danger to Customers"@en .

risk:DangertoPersonnel a rdfs:Class,
        skos:Concept,
        dpv:Impact ;
    dct:contributor "Harshvardhan J. Pandit" ;
    dct:created "2022-08-17"^^xsd:date ;
    dct:source "(ISO/IEC 27005:2018,https://www.iso.org/standard/75281.html)"@en ;
    rdfs:isDefinedBy risk: ;
    sw:term_status "accepted"@en ;
    skos:broader dpv:Harm ;
    skos:inScheme risk:risk-consequences-classes ;
    skos:prefLabel "Danger to Personnel"@en .

risk:DataBreach a rdfs:Class,
        skos:Concept,
        dpv:Consequence ;
    dct:contributor "Harshvardhan J. Pandit" ;
    dct:created "2022-08-17"^^xsd:date ;
    dct:source "(ISO/IEC 27005:2018,https://www.iso.org/standard/75281.html)"@en ;
    rdfs:isDefinedBy risk: ;
    sw:term_status "accepted"@en ;
    skos:broader dpv:Damage ;
    skos:inScheme risk:risk-consequences-classes ;
    skos:prefLabel "Data Breach"@en .

risk:DecisionTreeAnalysis a rdfs:Class,
        skos:Concept,
        risk:RiskAnalysis ;
    dct:contributor "Harshvardhan J. Pandit" ;
    dct:created "2022-08-18"^^xsd:date ;
    dct:source "(IEC 31010:2019,https://www.iso.org/standard/72140.html)"@en ;
    rdfs:isDefinedBy risk: ;
    sw:term_status "accepted"@en ;
    skos:broader risk:QuantitativeRiskAnalysis ;
    skos:definition "Uses a tree-like representation or model of decisions and their possible consequences. Outcomes are usually expressed in monetary terms or in terms of utility."@en ;
    skos:inScheme risk:risk-assessment-classes ;
    skos:prefLabel "Decision Tree Analysis"@en .

risk:DelphiTechnique a rdfs:Class,
        skos:Concept,
        risk:RiskAnalysis ;
    dct:contributor "Harshvardhan J. Pandit" ;
    dct:created "2022-08-18"^^xsd:date ;
    dct:source "(IEC 31010:2019,https://www.iso.org/standard/72140.html)"@en ;
    rdfs:isDefinedBy risk: ;
    sw:term_status "accepted"@en ;
    skos:broader risk:QualitativeRiskAnalysis ;
    skos:definition "Collects judgements through a set of sequential questionnaires. People participate individually but receive feedback on the responses of others after each set of questions."@en ;
    skos:inScheme risk:risk-assessment-classes ;
    skos:prefLabel "Delphi Technique"@en .

risk:DenialServiceAttack a rdfs:Class,
        skos:Concept,
        dpv:Consequence ;
    dct:contributor "Harshvardhan J. Pandit" ;
    dct:created "2022-08-17"^^xsd:date ;
    dct:source "(ISO/IEC 27005:2018,https://www.iso.org/standard/75281.html)"@en ;
    rdfs:isDefinedBy risk: ;
    sw:term_status "accepted"@en ;
    skos:broader dpv:Detriment ;
    skos:inScheme risk:risk-consequences-classes ;
    skos:prefLabel "Denial of Service Attack (DoS)"@en .

risk:DetrimentToRecovery a rdfs:Class,
        skos:Concept,
        dpv:Consequence ;
    dct:contributor "Harshvardhan J. Pandit" ;
    dct:created "2022-08-17"^^xsd:date ;
    dct:source "(ENISA Threat Taxonomy 2016,https://www.enisa.europa.eu/topics/threat-risk-management/threats-and-trends/enisa-threat-landscape/threat-taxonomy/view)"@en ;
    rdfs:isDefinedBy risk: ;
    sw:term_status "accepted"@en ;
    skos:broader dpv:Detriment ;
    skos:inScheme risk:risk-consequences-classes ;
    skos:prefLabel "Detriment to Recovery"@en .

risk:Discrimination a rdfs:Class,
        skos:Concept,
        dpv:Impact ;
    dct:contributor "Georg P Krog" ;
    dct:created "2022-08-19"^^xsd:date ;
    rdfs:isDefinedBy risk: ;
    sw:term_status "accepted"@en ;
    skos:broader dpv:Harm ;
    skos:inScheme risk:risk-consequences-classes ;
    skos:prefLabel "Discrimination"@en .

risk:DistributedDenialServiceAttack a rdfs:Class,
        skos:Concept,
        dpv:Consequence ;
    dct:contributor "Harshvardhan J. Pandit" ;
    dct:created "2022-08-17"^^xsd:date ;
    dct:source "(ISO/IEC 27005:2018,https://www.iso.org/standard/75281.html)"@en ;
    rdfs:isDefinedBy risk: ;
    sw:term_status "accepted"@en ;
    skos:broader dpv:Detriment ;
    skos:inScheme risk:risk-consequences-classes ;
    skos:prefLabel "Distributed Denial of Service Attack (DDoS)"@en .

risk:EBIOS a rdfs:Class,
        skos:Concept,
        risk:RiskManagement ;
    dct:contributor "Harshvardhan J. Pandit" ;
    dct:created "2022-08-18"^^xsd:date ;
    dct:source "(ENISA Risk Management Standards,https://www.enisa.europa.eu/publications/risk-management-standards)"@en ;
    rdfs:isDefinedBy risk: ;
    sw:term_status "accepted"@en ;
    skos:broader risk:RiskManagement ;
    skos:definition "Expression des Besoins et Identification des Objectifs de Sécurité (EBIOS) Risk Manager is an information security risk management method, created under the French General Secretariat of National Defence, consistent with ISO 31000 and ISO/IEC 27005, and enables the risk management requirements of ISO/IEC 27001 to be met"@en ;
    skos:inScheme risk:risk-methodology-classes ;
    skos:prefLabel "EBIOS"@en .

risk:ERM-IF a rdfs:Class,
        skos:Concept,
        risk:RiskManagement ;
    dct:contributor "Harshvardhan J. Pandit" ;
    dct:created "2022-08-18"^^xsd:date ;
    dct:source "(ENISA Compendium of Risk Management Frameworks with Potential Interoperability,https://www.enisa.europa.eu/publications/compendium-of-risk-management-frameworks)"@en ;
    rdfs:isDefinedBy risk: ;
    sw:term_status "accepted"@en ;
    skos:broader risk:RiskManagement ;
    skos:definition "Enterprise Risk Management - Integrated Framework (ERM-IF) defines the essential components of enterprise risk management. It is based on a set of principles and concepts for the enterprise and has as its objective to offer a common language for enterprise risk"@en ;
    skos:inScheme risk:risk-methodology-classes ;
    skos:prefLabel "ERM-IF"@en .

risk:ETSI-TS-102-165-1 a rdfs:Class,
        skos:Concept,
        risk:RiskManagement ;
    dct:contributor "Harshvardhan J. Pandit" ;
    dct:created "2022-08-18"^^xsd:date ;
    dct:source "(ENISA Compendium of Risk Management Frameworks with Potential Interoperability,https://www.enisa.europa.eu/publications/compendium-of-risk-management-frameworks)"@en ;
    rdfs:isDefinedBy risk: ;
    sw:term_status "accepted"@en ;
    skos:broader risk:RiskManagement ;
    skos:definition "ETSI TS 102 165-1 offers methodology and pro-forma for threat, vulnerability and risk analysis (TVRA). According to ETSI TS 102 165-1, threat vulnerability and risk analysis (TVRA) is used to identify risk to an information system based upon the product of the likelihood of an attack and the impact that such an attack will have on the system"@en ;
    skos:inScheme risk:risk-methodology-classes ;
    skos:prefLabel "ETSI TS 102 165-1"@en .

risk:EU-ITSRM a rdfs:Class,
        skos:Concept,
        risk:RiskManagement ;
    dct:contributor "Harshvardhan J. Pandit" ;
    dct:created "2022-08-18"^^xsd:date ;
    dct:source "(ENISA Compendium of Risk Management Frameworks with Potential Interoperability,https://www.enisa.europa.eu/publications/compendium-of-risk-management-frameworks)"@en ;
    rdfs:isDefinedBy risk: ;
    sw:term_status "accepted"@en ;
    skos:broader risk:RiskManagement ;
    skos:definition "ITSRM² IT Security Risk Management Methodology is a methodology provided by DG DIGIT and the European Commission as part of a set of standards for information security"@en ;
    skos:inScheme risk:risk-methodology-classes ;
    skos:prefLabel "ITSRM²"@en .

risk:Eavesdropping a rdfs:Class,
        skos:Concept,
        dpv:Impact ;
    dct:contributor "Harshvardhan J. Pandit" ;
    dct:created "2022-08-17"^^xsd:date ;
    dct:source "(ISO/IEC 27005:2018,https://www.iso.org/standard/75281.html)"@en ;
    rdfs:isDefinedBy risk: ;
    sw:term_status "accepted"@en ;
    skos:broader dpv:NonMaterialDamage ;
    skos:inScheme risk:risk-consequences-classes ;
    skos:prefLabel "Eavesdropping"@en .

risk:EconomicDisadvantage a rdfs:Class,
        skos:Concept,
        dpv:Impact ;
    dct:contributor "Georg P Krog" ;
    dct:created "2022-08-19"^^xsd:date ;
    rdfs:isDefinedBy risk: ;
    sw:term_status "accepted"@en ;
    skos:broader dpv:Impact ;
    skos:inScheme risk:risk-consequences-classes ;
    skos:prefLabel "Economic Disadvantage"@en .

risk:EnvironmentalSafetyEndangerment a rdfs:Class,
        skos:Concept,
        dpv:Impact ;
    dct:contributor "Harshvardhan J. Pandit" ;
    dct:created "2022-08-17"^^xsd:date ;
    dct:source "(ISO/IEC 27005:2018,https://www.iso.org/standard/75281.html)"@en ;
    rdfs:isDefinedBy risk: ;
    sw:term_status "accepted"@en ;
    skos:broader dpv:Harm ;
    skos:inScheme risk:risk-consequences-classes ;
    skos:prefLabel "Environmental Safety Endangerment"@en .

risk:EquipmentFailure a rdfs:Class,
        skos:Concept,
        dpv:Consequence ;
    dct:contributor "Harshvardhan J. Pandit" ;
    dct:created "2022-08-17"^^xsd:date ;
    dct:source "(ISO/IEC 27005:2018,https://www.iso.org/standard/75281.html)"@en ;
    rdfs:isDefinedBy risk: ;
    sw:term_status "accepted"@en ;
    skos:broader dpv:Damage ;
    skos:inScheme risk:risk-consequences-classes ;
    skos:prefLabel "Equipment Failure"@en .

risk:EquipmentMalfunction a rdfs:Class,
        skos:Concept,
        dpv:Consequence ;
    dct:contributor "Harshvardhan J. Pandit" ;
    dct:created "2022-08-17"^^xsd:date ;
    dct:source "(ISO/IEC 27005:2018,https://www.iso.org/standard/75281.html)"@en ;
    rdfs:isDefinedBy risk: ;
    sw:term_status "accepted"@en ;
    skos:broader dpv:Detriment ;
    skos:inScheme risk:risk-consequences-classes ;
    skos:prefLabel "Equipment Malfunction"@en .

risk:ErrornousSystemUse a rdfs:Class,
        skos:Concept,
        dpv:Consequence ;
    dct:contributor "Harshvardhan J. Pandit" ;
    dct:created "2022-08-17"^^xsd:date ;
    dct:source "(ISO/IEC 27005:2018,https://www.iso.org/standard/75281.html)"@en ;
    rdfs:isDefinedBy risk: ;
    sw:term_status "accepted"@en ;
    skos:broader dpv:Detriment ;
    skos:inScheme risk:risk-consequences-classes ;
    skos:prefLabel "Errornous System Use"@en .

risk:EventTreeAnalysis a rdfs:Class,
        skos:Concept,
        risk:RiskAnalysis ;
    dct:contributor "Harshvardhan J. Pandit" ;
    dct:created "2022-08-18"^^xsd:date ;
    dct:source "(IEC 31010:2019,https://www.iso.org/standard/72140.html)"@en ;
    rdfs:isDefinedBy risk: ;
    sw:term_status "accepted"@en ;
    skos:broader risk:QualitativeRiskAnalysis,
        risk:QuantitativeRiskAnalysis ;
    skos:definition "Models the possible outcomes from a given initiating event and the status of controls thus analysing the frequency or probability of the various possible outcomes."@en ;
    skos:inScheme risk:risk-assessment-classes ;
    skos:prefLabel "Event Tree Analysis"@en .

risk:Extorsion a rdfs:Class,
        skos:Concept,
        dpv:Impact ;
    dct:contributor "Harshvardhan J. Pandit" ;
    dct:created "2022-08-17"^^xsd:date ;
    dct:source "(ENISA Threat Taxonomy 2016,https://www.enisa.europa.eu/topics/threat-risk-management/threats-and-trends/enisa-threat-landscape/threat-taxonomy/view)"@en ;
    rdfs:isDefinedBy risk: ;
    sw:term_status "accepted"@en ;
    skos:broader dpv:Harm ;
    skos:inScheme risk:risk-consequences-classes ;
    skos:prefLabel "Extorsion"@en .

risk:ExtremelyHighLikelihood a rdfs:Class,
        skos:Concept,
        dpv:Likelihood ;
    dct:contributor "Harshvardhan J. Pandit" ;
    dct:created "2022-08-18"^^xsd:date ;
    rdf:value "0.99,xsd:decimal" ;
    rdfs:isDefinedBy risk: ;
    sw:term_status "accepted"@en ;
    skos:broader risk:7LikelihoodLevels ;
    skos:definition "Level where Likelihood is Extremely High"@en ;
    skos:inScheme risk:risk-levels-classes ;
    skos:prefLabel "Extremely High Likelihood"@en ;
    skos:scopeNote "The suggested quantitative value for this concept is 0.99 on a scale of 0 to 1"@en .

risk:ExtremelyHighRisk a rdfs:Class,
        skos:Concept,
        dpv:RiskLevel ;
    dct:contributor "Harshvardhan J. Pandit" ;
    dct:created "2022-08-18"^^xsd:date ;
    rdf:value "0.99,xsd:decimal" ;
    rdfs:isDefinedBy risk: ;
    sw:term_status "accepted"@en ;
    skos:broader risk:7RiskLevels ;
    skos:definition "Level where Risk is Extremely High"@en ;
    skos:inScheme risk:risk-levels-classes ;
    skos:prefLabel "Extremely High Risk"@en ;
    skos:scopeNote "The suggested quantitative value for this concept is 0.99 on a scale of 0 to 1"@en .

risk:ExtremelyHighSeverity a rdfs:Class,
        skos:Concept,
        dpv:Severity ;
    dct:contributor "Harshvardhan J. Pandit" ;
    dct:created "2022-08-18"^^xsd:date ;
    rdf:value "0.99,xsd:decimal" ;
    rdfs:isDefinedBy risk: ;
    sw:term_status "accepted"@en ;
    skos:broader risk:7SeverityLevels ;
    skos:definition "Level where Severity is Extremely High"@en ;
    skos:inScheme risk:risk-levels-classes ;
    skos:prefLabel "Extremely High Severity"@en ;
    skos:scopeNote "The suggested quantitative value for this concept is 0.99 on a scale of 0 to 1"@en .

risk:ExtremelyLowLikelihood a rdfs:Class,
        skos:Concept,
        dpv:Likelihood ;
    dct:contributor "Harshvardhan J. Pandit" ;
    dct:created "2022-08-18"^^xsd:date ;
    rdf:value "0.01,xsd:decimal" ;
    rdfs:isDefinedBy risk: ;
    sw:term_status "accepted"@en ;
    skos:broader risk:7LikelihoodLevels ;
    skos:definition "Level where Likelihood is Extremely Low"@en ;
    skos:inScheme risk:risk-levels-classes ;
    skos:prefLabel "Extremely Low Likelihood"@en ;
    skos:scopeNote "The suggested quantitative value for this concept is 0.01 on a scale of 0 to 1"@en .

risk:ExtremelyLowRisk a rdfs:Class,
        skos:Concept,
        dpv:RiskLevel ;
    dct:contributor "Harshvardhan J. Pandit" ;
    dct:created "2022-08-18"^^xsd:date ;
    rdf:value "0.01,xsd:decimal" ;
    rdfs:isDefinedBy risk: ;
    sw:term_status "accepted"@en ;
    skos:broader risk:7RiskLevels ;
    skos:definition "Level where Risk is Extremely Low"@en ;
    skos:inScheme risk:risk-levels-classes ;
    skos:prefLabel "Extremely Low Risk"@en ;
    skos:scopeNote "The suggested quantitative value for this concept is 0.01 on a scale of 0 to 1"@en .

risk:ExtremelyLowSeverity a rdfs:Class,
        skos:Concept,
        dpv:Severity ;
    dct:contributor "Harshvardhan J. Pandit" ;
    dct:created "2022-08-18"^^xsd:date ;
    rdf:value "0.01,xsd:decimal" ;
    rdfs:isDefinedBy risk: ;
    sw:term_status "accepted"@en ;
    skos:broader risk:7SeverityLevels ;
    skos:definition "Level where Severity is Extremely Low"@en ;
    skos:inScheme risk:risk-levels-classes ;
    skos:prefLabel "Extremely Low Severity"@en ;
    skos:scopeNote "The suggested quantitative value for this concept is 0.01 on a scale of 0 to 1"@en .

risk:FAIR a rdfs:Class,
        skos:Concept,
        risk:RiskManagement ;
    dct:contributor "Harshvardhan J. Pandit" ;
    dct:created "2022-08-18"^^xsd:date ;
    dct:source "(ENISA Compendium of Risk Management Frameworks with Potential Interoperability,https://www.enisa.europa.eu/publications/compendium-of-risk-management-frameworks)"@en ;
    rdfs:isDefinedBy risk: ;
    sw:term_status "accepted"@en ;
    skos:broader risk:RiskManagement ;
    skos:definition "The purpose of the FAIR (Factor Analysis of Information Risk) model is to help organisations understand, analyse, and measure information risk. The model provides an approach to quantify risk and defines the necessary building blocks for implementing effective cyber risk management programmes"@en ;
    skos:inScheme risk:risk-methodology-classes ;
    skos:prefLabel "FAIR"@en .

risk:FAIR-Privacy a rdfs:Class,
        skos:Concept,
        risk:RiskManagement ;
    dct:contributor "Harshvardhan J. Pandit" ;
    dct:created "2022-08-18"^^xsd:date ;
    dct:source "(ENISA Risk Management Standards,https://www.enisa.europa.eu/publications/risk-management-standards)"@en ;
    rdfs:isDefinedBy risk: ;
    sw:term_status "accepted"@en ;
    skos:broader risk:RiskManagement ;
    skos:definition "Factors Analysis in Information Risk (FAIR Privacy) is a quantitative privacy risk framework based on FAIR (Factors Analysis in Information Risk) that examines personal privacy risks (to individuals), not organisational risks"@en ;
    skos:inScheme risk:risk-methodology-classes ;
    skos:prefLabel "FAIR Privacy"@en .

risk:FMEA a rdfs:Class,
        skos:Concept,
        risk:RiskAnalysis ;
    dct:contributor "Harshvardhan J. Pandit" ;
    dct:created "2022-08-18"^^xsd:date ;
    dct:source "(IEC 31010:2019,https://www.iso.org/standard/72140.html)"@en ;
    rdfs:isDefinedBy risk: ;
    sw:term_status "accepted"@en ;
    skos:broader risk:QualitativeRiskAnalysis,
        risk:QuantitativeRiskAnalysis ;
    skos:definition "Considers the ways in which each component of a system might fail and the failure causes and effects."@en ;
    skos:inScheme risk:risk-assessment-classes ;
    skos:prefLabel "Failure Modes And Effects Analysis (FMEA)"@en .

risk:FMECA a rdfs:Class,
        skos:Concept,
        risk:RiskAnalysis ;
    dct:contributor "Harshvardhan J. Pandit" ;
    dct:created "2022-08-18"^^xsd:date ;
    dct:source "(IEC 31010:2019,https://www.iso.org/standard/72140.html)"@en ;
    rdfs:isDefinedBy risk: ;
    sw:term_status "accepted"@en ;
    skos:broader risk:QualitativeRiskAnalysis,
        risk:QuantitativeRiskAnalysis ;
    skos:definition "Considers the ways in which each component of a system might fail and the failure causes and effects. FMEA followed by a criticality analysis which defines the significance of each failure mode (FMECA)."@en ;
    skos:inScheme risk:risk-assessment-classes ;
    skos:prefLabel "Failure Modes And Effects And Criticality Analysis (FMECA)"@en .

risk:FNDiagrams a rdfs:Class,
        skos:Concept,
        risk:RiskAnalysis ;
    dct:contributor "Harshvardhan J. Pandit" ;
    dct:created "2022-08-18"^^xsd:date ;
    dct:source "(IEC 31010:2019,https://www.iso.org/standard/72140.html)"@en ;
    rdfs:isDefinedBy risk: ;
    sw:term_status "accepted"@en ;
    skos:broader risk:QuantitativeRiskAnalysis ;
    skos:definition "Special case of quantitative consequence/likelihood graph applied to consideration of tolerability of risk to human life."@en ;
    skos:inScheme risk:risk-assessment-classes ;
    skos:prefLabel "F-N Diagrams"@en .

risk:FaultTreeAnalysis a rdfs:Class,
        skos:Concept,
        risk:RiskAnalysis ;
    dct:contributor "Harshvardhan J. Pandit" ;
    dct:created "2022-08-18"^^xsd:date ;
    dct:source "(IEC 31010:2019,https://www.iso.org/standard/72140.html)"@en ;
    rdfs:isDefinedBy risk: ;
    sw:term_status "accepted"@en ;
    skos:broader risk:QualitativeRiskAnalysis,
        risk:QuantitativeRiskAnalysis ;
    skos:definition "Analyses causes of a focus event using Boolean logic to describe combinations of faults. Variations include a success tree where the top event is desired and a cause tree used to investigate past events."@en ;
    skos:inScheme risk:risk-assessment-classes ;
    skos:prefLabel "Fault Tree Analysis"@en .

risk:FinancialEquipmentCosts a rdfs:Class,
        skos:Concept,
        dpv:Consequence ;
    dct:contributor "Harshvardhan J. Pandit" ;
    dct:created "2022-08-17"^^xsd:date ;
    dct:source "(ISO/IEC 27005:2018,https://www.iso.org/standard/75281.html)"@en ;
    rdfs:isDefinedBy risk: ;
    sw:term_status "accepted"@en ;
    skos:broader dpv:Detriment ;
    skos:inScheme risk:risk-consequences-classes ;
    skos:prefLabel "Financial Equipment Costs"@en .

risk:FinancialInvestigationCosts a rdfs:Class,
        skos:Concept,
        dpv:Consequence ;
    dct:contributor "Harshvardhan J. Pandit" ;
    dct:created "2022-08-17"^^xsd:date ;
    dct:source "(ISO/IEC 27005:2018,https://www.iso.org/standard/75281.html)"@en ;
    rdfs:isDefinedBy risk: ;
    sw:term_status "accepted"@en ;
    skos:broader dpv:Detriment ;
    skos:inScheme risk:risk-consequences-classes ;
    skos:prefLabel "Financial Investigation Costs"@en .

risk:FinancialLoss a rdfs:Class,
        skos:Concept,
        dpv:Consequence ;
    dct:contributor "Harshvardhan J. Pandit" ;
    dct:created "2022-08-17"^^xsd:date ;
    dct:source "(ISO/IEC 27005:2018,https://www.iso.org/standard/75281.html)"@en ;
    rdfs:isDefinedBy risk: ;
    sw:term_status "accepted"@en ;
    skos:broader dpv:Damage ;
    skos:inScheme risk:risk-consequences-classes ;
    skos:prefLabel "Financial Loss"@en .

risk:FinancialPersonnelCosts a rdfs:Class,
        skos:Concept,
        dpv:Consequence ;
    dct:contributor "Harshvardhan J. Pandit" ;
    dct:created "2022-08-17"^^xsd:date ;
    dct:source "(ISO/IEC 27005:2018,https://www.iso.org/standard/75281.html)"@en ;
    rdfs:isDefinedBy risk: ;
    sw:term_status "accepted"@en ;
    skos:broader dpv:Detriment ;
    skos:inScheme risk:risk-consequences-classes ;
    skos:prefLabel "Financial Personnel Costs"@en .

risk:FinancialRepairCosts a rdfs:Class,
        skos:Concept,
        dpv:Consequence ;
    dct:contributor "Harshvardhan J. Pandit" ;
    dct:created "2022-08-17"^^xsd:date ;
    dct:source "(ISO/IEC 27005:2018,https://www.iso.org/standard/75281.html)"@en ;
    rdfs:isDefinedBy risk: ;
    sw:term_status "accepted"@en ;
    skos:broader dpv:Detriment ;
    skos:inScheme risk:risk-consequences-classes ;
    skos:prefLabel "Financial Repair Costs"@en .

risk:Fishbone a rdfs:Class,
        skos:Concept,
        risk:RiskAnalysis ;
    dct:contributor "Harshvardhan J. Pandit" ;
    dct:created "2022-08-18"^^xsd:date ;
    dct:source "(IEC 31010:2019,https://www.iso.org/standard/72140.html)"@en ;
    rdfs:isDefinedBy risk: ;
    sw:term_status "accepted"@en ;
    skos:broader risk:QualitativeRiskAnalysis ;
    skos:definition "Identifies contributory factors to a defined outcome (wanted or unwanted). Contributory factors are usually divided into predefined categories and displayed in a tree structure or a fishbone diagram."@en ;
    skos:inScheme risk:risk-assessment-classes ;
    skos:prefLabel "Ishikawa (Fishbone)"@en .

risk:Fraud a rdfs:Class,
        skos:Concept,
        dpv:Impact ;
    dct:contributor "Harshvardhan J. Pandit" ;
    dct:created "2022-08-17"^^xsd:date ;
    dct:source "(ISO/IEC 27005:2018,https://www.iso.org/standard/75281.html)"@en ;
    rdfs:isDefinedBy risk: ;
    sw:term_status "accepted"@en ;
    skos:broader dpv:Harm ;
    skos:inScheme risk:risk-consequences-classes ;
    skos:prefLabel "Fraud"@en .

risk:GCSOS a rdfs:Class,
        skos:Concept,
        risk:RiskManagement ;
    dct:contributor "Harshvardhan J. Pandit" ;
    dct:created "2022-08-18"^^xsd:date ;
    dct:source "(ENISA Compendium of Risk Management Frameworks with Potential Interoperability,https://www.enisa.europa.eu/publications/compendium-of-risk-management-frameworks)"@en ;
    rdfs:isDefinedBy risk: ;
    sw:term_status "accepted"@en ;
    skos:broader risk:RiskManagement ;
    skos:definition "The Guidelines on Cyber Security Onboard Ships (GCSOS) guidelines explain why and how cyber risks should be managed in a shipping context. They outline the risk assessment process with an explanation of the part played by each component of cyber risk and offer advice on how to respond to and recover from cyber incidents"@en ;
    skos:inScheme risk:risk-methodology-classes ;
    skos:prefLabel "GCSOS"@en .

risk:GameTheory a rdfs:Class,
        skos:Concept,
        risk:RiskAnalysis ;
    dct:contributor "Harshvardhan J. Pandit" ;
    dct:created "2022-08-18"^^xsd:date ;
    dct:source "(IEC 31010:2019,https://www.iso.org/standard/72140.html)"@en ;
    rdfs:isDefinedBy risk: ;
    sw:term_status "accepted"@en ;
    skos:broader risk:QuantitativeRiskAnalysis ;
    skos:definition "The study of strategic decision making to model the impact of the decisions of different players involved in the game. Example application area can be risk based pricing."@en ;
    skos:inScheme risk:risk-assessment-classes ;
    skos:prefLabel "Game Theory"@en .

risk:GovernmentCrisis a rdfs:Class,
        skos:Concept,
        dpv:Consequence ;
    dct:contributor "Harshvardhan J. Pandit" ;
    dct:created "2022-08-17"^^xsd:date ;
    dct:source "(ISO/IEC 27005:2018,https://www.iso.org/standard/75281.html)"@en ;
    rdfs:isDefinedBy risk: ;
    sw:term_status "accepted"@en ;
    skos:broader dpv:Detriment ;
    skos:inScheme risk:risk-consequences-classes ;
    skos:prefLabel "Government Crisis"@en .

risk:HACCP a rdfs:Class,
        skos:Concept,
        risk:RiskAnalysis ;
    dct:contributor "Harshvardhan J. Pandit" ;
    dct:created "2022-08-18"^^xsd:date ;
    dct:source "(IEC 31010:2019,https://www.iso.org/standard/72140.html)"@en ;
    rdfs:isDefinedBy risk: ;
    sw:term_status "accepted"@en ;
    skos:broader risk:QualitativeRiskAnalysis ;
    skos:definition "Analyses the risk reduction that can be achieved by various layers of protection."@en ;
    skos:inScheme risk:risk-assessment-classes ;
    skos:prefLabel "Hazard Analysis And Critical Control Points (HACCP)"@en .

risk:HAZOP a rdfs:Class,
        skos:Concept,
        risk:RiskAnalysis ;
    dct:contributor "Harshvardhan J. Pandit" ;
    dct:created "2022-08-18"^^xsd:date ;
    dct:source "(IEC 31010:2019,https://www.iso.org/standard/72140.html)"@en ;
    rdfs:isDefinedBy risk: ;
    sw:term_status "accepted"@en ;
    skos:broader risk:QualitativeRiskAnalysis ;
    skos:definition "A structured and systematic examination of a planned or existing process or operation in order to identify and evaluate problems that might represent risk to personnel or equipment, or prevent efficient operation"@en ;
    skos:inScheme risk:risk-assessment-classes ;
    skos:prefLabel "Hazard And Operability Studies (HAZOP)"@en .

risk:HITRUST-CSF a rdfs:Class,
        skos:Concept,
        risk:RiskManagement ;
    dct:contributor "Harshvardhan J. Pandit" ;
    dct:created "2022-08-18"^^xsd:date ;
    dct:source "(ENISA Compendium of Risk Management Frameworks with Potential Interoperability,https://www.enisa.europa.eu/publications/compendium-of-risk-management-frameworks)"@en ;
    rdfs:isDefinedBy risk: ;
    sw:term_status "accepted"@en ;
    skos:broader risk:RiskManagement ;
    skos:definition "The HITRUST Cyber-Security Framework (CSF) is a framework created by security industry experts to safeguard sensitive information and manage information risk for organisations across all industries and throughout the third-party supply chain"@en ;
    skos:inScheme risk:risk-methodology-classes ;
    skos:prefLabel "HITRUST-CSF"@en .

risk:HaltSource a rdfs:Class,
        skos:Concept,
        dpv:RiskMitigationMeasure ;
    dct:contributor "Harshvardhan J. Pandit" ;
    dct:created "2022-08-19"^^xsd:date ;
    rdfs:isDefinedBy risk: ;
    sw:term_status "accepted"@en ;
    skos:broader risk:ControlRiskSource ;
    skos:definition "Risk Control that halts the risk source or prevents it from materialising"@en ;
    skos:inScheme risk:risk-controls-classes ;
    skos:prefLabel "Halt Source"@en .

risk:HarmfulSpeech a rdfs:Class,
        skos:Concept,
        dpv:Impact ;
    dct:contributor "Harshvardhan J. Pandit" ;
    dct:created "2022-08-17"^^xsd:date ;
    dct:source "(ENISA Reference Incident Classification Taxonomy 2018,https://www.enisa.europa.eu/publications/reference-incident-classification-taxonomy/)"@en ;
    rdfs:isDefinedBy risk: ;
    sw:term_status "accepted"@en ;
    skos:broader dpv:Harm ;
    skos:inScheme risk:risk-consequences-classes ;
    skos:prefLabel "Harmful Spech"@en .

risk:HealthLifeImpact a rdfs:Class,
        skos:Concept,
        dpv:Impact ;
    dct:contributor "Harshvardhan J. Pandit" ;
    dct:created "2022-08-17"^^xsd:date ;
    dct:source "(ENISA Methodology for Sectoral Cybersecurity Assessments,https://www.enisa.europa.eu/publications/methodology-for-a-sectoral-cybersecurity-assessment)"@en ;
    rdfs:isDefinedBy risk: ;
    sw:term_status "accepted"@en ;
    skos:broader dpv:Impact ;
    skos:inScheme risk:risk-consequences-classes ;
    skos:prefLabel "Health and life impact"@en .

risk:HighLikelihood a rdfs:Class,
        skos:Concept,
        dpv:Likelihood ;
    dct:contributor "Harshvardhan J. Pandit" ;
    dct:created "2022-08-18"^^xsd:date ;
    rdf:value "0.75,xsd:decimal" ;
    rdfs:isDefinedBy risk: ;
    sw:term_status "accepted"@en ;
    skos:broader risk:3LikelihoodLevels,
        risk:5LikelihoodLevels,
        risk:7LikelihoodLevels ;
    skos:definition "Level where Likelihood is High"@en ;
    skos:inScheme risk:risk-levels-classes ;
    skos:prefLabel "High Likelihood"@en ;
    skos:scopeNote "The suggested quantitative value for this concept is 0.75 on a scale of 0 to 1"@en .

risk:HighRisk a rdfs:Class,
        skos:Concept,
        dpv:RiskLevel ;
    dct:contributor "Harshvardhan J. Pandit" ;
    dct:created "2022-08-18"^^xsd:date ;
    rdf:value "0.75,xsd:decimal" ;
    rdfs:isDefinedBy risk: ;
    sw:term_status "accepted"@en ;
    skos:broader risk:3RiskLevels,
        risk:5RiskLevels,
        risk:7RiskLevels ;
    skos:definition "Level where Risk is High"@en ;
    skos:inScheme risk:risk-levels-classes ;
    skos:prefLabel "High Risk"@en ;
    skos:scopeNote "The suggested quantitative value for this concept is 0.75 on a scale of 0 to 1"@en .

risk:HighSeverity a rdfs:Class,
        skos:Concept,
        dpv:Severity ;
    dct:contributor "Harshvardhan J. Pandit" ;
    dct:created "2022-08-18"^^xsd:date ;
    rdf:value "0.75,xsd:decimal" ;
    rdfs:isDefinedBy risk: ;
    sw:term_status "accepted"@en ;
    skos:broader risk:3SeverityLevels,
        risk:5SeverityLevels,
        risk:7SeverityLevels ;
    skos:definition "Level where Severity is High"@en ;
    skos:inScheme risk:risk-levels-classes ;
    skos:prefLabel "High Severity"@en ;
    skos:scopeNote "The suggested quantitative value for this concept is 0.75 on a scale of 0 to 1"@en .

risk:HumanErrors a rdfs:Class,
        skos:Concept,
        dpv:Consequence ;
    dct:contributor "Harshvardhan J. Pandit" ;
    dct:created "2022-08-17"^^xsd:date ;
    dct:source "(ENISA Reference Incident Classification Taxonomy 2018,https://www.enisa.europa.eu/publications/reference-incident-classification-taxonomy/)"@en ;
    rdfs:isDefinedBy risk: ;
    sw:term_status "accepted"@en ;
    skos:broader dpv:Detriment ;
    skos:inScheme risk:risk-consequences-classes ;
    skos:prefLabel "Human Errors"@en .

risk:HumanReliabilityAnalysis a rdfs:Class,
        skos:Concept,
        risk:RiskAnalysis ;
    dct:contributor "Harshvardhan J. Pandit" ;
    dct:created "2022-08-18"^^xsd:date ;
    dct:source "(IEC 31010:2019,https://www.iso.org/standard/72140.html)"@en ;
    rdfs:isDefinedBy risk: ;
    sw:term_status "accepted"@en ;
    skos:broader risk:QualitativeRiskAnalysis,
        risk:QuantitativeRiskAnalysis ;
    skos:definition "A set of techniques for identifying the potential for human error and estimating the likelihood of failure."@en ;
    skos:inScheme risk:risk-assessment-classes ;
    skos:prefLabel "Human Reliability Analysis"@en .

risk:IMO-MSC-FAL1-CIRC3 a rdfs:Class,
        skos:Concept,
        risk:RiskManagement ;
    dct:contributor "Harshvardhan J. Pandit" ;
    dct:created "2022-08-18"^^xsd:date ;
    dct:source "(ENISA Compendium of Risk Management Frameworks with Potential Interoperability,https://www.enisa.europa.eu/publications/compendium-of-risk-management-frameworks)"@en ;
    rdfs:isDefinedBy risk: ;
    sw:term_status "accepted"@en ;
    skos:broader risk:RiskManagement ;
    skos:definition "The official International Maritime Organization guidelines IMO MSC-FAL.1/CIRC.3 provide a high-level approach to the management pf maritime cyber risk which refers to the extent a technology asset is exposed to risks during an event that could result in shipping-related operational failure"@en ;
    skos:inScheme risk:risk-methodology-classes ;
    skos:prefLabel "IMO MSC-FAL.1/CIRC.3"@en .

risk:IRAM2 a rdfs:Class,
        skos:Concept,
        risk:RiskManagement ;
    dct:contributor "Harshvardhan J. Pandit" ;
    dct:created "2022-08-18"^^xsd:date ;
    dct:source "(ENISA Compendium of Risk Management Frameworks with Potential Interoperability,https://www.enisa.europa.eu/publications/compendium-of-risk-management-frameworks)"@en ;
    rdfs:isDefinedBy risk: ;
    sw:term_status "accepted"@en ;
    skos:broader risk:RiskManagement ;
    skos:definition "Information Risk Assessment Methodology (IRAM2) supports risk assessment and treatment and entails a six-phase process, and is is implemented by an automated toolset"@en ;
    skos:inScheme risk:risk-methodology-classes ;
    skos:prefLabel "IRAM2"@en .

risk:IS-BM a rdfs:Class,
        skos:Concept,
        risk:RiskManagement ;
    dct:contributor "Harshvardhan J. Pandit" ;
    dct:created "2022-08-18"^^xsd:date ;
    dct:source "(ENISA Compendium of Risk Management Frameworks with Potential Interoperability,https://www.enisa.europa.eu/publications/compendium-of-risk-management-frameworks)"@en ;
    rdfs:isDefinedBy risk: ;
    sw:term_status "accepted"@en ;
    skos:broader risk:RiskManagement ;
    skos:definition "The IS risk analysis method is based on a business model using a quantitative approach. The values of IS assets come from their importance towards operational continuity, as well as from their replacement costs"@en ;
    skos:inScheme risk:risk-methodology-classes ;
    skos:prefLabel "IS-BM"@en .

risk:ISACA-RISK-IT a rdfs:Class,
        skos:Concept,
        risk:RiskManagement ;
    dct:contributor "Harshvardhan J. Pandit" ;
    dct:created "2022-08-18"^^xsd:date ;
    dct:source "(ENISA Compendium of Risk Management Frameworks with Potential Interoperability,https://www.enisa.europa.eu/publications/compendium-of-risk-management-frameworks)"@en ;
    rdfs:isDefinedBy risk: ;
    sw:term_status "accepted"@en ;
    skos:broader risk:RiskManagement ;
    skos:definition "The ISACA Risk IT Framework provides a set of guiding principles and supporting practices for enterprise management, combined to deliver a comprehensive process model for governing and managing IT risk"@en ;
    skos:inScheme risk:risk-methodology-classes ;
    skos:prefLabel "ISACA-RISK-IT"@en .

risk:ISAMM a rdfs:Class,
        skos:Concept,
        risk:RiskManagement ;
    dct:contributor "Harshvardhan J. Pandit" ;
    dct:created "2022-08-18"^^xsd:date ;
    dct:source "(ENISA Risk Management Standards,https://www.enisa.europa.eu/publications/risk-management-standards)"@en ;
    rdfs:isDefinedBy risk: ;
    sw:term_status "accepted"@en ;
    skos:broader risk:RiskManagement ;
    skos:definition "Information Security Assessment and Monitoring Method (ISAMM) is a quantitative type of risk management methodology that can be applied by various organisations such as governmental agencies, large companies and small and medium size enterprises"@en ;
    skos:inScheme risk:risk-methodology-classes ;
    skos:prefLabel "ISAMM"@en .

risk:ISO-IEC-27005-2018 a rdfs:Class,
        skos:Concept,
        risk:RiskManagement ;
    dct:contributor "Harshvardhan J. Pandit" ;
    dct:created "2022-08-18"^^xsd:date ;
    dct:source "(ENISA Compendium of Risk Management Frameworks with Potential Interoperability,https://www.enisa.europa.eu/publications/compendium-of-risk-management-frameworks)"@en ;
    rdfs:isDefinedBy risk: ;
    sw:term_status "accepted"@en ;
    skos:broader risk:RiskManagement ;
    skos:definition "ISO/IEC 27005:2018 ‘Information technology — Security techniques — Information security risk management’ is a risk management framework applicable to all types of organisations (e.g. commercial enterprises, government agencies, non-profit organisations) which intend to manage risks that could compromise the organisation’s information security"@en ;
    skos:inScheme risk:risk-methodology-classes ;
    skos:prefLabel "ISO/IEC 27005:2018"@en .

risk:ISRAM a rdfs:Class,
        skos:Concept,
        risk:RiskManagement ;
    dct:contributor "Harshvardhan J. Pandit" ;
    dct:created "2022-08-18"^^xsd:date ;
    dct:source "(ENISA Compendium of Risk Management Frameworks with Potential Interoperability,https://www.enisa.europa.eu/publications/compendium-of-risk-management-frameworks)"@en ;
    rdfs:isDefinedBy risk: ;
    sw:term_status "accepted"@en ;
    skos:broader risk:RiskManagement ;
    skos:definition "ISRAM is a quantitative, paper-based risk analysis method that is designed to allow effective participation of managers and staff in the process"@en ;
    skos:inScheme risk:risk-methodology-classes ;
    skos:prefLabel "ISRAM"@en .

risk:IT-Grundschutz a rdfs:Class,
        skos:Concept,
        risk:RiskManagement ;
    dct:contributor "Harshvardhan J. Pandit" ;
    dct:created "2022-08-18"^^xsd:date ;
    dct:source "(ENISA Risk Management Standards,https://www.enisa.europa.eu/publications/risk-management-standards)"@en ;
    rdfs:isDefinedBy risk: ;
    sw:term_status "accepted"@en ;
    skos:broader risk:RiskManagement ;
    skos:definition "IT-Grundschutz has been developed by the Federal Office for Information Security in Germany. IT-Grundschutz provides a configuration for the establishment of an integrated and effective IT security managemen"@en ;
    skos:inScheme risk:risk-methodology-classes ;
    skos:prefLabel "IT-Grundschutz"@en .

risk:IdentityDispute a rdfs:Class,
        skos:Concept,
        dpv:Consequence ;
    dct:contributor "Harshvardhan J. Pandit" ;
    dct:created "2022-08-24"^^xsd:date ;
    rdfs:isDefinedBy risk: ;
    sw:term_status "accepted"@en ;
    skos:broader dpv:Detriment ;
    skos:inScheme risk:risk-consequences-classes ;
    skos:prefLabel "Identity Dispute"@en .

risk:IdentityFraud a rdfs:Class,
        skos:Concept,
        dpv:Impact ;
    dct:contributor "Harshvardhan J. Pandit" ;
    dct:created "2022-08-17"^^xsd:date ;
    dct:source "(ENISA Threat Taxonomy 2016,https://www.enisa.europa.eu/topics/threat-risk-management/threats-and-trends/enisa-threat-landscape/threat-taxonomy/view)"@en ;
    rdfs:isDefinedBy risk: ;
    sw:term_status "accepted"@en ;
    skos:broader dpv:Harm ;
    skos:inScheme risk:risk-consequences-classes ;
    skos:prefLabel "Identity Fraud"@en .

risk:IdentityTheft a rdfs:Class,
        skos:Concept,
        dpv:Impact ;
    dct:contributor "Harshvardhan J. Pandit" ;
    dct:created "2022-08-17"^^xsd:date ;
    dct:source "(ENISA Threat Taxonomy 2016,https://www.enisa.europa.eu/topics/threat-risk-management/threats-and-trends/enisa-threat-landscape/threat-taxonomy/view)"@en ;
    rdfs:isDefinedBy risk: ;
    sw:term_status "accepted"@en ;
    skos:broader dpv:Harm ;
    skos:inScheme risk:risk-consequences-classes ;
    skos:prefLabel "Identity Theft"@en .

risk:IllegalProcessingData a rdfs:Class,
        skos:Concept,
        dpv:Consequence ;
    dct:contributor "Harshvardhan J. Pandit" ;
    dct:created "2022-08-17"^^xsd:date ;
    dct:source "(ISO/IEC 27005:2018,https://www.iso.org/standard/75281.html)"@en ;
    rdfs:isDefinedBy risk: ;
    sw:term_status "accepted"@en ;
    skos:broader dpv:Damage ;
    skos:inScheme risk:risk-consequences-classes ;
    skos:prefLabel "Illegal Processing of Data"@en .

risk:ImpactOnDataSubject a rdfs:Class,
        skos:Concept,
        dpv:Impact ;
    dct:contributor "Harshvardhan J. Pandit, Georg P Krog" ;
    dct:created "2022-10-22"^^xsd:date ;
    rdfs:isDefinedBy risk: ;
    sw:term_status "accepted"@en ;
    skos:broader dpv:Impact ;
    skos:inScheme risk:risk-consequences-classes ;
    skos:prefLabel "Impact on Data Subject"@en .

risk:ImpacttoRights a rdfs:Class,
        skos:Concept,
        dpv:Impact ;
    dct:contributor "Harshvardhan J. Pandit" ;
    dct:created "2022-08-17"^^xsd:date ;
    dct:source "(ISO/IEC 27005:2018,https://www.iso.org/standard/75281.html)"@en ;
    rdfs:isDefinedBy risk: ;
    sw:term_status "accepted"@en ;
    skos:broader dpv:Impact ;
    skos:inScheme risk:risk-consequences-classes ;
    skos:prefLabel "Impact to Rights"@en .

risk:IncreaseInternalCost a rdfs:Class,
        skos:Concept,
        dpv:Consequence ;
    dct:contributor "Harshvardhan J. Pandit" ;
    dct:created "2022-08-17"^^xsd:date ;
    dct:source "(ISO/IEC 27005:2018,https://www.iso.org/standard/75281.html)"@en ;
    rdfs:isDefinedBy risk: ;
    sw:term_status "accepted"@en ;
    skos:broader dpv:Detriment ;
    skos:inScheme risk:risk-consequences-classes ;
    skos:prefLabel "Increase Internal Cost"@en .

risk:IndustrialCrisis a rdfs:Class,
        skos:Concept,
        dpv:Consequence ;
    dct:contributor "Harshvardhan J. Pandit" ;
    dct:created "2022-08-17"^^xsd:date ;
    dct:source "(ISO/IEC 27005:2018,https://www.iso.org/standard/75281.html)"@en ;
    rdfs:isDefinedBy risk: ;
    sw:term_status "accepted"@en ;
    skos:broader dpv:Detriment ;
    skos:inScheme risk:risk-consequences-classes ;
    skos:prefLabel "Industrial Crisis"@en .

risk:InfluenceDiagrams a rdfs:Class,
        skos:Concept,
        risk:RiskAnalysis ;
    dct:contributor "Harshvardhan J. Pandit" ;
    dct:created "2022-08-18"^^xsd:date ;
    dct:source "(IEC 31010:2019,https://www.iso.org/standard/72140.html)"@en ;
    rdfs:isDefinedBy risk: ;
    sw:term_status "accepted"@en ;
    skos:broader risk:QuantitativeRiskAnalysis ;
    skos:definition "An extended version of Bayesian networks that includes variables representing uncertainties, consequences and actions"@en ;
    skos:inScheme risk:risk-assessment-classes ;
    skos:prefLabel "Influence Diagrams"@en .

risk:Injury a rdfs:Class,
        skos:Concept,
        dpv:Impact ;
    dct:contributor "Harshvardhan J. Pandit" ;
    dct:created "2022-08-17"^^xsd:date ;
    dct:source "(ISO/IEC 27005:2018,https://www.iso.org/standard/75281.html)"@en ;
    rdfs:isDefinedBy risk: ;
    sw:term_status "accepted"@en ;
    skos:broader dpv:Harm ;
    skos:inScheme risk:risk-consequences-classes ;
    skos:prefLabel "Injury"@en .

risk:InterceptionCommunications a rdfs:Class,
        skos:Concept,
        dpv:Consequence ;
    dct:contributor "Harshvardhan J. Pandit" ;
    dct:created "2022-08-17"^^xsd:date ;
    dct:source "(ISO/IEC 27005:2018,https://www.iso.org/standard/75281.html)"@en ;
    rdfs:isDefinedBy risk: ;
    sw:term_status "accepted"@en ;
    skos:broader dpv:Damage ;
    skos:inScheme risk:risk-consequences-classes ;
    skos:prefLabel "Interception of Communications"@en .

risk:InternalOperationDisruption a rdfs:Class,
        skos:Concept,
        dpv:Consequence ;
    dct:contributor "Harshvardhan J. Pandit" ;
    dct:created "2022-08-17"^^xsd:date ;
    dct:source "(ISO/IEC 27005:2018,https://www.iso.org/standard/75281.html)"@en ;
    rdfs:isDefinedBy risk: ;
    sw:term_status "accepted"@en ;
    skos:broader dpv:Detriment ;
    skos:inScheme risk:risk-consequences-classes ;
    skos:prefLabel "Internal Operation Disruption"@en .

risk:Interviews a rdfs:Class,
        skos:Concept,
        risk:RiskAnalysis ;
    dct:contributor "Harshvardhan J. Pandit" ;
    dct:created "2022-08-18"^^xsd:date ;
    dct:source "(IEC 31010:2019,https://www.iso.org/standard/72140.html)"@en ;
    rdfs:isDefinedBy risk: ;
    sw:term_status "accepted"@en ;
    skos:broader risk:QualitativeRiskAnalysis ;
    skos:definition "Structured or semi- structured one-to-one conversations to elicit views."@en ;
    skos:inScheme risk:risk-assessment-classes ;
    skos:prefLabel "Interviews"@en .

risk:KnownVulnerabilityExploited a rdfs:Class,
        skos:Concept,
        dpv:Consequence ;
    dct:contributor "Harshvardhan J. Pandit" ;
    dct:created "2022-08-17"^^xsd:date ;
    dct:source "(ENISA Reference Incident Classification Taxonomy 2018,https://www.enisa.europa.eu/publications/reference-incident-classification-taxonomy/)"@en ;
    rdfs:isDefinedBy risk: ;
    sw:term_status "accepted"@en ;
    skos:broader dpv:Detriment ;
    skos:inScheme risk:risk-consequences-classes ;
    skos:prefLabel "Known Vulnerability Exploited"@en .

risk:LOPA a rdfs:Class,
        skos:Concept,
        risk:RiskAnalysis ;
    dct:contributor "Harshvardhan J. Pandit" ;
    dct:created "2022-08-18"^^xsd:date ;
    dct:source "(IEC 31010:2019,https://www.iso.org/standard/72140.html)"@en ;
    rdfs:isDefinedBy risk: ;
    sw:term_status "accepted"@en ;
    skos:broader risk:QualitativeRiskAnalysis,
        risk:QuantitativeRiskAnalysis ;
    skos:definition "Analyses the risk reduction that can be achieved by various layers of protection."@en ;
    skos:inScheme risk:risk-assessment-classes ;
    skos:prefLabel "Layer Protection Analysis (LOPA)"@en .

risk:LawEnforcementAdverseEffects a rdfs:Class,
        skos:Concept,
        dpv:Consequence ;
    dct:contributor "Harshvardhan J. Pandit" ;
    dct:created "2022-08-17"^^xsd:date ;
    dct:source "(ISO/IEC 27005:2018,https://www.iso.org/standard/75281.html)"@en ;
    rdfs:isDefinedBy risk: ;
    sw:term_status "accepted"@en ;
    skos:broader dpv:Detriment ;
    skos:inScheme risk:risk-consequences-classes ;
    skos:prefLabel "Law Enforcement Adverse Effects"@en .

risk:LimitationOfRights a rdfs:Class,
        skos:Concept,
        dpv:Impact ;
    dct:contributor "Georg P Krog, Harshvardhan J. Pandit" ;
    dct:created "2022-08-18"^^xsd:date ;
    rdfs:isDefinedBy risk: ;
    sw:term_status "accepted"@en ;
    skos:broader dpv:Harm ;
    skos:inScheme risk:risk-consequences-classes ;
    skos:prefLabel "Limitation of Rights"@en .

risk:LossAssets a rdfs:Class,
        skos:Concept,
        dpv:Impact ;
    dct:contributor "Harshvardhan J. Pandit" ;
    dct:created "2022-08-17"^^xsd:date ;
    dct:source "(ISO/IEC 27005:2018,https://www.iso.org/standard/75281.html)"@en ;
    rdfs:isDefinedBy risk: ;
    sw:term_status "accepted"@en ;
    skos:broader dpv:MaterialDamage ;
    skos:inScheme risk:risk-consequences-classes ;
    skos:prefLabel "Loss of Assets"@en .

risk:LossCompetitiveAdvantage a rdfs:Class,
        skos:Concept,
        dpv:Impact ;
    dct:contributor "Harshvardhan J. Pandit" ;
    dct:created "2022-08-17"^^xsd:date ;
    dct:source "(ISO/IEC 27005:2018,https://www.iso.org/standard/75281.html)"@en ;
    rdfs:isDefinedBy risk: ;
    sw:term_status "accepted"@en ;
    skos:broader dpv:NonMaterialDamage ;
    skos:inScheme risk:risk-consequences-classes ;
    skos:prefLabel "Loss of Competitive Advantage"@en .

risk:LossControlOverData a rdfs:Class,
        skos:Concept,
        dpv:Impact ;
    dct:contributor "Georg P Krog, Harshvardhan J. Pandit" ;
    dct:created "2022-08-19"^^xsd:date ;
    rdfs:isDefinedBy risk: ;
    sw:term_status "accepted"@en ;
    skos:broader dpv:NonMaterialDamage ;
    skos:inScheme risk:risk-consequences-classes ;
    skos:prefLabel "Loss of Control over Data"@en .

risk:LossCredibility a rdfs:Class,
        skos:Concept,
        dpv:Consequence ;
    dct:contributor "Harshvardhan J. Pandit" ;
    dct:created "2022-08-17"^^xsd:date ;
    dct:source "(ISO/IEC 27005:2018,https://www.iso.org/standard/75281.html)"@en ;
    rdfs:isDefinedBy risk: ;
    sw:term_status "accepted"@en ;
    skos:broader dpv:Detriment ;
    skos:inScheme risk:risk-consequences-classes ;
    skos:prefLabel "Loss of Credibility"@en .

risk:LossCustomerConfidence a rdfs:Class,
        skos:Concept,
        dpv:Consequence ;
    dct:contributor "Harshvardhan J. Pandit" ;
    dct:created "2022-08-17"^^xsd:date ;
    dct:source "(ISO/IEC 27005:2018,https://www.iso.org/standard/75281.html)"@en ;
    rdfs:isDefinedBy risk: ;
    sw:term_status "accepted"@en ;
    skos:broader dpv:Detriment ;
    skos:inScheme risk:risk-consequences-classes ;
    skos:prefLabel "Loss of Customer Confidence"@en .

risk:LossCustomers a rdfs:Class,
        skos:Concept,
        dpv:Impact ;
    dct:contributor "Harshvardhan J. Pandit" ;
    dct:created "2022-08-17"^^xsd:date ;
    dct:source "(ISO/IEC 27005:2018,https://www.iso.org/standard/75281.html)"@en ;
    rdfs:isDefinedBy risk: ;
    sw:term_status "accepted"@en ;
    skos:broader dpv:NonMaterialDamage ;
    skos:inScheme risk:risk-consequences-classes ;
    skos:prefLabel "Loss of Customers"@en .

risk:LossData a rdfs:Class,
        skos:Concept,
        dpv:Impact ;
    dct:contributor "Harshvardhan J. Pandit" ;
    dct:created "2022-08-17"^^xsd:date ;
    dct:source "(ENISA Threat Taxonomy 2016,https://www.enisa.europa.eu/topics/threat-risk-management/threats-and-trends/enisa-threat-landscape/threat-taxonomy/view)"@en ;
    rdfs:isDefinedBy risk: ;
    sw:term_status "accepted"@en ;
    skos:broader dpv:NonMaterialDamage ;
    skos:inScheme risk:risk-consequences-classes ;
    skos:prefLabel "Loss of Data"@en .

risk:LossFunds a rdfs:Class,
        skos:Concept,
        dpv:Impact ;
    dct:contributor "Harshvardhan J. Pandit" ;
    dct:created "2022-08-17"^^xsd:date ;
    dct:source "(ISO/IEC 27005:2018,https://www.iso.org/standard/75281.html)"@en ;
    rdfs:isDefinedBy risk: ;
    sw:term_status "accepted"@en ;
    skos:broader dpv:MaterialDamage ;
    skos:inScheme risk:risk-consequences-classes ;
    skos:prefLabel "Loss of Funds"@en .

risk:LossGoods a rdfs:Class,
        skos:Concept,
        dpv:Impact ;
    dct:contributor "Harshvardhan J. Pandit" ;
    dct:created "2022-08-17"^^xsd:date ;
    dct:source "(ISO/IEC 27005:2018,https://www.iso.org/standard/75281.html)"@en ;
    rdfs:isDefinedBy risk: ;
    sw:term_status "accepted"@en ;
    skos:broader dpv:MaterialDamage ;
    skos:inScheme risk:risk-consequences-classes ;
    skos:prefLabel "Loss of Goods"@en .

risk:LossGoodwill a rdfs:Class,
        skos:Concept,
        dpv:Consequence ;
    dct:contributor "Harshvardhan J. Pandit" ;
    dct:created "2022-08-17"^^xsd:date ;
    dct:source "(ISO/IEC 27005:2018,https://www.iso.org/standard/75281.html)"@en ;
    rdfs:isDefinedBy risk: ;
    sw:term_status "accepted"@en ;
    skos:broader dpv:Detriment ;
    skos:inScheme risk:risk-consequences-classes ;
    skos:prefLabel "Loss of Goodwill"@en .

risk:LossNegotiatingCapacity a rdfs:Class,
        skos:Concept,
        dpv:Consequence ;
    dct:contributor "Harshvardhan J. Pandit" ;
    dct:created "2022-08-17"^^xsd:date ;
    dct:source "(ISO/IEC 27005:2018,https://www.iso.org/standard/75281.html)"@en ;
    rdfs:isDefinedBy risk: ;
    sw:term_status "accepted"@en ;
    skos:broader dpv:Detriment ;
    skos:inScheme risk:risk-consequences-classes ;
    skos:prefLabel "Loss of Negotiating Capacity"@en .

risk:LossOpportunity a rdfs:Class,
        skos:Concept,
        dpv:Consequence ;
    dct:contributor "Harshvardhan J. Pandit" ;
    dct:created "2022-08-17"^^xsd:date ;
    dct:source "(ISO/IEC 27005:2018,https://www.iso.org/standard/75281.html)"@en ;
    rdfs:isDefinedBy risk: ;
    sw:term_status "accepted"@en ;
    skos:broader dpv:Detriment ;
    skos:inScheme risk:risk-consequences-classes ;
    skos:prefLabel "Loss of Opportunity"@en .

risk:LossProprietaryInformation a rdfs:Class,
        skos:Concept,
        dpv:Impact ;
    dct:contributor "Harshvardhan J. Pandit" ;
    dct:created "2022-08-17"^^xsd:date ;
    dct:source "(ISO/IEC 27005:2018,https://www.iso.org/standard/75281.html)"@en ;
    rdfs:isDefinedBy risk: ;
    sw:term_status "accepted"@en ;
    skos:broader dpv:NonMaterialDamage ;
    skos:inScheme risk:risk-consequences-classes ;
    skos:prefLabel "Loss of Proprietary Information"@en .

risk:LossReputation a rdfs:Class,
        skos:Concept,
        dpv:Consequence ;
    dct:contributor "Harshvardhan J. Pandit" ;
    dct:created "2022-08-17"^^xsd:date ;
    dct:source "(ISO/IEC 27005:2018,https://www.iso.org/standard/75281.html)"@en ;
    rdfs:isDefinedBy risk: ;
    sw:term_status "accepted"@en ;
    skos:broader dpv:Detriment ;
    skos:inScheme risk:risk-consequences-classes ;
    skos:prefLabel "Loss of Reputation"@en .

risk:LossResources a rdfs:Class,
        skos:Concept,
        dpv:Impact ;
    dct:contributor "Harshvardhan J. Pandit" ;
    dct:created "2022-08-17"^^xsd:date ;
    dct:source "(ENISA Threat Taxonomy 2016,https://www.enisa.europa.eu/topics/threat-risk-management/threats-and-trends/enisa-threat-landscape/threat-taxonomy/view)"@en ;
    rdfs:isDefinedBy risk: ;
    sw:term_status "accepted"@en ;
    skos:broader dpv:NonMaterialDamage ;
    skos:inScheme risk:risk-consequences-classes ;
    skos:prefLabel "Loss of Resources"@en .

risk:LossSuppliers a rdfs:Class,
        skos:Concept,
        dpv:Impact ;
    dct:contributor "Harshvardhan J. Pandit" ;
    dct:created "2022-08-17"^^xsd:date ;
    dct:source "(ISO/IEC 27005:2018,https://www.iso.org/standard/75281.html)"@en ;
    rdfs:isDefinedBy risk: ;
    sw:term_status "accepted"@en ;
    skos:broader dpv:NonMaterialDamage ;
    skos:inScheme risk:risk-consequences-classes ;
    skos:prefLabel "Loss of Suppliers"@en .

risk:LossTechnologicalAdvantage a rdfs:Class,
        skos:Concept,
        dpv:Impact ;
    dct:contributor "Harshvardhan J. Pandit" ;
    dct:created "2022-08-17"^^xsd:date ;
    dct:source "(ISO/IEC 27005:2018,https://www.iso.org/standard/75281.html)"@en ;
    rdfs:isDefinedBy risk: ;
    sw:term_status "accepted"@en ;
    skos:broader dpv:NonMaterialDamage ;
    skos:inScheme risk:risk-consequences-classes ;
    skos:prefLabel "Loss of Technological Advantage"@en .

risk:LossTrust a rdfs:Class,
        skos:Concept,
        dpv:Consequence ;
    dct:contributor "Harshvardhan J. Pandit" ;
    dct:created "2022-08-17"^^xsd:date ;
    dct:source "(ISO/IEC 27005:2018,https://www.iso.org/standard/75281.html)"@en ;
    rdfs:isDefinedBy risk: ;
    sw:term_status "accepted"@en ;
    skos:broader dpv:Detriment ;
    skos:inScheme risk:risk-consequences-classes ;
    skos:prefLabel "Loss of Trust"@en .

risk:LowLikelihood a rdfs:Class,
        skos:Concept,
        dpv:Likelihood ;
    dct:contributor "Harshvardhan J. Pandit" ;
    dct:created "2022-08-18"^^xsd:date ;
    rdf:value "0.25,xsd:decimal" ;
    rdfs:isDefinedBy risk: ;
    sw:term_status "accepted"@en ;
    skos:broader risk:3LikelihoodLevels,
        risk:5LikelihoodLevels,
        risk:7LikelihoodLevels ;
    skos:definition "Level where Likelihood is Low"@en ;
    skos:inScheme risk:risk-levels-classes ;
    skos:prefLabel "Low Likelihood"@en ;
    skos:scopeNote "The suggested quantitative value for this concept is 0.25 on a scale of 0 to 1"@en .

risk:LowRisk a rdfs:Class,
        skos:Concept,
        dpv:RiskLevel ;
    dct:contributor "Harshvardhan J. Pandit" ;
    dct:created "2022-08-18"^^xsd:date ;
    rdf:value "0.25,xsd:decimal" ;
    rdfs:isDefinedBy risk: ;
    sw:term_status "accepted"@en ;
    skos:broader risk:3RiskLevels,
        risk:5RiskLevels,
        risk:7RiskLevels ;
    skos:definition "Level where Risk is Low"@en ;
    skos:inScheme risk:risk-levels-classes ;
    skos:prefLabel "Low Risk"@en ;
    skos:scopeNote "The suggested quantitative value for this concept is 0.25 on a scale of 0 to 1"@en .

risk:LowSeverity a rdfs:Class,
        skos:Concept,
        dpv:Severity ;
    dct:contributor "Harshvardhan J. Pandit" ;
    dct:created "2022-08-18"^^xsd:date ;
    rdf:value "0.25,xsd:decimal" ;
    rdfs:isDefinedBy risk: ;
    sw:term_status "accepted"@en ;
    skos:broader risk:3SeverityLevels,
        risk:5SeverityLevels,
        risk:7SeverityLevels ;
    skos:definition "Level where Severity is Low"@en ;
    skos:inScheme risk:risk-levels-classes ;
    skos:prefLabel "Low Severity"@en ;
    skos:scopeNote "The suggested quantitative value for this concept is 0.25 on a scale of 0 to 1"@en .

risk:MAGERIT a rdfs:Class,
        skos:Concept,
        risk:RiskManagement ;
    dct:contributor "Harshvardhan J. Pandit" ;
    dct:created "2022-08-18"^^xsd:date ;
    dct:source "(ENISA Risk Management Standards,https://www.enisa.europa.eu/publications/risk-management-standards)"@en ;
    rdfs:isDefinedBy risk: ;
    sw:term_status "accepted"@en ;
    skos:broader risk:RiskManagement ;
    skos:definition "Method for the Harmonised Analysis of Risk (MAGERIT) is an open methodology for risk analysis and management developed by the Spanish Higher Council for Electronic Government and offered as a framework and guide to the public administration"@en ;
    skos:inScheme risk:risk-methodology-classes ;
    skos:prefLabel "MAGERIT"@en .

risk:MCA a rdfs:Class,
        skos:Concept,
        risk:RiskAnalysis ;
    dct:contributor "Harshvardhan J. Pandit" ;
    dct:created "2022-08-18"^^xsd:date ;
    dct:source "(IEC 31010:2019,https://www.iso.org/standard/72140.html)"@en ;
    rdfs:isDefinedBy risk: ;
    sw:term_status "accepted"@en ;
    skos:broader risk:QualitativeRiskAnalysis ;
    skos:definition "Compares options in a way that makes trade-offs explicit. Provides an alternative to cost/benefit analysis that does not need a monetary value to be allocated to all inputs."@en ;
    skos:inScheme risk:risk-assessment-classes ;
    skos:prefLabel "Multi-criteria Analysis (MCA)"@en .

risk:MEHARI a rdfs:Class,
        skos:Concept,
        risk:RiskManagement ;
    dct:contributor "Harshvardhan J. Pandit" ;
    dct:created "2022-08-18"^^xsd:date ;
    dct:source "(ENISA Risk Management Standards,https://www.enisa.europa.eu/publications/risk-management-standards)"@en ;
    rdfs:isDefinedBy risk: ;
    sw:term_status "accepted"@en ;
    skos:broader risk:RiskManagement ;
    skos:definition "MEHARI is a free of charge qualitative risk analysis and management method developed by CLUSIF (Club for the Security of Information in France/Club de la Sécurité de l'Information Français)"@en ;
    skos:inScheme risk:risk-methodology-classes ;
    skos:prefLabel "MEHARI"@en .

risk:MONARC a rdfs:Class,
        skos:Concept,
        risk:RiskManagement ;
    dct:contributor "Harshvardhan J. Pandit" ;
    dct:created "2022-08-18"^^xsd:date ;
    dct:source "(ENISA Compendium of Risk Management Frameworks with Potential Interoperability,https://www.enisa.europa.eu/publications/compendium-of-risk-management-frameworks)"@en ;
    rdfs:isDefinedBy risk: ;
    sw:term_status "accepted"@en ;
    skos:broader risk:RiskManagement ;
    skos:definition "MONARC (Méthode Optimisée d’analyse des risques CASES – ‘Method for an Optimised Analysis of Risks by CASES’ is a tool and a method allowing precise and repeatable risk assessments to take place"@en ;
    skos:inScheme risk:risk-methodology-classes ;
    skos:prefLabel "MONARC"@en .

risk:MaliciousCodeAttack a rdfs:Class,
        skos:Concept,
        dpv:Consequence ;
    dct:contributor "Harshvardhan J. Pandit" ;
    dct:created "2022-08-17"^^xsd:date ;
    dct:source "(ENISA Reference Incident Classification Taxonomy 2018,https://www.enisa.europa.eu/publications/reference-incident-classification-taxonomy/)"@en ;
    rdfs:isDefinedBy risk: ;
    sw:term_status "accepted"@en ;
    skos:broader dpv:Detriment ;
    skos:definition "Intentional use of software by including or inserting in a system for a harmful purpose"@en ;
    skos:inScheme risk:risk-consequences-classes ;
    skos:prefLabel "Malicious Code Attack"@en .

risk:MalwareAttack a rdfs:Class,
        skos:Concept,
        dpv:Consequence ;
    dct:contributor "Harshvardhan J. Pandit" ;
    dct:created "2022-08-17"^^xsd:date ;
    dct:source "(ENISA Methodology for Sectoral Cybersecurity Assessments,https://www.enisa.europa.eu/publications/methodology-for-a-sectoral-cybersecurity-assessment)"@en ;
    rdfs:isDefinedBy risk: ;
    sw:term_status "accepted"@en ;
    skos:broader dpv:Detriment ;
    skos:definition "Malware is software or firmware intended to perform an unauthorised process that will have an adverse impact on the confidentiality, integrity, or availability of a system"@en ;
    skos:inScheme risk:risk-consequences-classes ;
    skos:prefLabel "Malware Attack"@en .

risk:MarkovAnalysis a rdfs:Class,
        skos:Concept,
        risk:RiskAnalysis ;
    dct:contributor "Harshvardhan J. Pandit" ;
    dct:created "2022-08-18"^^xsd:date ;
    dct:source "(IEC 31010:2019,https://www.iso.org/standard/72140.html)"@en ;
    rdfs:isDefinedBy risk: ;
    sw:term_status "accepted"@en ;
    skos:broader risk:QuantitativeRiskAnalysis ;
    skos:definition "Calculates the probability that a system that has the capacity to be in one of a number of states will be in a particular state at a time t in the future."@en ;
    skos:inScheme risk:risk-assessment-classes ;
    skos:prefLabel "Markov Analysis"@en .

risk:MisinformationDisinformation a rdfs:Class,
        skos:Concept,
        dpv:Consequence ;
    dct:contributor "Harshvardhan J. Pandit" ;
    dct:created "2022-08-17"^^xsd:date ;
    dct:source "(ENISA Threat Landscape 2021,https://www.enisa.europa.eu/publications/enisa-threat-landscape-2021)"@en ;
    rdfs:isDefinedBy risk: ;
    sw:term_status "accepted"@en ;
    skos:broader dpv:Detriment ;
    skos:definition "Information that is untrue, misleading, or false and used intentionally (disinformation) or unintentionally (misinformation)"@en ;
    skos:inScheme risk:risk-consequences-classes ;
    skos:prefLabel "MisinformationDisinformation"@en .

risk:MisuseBreachedInformation a rdfs:Class,
        skos:Concept,
        dpv:Consequence ;
    dct:contributor "Harshvardhan J. Pandit" ;
    dct:created "2022-08-17"^^xsd:date ;
    dct:source "(ISO/IEC 27005:2018,https://www.iso.org/standard/75281.html)"@en ;
    rdfs:isDefinedBy risk: ;
    sw:term_status "accepted"@en ;
    skos:broader dpv:Detriment ;
    skos:inScheme risk:risk-consequences-classes ;
    skos:prefLabel "Misuse of Breached Information"@en .

risk:ModerateLikelihood a rdfs:Class,
        skos:Concept,
        dpv:Likelihood ;
    dct:contributor "Harshvardhan J. Pandit" ;
    dct:created "2022-08-18"^^xsd:date ;
    rdf:value "0.5,xsd:decimal" ;
    rdfs:isDefinedBy risk: ;
    sw:term_status "accepted"@en ;
    skos:broader risk:3LikelihoodLevels,
        risk:5LikelihoodLevels,
        risk:7LikelihoodLevels ;
    skos:definition "Level where Likelihood is Moderate"@en ;
    skos:inScheme risk:risk-levels-classes ;
    skos:prefLabel "Moderate Likelihood"@en ;
    skos:scopeNote "The suggested quantitative value for this concept is 0.5 on a scale of 0 to 1"@en .

risk:ModerateRisk a rdfs:Class,
        skos:Concept,
        dpv:RiskLevel ;
    dct:contributor "Harshvardhan J. Pandit" ;
    dct:created "2022-08-18"^^xsd:date ;
    rdf:value "0.5,xsd:decimal" ;
    rdfs:isDefinedBy risk: ;
    sw:term_status "accepted"@en ;
    skos:broader risk:3RiskLevels,
        risk:5RiskLevels,
        risk:7RiskLevels ;
    skos:definition "Level where Risk is Moderate"@en ;
    skos:inScheme risk:risk-levels-classes ;
    skos:prefLabel "Moderate Risk"@en ;
    skos:scopeNote "The suggested quantitative value for this concept is 0.5 on a scale of 0 to 1"@en .

risk:ModerateSeverity a rdfs:Class,
        skos:Concept,
        dpv:Severity ;
    dct:contributor "Harshvardhan J. Pandit" ;
    dct:created "2022-08-18"^^xsd:date ;
    rdf:value "0.5,xsd:decimal" ;
    rdfs:isDefinedBy risk: ;
    sw:term_status "accepted"@en ;
    skos:broader risk:3SeverityLevels,
        risk:5SeverityLevels,
        risk:7SeverityLevels ;
    skos:definition "Level where Severity is Moderate"@en ;
    skos:inScheme risk:risk-levels-classes ;
    skos:prefLabel "Moderate Severity"@en ;
    skos:scopeNote "The suggested quantitative value for this concept is 0.5 on a scale of 0 to 1"@en .

risk:MonitorConsequence a rdfs:Class,
        skos:Concept,
        dpv:RiskMitigationMeasure ;
    dct:contributor "Harshvardhan J. Pandit" ;
    dct:created "2022-09-03"^^xsd:date ;
    rdfs:isDefinedBy risk: ;
    sw:term_status "accepted"@en ;
    skos:broader risk:ControlMonitors ;
    skos:definition "Risk Control that monitors a Risk Consequence"@en ;
    skos:inScheme risk:risk-controls-classes ;
    skos:prefLabel "Monitor Consequence"@en .

risk:MonitorImpact a rdfs:Class,
        skos:Concept,
        dpv:RiskMitigationMeasure ;
    dct:contributor "Harshvardhan J. Pandit" ;
    dct:created "2022-09-04"^^xsd:date ;
    rdfs:isDefinedBy risk: ;
    sw:term_status "accepted"@en ;
    skos:broader risk:ControlMonitors ;
    skos:definition "Risk Control that monitors a Risk Impact"@en ;
    skos:inScheme risk:risk-controls-classes ;
    skos:prefLabel "Monitor Impact"@en .

risk:MonitorRisk a rdfs:Class,
        skos:Concept,
        dpv:RiskMitigationMeasure ;
    dct:contributor "Harshvardhan J. Pandit" ;
    dct:created "2022-08-31"^^xsd:date ;
    rdfs:isDefinedBy risk: ;
    sw:term_status "accepted"@en ;
    skos:broader risk:ControlMonitors ;
    skos:definition "Risk Control that monitors a Risk"@en ;
    skos:inScheme risk:risk-controls-classes ;
    skos:prefLabel "Monitor Risk"@en .

risk:MonitorRiskControl a rdfs:Class,
        skos:Concept,
        dpv:RiskMitigationMeasure ;
    dct:contributor "Harshvardhan J. Pandit" ;
    dct:created "2022-09-05"^^xsd:date ;
    rdfs:isDefinedBy risk: ;
    sw:term_status "accepted"@en ;
    skos:broader risk:ControlMonitors ;
    skos:definition "Risk Control that monitors another Risk Control"@en ;
    skos:inScheme risk:risk-controls-classes ;
    skos:prefLabel "Monitor Risk Control"@en .

risk:MonitorRiskSource a rdfs:Class,
        skos:Concept,
        dpv:RiskMitigationMeasure ;
    dct:contributor "Harshvardhan J. Pandit" ;
    dct:created "2022-09-01"^^xsd:date ;
    rdfs:isDefinedBy risk: ;
    sw:term_status "accepted"@en ;
    skos:broader risk:ControlMonitors ;
    skos:definition "Risk Control that monitors a Risk Source"@en ;
    skos:inScheme risk:risk-controls-classes ;
    skos:prefLabel "Monitor Risk Source"@en .

risk:MonitorVulnerabilities a rdfs:Class,
        skos:Concept,
        dpv:RiskMitigationMeasure ;
    dct:contributor "Harshvardhan J. Pandit" ;
    dct:created "2022-09-02"^^xsd:date ;
    rdfs:isDefinedBy risk: ;
    sw:term_status "accepted"@en ;
    skos:broader risk:ControlMonitors ;
    skos:definition "Risk Control that monitors a Risk Vulnerability"@en ;
    skos:inScheme risk:risk-controls-classes ;
    skos:prefLabel "Monitor Vulnerabilities"@en .

risk:MonteCarloSimulation a rdfs:Class,
        skos:Concept,
        risk:RiskAnalysis ;
    dct:contributor "Harshvardhan J. Pandit" ;
    dct:created "2022-08-18"^^xsd:date ;
    dct:source "(IEC 31010:2019,https://www.iso.org/standard/72140.html)"@en ;
    rdfs:isDefinedBy risk: ;
    sw:term_status "accepted"@en ;
    skos:broader risk:QuantitativeRiskAnalysis ;
    skos:definition "Calculates the probability of outcomes by running multiple simulations using random variables."@en ;
    skos:inScheme risk:risk-assessment-classes ;
    skos:prefLabel "Monte Carlo Simulation"@en .

risk:NIST-SP-800-30 a rdfs:Class,
        skos:Concept,
        risk:RiskManagement ;
    dct:contributor "Harshvardhan J. Pandit" ;
    dct:created "2022-08-18"^^xsd:date ;
    dct:source "(ENISA Risk Management Standards,https://www.enisa.europa.eu/publications/risk-management-standards)"@en ;
    rdfs:isDefinedBy risk: ;
    sw:term_status "accepted"@en ;
    skos:broader risk:RiskManagement ;
    skos:definition "NIST 800-30 is a free guide that provides a foundation for the development of an effective risk management programme, containing both the definitions and the practical guidance necessary for assessing and mitigating risks identified within IT systems"@en ;
    skos:inScheme risk:risk-methodology-classes ;
    skos:prefLabel "NIST SP 800-30"@en .

risk:NIST-SP-800-37 a rdfs:Class,
        skos:Concept,
        risk:RiskManagement ;
    dct:contributor "Harshvardhan J. Pandit" ;
    dct:created "2022-08-18"^^xsd:date ;
    dct:source "(ENISA Risk Management Standards,https://www.enisa.europa.eu/publications/risk-management-standards)"@en ;
    rdfs:isDefinedBy risk: ;
    sw:term_status "accepted"@en ;
    skos:broader risk:RiskManagement ;
    skos:definition "NIST SP 800-37 Rev. 2 is an asset-based RMF which comprises 7 steps, namely Prepare, Categorise, Select, Implement, Assess, Authorise and Monitor. It does not adopt a specific risk assessment methodology, although the NIST 800-30 guide is extensively referenced"@en ;
    skos:inScheme risk:risk-methodology-classes ;
    skos:prefLabel "NIST SP 800-37"@en .

risk:NIST-SP-800-39 a rdfs:Class,
        skos:Concept,
        risk:RiskManagement ;
    dct:contributor "Harshvardhan J. Pandit" ;
    dct:created "2022-08-18"^^xsd:date ;
    dct:source "(ENISA Risk Management Standards,https://www.enisa.europa.eu/publications/risk-management-standards)"@en ;
    rdfs:isDefinedBy risk: ;
    sw:term_status "accepted"@en ;
    skos:broader risk:RiskManagement ;
    skos:definition "The purpose of NIST SP 800-39 is to provide a structured, yet flexible approach for an integrated, enterprise-wide programme for managing the risk to information security of organisational operations (i.e. mission, functions, image, and reputation) and assets, individuals, other organisations etc. on an ongoing basis"@en ;
    skos:inScheme risk:risk-methodology-classes ;
    skos:prefLabel "NIST SP 800–39"@en .

risk:NIST-SP-800-82 a rdfs:Class,
        skos:Concept,
        risk:RiskManagement ;
    dct:contributor "Harshvardhan J. Pandit" ;
    dct:created "2022-08-18"^^xsd:date ;
    dct:source "(ENISA Compendium of Risk Management Frameworks with Potential Interoperability,https://www.enisa.europa.eu/publications/compendium-of-risk-management-frameworks)"@en ;
    rdfs:isDefinedBy risk: ;
    sw:term_status "accepted"@en ;
    skos:broader risk:RiskManagement ;
    skos:definition "NIST SP 800-82 Rev. 2 (Stouffer, et al., 2015), entitled ‘Guide to industrial control systems (ISC) security’, is an Industrial Control Systems Security Guide"@en ;
    skos:inScheme risk:risk-methodology-classes ;
    skos:prefLabel "NIST SP 800–82"@en .

risk:NominalGroupTechnique a rdfs:Class,
        skos:Concept,
        risk:RiskAnalysis ;
    dct:contributor "Harshvardhan J. Pandit" ;
    dct:created "2022-08-18"^^xsd:date ;
    dct:source "(IEC 31010:2019,https://www.iso.org/standard/72140.html)"@en ;
    rdfs:isDefinedBy risk: ;
    sw:term_status "accepted"@en ;
    skos:broader risk:QualitativeRiskAnalysis ;
    skos:definition "Technique for eliciting views from a group of people where initial participation is as individuals with no interaction, then group discussion of ideas follows."@en ;
    skos:inScheme risk:risk-assessment-classes ;
    skos:prefLabel "Nominal Group Technique"@en .

risk:O-RA a rdfs:Class,
        skos:Concept,
        risk:RiskManagement ;
    dct:contributor "Harshvardhan J. Pandit" ;
    dct:created "2022-08-18"^^xsd:date ;
    dct:source "(ENISA Compendium of Risk Management Frameworks with Potential Interoperability,https://www.enisa.europa.eu/publications/compendium-of-risk-management-frameworks)"@en ;
    rdfs:isDefinedBy risk: ;
    sw:term_status "accepted"@en ;
    skos:broader risk:RiskManagement ;
    skos:definition "The Open Group Standard for Risk Analysis (O-RA) provides a set of standards for various aspects of information security risk analysis that is based on the Open FAIR framework and can be applied to any risk scenario"@en ;
    skos:inScheme risk:risk-methodology-classes ;
    skos:prefLabel "O-RA"@en .

risk:OCTAVE a rdfs:Class,
        skos:Concept,
        risk:RiskManagement ;
    dct:contributor "Harshvardhan J. Pandit" ;
    dct:created "2022-08-18"^^xsd:date ;
    dct:source "(ENISA Risk Management Standards,https://www.enisa.europa.eu/publications/risk-management-standards)"@en ;
    rdfs:isDefinedBy risk: ;
    sw:term_status "accepted"@en ;
    skos:broader risk:RiskManagement ;
    skos:definition "Operationally Critical Threat, Asset, and Vulnerability Evaluation (OCTAVE) is a free of charge approach to evaluations of information security risk that is comprehensive, systematic, context-driven, and self-directed"@en ;
    skos:inScheme risk:risk-methodology-classes ;
    skos:prefLabel "OCTAVE"@en .

risk:OCTAVE-ALLEGRO a rdfs:Class,
        skos:Concept,
        risk:RiskManagement ;
    dct:contributor "Harshvardhan J. Pandit" ;
    dct:created "2022-08-18"^^xsd:date ;
    dct:source "(ENISA Compendium of Risk Management Frameworks with Potential Interoperability,https://www.enisa.europa.eu/publications/compendium-of-risk-management-frameworks)"@en ;
    rdfs:isDefinedBy risk: ;
    sw:term_status "accepted"@en ;
    skos:broader risk:RiskManagement ;
    skos:definition "OCTAVE Allegro is designed to allow broad assessment of an organisation’s operational risk environment, with the goal of producing robust results without the need for extensive knowledge of risk assessment"@en ;
    skos:inScheme risk:risk-methodology-classes ;
    skos:prefLabel "OCTAVE ALLEGRO"@en .

risk:OCTAVE-FORTE a rdfs:Class,
        skos:Concept,
        risk:RiskManagement ;
    dct:contributor "Harshvardhan J. Pandit" ;
    dct:created "2022-08-18"^^xsd:date ;
    dct:source "(ENISA Compendium of Risk Management Frameworks with Potential Interoperability,https://www.enisa.europa.eu/publications/compendium-of-risk-management-frameworks)"@en ;
    rdfs:isDefinedBy risk: ;
    sw:term_status "accepted"@en ;
    skos:broader risk:RiskManagement ;
    skos:definition "The OCTAVE FORTE process model was developed to support organisations in evaluating their security risks. It applies Enterprise Risk Management (ERM) principles to bridge the gap between executives and practitioners acting as decision makers"@en ;
    skos:inScheme risk:risk-methodology-classes ;
    skos:prefLabel "OCTAVE FORTE"@en .

risk:OCTAVE-S a rdfs:Class,
        skos:Concept,
        risk:RiskManagement ;
    dct:contributor "Harshvardhan J. Pandit" ;
    dct:created "2022-08-18"^^xsd:date ;
    dct:source "(ENISA Compendium of Risk Management Frameworks with Potential Interoperability,https://www.enisa.europa.eu/publications/compendium-of-risk-management-frameworks)"@en ;
    rdfs:isDefinedBy risk: ;
    sw:term_status "accepted"@en ;
    skos:broader risk:RiskManagement ;
    skos:definition "The OCTAVE-S is based on the OCTAVE approach and is a self-directed approach, meaning that people from an organisation assume responsibility for setting the organisation’s security strategy"@en ;
    skos:inScheme risk:risk-methodology-classes ;
    skos:prefLabel "OCTAVE-S"@en .

risk:OrganisationDisruption a rdfs:Class,
        skos:Concept,
        dpv:Consequence ;
    dct:contributor "Harshvardhan J. Pandit" ;
    dct:created "2022-08-17"^^xsd:date ;
    dct:source "(ISO/IEC 27005:2018,https://www.iso.org/standard/75281.html)"@en ;
    rdfs:isDefinedBy risk: ;
    sw:term_status "accepted"@en ;
    skos:broader dpv:Detriment ;
    skos:inScheme risk:risk-consequences-classes ;
    skos:prefLabel "Organisation Disruption"@en .

risk:PIA a rdfs:Class,
        skos:Concept,
        risk:RiskAnalysis ;
    dct:contributor "Harshvardhan J. Pandit" ;
    dct:created "2022-08-18"^^xsd:date ;
    dct:source "(IEC 31010:2019,https://www.iso.org/standard/72140.html)"@en ;
    rdfs:isDefinedBy risk: ;
    sw:term_status "accepted"@en ;
    skos:broader risk:QualitativeRiskAnalysis ;
    skos:definition "Analyses how incidents and events could affect a person's privacy and identifies and quantifies the capabilities that would be needed to manage it."@en ;
    skos:inScheme risk:risk-assessment-classes ;
    skos:prefLabel "Privacy Impact Analysis (PIA)"@en .

risk:ParetoCharts a rdfs:Class,
        skos:Concept,
        risk:RiskAnalysis ;
    dct:contributor "Harshvardhan J. Pandit" ;
    dct:created "2022-08-18"^^xsd:date ;
    dct:source "(IEC 31010:2019,https://www.iso.org/standard/72140.html)"@en ;
    rdfs:isDefinedBy risk: ;
    sw:term_status "accepted"@en ;
    skos:broader risk:QuantitativeRiskAnalysis ;
    skos:definition "The Pareto principle (the 80–20 rule) states that, for many events, roughly 80 % of the effects come from 20 % of the causes."@en ;
    skos:inScheme risk:risk-assessment-classes ;
    skos:prefLabel "Pareto Charts"@en .

risk:PersonalSafetyEndangerment a rdfs:Class,
        skos:Concept,
        dpv:Impact ;
    dct:contributor "Harshvardhan J. Pandit" ;
    dct:created "2022-08-17"^^xsd:date ;
    dct:source "(ISO/IEC 27005:2018,https://www.iso.org/standard/75281.html)"@en ;
    rdfs:isDefinedBy risk: ;
    sw:term_status "accepted"@en ;
    skos:broader dpv:Harm ;
    skos:inScheme risk:risk-consequences-classes ;
    skos:prefLabel "Personal Safety Endangerment"@en .

risk:PersonnelAbsence a rdfs:Class,
        skos:Concept,
        dpv:Impact ;
    dct:contributor "Harshvardhan J. Pandit" ;
    dct:created "2022-08-17"^^xsd:date ;
    dct:source "(ENISA Threat Taxonomy 2016,https://www.enisa.europa.eu/topics/threat-risk-management/threats-and-trends/enisa-threat-landscape/threat-taxonomy/view)"@en ;
    rdfs:isDefinedBy risk: ;
    sw:term_status "accepted"@en ;
    skos:broader dpv:NonMaterialDamage ;
    skos:inScheme risk:risk-consequences-classes ;
    skos:prefLabel "Personnel Absence"@en .

risk:PhishingScam a rdfs:Class,
        skos:Concept,
        dpv:Impact ;
    dct:contributor "Harshvardhan J. Pandit" ;
    dct:created "2022-08-17"^^xsd:date ;
    dct:source "(ENISA Threat Landscape for Ransomware Attacks 2022,https://www.enisa.europa.eu/publications/enisa-threat-landscape-for-ransomware-attacks)"@en ;
    rdfs:isDefinedBy risk: ;
    sw:term_status "accepted"@en ;
    skos:broader dpv:Harm ;
    skos:definition "A type of social engineering attack involving deceptive messages intended to reveal sensitive information"@en ;
    skos:inScheme risk:risk-consequences-classes ;
    skos:prefLabel "Phishing Scam"@en .

risk:PhysicalAssault a rdfs:Class,
        skos:Concept,
        dpv:Impact ;
    dct:contributor "Harshvardhan J. Pandit" ;
    dct:created "2022-08-17"^^xsd:date ;
    dct:source "(ISO/IEC 27005:2018,https://www.iso.org/standard/75281.html)"@en ;
    rdfs:isDefinedBy risk: ;
    sw:term_status "accepted"@en ;
    skos:broader dpv:Harm ;
    skos:inScheme risk:risk-consequences-classes ;
    skos:prefLabel "Physical Assault"@en .

risk:PhysicalSpying a rdfs:Class,
        skos:Concept,
        dpv:Impact ;
    dct:contributor "Harshvardhan J. Pandit" ;
    dct:created "2022-08-17"^^xsd:date ;
    dct:source "(ISO/IEC 27005:2018,https://www.iso.org/standard/75281.html)"@en ;
    rdfs:isDefinedBy risk: ;
    sw:term_status "accepted"@en ;
    skos:broader dpv:NonMaterialDamage ;
    skos:inScheme risk:risk-consequences-classes ;
    skos:prefLabel "Physical Spying"@en .

risk:PhysicalStalking a rdfs:Class,
        skos:Concept,
        dpv:Impact ;
    dct:contributor "Harshvardhan J. Pandit" ;
    dct:created "2022-08-17"^^xsd:date ;
    dct:source "(ISO/IEC 27005:2018,https://www.iso.org/standard/75281.html)"@en ;
    rdfs:isDefinedBy risk: ;
    sw:term_status "accepted"@en ;
    skos:broader dpv:NonMaterialDamage ;
    skos:inScheme risk:risk-consequences-classes ;
    skos:prefLabel "Physical Stalking"@en .

risk:PreventExercisingOfRights a rdfs:Class,
        skos:Concept,
        dpv:Impact ;
    dct:contributor "Georg P Krog, Harshvardhan J. Pandit" ;
    dct:created "2022-08-18"^^xsd:date ;
    rdfs:isDefinedBy risk: ;
    sw:term_status "accepted"@en ;
    skos:broader dpv:Harm ;
    skos:inScheme risk:risk-consequences-classes ;
    skos:prefLabel "Prevent Exercising of Rights"@en .

risk:PrivacyImpact a rdfs:Class,
        skos:Concept,
        dpv:Impact ;
    dct:contributor "Harshvardhan J. Pandit" ;
    dct:created "2022-08-17"^^xsd:date ;
    dct:source "(ENISA Methodology for Sectoral Cybersecurity Assessments,https://www.enisa.europa.eu/publications/methodology-for-a-sectoral-cybersecurity-assessment)"@en ;
    rdfs:isDefinedBy risk: ;
    sw:term_status "accepted"@en ;
    skos:broader dpv:Impact ;
    skos:inScheme risk:risk-consequences-classes ;
    skos:prefLabel "Privacy impact"@en .

risk:PsychologicalHarm a rdfs:Class,
        skos:Concept,
        dpv:Impact ;
    dct:contributor "Harshvardhan J. Pandit" ;
    dct:created "2022-08-17"^^xsd:date ;
    dct:source "(ENISA Reference Incident Classification Taxonomy 2018,https://www.enisa.europa.eu/publications/reference-incident-classification-taxonomy/)"@en ;
    rdfs:isDefinedBy risk: ;
    sw:term_status "accepted"@en ;
    skos:broader dpv:Harm ;
    skos:inScheme risk:risk-consequences-classes ;
    skos:prefLabel "Psychological Harm"@en .

risk:PublicOrderBreach a rdfs:Class,
        skos:Concept,
        dpv:Consequence ;
    dct:contributor "Harshvardhan J. Pandit" ;
    dct:created "2022-08-17"^^xsd:date ;
    dct:source "(ISO/IEC 27005:2018,https://www.iso.org/standard/75281.html)"@en ;
    rdfs:isDefinedBy risk: ;
    sw:term_status "accepted"@en ;
    skos:broader dpv:Damage ;
    skos:inScheme risk:risk-consequences-classes ;
    skos:prefLabel "Public Order Breach"@en .

risk:QualitativeRiskAnalysis a rdfs:Class,
        skos:Concept,
        risk:RiskAnalysis ;
    dct:contributor "Harshvardhan J. Pandit" ;
    dct:created "2022-08-18"^^xsd:date ;
    dct:source "(IEC 31010:2019,https://www.iso.org/standard/72140.html)"@en ;
    rdfs:isDefinedBy risk: ;
    sw:term_status "accepted"@en ;
    skos:broader risk:RiskAnalysis ;
    skos:definition "A risk analysis technique that uses qualitative methods"@en ;
    skos:inScheme risk:risk-assessment-classes ;
    skos:narrower risk:ALARA,
        risk:ALARP,
        risk:BowTie,
        risk:Brainstorming,
        risk:BusinessImpactAnalysis,
        risk:CausalMapping,
        risk:Checklists,
        risk:Cindynic,
        risk:Classifications,
        risk:DPIA,
        risk:DelphiTechnique,
        risk:EventTreeAnalysis,
        risk:FMEA,
        risk:FMECA,
        risk:FaultTreeAnalysis,
        risk:Fishbone,
        risk:HACCP,
        risk:HAZOP,
        risk:HumanReliabilityAnalysis,
        risk:Interviews,
        risk:LOPA,
        risk:MCA,
        risk:NominalGroupTechnique,
        risk:PIA,
        risk:ReliabilityCentredMaintenance,
        risk:RiskMatrix,
        risk:RiskRegisters,
        risk:SFAIRP,
        risk:SWIFT,
        risk:ScenarioAnalysis,
        risk:Surveys,
        risk:Taxonomies ;
    skos:prefLabel "Qualitative Risk Analysis"@en .

risk:QuantitativeRiskAnalysis a rdfs:Class,
        skos:Concept,
        risk:RiskAnalysis ;
    dct:contributor "Harshvardhan J. Pandit" ;
    dct:created "2022-08-18"^^xsd:date ;
    dct:source "(IEC 31010:2019,https://www.iso.org/standard/72140.html)"@en ;
    rdfs:isDefinedBy risk: ;
    sw:term_status "accepted"@en ;
    skos:broader risk:RiskAnalysis ;
    skos:definition "A risk analysis technique that uses quantitative methods"@en ;
    skos:inScheme risk:risk-assessment-classes ;
    skos:narrower risk:ALARA,
        risk:ALARP,
        risk:BayesianAnalysis,
        risk:BayesianNetworks,
        risk:BowTie,
        risk:BusinessImpactAnalysis,
        risk:CVaR,
        risk:CauseConsequenceAnalysis,
        risk:CostBenefitAnalysis,
        risk:CrossImpactAnalysis,
        risk:DecisionTreeAnalysis,
        risk:EventTreeAnalysis,
        risk:FMEA,
        risk:FMECA,
        risk:FNDiagrams,
        risk:FaultTreeAnalysis,
        risk:GameTheory,
        risk:HumanReliabilityAnalysis,
        risk:InfluenceDiagrams,
        risk:LOPA,
        risk:MarkovAnalysis,
        risk:MonteCarloSimulation,
        risk:ParetoCharts,
        risk:ReliabilityCentredMaintenance,
        risk:RiskIndices,
        risk:RiskMatrix,
        risk:SCurves,
        risk:SFAIRP,
        risk:Toxicological,
        risk:VaR ;
    skos:prefLabel "Quantitative Risk Analysis"@en .

risk:RM3x3S1L1 a rdfs:Class,
        skos:Concept,
        risk:RiskAnalysis ;
    dct:contributor "Harshvardhan J. Pandit" ;
    dct:created "2022-08-17"^^xsd:date ;
    rdf:value "0.11,xsd:decimal" ;
    rdfs:isDefinedBy risk: ;
    sw:term_status "accepted"@en ;
    skos:broader risk:RiskMatrix3x3 ;
    skos:definition "Node in a 3x3 Risk Matrix with Risk Severity: Low; Likelihood: Low; and Risk Level: Low"@en ;
    skos:inScheme risk:risk-matrix-classes ;
    skos:prefLabel "Low Risk (RM3x3 S:1 L:1)"@en .

risk:RM3x3S1L2 a rdfs:Class,
        skos:Concept,
        risk:RiskAnalysis ;
    dct:contributor "Harshvardhan J. Pandit" ;
    dct:created "2022-08-17"^^xsd:date ;
    rdf:value "0.22,xsd:decimal" ;
    rdfs:isDefinedBy risk: ;
    sw:term_status "accepted"@en ;
    skos:broader risk:RiskMatrix3x3 ;
    skos:definition "Node in a 3x3 Risk Matrix with Risk Severity: Low; Likelihood: Moderate; and Risk Level: Low"@en ;
    skos:inScheme risk:risk-matrix-classes ;
    skos:prefLabel "Low Risk (RM3x3 S:1 L:2)"@en .

risk:RM3x3S1L3 a rdfs:Class,
        skos:Concept,
        risk:RiskAnalysis ;
    dct:contributor "Harshvardhan J. Pandit" ;
    dct:created "2022-08-17"^^xsd:date ;
    rdf:value "0.33,xsd:decimal" ;
    rdfs:isDefinedBy risk: ;
    sw:term_status "accepted"@en ;
    skos:broader risk:RiskMatrix3x3 ;
    skos:definition "Node in a 3x3 Risk Matrix with Risk Severity: Low; Likelihood: High; and Risk Level: Moderate"@en ;
    skos:inScheme risk:risk-matrix-classes ;
    skos:prefLabel "Moderate Risk (RM3x3 S:1 L:3)"@en .

risk:RM3x3S2L1 a rdfs:Class,
        skos:Concept,
        risk:RiskAnalysis ;
    dct:contributor "Harshvardhan J. Pandit" ;
    dct:created "2022-08-17"^^xsd:date ;
    rdf:value "0.22,xsd:decimal" ;
    rdfs:isDefinedBy risk: ;
    sw:term_status "accepted"@en ;
    skos:broader risk:RiskMatrix3x3 ;
    skos:definition "Node in a 3x3 Risk Matrix with Risk Severity: Moderate; Likelihood: Low; and Risk Level: Low"@en ;
    skos:inScheme risk:risk-matrix-classes ;
    skos:prefLabel "Low Risk (RM3x3 S:2 L:1)"@en .

risk:RM3x3S2L2 a rdfs:Class,
        skos:Concept,
        risk:RiskAnalysis ;
    dct:contributor "Harshvardhan J. Pandit" ;
    dct:created "2022-08-17"^^xsd:date ;
    rdf:value "0.44,xsd:decimal" ;
    rdfs:isDefinedBy risk: ;
    sw:term_status "accepted"@en ;
    skos:broader risk:RiskMatrix3x3 ;
    skos:definition "Node in a 3x3 Risk Matrix with Risk Severity: Moderate; Likelihood: Moderate; and Risk Level: Moderate"@en ;
    skos:inScheme risk:risk-matrix-classes ;
    skos:prefLabel "Moderate Risk (RM3x3 S:2 L:2)"@en .

risk:RM3x3S2L3 a rdfs:Class,
        skos:Concept,
        risk:RiskAnalysis ;
    dct:contributor "Harshvardhan J. Pandit" ;
    dct:created "2022-08-17"^^xsd:date ;
    rdf:value "0.67,xsd:decimal" ;
    rdfs:isDefinedBy risk: ;
    sw:term_status "accepted"@en ;
    skos:broader risk:RiskMatrix3x3 ;
    skos:definition "Node in a 3x3 Risk Matrix with Risk Severity: Moderate; Likelihood: High; and Risk Level: High"@en ;
    skos:inScheme risk:risk-matrix-classes ;
    skos:prefLabel "High Risk (RM3x3 S:2 L:3)"@en .

risk:RM3x3S3L1 a rdfs:Class,
        skos:Concept,
        risk:RiskAnalysis ;
    dct:contributor "Harshvardhan J. Pandit" ;
    dct:created "2022-08-17"^^xsd:date ;
    rdf:value "0.33,xsd:decimal" ;
    rdfs:isDefinedBy risk: ;
    sw:term_status "accepted"@en ;
    skos:broader risk:RiskMatrix3x3 ;
    skos:definition "Node in a 3x3 Risk Matrix with Risk Severity: High; Likelihood: Low; and Risk Level: Moderate"@en ;
    skos:inScheme risk:risk-matrix-classes ;
    skos:prefLabel "Moderate Risk (RM3x3 S:3 L:1)"@en .

risk:RM3x3S3L2 a rdfs:Class,
        skos:Concept,
        risk:RiskAnalysis ;
    dct:contributor "Harshvardhan J. Pandit" ;
    dct:created "2022-08-17"^^xsd:date ;
    rdf:value "0.67,xsd:decimal" ;
    rdfs:isDefinedBy risk: ;
    sw:term_status "accepted"@en ;
    skos:broader risk:RiskMatrix3x3 ;
    skos:definition "Node in a 3x3 Risk Matrix with Risk Severity: High; Likelihood: Moderate; and Risk Level: High"@en ;
    skos:inScheme risk:risk-matrix-classes ;
    skos:prefLabel "High Risk (RM3x3 S:3 L:2)"@en .

risk:RM3x3S3L3 a rdfs:Class,
        skos:Concept,
        risk:RiskAnalysis ;
    dct:contributor "Harshvardhan J. Pandit" ;
    dct:created "2022-08-17"^^xsd:date ;
    rdf:value "1.00,xsd:decimal" ;
    rdfs:isDefinedBy risk: ;
    sw:term_status "accepted"@en ;
    skos:broader risk:RiskMatrix3x3 ;
    skos:definition "Node in a 3x3 Risk Matrix with Risk Severity: High; Likelihood: High; and Risk Level: High"@en ;
    skos:inScheme risk:risk-matrix-classes ;
    skos:prefLabel "High Risk (RM3x3 S:3 L:3)"@en .

risk:RM5x5S1L1 a rdfs:Class,
        skos:Concept,
        risk:RiskAnalysis ;
    dct:contributor "Harshvardhan J. Pandit" ;
    dct:created "2022-08-17"^^xsd:date ;
    rdf:value "0.04,xsd:decimal" ;
    rdfs:isDefinedBy risk: ;
    sw:term_status "accepted"@en ;
    skos:broader risk:RiskMatrix5x5 ;
    skos:definition "Node in a 5x5 Risk Matrix with Risk Severity: VeryLow; Likelihood: VeryLow; and Risk Level: VeryLow"@en ;
    skos:inScheme risk:risk-matrix-classes ;
    skos:prefLabel "Very Low Risk (RM5x5 S:1 L:1)"@en .

risk:RM5x5S1L2 a rdfs:Class,
        skos:Concept,
        risk:RiskAnalysis ;
    dct:contributor "Harshvardhan J. Pandit" ;
    dct:created "2022-08-17"^^xsd:date ;
    rdf:value "0.08,xsd:decimal" ;
    rdfs:isDefinedBy risk: ;
    sw:term_status "accepted"@en ;
    skos:broader risk:RiskMatrix5x5 ;
    skos:definition "Node in a 5x5 Risk Matrix with Risk Severity: VeryLow; Likelihood: Low; and Risk Level: VeryLow"@en ;
    skos:inScheme risk:risk-matrix-classes ;
    skos:prefLabel "Very Low Risk (RM5x5 S:1 L:2)"@en .

risk:RM5x5S1L3 a rdfs:Class,
        skos:Concept,
        risk:RiskAnalysis ;
    dct:contributor "Harshvardhan J. Pandit" ;
    dct:created "2022-08-17"^^xsd:date ;
    rdf:value "0.12,xsd:decimal" ;
    rdfs:isDefinedBy risk: ;
    sw:term_status "accepted"@en ;
    skos:broader risk:RiskMatrix5x5 ;
    skos:definition "Node in a 5x5 Risk Matrix with Risk Severity: VeryLow; Likelihood: Moderate; and Risk Level: VeryLow"@en ;
    skos:inScheme risk:risk-matrix-classes ;
    skos:prefLabel "Very Low Risk (RM5x5 S:1 L:3)"@en .

risk:RM5x5S1L4 a rdfs:Class,
        skos:Concept,
        risk:RiskAnalysis ;
    dct:contributor "Harshvardhan J. Pandit" ;
    dct:created "2022-08-17"^^xsd:date ;
    rdf:value "0.16,xsd:decimal" ;
    rdfs:isDefinedBy risk: ;
    sw:term_status "accepted"@en ;
    skos:broader risk:RiskMatrix5x5 ;
    skos:definition "Node in a 5x5 Risk Matrix with Risk Severity: VeryLow; Likelihood: High; and Risk Level: Low"@en ;
    skos:inScheme risk:risk-matrix-classes ;
    skos:prefLabel "Low Risk (RM5x5 S:1 L:4)"@en .

risk:RM5x5S1L5 a rdfs:Class,
        skos:Concept,
        risk:RiskAnalysis ;
    dct:contributor "Harshvardhan J. Pandit" ;
    dct:created "2022-08-17"^^xsd:date ;
    rdf:value "0.20,xsd:decimal" ;
    rdfs:isDefinedBy risk: ;
    sw:term_status "accepted"@en ;
    skos:broader risk:RiskMatrix5x5 ;
    skos:definition "Node in a 5x5 Risk Matrix with Risk Severity: VeryLow; Likelihood: VeryHigh; and Risk Level: Low"@en ;
    skos:inScheme risk:risk-matrix-classes ;
    skos:prefLabel "Low Risk (RM5x5 S:1 L:5)"@en .

risk:RM5x5S2L1 a rdfs:Class,
        skos:Concept,
        risk:RiskAnalysis ;
    dct:contributor "Harshvardhan J. Pandit" ;
    dct:created "2022-08-17"^^xsd:date ;
    rdf:value "0.08,xsd:decimal" ;
    rdfs:isDefinedBy risk: ;
    sw:term_status "accepted"@en ;
    skos:broader risk:RiskMatrix5x5 ;
    skos:definition "Node in a 5x5 Risk Matrix with Risk Severity: Low; Likelihood: VeryLow; and Risk Level: VeryLow"@en ;
    skos:inScheme risk:risk-matrix-classes ;
    skos:prefLabel "Very Low Risk (RM5x5 S:2 L:1)"@en .

risk:RM5x5S2L2 a rdfs:Class,
        skos:Concept,
        risk:RiskAnalysis ;
    dct:contributor "Harshvardhan J. Pandit" ;
    dct:created "2022-08-17"^^xsd:date ;
    rdf:value "0.16,xsd:decimal" ;
    rdfs:isDefinedBy risk: ;
    sw:term_status "accepted"@en ;
    skos:broader risk:RiskMatrix5x5 ;
    skos:definition "Node in a 5x5 Risk Matrix with Risk Severity: Low; Likelihood: Low; and Risk Level: Low"@en ;
    skos:inScheme risk:risk-matrix-classes ;
    skos:prefLabel "Low Risk (RM5x5 S:2 L:2)"@en .

risk:RM5x5S2L3 a rdfs:Class,
        skos:Concept,
        risk:RiskAnalysis ;
    dct:contributor "Harshvardhan J. Pandit" ;
    dct:created "2022-08-17"^^xsd:date ;
    rdf:value "0.24,xsd:decimal" ;
    rdfs:isDefinedBy risk: ;
    sw:term_status "accepted"@en ;
    skos:broader risk:RiskMatrix5x5 ;
    skos:definition "Node in a 5x5 Risk Matrix with Risk Severity: Low; Likelihood: Moderate; and Risk Level: Moderate"@en ;
    skos:inScheme risk:risk-matrix-classes ;
    skos:prefLabel "Moderate Risk (RM5x5 S:2 L:3)"@en .

risk:RM5x5S2L4 a rdfs:Class,
        skos:Concept,
        risk:RiskAnalysis ;
    dct:contributor "Harshvardhan J. Pandit" ;
    dct:created "2022-08-17"^^xsd:date ;
    rdf:value "0.32,xsd:decimal" ;
    rdfs:isDefinedBy risk: ;
    sw:term_status "accepted"@en ;
    skos:broader risk:RiskMatrix5x5 ;
    skos:definition "Node in a 5x5 Risk Matrix with Risk Severity: Low; Likelihood: High; and Risk Level: Moderate"@en ;
    skos:inScheme risk:risk-matrix-classes ;
    skos:prefLabel "Moderate Risk (RM5x5 S:2 L:4)"@en .

risk:RM5x5S2L5 a rdfs:Class,
        skos:Concept,
        risk:RiskAnalysis ;
    dct:contributor "Harshvardhan J. Pandit" ;
    dct:created "2022-08-17"^^xsd:date ;
    rdf:value "0.40,xsd:decimal" ;
    rdfs:isDefinedBy risk: ;
    sw:term_status "accepted"@en ;
    skos:broader risk:RiskMatrix5x5 ;
    skos:definition "Node in a 5x5 Risk Matrix with Risk Severity: Low; Likelihood: VeryHigh; and Risk Level: High"@en ;
    skos:inScheme risk:risk-matrix-classes ;
    skos:prefLabel "High Risk (RM5x5 S:2 L:5)"@en .

risk:RM5x5S3L1 a rdfs:Class,
        skos:Concept,
        risk:RiskAnalysis ;
    dct:contributor "Harshvardhan J. Pandit" ;
    dct:created "2022-08-17"^^xsd:date ;
    rdf:value "0.12,xsd:decimal" ;
    rdfs:isDefinedBy risk: ;
    sw:term_status "accepted"@en ;
    skos:broader risk:RiskMatrix5x5 ;
    skos:definition "Node in a 5x5 Risk Matrix with Risk Severity: Moderate; Likelihood: VeryLow; and Risk Level: VeryLow"@en ;
    skos:inScheme risk:risk-matrix-classes ;
    skos:prefLabel "Very Low Risk (RM5x5 S:3 L:1)"@en .

risk:RM5x5S3L2 a rdfs:Class,
        skos:Concept,
        risk:RiskAnalysis ;
    dct:contributor "Harshvardhan J. Pandit" ;
    dct:created "2022-08-17"^^xsd:date ;
    rdf:value "0.24,xsd:decimal" ;
    rdfs:isDefinedBy risk: ;
    sw:term_status "accepted"@en ;
    skos:broader risk:RiskMatrix5x5 ;
    skos:definition "Node in a 5x5 Risk Matrix with Risk Severity: Moderate; Likelihood: Low; and Risk Level: Moderate"@en ;
    skos:inScheme risk:risk-matrix-classes ;
    skos:prefLabel "Moderate Risk (RM5x5 S:3 L:2)"@en .

risk:RM5x5S3L3 a rdfs:Class,
        skos:Concept,
        risk:RiskAnalysis ;
    dct:contributor "Harshvardhan J. Pandit" ;
    dct:created "2022-08-17"^^xsd:date ;
    rdf:value "0.36,xsd:decimal" ;
    rdfs:isDefinedBy risk: ;
    sw:term_status "accepted"@en ;
    skos:broader risk:RiskMatrix5x5 ;
    skos:definition "Node in a 5x5 Risk Matrix with Risk Severity: Moderate; Likelihood: Moderate; and Risk Level: Moderate"@en ;
    skos:inScheme risk:risk-matrix-classes ;
    skos:prefLabel "Moderate Risk (RM5x5 S:3 L:3)"@en .

risk:RM5x5S3L4 a rdfs:Class,
        skos:Concept,
        risk:RiskAnalysis ;
    dct:contributor "Harshvardhan J. Pandit" ;
    dct:created "2022-08-17"^^xsd:date ;
    rdf:value "0.48,xsd:decimal" ;
    rdfs:isDefinedBy risk: ;
    sw:term_status "accepted"@en ;
    skos:broader risk:RiskMatrix5x5 ;
    skos:definition "Node in a 5x5 Risk Matrix with Risk Severity: Moderate; Likelihood: High; and Risk Level: High"@en ;
    skos:inScheme risk:risk-matrix-classes ;
    skos:prefLabel "High Risk (RM5x5 S:3 L:4)"@en .

risk:RM5x5S3L5 a rdfs:Class,
        skos:Concept,
        risk:RiskAnalysis ;
    dct:contributor "Harshvardhan J. Pandit" ;
    dct:created "2022-08-17"^^xsd:date ;
    rdf:value "0.60,xsd:decimal" ;
    rdfs:isDefinedBy risk: ;
    sw:term_status "accepted"@en ;
    skos:broader risk:RiskMatrix5x5 ;
    skos:definition "Node in a 5x5 Risk Matrix with Risk Severity: Moderate; Likelihood: VeryHigh; and Risk Level: VeryHigh"@en ;
    skos:inScheme risk:risk-matrix-classes ;
    skos:prefLabel "Very High Risk (RM5x5 S:3 L:5)"@en .

risk:RM5x5S4L1 a rdfs:Class,
        skos:Concept,
        risk:RiskAnalysis ;
    dct:contributor "Harshvardhan J. Pandit" ;
    dct:created "2022-08-17"^^xsd:date ;
    rdf:value "0.16,xsd:decimal" ;
    rdfs:isDefinedBy risk: ;
    sw:term_status "accepted"@en ;
    skos:broader risk:RiskMatrix5x5 ;
    skos:definition "Node in a 5x5 Risk Matrix with Risk Severity: High; Likelihood: VeryLow; and Risk Level: Low"@en ;
    skos:inScheme risk:risk-matrix-classes ;
    skos:prefLabel "Low Risk (RM5x5 S:4 L:1)"@en .

risk:RM5x5S4L2 a rdfs:Class,
        skos:Concept,
        risk:RiskAnalysis ;
    dct:contributor "Harshvardhan J. Pandit" ;
    dct:created "2022-08-17"^^xsd:date ;
    rdf:value "0.32,xsd:decimal" ;
    rdfs:isDefinedBy risk: ;
    sw:term_status "accepted"@en ;
    skos:broader risk:RiskMatrix5x5 ;
    skos:definition "Node in a 5x5 Risk Matrix with Risk Severity: High; Likelihood: Low; and Risk Level: Moderate"@en ;
    skos:inScheme risk:risk-matrix-classes ;
    skos:prefLabel "Moderate Risk (RM5x5 S:4 L:2)"@en .

risk:RM5x5S4L3 a rdfs:Class,
        skos:Concept,
        risk:RiskAnalysis ;
    dct:contributor "Harshvardhan J. Pandit" ;
    dct:created "2022-08-17"^^xsd:date ;
    rdf:value "0.48,xsd:decimal" ;
    rdfs:isDefinedBy risk: ;
    sw:term_status "accepted"@en ;
    skos:broader risk:RiskMatrix5x5 ;
    skos:definition "Node in a 5x5 Risk Matrix with Risk Severity: High; Likelihood: Moderate; and Risk Level: High"@en ;
    skos:inScheme risk:risk-matrix-classes ;
    skos:prefLabel "High Risk (RM5x5 S:4 L:3)"@en .

risk:RM5x5S4L4 a rdfs:Class,
        skos:Concept,
        risk:RiskAnalysis ;
    dct:contributor "Harshvardhan J. Pandit" ;
    dct:created "2022-08-17"^^xsd:date ;
    rdf:value "0.64,xsd:decimal" ;
    rdfs:isDefinedBy risk: ;
    sw:term_status "accepted"@en ;
    skos:broader risk:RiskMatrix5x5 ;
    skos:definition "Node in a 5x5 Risk Matrix with Risk Severity: High; Likelihood: High; and Risk Level: VeryHigh"@en ;
    skos:inScheme risk:risk-matrix-classes ;
    skos:prefLabel "Very High Risk (RM5x5 S:4 L:4)"@en .

risk:RM5x5S4L5 a rdfs:Class,
        skos:Concept,
        risk:RiskAnalysis ;
    dct:contributor "Harshvardhan J. Pandit" ;
    dct:created "2022-08-17"^^xsd:date ;
    rdf:value "0.80,xsd:decimal" ;
    rdfs:isDefinedBy risk: ;
    sw:term_status "accepted"@en ;
    skos:broader risk:RiskMatrix5x5 ;
    skos:definition "Node in a 5x5 Risk Matrix with Risk Severity: High; Likelihood: VeryHigh; and Risk Level: VeryHigh"@en ;
    skos:inScheme risk:risk-matrix-classes ;
    skos:prefLabel "Very High Risk (RM5x5 S:4 L:5)"@en .

risk:RM5x5S5L1 a rdfs:Class,
        skos:Concept,
        risk:RiskAnalysis ;
    dct:contributor "Harshvardhan J. Pandit" ;
    dct:created "2022-08-17"^^xsd:date ;
    rdf:value "0.20,xsd:decimal" ;
    rdfs:isDefinedBy risk: ;
    sw:term_status "accepted"@en ;
    skos:broader risk:RiskMatrix5x5 ;
    skos:definition "Node in a 5x5 Risk Matrix with Risk Severity: VeryHigh; Likelihood: VeryLow; and Risk Level: Low"@en ;
    skos:inScheme risk:risk-matrix-classes ;
    skos:prefLabel "Low Risk (RM5x5 S:5 L:1)"@en .

risk:RM5x5S5L2 a rdfs:Class,
        skos:Concept,
        risk:RiskAnalysis ;
    dct:contributor "Harshvardhan J. Pandit" ;
    dct:created "2022-08-17"^^xsd:date ;
    rdf:value "0.40,xsd:decimal" ;
    rdfs:isDefinedBy risk: ;
    sw:term_status "accepted"@en ;
    skos:broader risk:RiskMatrix5x5 ;
    skos:definition "Node in a 5x5 Risk Matrix with Risk Severity: VeryHigh; Likelihood: Low; and Risk Level: High"@en ;
    skos:inScheme risk:risk-matrix-classes ;
    skos:prefLabel "High Risk (RM5x5 S:5 L:2)"@en .

risk:RM5x5S5L3 a rdfs:Class,
        skos:Concept,
        risk:RiskAnalysis ;
    dct:contributor "Harshvardhan J. Pandit" ;
    dct:created "2022-08-17"^^xsd:date ;
    rdf:value "0.60,xsd:decimal" ;
    rdfs:isDefinedBy risk: ;
    sw:term_status "accepted"@en ;
    skos:broader risk:RiskMatrix5x5 ;
    skos:definition "Node in a 5x5 Risk Matrix with Risk Severity: VeryHigh; Likelihood: Moderate; and Risk Level: High"@en ;
    skos:inScheme risk:risk-matrix-classes ;
    skos:prefLabel "High Risk (RM5x5 S:5 L:3)"@en .

risk:RM5x5S5L4 a rdfs:Class,
        skos:Concept,
        risk:RiskAnalysis ;
    dct:contributor "Harshvardhan J. Pandit" ;
    dct:created "2022-08-17"^^xsd:date ;
    rdf:value "0.80,xsd:decimal" ;
    rdfs:isDefinedBy risk: ;
    sw:term_status "accepted"@en ;
    skos:broader risk:RiskMatrix5x5 ;
    skos:definition "Node in a 5x5 Risk Matrix with Risk Severity: VeryHigh; Likelihood: High; and Risk Level: VeryHigh"@en ;
    skos:inScheme risk:risk-matrix-classes ;
    skos:prefLabel "Very High Risk (RM5x5 S:5 L:4)"@en .

risk:RM5x5S5L5 a rdfs:Class,
        skos:Concept,
        risk:RiskAnalysis ;
    dct:contributor "Harshvardhan J. Pandit" ;
    dct:created "2022-08-17"^^xsd:date ;
    rdf:value "1.00,xsd:decimal" ;
    rdfs:isDefinedBy risk: ;
    sw:term_status "accepted"@en ;
    skos:broader risk:RiskMatrix5x5 ;
    skos:definition "Node in a 5x5 Risk Matrix with Risk Severity: VeryHigh; Likelihood: VeryHigh; and Risk Level: VeryHigh"@en ;
    skos:inScheme risk:risk-matrix-classes ;
    skos:prefLabel "Very High Risk (RM5x5 S:5 L:5)"@en .

risk:RM7x7S1L1 a rdfs:Class,
        skos:Concept,
        risk:RiskAnalysis ;
    dct:contributor "Harshvardhan J. Pandit" ;
    dct:created "2022-08-17"^^xsd:date ;
    rdf:value "0.02,xsd:decimal" ;
    rdfs:isDefinedBy risk: ;
    sw:term_status "accepted"@en ;
    skos:broader risk:RiskMatrix7x7 ;
    skos:definition "Node in a 7x7 Risk Matrix with Risk Severity: ExtremelyLow; Likelihood: ExtremelyLow; and Risk Level: ExtremelyLow"@en ;
    skos:inScheme risk:risk-matrix-classes ;
    skos:prefLabel "Extremely Low Risk (RM7x7 S:1 L:1)"@en .

risk:RM7x7S1L2 a rdfs:Class,
        skos:Concept,
        risk:RiskAnalysis ;
    dct:contributor "Harshvardhan J. Pandit" ;
    dct:created "2022-08-17"^^xsd:date ;
    rdf:value "0.04,xsd:decimal" ;
    rdfs:isDefinedBy risk: ;
    sw:term_status "accepted"@en ;
    skos:broader risk:RiskMatrix7x7 ;
    skos:definition "Node in a 7x7 Risk Matrix with Risk Severity: ExtremelyLow; Likelihood: VeryLow; and Risk Level: ExtremelyLow"@en ;
    skos:inScheme risk:risk-matrix-classes ;
    skos:prefLabel "Extremely Low Risk (RM7x7 S:1 L:2)"@en .

risk:RM7x7S1L3 a rdfs:Class,
        skos:Concept,
        risk:RiskAnalysis ;
    dct:contributor "Harshvardhan J. Pandit" ;
    dct:created "2022-08-17"^^xsd:date ;
    rdf:value "0.06,xsd:decimal" ;
    rdfs:isDefinedBy risk: ;
    sw:term_status "accepted"@en ;
    skos:broader risk:RiskMatrix7x7 ;
    skos:definition "Node in a 7x7 Risk Matrix with Risk Severity: ExtremelyLow; Likelihood: Low; and Risk Level: ExtremelyLow"@en ;
    skos:inScheme risk:risk-matrix-classes ;
    skos:prefLabel "Extremely Low Risk (RM7x7 S:1 L:3)"@en .

risk:RM7x7S1L4 a rdfs:Class,
        skos:Concept,
        risk:RiskAnalysis ;
    dct:contributor "Harshvardhan J. Pandit" ;
    dct:created "2022-08-17"^^xsd:date ;
    rdf:value "0.08,xsd:decimal" ;
    rdfs:isDefinedBy risk: ;
    sw:term_status "accepted"@en ;
    skos:broader risk:RiskMatrix7x7 ;
    skos:definition "Node in a 7x7 Risk Matrix with Risk Severity: ExtremelyLow; Likelihood: Moderate; and Risk Level: VeryLow"@en ;
    skos:inScheme risk:risk-matrix-classes ;
    skos:prefLabel "Very Low Risk (RM7x7 S:1 L:4)"@en .

risk:RM7x7S1L5 a rdfs:Class,
        skos:Concept,
        risk:RiskAnalysis ;
    dct:contributor "Harshvardhan J. Pandit" ;
    dct:created "2022-08-17"^^xsd:date ;
    rdf:value "0.10,xsd:decimal" ;
    rdfs:isDefinedBy risk: ;
    sw:term_status "accepted"@en ;
    skos:broader risk:RiskMatrix7x7 ;
    skos:definition "Node in a 7x7 Risk Matrix with Risk Severity: ExtremelyLow; Likelihood: High; and Risk Level: VeryLow"@en ;
    skos:inScheme risk:risk-matrix-classes ;
    skos:prefLabel "Very Low Risk (RM7x7 S:1 L:5)"@en .

risk:RM7x7S1L6 a rdfs:Class,
        skos:Concept,
        risk:RiskAnalysis ;
    dct:contributor "Harshvardhan J. Pandit" ;
    dct:created "2022-08-17"^^xsd:date ;
    rdf:value "0.12,xsd:decimal" ;
    rdfs:isDefinedBy risk: ;
    sw:term_status "accepted"@en ;
    skos:broader risk:RiskMatrix7x7 ;
    skos:definition "Node in a 7x7 Risk Matrix with Risk Severity: ExtremelyLow; Likelihood: VeryHigh; and Risk Level: VeryLow"@en ;
    skos:inScheme risk:risk-matrix-classes ;
    skos:prefLabel "Very Low Risk (RM7x7 S:1 L:6)"@en .

risk:RM7x7S1L7 a rdfs:Class,
        skos:Concept,
        risk:RiskAnalysis ;
    dct:contributor "Harshvardhan J. Pandit" ;
    dct:created "2022-08-17"^^xsd:date ;
    rdf:value "0.14,xsd:decimal" ;
    rdfs:isDefinedBy risk: ;
    sw:term_status "accepted"@en ;
    skos:broader risk:RiskMatrix7x7 ;
    skos:definition "Node in a 7x7 Risk Matrix with Risk Severity: ExtremelyLow; Likelihood: ExtremelyHigh; and Risk Level: Low"@en ;
    skos:inScheme risk:risk-matrix-classes ;
    skos:prefLabel "Low Risk (RM7x7 S:1 L:7)"@en .

risk:RM7x7S2L1 a rdfs:Class,
        skos:Concept,
        risk:RiskAnalysis ;
    dct:contributor "Harshvardhan J. Pandit" ;
    dct:created "2022-08-17"^^xsd:date ;
    rdf:value "0.04,xsd:decimal" ;
    rdfs:isDefinedBy risk: ;
    sw:term_status "accepted"@en ;
    skos:broader risk:RiskMatrix7x7 ;
    skos:definition "Node in a 7x7 Risk Matrix with Risk Severity: VeryLow; Likelihood: ExtremelyLow; and Risk Level: ExtremelyLow"@en ;
    skos:inScheme risk:risk-matrix-classes ;
    skos:prefLabel "Extremely Low Risk (RM7x7 S:2 L:1)"@en .

risk:RM7x7S2L2 a rdfs:Class,
        skos:Concept,
        risk:RiskAnalysis ;
    dct:contributor "Harshvardhan J. Pandit" ;
    dct:created "2022-08-17"^^xsd:date ;
    rdf:value "0.08,xsd:decimal" ;
    rdfs:isDefinedBy risk: ;
    sw:term_status "accepted"@en ;
    skos:broader risk:RiskMatrix7x7 ;
    skos:definition "Node in a 7x7 Risk Matrix with Risk Severity: VeryLow; Likelihood: VeryLow; and Risk Level: ExtremelyLow"@en ;
    skos:inScheme risk:risk-matrix-classes ;
    skos:prefLabel "Extremely Low Risk (RM7x7 S:2 L:2)"@en .

risk:RM7x7S2L3 a rdfs:Class,
        skos:Concept,
        risk:RiskAnalysis ;
    dct:contributor "Harshvardhan J. Pandit" ;
    dct:created "2022-08-17"^^xsd:date ;
    rdf:value "0.12,xsd:decimal" ;
    rdfs:isDefinedBy risk: ;
    sw:term_status "accepted"@en ;
    skos:broader risk:RiskMatrix7x7 ;
    skos:definition "Node in a 7x7 Risk Matrix with Risk Severity: VeryLow; Likelihood: Low; and Risk Level: VeryLow"@en ;
    skos:inScheme risk:risk-matrix-classes ;
    skos:prefLabel "Very Low Risk (RM7x7 S:2 L:3)"@en .

risk:RM7x7S2L4 a rdfs:Class,
        skos:Concept,
        risk:RiskAnalysis ;
    dct:contributor "Harshvardhan J. Pandit" ;
    dct:created "2022-08-17"^^xsd:date ;
    rdf:value "0.16,xsd:decimal" ;
    rdfs:isDefinedBy risk: ;
    sw:term_status "accepted"@en ;
    skos:broader risk:RiskMatrix7x7 ;
    skos:definition "Node in a 7x7 Risk Matrix with Risk Severity: VeryLow; Likelihood: Moderate; and Risk Level: Low"@en ;
    skos:inScheme risk:risk-matrix-classes ;
    skos:prefLabel "Low Risk (RM7x7 S:2 L:4)"@en .

risk:RM7x7S2L5 a rdfs:Class,
        skos:Concept,
        risk:RiskAnalysis ;
    dct:contributor "Harshvardhan J. Pandit" ;
    dct:created "2022-08-17"^^xsd:date ;
    rdf:value "0.20,xsd:decimal" ;
    rdfs:isDefinedBy risk: ;
    sw:term_status "accepted"@en ;
    skos:broader risk:RiskMatrix7x7 ;
    skos:definition "Node in a 7x7 Risk Matrix with Risk Severity: VeryLow; Likelihood: High; and Risk Level: Low"@en ;
    skos:inScheme risk:risk-matrix-classes ;
    skos:prefLabel "Low Risk (RM7x7 S:2 L:5)"@en .

risk:RM7x7S2L6 a rdfs:Class,
        skos:Concept,
        risk:RiskAnalysis ;
    dct:contributor "Harshvardhan J. Pandit" ;
    dct:created "2022-08-17"^^xsd:date ;
    rdf:value "0.24,xsd:decimal" ;
    rdfs:isDefinedBy risk: ;
    sw:term_status "accepted"@en ;
    skos:broader risk:RiskMatrix7x7 ;
    skos:definition "Node in a 7x7 Risk Matrix with Risk Severity: VeryLow; Likelihood: VeryHigh; and Risk Level: Moderate"@en ;
    skos:inScheme risk:risk-matrix-classes ;
    skos:prefLabel "Moderate Risk (RM7x7 S:2 L:6)"@en .

risk:RM7x7S2L7 a rdfs:Class,
        skos:Concept,
        risk:RiskAnalysis ;
    dct:contributor "Harshvardhan J. Pandit" ;
    dct:created "2022-08-17"^^xsd:date ;
    rdf:value "0.29,xsd:decimal" ;
    rdfs:isDefinedBy risk: ;
    sw:term_status "accepted"@en ;
    skos:broader risk:RiskMatrix7x7 ;
    skos:definition "Node in a 7x7 Risk Matrix with Risk Severity: VeryLow; Likelihood: ExtremelyHigh; and Risk Level: Moderate"@en ;
    skos:inScheme risk:risk-matrix-classes ;
    skos:prefLabel "Moderate Risk (RM7x7 S:2 L:7)"@en .

risk:RM7x7S3L1 a rdfs:Class,
        skos:Concept,
        risk:RiskAnalysis ;
    dct:contributor "Harshvardhan J. Pandit" ;
    dct:created "2022-08-17"^^xsd:date ;
    rdf:value "0.06,xsd:decimal" ;
    rdfs:isDefinedBy risk: ;
    sw:term_status "accepted"@en ;
    skos:broader risk:RiskMatrix7x7 ;
    skos:definition "Node in a 7x7 Risk Matrix with Risk Severity: Low; Likelihood: ExtremelyLow; and Risk Level: ExtremelyLow"@en ;
    skos:inScheme risk:risk-matrix-classes ;
    skos:prefLabel "Extremely Low Risk (RM7x7 S:3 L:1)"@en .

risk:RM7x7S3L2 a rdfs:Class,
        skos:Concept,
        risk:RiskAnalysis ;
    dct:contributor "Harshvardhan J. Pandit" ;
    dct:created "2022-08-17"^^xsd:date ;
    rdf:value "0.12,xsd:decimal" ;
    rdfs:isDefinedBy risk: ;
    sw:term_status "accepted"@en ;
    skos:broader risk:RiskMatrix7x7 ;
    skos:definition "Node in a 7x7 Risk Matrix with Risk Severity: Low; Likelihood: VeryLow; and Risk Level: VeryLow"@en ;
    skos:inScheme risk:risk-matrix-classes ;
    skos:prefLabel "Very Low Risk (RM7x7 S:3 L:2)"@en .

risk:RM7x7S3L3 a rdfs:Class,
        skos:Concept,
        risk:RiskAnalysis ;
    dct:contributor "Harshvardhan J. Pandit" ;
    dct:created "2022-08-17"^^xsd:date ;
    rdf:value "0.18,xsd:decimal" ;
    rdfs:isDefinedBy risk: ;
    sw:term_status "accepted"@en ;
    skos:broader risk:RiskMatrix7x7 ;
    skos:definition "Node in a 7x7 Risk Matrix with Risk Severity: Low; Likelihood: Low; and Risk Level: Low"@en ;
    skos:inScheme risk:risk-matrix-classes ;
    skos:prefLabel "Low Risk (RM7x7 S:3 L:3)"@en .

risk:RM7x7S3L4 a rdfs:Class,
        skos:Concept,
        risk:RiskAnalysis ;
    dct:contributor "Harshvardhan J. Pandit" ;
    dct:created "2022-08-17"^^xsd:date ;
    rdf:value "0.24,xsd:decimal" ;
    rdfs:isDefinedBy risk: ;
    sw:term_status "accepted"@en ;
    skos:broader risk:RiskMatrix7x7 ;
    skos:definition "Node in a 7x7 Risk Matrix with Risk Severity: Low; Likelihood: Moderate; and Risk Level: Moderate"@en ;
    skos:inScheme risk:risk-matrix-classes ;
    skos:prefLabel "Moderate Risk (RM7x7 S:3 L:4)"@en .

risk:RM7x7S3L5 a rdfs:Class,
        skos:Concept,
        risk:RiskAnalysis ;
    dct:contributor "Harshvardhan J. Pandit" ;
    dct:created "2022-08-17"^^xsd:date ;
    rdf:value "0.31,xsd:decimal" ;
    rdfs:isDefinedBy risk: ;
    sw:term_status "accepted"@en ;
    skos:broader risk:RiskMatrix7x7 ;
    skos:definition "Node in a 7x7 Risk Matrix with Risk Severity: Low; Likelihood: High; and Risk Level: High"@en ;
    skos:inScheme risk:risk-matrix-classes ;
    skos:prefLabel "High Risk (RM7x7 S:3 L:5)"@en .

risk:RM7x7S3L6 a rdfs:Class,
        skos:Concept,
        risk:RiskAnalysis ;
    dct:contributor "Harshvardhan J. Pandit" ;
    dct:created "2022-08-17"^^xsd:date ;
    rdf:value "0.37,xsd:decimal" ;
    rdfs:isDefinedBy risk: ;
    sw:term_status "accepted"@en ;
    skos:broader risk:RiskMatrix7x7 ;
    skos:definition "Node in a 7x7 Risk Matrix with Risk Severity: Low; Likelihood: VeryHigh; and Risk Level: High"@en ;
    skos:inScheme risk:risk-matrix-classes ;
    skos:prefLabel "High Risk (RM7x7 S:3 L:6)"@en .

risk:RM7x7S3L7 a rdfs:Class,
        skos:Concept,
        risk:RiskAnalysis ;
    dct:contributor "Harshvardhan J. Pandit" ;
    dct:created "2022-08-17"^^xsd:date ;
    rdf:value "0.43,xsd:decimal" ;
    rdfs:isDefinedBy risk: ;
    sw:term_status "accepted"@en ;
    skos:broader risk:RiskMatrix7x7 ;
    skos:definition "Node in a 7x7 Risk Matrix with Risk Severity: Low; Likelihood: ExtremelyHigh; and Risk Level: VeryHigh"@en ;
    skos:inScheme risk:risk-matrix-classes ;
    skos:prefLabel "Very High Risk (RM7x7 S:3 L:7)"@en .

risk:RM7x7S4L1 a rdfs:Class,
        skos:Concept,
        risk:RiskAnalysis ;
    dct:contributor "Harshvardhan J. Pandit" ;
    dct:created "2022-08-17"^^xsd:date ;
    rdf:value "0.08,xsd:decimal" ;
    rdfs:isDefinedBy risk: ;
    sw:term_status "accepted"@en ;
    skos:broader risk:RiskMatrix7x7 ;
    skos:definition "Node in a 7x7 Risk Matrix with Risk Severity: Moderate; Likelihood: ExtremelyLow; and Risk Level: ExtremelyLow"@en ;
    skos:inScheme risk:risk-matrix-classes ;
    skos:prefLabel "Extremely Low Risk (RM7x7 S:4 L:1)"@en .

risk:RM7x7S4L2 a rdfs:Class,
        skos:Concept,
        risk:RiskAnalysis ;
    dct:contributor "Harshvardhan J. Pandit" ;
    dct:created "2022-08-17"^^xsd:date ;
    rdf:value "0.16,xsd:decimal" ;
    rdfs:isDefinedBy risk: ;
    sw:term_status "accepted"@en ;
    skos:broader risk:RiskMatrix7x7 ;
    skos:definition "Node in a 7x7 Risk Matrix with Risk Severity: Moderate; Likelihood: VeryLow; and Risk Level: Low"@en ;
    skos:inScheme risk:risk-matrix-classes ;
    skos:prefLabel "Low Risk (RM7x7 S:4 L:2)"@en .

risk:RM7x7S4L3 a rdfs:Class,
        skos:Concept,
        risk:RiskAnalysis ;
    dct:contributor "Harshvardhan J. Pandit" ;
    dct:created "2022-08-17"^^xsd:date ;
    rdf:value "0.24,xsd:decimal" ;
    rdfs:isDefinedBy risk: ;
    sw:term_status "accepted"@en ;
    skos:broader risk:RiskMatrix7x7 ;
    skos:definition "Node in a 7x7 Risk Matrix with Risk Severity: Moderate; Likelihood: Low; and Risk Level: Moderate"@en ;
    skos:inScheme risk:risk-matrix-classes ;
    skos:prefLabel "Moderate Risk (RM7x7 S:4 L:3)"@en .

risk:RM7x7S4L4 a rdfs:Class,
        skos:Concept,
        risk:RiskAnalysis ;
    dct:contributor "Harshvardhan J. Pandit" ;
    dct:created "2022-08-17"^^xsd:date ;
    rdf:value "0.33,xsd:decimal" ;
    rdfs:isDefinedBy risk: ;
    sw:term_status "accepted"@en ;
    skos:broader risk:RiskMatrix7x7 ;
    skos:definition "Node in a 7x7 Risk Matrix with Risk Severity: Moderate; Likelihood: Moderate; and Risk Level: High"@en ;
    skos:inScheme risk:risk-matrix-classes ;
    skos:prefLabel "High Risk (RM7x7 S:4 L:4)"@en .

risk:RM7x7S4L5 a rdfs:Class,
        skos:Concept,
        risk:RiskAnalysis ;
    dct:contributor "Harshvardhan J. Pandit" ;
    dct:created "2022-08-17"^^xsd:date ;
    rdf:value "0.41,xsd:decimal" ;
    rdfs:isDefinedBy risk: ;
    sw:term_status "accepted"@en ;
    skos:broader risk:RiskMatrix7x7 ;
    skos:definition "Node in a 7x7 Risk Matrix with Risk Severity: Moderate; Likelihood: High; and Risk Level: High"@en ;
    skos:inScheme risk:risk-matrix-classes ;
    skos:prefLabel "High Risk (RM7x7 S:4 L:5)"@en .

risk:RM7x7S4L6 a rdfs:Class,
        skos:Concept,
        risk:RiskAnalysis ;
    dct:contributor "Harshvardhan J. Pandit" ;
    dct:created "2022-08-17"^^xsd:date ;
    rdf:value "0.49,xsd:decimal" ;
    rdfs:isDefinedBy risk: ;
    sw:term_status "accepted"@en ;
    skos:broader risk:RiskMatrix7x7 ;
    skos:definition "Node in a 7x7 Risk Matrix with Risk Severity: Moderate; Likelihood: VeryHigh; and Risk Level: VeryHigh"@en ;
    skos:inScheme risk:risk-matrix-classes ;
    skos:prefLabel "Very High Risk (RM7x7 S:4 L:6)"@en .

risk:RM7x7S4L7 a rdfs:Class,
        skos:Concept,
        risk:RiskAnalysis ;
    dct:contributor "Harshvardhan J. Pandit" ;
    dct:created "2022-08-17"^^xsd:date ;
    rdf:value "0.57,xsd:decimal" ;
    rdfs:isDefinedBy risk: ;
    sw:term_status "accepted"@en ;
    skos:broader risk:RiskMatrix7x7 ;
    skos:definition "Node in a 7x7 Risk Matrix with Risk Severity: Moderate; Likelihood: ExtremelyHigh; and Risk Level: VeryHigh"@en ;
    skos:inScheme risk:risk-matrix-classes ;
    skos:prefLabel "Very High Risk (RM7x7 S:4 L:7)"@en .

risk:RM7x7S5L1 a rdfs:Class,
        skos:Concept,
        risk:RiskAnalysis ;
    dct:contributor "Harshvardhan J. Pandit" ;
    dct:created "2022-08-17"^^xsd:date ;
    rdf:value "0.10,xsd:decimal" ;
    rdfs:isDefinedBy risk: ;
    sw:term_status "accepted"@en ;
    skos:broader risk:RiskMatrix7x7 ;
    skos:definition "Node in a 7x7 Risk Matrix with Risk Severity: High; Likelihood: ExtremelyLow; and Risk Level: VeryLow"@en ;
    skos:inScheme risk:risk-matrix-classes ;
    skos:prefLabel "Very Low Risk (RM7x7 S:5 L:1)"@en .

risk:RM7x7S5L2 a rdfs:Class,
        skos:Concept,
        risk:RiskAnalysis ;
    dct:contributor "Harshvardhan J. Pandit" ;
    dct:created "2022-08-17"^^xsd:date ;
    rdf:value "0.20,xsd:decimal" ;
    rdfs:isDefinedBy risk: ;
    sw:term_status "accepted"@en ;
    skos:broader risk:RiskMatrix7x7 ;
    skos:definition "Node in a 7x7 Risk Matrix with Risk Severity: High; Likelihood: VeryLow; and Risk Level: Low"@en ;
    skos:inScheme risk:risk-matrix-classes ;
    skos:prefLabel "Low Risk (RM7x7 S:5 L:2)"@en .

risk:RM7x7S5L3 a rdfs:Class,
        skos:Concept,
        risk:RiskAnalysis ;
    dct:contributor "Harshvardhan J. Pandit" ;
    dct:created "2022-08-17"^^xsd:date ;
    rdf:value "0.31,xsd:decimal" ;
    rdfs:isDefinedBy risk: ;
    sw:term_status "accepted"@en ;
    skos:broader risk:RiskMatrix7x7 ;
    skos:definition "Node in a 7x7 Risk Matrix with Risk Severity: High; Likelihood: Low; and Risk Level: Moderate"@en ;
    skos:inScheme risk:risk-matrix-classes ;
    skos:prefLabel "Moderate Risk (RM7x7 S:5 L:3)"@en .

risk:RM7x7S5L4 a rdfs:Class,
        skos:Concept,
        risk:RiskAnalysis ;
    dct:contributor "Harshvardhan J. Pandit" ;
    dct:created "2022-08-17"^^xsd:date ;
    rdf:value "0.41,xsd:decimal" ;
    rdfs:isDefinedBy risk: ;
    sw:term_status "accepted"@en ;
    skos:broader risk:RiskMatrix7x7 ;
    skos:definition "Node in a 7x7 Risk Matrix with Risk Severity: High; Likelihood: Moderate; and Risk Level: High"@en ;
    skos:inScheme risk:risk-matrix-classes ;
    skos:prefLabel "High Risk (RM7x7 S:5 L:4)"@en .

risk:RM7x7S5L5 a rdfs:Class,
        skos:Concept,
        risk:RiskAnalysis ;
    dct:contributor "Harshvardhan J. Pandit" ;
    dct:created "2022-08-17"^^xsd:date ;
    rdf:value "0.51,xsd:decimal" ;
    rdfs:isDefinedBy risk: ;
    sw:term_status "accepted"@en ;
    skos:broader risk:RiskMatrix7x7 ;
    skos:definition "Node in a 7x7 Risk Matrix with Risk Severity: High; Likelihood: High; and Risk Level: VeryHigh"@en ;
    skos:inScheme risk:risk-matrix-classes ;
    skos:prefLabel "Very High Risk (RM7x7 S:5 L:5)"@en .

risk:RM7x7S5L6 a rdfs:Class,
        skos:Concept,
        risk:RiskAnalysis ;
    dct:contributor "Harshvardhan J. Pandit" ;
    dct:created "2022-08-17"^^xsd:date ;
    rdf:value "0.61,xsd:decimal" ;
    rdfs:isDefinedBy risk: ;
    sw:term_status "accepted"@en ;
    skos:broader risk:RiskMatrix7x7 ;
    skos:definition "Node in a 7x7 Risk Matrix with Risk Severity: High; Likelihood: VeryHigh; and Risk Level: ExtremelyHigh"@en ;
    skos:inScheme risk:risk-matrix-classes ;
    skos:prefLabel "Extremely High Risk (RM7x7 S:5 L:6)"@en .

risk:RM7x7S5L7 a rdfs:Class,
        skos:Concept,
        risk:RiskAnalysis ;
    dct:contributor "Harshvardhan J. Pandit" ;
    dct:created "2022-08-17"^^xsd:date ;
    rdf:value "0.71,xsd:decimal" ;
    rdfs:isDefinedBy risk: ;
    sw:term_status "accepted"@en ;
    skos:broader risk:RiskMatrix7x7 ;
    skos:definition "Node in a 7x7 Risk Matrix with Risk Severity: High; Likelihood: ExtremelyHigh; and Risk Level: ExtremelyHigh"@en ;
    skos:inScheme risk:risk-matrix-classes ;
    skos:prefLabel "Extremely High Risk (RM7x7 S:5 L:7)"@en .

risk:RM7x7S6L1 a rdfs:Class,
        skos:Concept,
        risk:RiskAnalysis ;
    dct:contributor "Harshvardhan J. Pandit" ;
    dct:created "2022-08-17"^^xsd:date ;
    rdf:value "0.12,xsd:decimal" ;
    rdfs:isDefinedBy risk: ;
    sw:term_status "accepted"@en ;
    skos:broader risk:RiskMatrix7x7 ;
    skos:definition "Node in a 7x7 Risk Matrix with Risk Severity: VeryHigh; Likelihood: ExtremelyLow; and Risk Level: VeryLow"@en ;
    skos:inScheme risk:risk-matrix-classes ;
    skos:prefLabel "Very Low Risk (RM7x7 S:6 L:1)"@en .

risk:RM7x7S6L2 a rdfs:Class,
        skos:Concept,
        risk:RiskAnalysis ;
    dct:contributor "Harshvardhan J. Pandit" ;
    dct:created "2022-08-17"^^xsd:date ;
    rdf:value "0.24,xsd:decimal" ;
    rdfs:isDefinedBy risk: ;
    sw:term_status "accepted"@en ;
    skos:broader risk:RiskMatrix7x7 ;
    skos:definition "Node in a 7x7 Risk Matrix with Risk Severity: VeryHigh; Likelihood: VeryLow; and Risk Level: Moderate"@en ;
    skos:inScheme risk:risk-matrix-classes ;
    skos:prefLabel "Moderate Risk (RM7x7 S:6 L:2)"@en .

risk:RM7x7S6L3 a rdfs:Class,
        skos:Concept,
        risk:RiskAnalysis ;
    dct:contributor "Harshvardhan J. Pandit" ;
    dct:created "2022-08-17"^^xsd:date ;
    rdf:value "0.37,xsd:decimal" ;
    rdfs:isDefinedBy risk: ;
    sw:term_status "accepted"@en ;
    skos:broader risk:RiskMatrix7x7 ;
    skos:definition "Node in a 7x7 Risk Matrix with Risk Severity: VeryHigh; Likelihood: Low; and Risk Level: High"@en ;
    skos:inScheme risk:risk-matrix-classes ;
    skos:prefLabel "High Risk (RM7x7 S:6 L:3)"@en .

risk:RM7x7S6L4 a rdfs:Class,
        skos:Concept,
        risk:RiskAnalysis ;
    dct:contributor "Harshvardhan J. Pandit" ;
    dct:created "2022-08-17"^^xsd:date ;
    rdf:value "0.49,xsd:decimal" ;
    rdfs:isDefinedBy risk: ;
    sw:term_status "accepted"@en ;
    skos:broader risk:RiskMatrix7x7 ;
    skos:definition "Node in a 7x7 Risk Matrix with Risk Severity: VeryHigh; Likelihood: Moderate; and Risk Level: VeryHigh"@en ;
    skos:inScheme risk:risk-matrix-classes ;
    skos:prefLabel "Very High Risk (RM7x7 S:6 L:4)"@en .

risk:RM7x7S6L5 a rdfs:Class,
        skos:Concept,
        risk:RiskAnalysis ;
    dct:contributor "Harshvardhan J. Pandit" ;
    dct:created "2022-08-17"^^xsd:date ;
    rdf:value "0.61,xsd:decimal" ;
    rdfs:isDefinedBy risk: ;
    sw:term_status "accepted"@en ;
    skos:broader risk:RiskMatrix7x7 ;
    skos:definition "Node in a 7x7 Risk Matrix with Risk Severity: VeryHigh; Likelihood: High; and Risk Level: VeryHigh"@en ;
    skos:inScheme risk:risk-matrix-classes ;
    skos:prefLabel "Very High Risk (RM7x7 S:6 L:5)"@en .

risk:RM7x7S6L6 a rdfs:Class,
        skos:Concept,
        risk:RiskAnalysis ;
    dct:contributor "Harshvardhan J. Pandit" ;
    dct:created "2022-08-17"^^xsd:date ;
    rdf:value "0.73,xsd:decimal" ;
    rdfs:isDefinedBy risk: ;
    sw:term_status "accepted"@en ;
    skos:broader risk:RiskMatrix7x7 ;
    skos:definition "Node in a 7x7 Risk Matrix with Risk Severity: VeryHigh; Likelihood: VeryHigh; and Risk Level: ExtremelyHigh"@en ;
    skos:inScheme risk:risk-matrix-classes ;
    skos:prefLabel "Extremely High Risk (RM7x7 S:6 L:6)"@en .

risk:RM7x7S6L7 a rdfs:Class,
        skos:Concept,
        risk:RiskAnalysis ;
    dct:contributor "Harshvardhan J. Pandit" ;
    dct:created "2022-08-17"^^xsd:date ;
    rdf:value "0.86,xsd:decimal" ;
    rdfs:isDefinedBy risk: ;
    sw:term_status "accepted"@en ;
    skos:broader risk:RiskMatrix7x7 ;
    skos:definition "Node in a 7x7 Risk Matrix with Risk Severity: VeryHigh; Likelihood: ExtremelyHigh; and Risk Level: ExtremelyHigh"@en ;
    skos:inScheme risk:risk-matrix-classes ;
    skos:prefLabel "Extremely High Risk (RM7x7 S:6 L:7)"@en .

risk:RM7x7S7L1 a rdfs:Class,
        skos:Concept,
        risk:RiskAnalysis ;
    dct:contributor "Harshvardhan J. Pandit" ;
    dct:created "2022-08-17"^^xsd:date ;
    rdf:value "0.14,xsd:decimal" ;
    rdfs:isDefinedBy risk: ;
    sw:term_status "accepted"@en ;
    skos:broader risk:RiskMatrix7x7 ;
    skos:definition "Node in a 7x7 Risk Matrix with Risk Severity: ExtremelyHigh; Likelihood: ExtremelyLow; and Risk Level: Low"@en ;
    skos:inScheme risk:risk-matrix-classes ;
    skos:prefLabel "Low Risk (RM7x7 S:7 L:1)"@en .

risk:RM7x7S7L2 a rdfs:Class,
        skos:Concept,
        risk:RiskAnalysis ;
    dct:contributor "Harshvardhan J. Pandit" ;
    dct:created "2022-08-17"^^xsd:date ;
    rdf:value "0.29,xsd:decimal" ;
    rdfs:isDefinedBy risk: ;
    sw:term_status "accepted"@en ;
    skos:broader risk:RiskMatrix7x7 ;
    skos:definition "Node in a 7x7 Risk Matrix with Risk Severity: ExtremelyHigh; Likelihood: VeryLow; and Risk Level: Moderate"@en ;
    skos:inScheme risk:risk-matrix-classes ;
    skos:prefLabel "Moderate Risk (RM7x7 S:7 L:2)"@en .

risk:RM7x7S7L3 a rdfs:Class,
        skos:Concept,
        risk:RiskAnalysis ;
    dct:contributor "Harshvardhan J. Pandit" ;
    dct:created "2022-08-17"^^xsd:date ;
    rdf:value "0.43,xsd:decimal" ;
    rdfs:isDefinedBy risk: ;
    sw:term_status "accepted"@en ;
    skos:broader risk:RiskMatrix7x7 ;
    skos:definition "Node in a 7x7 Risk Matrix with Risk Severity: ExtremelyHigh; Likelihood: Low; and Risk Level: High"@en ;
    skos:inScheme risk:risk-matrix-classes ;
    skos:prefLabel "High Risk (RM7x7 S:7 L:3)"@en .

risk:RM7x7S7L4 a rdfs:Class,
        skos:Concept,
        risk:RiskAnalysis ;
    dct:contributor "Harshvardhan J. Pandit" ;
    dct:created "2022-08-17"^^xsd:date ;
    rdf:value "0.57,xsd:decimal" ;
    rdfs:isDefinedBy risk: ;
    sw:term_status "accepted"@en ;
    skos:broader risk:RiskMatrix7x7 ;
    skos:definition "Node in a 7x7 Risk Matrix with Risk Severity: ExtremelyHigh; Likelihood: Moderate; and Risk Level: VeryHigh"@en ;
    skos:inScheme risk:risk-matrix-classes ;
    skos:prefLabel "Very High Risk (RM7x7 S:7 L:4)"@en .

risk:RM7x7S7L5 a rdfs:Class,
        skos:Concept,
        risk:RiskAnalysis ;
    dct:contributor "Harshvardhan J. Pandit" ;
    dct:created "2022-08-17"^^xsd:date ;
    rdf:value "0.71,xsd:decimal" ;
    rdfs:isDefinedBy risk: ;
    sw:term_status "accepted"@en ;
    skos:broader risk:RiskMatrix7x7 ;
    skos:definition "Node in a 7x7 Risk Matrix with Risk Severity: ExtremelyHigh; Likelihood: High; and Risk Level: ExtremelyHigh"@en ;
    skos:inScheme risk:risk-matrix-classes ;
    skos:prefLabel "Extremely High Risk (RM7x7 S:7 L:5)"@en .

risk:RM7x7S7L6 a rdfs:Class,
        skos:Concept,
        risk:RiskAnalysis ;
    dct:contributor "Harshvardhan J. Pandit" ;
    dct:created "2022-08-17"^^xsd:date ;
    rdf:value "0.86,xsd:decimal" ;
    rdfs:isDefinedBy risk: ;
    sw:term_status "accepted"@en ;
    skos:broader risk:RiskMatrix7x7 ;
    skos:definition "Node in a 7x7 Risk Matrix with Risk Severity: ExtremelyHigh; Likelihood: VeryHigh; and Risk Level: ExtremelyHigh"@en ;
    skos:inScheme risk:risk-matrix-classes ;
    skos:prefLabel "Extremely High Risk (RM7x7 S:7 L:6)"@en .

risk:RM7x7S7L7 a rdfs:Class,
        skos:Concept,
        risk:RiskAnalysis ;
    dct:contributor "Harshvardhan J. Pandit" ;
    dct:created "2022-08-17"^^xsd:date ;
    rdf:value "1.00,xsd:decimal" ;
    rdfs:isDefinedBy risk: ;
    sw:term_status "accepted"@en ;
    skos:broader risk:RiskMatrix7x7 ;
    skos:definition "Node in a 7x7 Risk Matrix with Risk Severity: ExtremelyHigh; Likelihood: ExtremelyHigh; and Risk Level: ExtremelyHigh"@en ;
    skos:inScheme risk:risk-matrix-classes ;
    skos:prefLabel "Extremely High Risk (RM7x7 S:7 L:7)"@en .

risk:RansomwareAttack a rdfs:Class,
        skos:Concept,
        dpv:Impact ;
    dct:contributor "Harshvardhan J. Pandit" ;
    dct:created "2022-08-17"^^xsd:date ;
    dct:source "(ISO/IEC 27005:2018,https://www.iso.org/standard/75281.html),(ENISA Threat Landscape for Ransomware Attacks 2022,https://www.enisa.europa.eu/publications/enisa-threat-landscape-for-ransomware-attacks)"@en ;
    rdfs:isDefinedBy risk: ;
    sw:term_status "accepted"@en ;
    skos:broader dpv:NonMaterialDamage ;
    skos:definition "Ransomware is a type of attack where threat actors take control of a target’s assets and demand a ransom in exchange for the return of the asset’s availability and confidentiality"@en ;
    skos:inScheme risk:risk-consequences-classes ;
    skos:prefLabel "RansomwareAttack"@en .

risk:ReduceLikelihood a rdfs:Class,
        skos:Concept,
        dpv:RiskMitigationMeasure ;
    dct:contributor "Harshvardhan J. Pandit" ;
    dct:created "2022-08-22"^^xsd:date ;
    rdfs:isDefinedBy risk: ;
    sw:term_status "accepted"@en ;
    skos:broader dpv:RiskMitigationMeasure ;
    skos:definition "Risk Control that reduces the likelihood of an event"@en ;
    skos:inScheme risk:risk-controls-classes ;
    skos:prefLabel "Reduce Likelihood"@en .

risk:ReduceSeverity a rdfs:Class,
        skos:Concept,
        dpv:RiskMitigationMeasure ;
    dct:contributor "Harshvardhan J. Pandit" ;
    dct:created "2022-08-23"^^xsd:date ;
    rdfs:isDefinedBy risk: ;
    sw:term_status "accepted"@en ;
    skos:broader dpv:RiskMitigationMeasure ;
    skos:definition "Risk Control that reduces the severity of an event"@en ;
    skos:inScheme risk:risk-controls-classes ;
    skos:prefLabel "Reduce Severity"@en .

risk:ReliabilityCentredMaintenance a rdfs:Class,
        skos:Concept,
        risk:RiskAnalysis ;
    dct:contributor "Harshvardhan J. Pandit" ;
    dct:created "2022-08-18"^^xsd:date ;
    dct:source "(IEC 31010:2019,https://www.iso.org/standard/72140.html)"@en ;
    rdfs:isDefinedBy risk: ;
    sw:term_status "accepted"@en ;
    skos:broader risk:QualitativeRiskAnalysis,
        risk:QuantitativeRiskAnalysis ;
    skos:definition "A risk based assessment used to identify the appropriate maintenance tasks for a system and its components."@en ;
    skos:inScheme risk:risk-assessment-classes ;
    skos:prefLabel "Reliability Centred Maintenance"@en .

risk:RemoteSpying a rdfs:Class,
        skos:Concept,
        dpv:Impact ;
    dct:contributor "Harshvardhan J. Pandit" ;
    dct:created "2022-08-17"^^xsd:date ;
    dct:source "(ISO/IEC 27005:2018,https://www.iso.org/standard/75281.html)"@en ;
    rdfs:isDefinedBy risk: ;
    sw:term_status "accepted"@en ;
    skos:broader dpv:NonMaterialDamage ;
    skos:inScheme risk:risk-consequences-classes ;
    skos:prefLabel "Remote Spying"@en .

risk:RemoveConsequence a rdfs:Class,
        skos:Concept,
        dpv:RiskMitigationMeasure ;
    dct:contributor "Harshvardhan J. Pandit" ;
    dct:created "2022-08-27"^^xsd:date ;
    rdfs:isDefinedBy risk: ;
    sw:term_status "accepted"@en ;
    skos:broader risk:ControlConsequence ;
    skos:definition "Risk Control that removes Consequence i.e. prevents it from materialising"@en ;
    skos:inScheme risk:risk-controls-classes ;
    skos:prefLabel "Remove Consequence"@en .

risk:RemoveImpact a rdfs:Class,
        skos:Concept,
        dpv:RiskMitigationMeasure ;
    dct:contributor "Harshvardhan J. Pandit" ;
    dct:created "2022-08-28"^^xsd:date ;
    dct:modified "2023-07-31"^^xsd:date ;
    rdfs:isDefinedBy risk: ;
    sw:term_status "accepted"@en ;
    skos:broader risk:ControlImpact ;
    skos:definition "Risk Control that removes Impact i.e. prevents it from materialising"@en ;
    skos:inScheme risk:risk-controls-classes ;
    skos:prefLabel "Remove Impact"@en .

risk:RemoveSource a rdfs:Class,
        skos:Concept,
        dpv:RiskMitigationMeasure ;
    dct:contributor "Harshvardhan J. Pandit" ;
    dct:created "2022-08-20"^^xsd:date ;
    rdfs:isDefinedBy risk: ;
    sw:term_status "accepted"@en ;
    skos:broader risk:ControlRiskSource ;
    skos:definition "Risk Control that removes the risk source"@en ;
    skos:inScheme risk:risk-controls-classes ;
    skos:prefLabel "Remove Source"@en .

risk:ReplacementCosts a rdfs:Class,
        skos:Concept,
        dpv:Consequence ;
    dct:contributor "Harshvardhan J. Pandit" ;
    dct:created "2022-08-17"^^xsd:date ;
    dct:source "(ISO/IEC 27005:2018,https://www.iso.org/standard/75281.html)"@en ;
    rdfs:isDefinedBy risk: ;
    sw:term_status "accepted"@en ;
    skos:broader dpv:Detriment ;
    skos:inScheme risk:risk-consequences-classes ;
    skos:prefLabel "Replacement Costs"@en .

risk:ReputationTrustImpact a rdfs:Class,
        skos:Concept,
        dpv:Impact ;
    dct:contributor "Harshvardhan J. Pandit" ;
    dct:created "2022-08-17"^^xsd:date ;
    dct:source "(ENISA Methodology for Sectoral Cybersecurity Assessments,https://www.enisa.europa.eu/publications/methodology-for-a-sectoral-cybersecurity-assessment)"@en ;
    rdfs:isDefinedBy risk: ;
    sw:term_status "accepted"@en ;
    skos:broader dpv:Impact ;
    skos:inScheme risk:risk-consequences-classes ;
    skos:prefLabel "Reputation and trust impact"@en .

risk:RetrievalDeletedData a rdfs:Class,
        skos:Concept,
        dpv:Consequence ;
    dct:contributor "Harshvardhan J. Pandit" ;
    dct:created "2022-08-17"^^xsd:date ;
    dct:source "(ISO/IEC 27005:2018,https://www.iso.org/standard/75281.html)"@en ;
    rdfs:isDefinedBy risk: ;
    sw:term_status "accepted"@en ;
    skos:broader dpv:Detriment ;
    skos:inScheme risk:risk-consequences-classes ;
    skos:prefLabel "Retrieval of Deleted Data"@en .

risk:RetrievalDiscardedEquipment a rdfs:Class,
        skos:Concept,
        dpv:Consequence ;
    dct:contributor "Harshvardhan J. Pandit" ;
    dct:created "2022-08-17"^^xsd:date ;
    dct:source "(ISO/IEC 27005:2018,https://www.iso.org/standard/75281.html)"@en ;
    rdfs:isDefinedBy risk: ;
    sw:term_status "accepted"@en ;
    skos:broader dpv:Detriment ;
    skos:inScheme risk:risk-consequences-classes ;
    skos:prefLabel "Retrieval of Discarded Equipment"@en .

risk:RiskAnalysis a rdfs:Class,
        skos:Concept ;
    dct:contributor "Harshvardhan J. Pandit" ;
    dct:created "2022-08-18"^^xsd:date ;
    dct:source "(IEC 31010:2019,https://www.iso.org/standard/72140.html)"@en ;
    rdfs:isDefinedBy risk: ;
    rdfs:subClassOf dpv:RiskAssessment ;
    sw:term_status "accepted"@en ;
    skos:broader dpv:RiskAssessment ;
    skos:definition "A technique or method used to analyse and identify risk levels, sources, likelihoods, severities, and other necessary information required to conduct risk management procedures"@en ;
    skos:inScheme risk:risk-assessment-classes ;
    skos:narrower risk:QualitativeRiskAnalysis,
        risk:QuantitativeRiskAnalysis ;
    skos:prefLabel "RiskAnalysis"@en .

risk:RiskIndices a rdfs:Class,
        skos:Concept,
        risk:RiskAnalysis ;
    dct:contributor "Harshvardhan J. Pandit" ;
    dct:created "2022-08-18"^^xsd:date ;
    dct:source "(IEC 31010:2019,https://www.iso.org/standard/72140.html)"@en ;
    rdfs:isDefinedBy risk: ;
    sw:term_status "accepted"@en ;
    skos:broader risk:QuantitativeRiskAnalysis ;
    skos:definition "Rates the significance of risks based on ratings applied to factors which are believed to influence the magnitude of the risk."@en ;
    skos:inScheme risk:risk-assessment-classes ;
    skos:prefLabel "Risk Indices"@en .

risk:RiskMatrix a rdfs:Class,
        skos:Concept,
        risk:RiskAnalysis ;
    dct:contributor "Harshvardhan J. Pandit" ;
    dct:created "2022-08-18"^^xsd:date ;
    dct:source "(IEC 31010:2019,https://www.iso.org/standard/72140.html)"@en ;
    rdfs:isDefinedBy risk: ;
    sw:term_status "accepted"@en ;
    skos:broader risk:QualitativeRiskAnalysis,
        risk:QuantitativeRiskAnalysis ;
    skos:definition "Compares individual risks by selecting a consequence/ likelihood pair and displaying them on a matrix with consequence on one axis and likelihood on the other."@en ;
    skos:inScheme risk:risk-assessment-classes ;
    skos:narrower risk:RiskMatrix3x3,
        risk:RiskMatrix5x5,
        risk:RiskMatrix7x7 ;
    skos:prefLabel "Risk Matrix"@en .

risk:RiskMatrix3x3 a rdfs:Class,
        skos:Concept,
        risk:RiskAnalysis ;
    dct:contributor "Harshvardhan J. Pandit" ;
    dct:created "2022-08-17"^^xsd:date ;
    rdfs:isDefinedBy risk: ;
    sw:term_status "accepted"@en ;
    skos:broader risk:RiskMatrix ;
    skos:definition "A Risk Matrix with 3 Likelihood, 3 Severity, and 3 Risk Level types"@en ;
    skos:inScheme risk:risk-matrix-classes ;
    skos:narrower risk:RM3x3S1L1,
        risk:RM3x3S1L2,
        risk:RM3x3S1L3,
        risk:RM3x3S2L1,
        risk:RM3x3S2L2,
        risk:RM3x3S2L3,
        risk:RM3x3S3L1,
        risk:RM3x3S3L2,
        risk:RM3x3S3L3 ;
    skos:prefLabel "Risk Matrix 3x3"@en .

risk:RiskMatrix5x5 a rdfs:Class,
        skos:Concept,
        risk:RiskAnalysis ;
    dct:contributor "Harshvardhan J. Pandit" ;
    dct:created "2022-08-17"^^xsd:date ;
    rdfs:isDefinedBy risk: ;
    sw:term_status "accepted"@en ;
    skos:broader risk:RiskMatrix ;
    skos:definition "A Risk Matrix with 5 Likelihood, 5 Severity, and 5 Risk Level types"@en ;
    skos:inScheme risk:risk-matrix-classes ;
    skos:narrower risk:RM5x5S1L1,
        risk:RM5x5S1L2,
        risk:RM5x5S1L3,
        risk:RM5x5S1L4,
        risk:RM5x5S1L5,
        risk:RM5x5S2L1,
        risk:RM5x5S2L2,
        risk:RM5x5S2L3,
        risk:RM5x5S2L4,
        risk:RM5x5S2L5,
        risk:RM5x5S3L1,
        risk:RM5x5S3L2,
        risk:RM5x5S3L3,
        risk:RM5x5S3L4,
        risk:RM5x5S3L5,
        risk:RM5x5S4L1,
        risk:RM5x5S4L2,
        risk:RM5x5S4L3,
        risk:RM5x5S4L4,
        risk:RM5x5S4L5,
        risk:RM5x5S5L1,
        risk:RM5x5S5L2,
        risk:RM5x5S5L3,
        risk:RM5x5S5L4,
        risk:RM5x5S5L5 ;
    skos:prefLabel "Risk Matrix 5x5"@en .

risk:RiskMatrix7x7 a rdfs:Class,
        skos:Concept,
        risk:RiskAnalysis ;
    dct:contributor "Harshvardhan J. Pandit" ;
    dct:created "2022-08-17"^^xsd:date ;
    rdfs:isDefinedBy risk: ;
    sw:term_status "accepted"@en ;
    skos:broader risk:RiskMatrix ;
    skos:definition "A Risk Matrix with 7 Likelihood, 7 Severity, and 7 Risk Level types"@en ;
    skos:inScheme risk:risk-matrix-classes ;
    skos:narrower risk:RM7x7S1L1,
        risk:RM7x7S1L2,
        risk:RM7x7S1L3,
        risk:RM7x7S1L4,
        risk:RM7x7S1L5,
        risk:RM7x7S1L6,
        risk:RM7x7S1L7,
        risk:RM7x7S2L1,
        risk:RM7x7S2L2,
        risk:RM7x7S2L3,
        risk:RM7x7S2L4,
        risk:RM7x7S2L5,
        risk:RM7x7S2L6,
        risk:RM7x7S2L7,
        risk:RM7x7S3L1,
        risk:RM7x7S3L2,
        risk:RM7x7S3L3,
        risk:RM7x7S3L4,
        risk:RM7x7S3L5,
        risk:RM7x7S3L6,
        risk:RM7x7S3L7,
        risk:RM7x7S4L1,
        risk:RM7x7S4L2,
        risk:RM7x7S4L3,
        risk:RM7x7S4L4,
        risk:RM7x7S4L5,
        risk:RM7x7S4L6,
        risk:RM7x7S4L7,
        risk:RM7x7S5L1,
        risk:RM7x7S5L2,
        risk:RM7x7S5L3,
        risk:RM7x7S5L4,
        risk:RM7x7S5L5,
        risk:RM7x7S5L6,
        risk:RM7x7S5L7,
        risk:RM7x7S6L1,
        risk:RM7x7S6L2,
        risk:RM7x7S6L3,
        risk:RM7x7S6L4,
        risk:RM7x7S6L5,
        risk:RM7x7S6L6,
        risk:RM7x7S6L7,
        risk:RM7x7S7L1,
        risk:RM7x7S7L2,
        risk:RM7x7S7L3,
        risk:RM7x7S7L4,
        risk:RM7x7S7L5,
        risk:RM7x7S7L6,
        risk:RM7x7S7L7 ;
    skos:prefLabel "Risk Matrix 7x7"@en .

risk:RiskRegisters a rdfs:Class,
        skos:Concept,
        risk:RiskAnalysis ;
    dct:contributor "Harshvardhan J. Pandit" ;
    dct:created "2022-08-18"^^xsd:date ;
    dct:source "(IEC 31010:2019,https://www.iso.org/standard/72140.html)"@en ;
    rdfs:isDefinedBy risk: ;
    sw:term_status "accepted"@en ;
    skos:broader risk:QualitativeRiskAnalysis ;
    skos:definition "A means of recording information about risks and tracking actions."@en ;
    skos:inScheme risk:risk-assessment-classes ;
    skos:prefLabel "Risk Registers"@en .

risk:SCurves a rdfs:Class,
        skos:Concept,
        risk:RiskAnalysis ;
    dct:contributor "Harshvardhan J. Pandit" ;
    dct:created "2022-08-18"^^xsd:date ;
    dct:source "(IEC 31010:2019,https://www.iso.org/standard/72140.html)"@en ;
    rdfs:isDefinedBy risk: ;
    sw:term_status "accepted"@en ;
    skos:broader risk:QuantitativeRiskAnalysis ;
    skos:definition "A means of displaying the relationship between consequences and their likelihood plotted as a cumulative distribution function (S-curve)."@en ;
    skos:inScheme risk:risk-assessment-classes ;
    skos:prefLabel "S-curves"@en .

risk:SFAIRP a rdfs:Class,
        skos:Concept,
        risk:RiskAnalysis ;
    dct:contributor "Harshvardhan J. Pandit" ;
    dct:created "2022-08-18"^^xsd:date ;
    dct:source "(IEC 31010:2019,https://www.iso.org/standard/72140.html)"@en ;
    rdfs:isDefinedBy risk: ;
    sw:term_status "accepted"@en ;
    skos:broader risk:QualitativeRiskAnalysis,
        risk:QuantitativeRiskAnalysis ;
    skos:definition "So far as is Resonably Practiceable (ALARP) - A criteria for deciding significance of risk and means of evaluating tolerability of risk"@en ;
    skos:inScheme risk:risk-assessment-classes ;
    skos:prefLabel "SFAIRP"@en .

risk:SWIFT a rdfs:Class,
        skos:Concept,
        risk:RiskAnalysis ;
    dct:contributor "Harshvardhan J. Pandit" ;
    dct:created "2022-08-18"^^xsd:date ;
    dct:source "(IEC 31010:2019,https://www.iso.org/standard/72140.html)"@en ;
    rdfs:isDefinedBy risk: ;
    sw:term_status "accepted"@en ;
    skos:broader risk:QualitativeRiskAnalysis ;
    skos:definition "A simpler form of HAZOP with prompts of \"what if\" to identify deviations from the expected."@en ;
    skos:inScheme risk:risk-assessment-classes ;
    skos:prefLabel "Structured \"What If?\" (SWIFT)"@en .

risk:Sabotage a rdfs:Class,
        skos:Concept,
        dpv:Impact ;
    dct:contributor "Harshvardhan J. Pandit" ;
    dct:created "2022-08-17"^^xsd:date ;
    dct:source "(ENISA Reference Incident Classification Taxonomy 2018,https://www.enisa.europa.eu/publications/reference-incident-classification-taxonomy/)"@en ;
    rdfs:isDefinedBy risk: ;
    sw:term_status "accepted"@en ;
    skos:broader dpv:Harm ;
    skos:inScheme risk:risk-consequences-classes ;
    skos:prefLabel "Sabotage"@en .

risk:Scam a rdfs:Class,
        skos:Concept,
        dpv:Impact ;
    dct:contributor "Harshvardhan J. Pandit" ;
    dct:created "2022-08-17"^^xsd:date ;
    dct:source "(ISO/IEC 27005:2018,https://www.iso.org/standard/75281.html)"@en ;
    rdfs:isDefinedBy risk: ;
    sw:term_status "accepted"@en ;
    skos:broader dpv:Harm ;
    skos:inScheme risk:risk-consequences-classes ;
    skos:prefLabel "Scam"@en .

risk:ScenarioAnalysis a rdfs:Class,
        skos:Concept,
        risk:RiskAnalysis ;
    dct:contributor "Harshvardhan J. Pandit" ;
    dct:created "2022-08-18"^^xsd:date ;
    dct:source "(IEC 31010:2019,https://www.iso.org/standard/72140.html)"@en ;
    rdfs:isDefinedBy risk: ;
    sw:term_status "accepted"@en ;
    skos:broader risk:QualitativeRiskAnalysis ;
    skos:definition "Identifies possible future scenarios through imagination, extrapolation from the present or modelling. Risk is then considered for each of these scenarios."@en ;
    skos:inScheme risk:risk-assessment-classes ;
    skos:prefLabel "Scenario Analysis"@en .

risk:SecurityBreach a rdfs:Class,
        skos:Concept,
        dpv:Consequence ;
    dct:contributor "Harshvardhan J. Pandit" ;
    dct:created "2022-08-17"^^xsd:date ;
    dct:source "(ISO/IEC 27005:2018,https://www.iso.org/standard/75281.html)"@en ;
    rdfs:isDefinedBy risk: ;
    sw:term_status "accepted"@en ;
    skos:broader dpv:Consequence ;
    skos:inScheme risk:risk-consequences-classes ;
    skos:prefLabel "Security Breach"@en .

risk:ServiceInterruption a rdfs:Class,
        skos:Concept,
        dpv:Consequence ;
    dct:contributor "Harshvardhan J. Pandit" ;
    dct:created "2022-08-17"^^xsd:date ;
    dct:source "(ISO/IEC 27005:2018,https://www.iso.org/standard/75281.html)"@en ;
    rdfs:isDefinedBy risk: ;
    sw:term_status "accepted"@en ;
    skos:broader dpv:Detriment ;
    skos:inScheme risk:risk-consequences-classes ;
    skos:prefLabel "Service Interruption"@en .

risk:SexualViolence a rdfs:Class,
        skos:Concept,
        dpv:Impact ;
    dct:contributor "Harshvardhan J. Pandit" ;
    dct:created "2022-08-17"^^xsd:date ;
    dct:source "(ENISA Reference Incident Classification Taxonomy 2018,https://www.enisa.europa.eu/publications/reference-incident-classification-taxonomy/)"@en ;
    rdfs:isDefinedBy risk: ;
    sw:term_status "accepted"@en ;
    skos:broader dpv:Harm ;
    skos:inScheme risk:risk-consequences-classes ;
    skos:prefLabel "Sexual Violence"@en .

risk:ShareRisk a rdfs:Class,
        skos:Concept,
        dpv:RiskMitigationMeasure ;
    dct:contributor "Harshvardhan J. Pandit" ;
    dct:created "2022-08-29"^^xsd:date ;
    rdfs:isDefinedBy risk: ;
    sw:term_status "accepted"@en ;
    skos:broader dpv:RiskMitigationMeasure ;
    skos:definition "Risk Mitigation Measure that shares Risk e.g. amongst stakeholders"@en ;
    skos:inScheme risk:risk-controls-classes ;
    skos:prefLabel "Share Risk"@en .

risk:SocialDisadvantage a rdfs:Class,
        skos:Concept,
        dpv:Impact ;
    dct:contributor "Georg P Krog" ;
    dct:created "2022-08-19"^^xsd:date ;
    rdfs:isDefinedBy risk: ;
    sw:term_status "accepted"@en ;
    skos:broader dpv:Impact ;
    skos:inScheme risk:risk-consequences-classes ;
    skos:prefLabel "Social Disadvantage"@en .

risk:Spam a rdfs:Class,
        skos:Concept,
        dpv:Impact ;
    dct:contributor "Harshvardhan J. Pandit" ;
    dct:created "2022-08-17"^^xsd:date ;
    dct:source "(ENISA Reference Incident Classification Taxonomy 2018,https://www.enisa.europa.eu/publications/reference-incident-classification-taxonomy/)"@en ;
    rdfs:isDefinedBy risk: ;
    sw:term_status "accepted"@en ;
    skos:broader dpv:Harm ;
    skos:inScheme risk:risk-consequences-classes ;
    skos:prefLabel "Spam"@en .

risk:Spoofing a rdfs:Class,
        skos:Concept,
        dpv:Impact ;
    dct:contributor "Harshvardhan J. Pandit" ;
    dct:created "2022-08-17"^^xsd:date ;
    dct:source "(ISO/IEC 27005:2018,https://www.iso.org/standard/75281.html)"@en ;
    rdfs:isDefinedBy risk: ;
    sw:term_status "accepted"@en ;
    skos:broader dpv:Harm ;
    skos:inScheme risk:risk-consequences-classes ;
    skos:prefLabel "Spoofing"@en .

risk:Spying a rdfs:Class,
        skos:Concept,
        dpv:Impact ;
    dct:contributor "Harshvardhan J. Pandit" ;
    dct:created "2022-08-17"^^xsd:date ;
    dct:source "(ISO/IEC 27005:2018,https://www.iso.org/standard/75281.html)"@en ;
    rdfs:isDefinedBy risk: ;
    sw:term_status "accepted"@en ;
    skos:broader dpv:NonMaterialDamage ;
    skos:inScheme risk:risk-consequences-classes ;
    skos:prefLabel "Spying"@en .

risk:Stalking a rdfs:Class,
        skos:Concept,
        dpv:Impact ;
    dct:contributor "Harshvardhan J. Pandit" ;
    dct:created "2022-08-17"^^xsd:date ;
    dct:source "(ISO/IEC 27005:2018,https://www.iso.org/standard/75281.html)"@en ;
    rdfs:isDefinedBy risk: ;
    sw:term_status "accepted"@en ;
    skos:broader dpv:NonMaterialDamage ;
    skos:inScheme risk:risk-consequences-classes ;
    skos:prefLabel "Stalking"@en .

risk:Surveys a rdfs:Class,
        skos:Concept,
        risk:RiskAnalysis ;
    dct:contributor "Harshvardhan J. Pandit" ;
    dct:created "2022-08-18"^^xsd:date ;
    dct:source "(IEC 31010:2019,https://www.iso.org/standard/72140.html)"@en ;
    rdfs:isDefinedBy risk: ;
    sw:term_status "accepted"@en ;
    skos:broader risk:QualitativeRiskAnalysis ;
    skos:definition "Paper- or computer-based questionnaires to elicit views."@en ;
    skos:inScheme risk:risk-assessment-classes ;
    skos:prefLabel "Surveys"@en .

risk:SystemFailure a rdfs:Class,
        skos:Concept,
        dpv:Consequence ;
    dct:contributor "Harshvardhan J. Pandit" ;
    dct:created "2022-08-17"^^xsd:date ;
    dct:source "(ENISA Threat Landscape for Ransomware Attacks 2022,https://www.enisa.europa.eu/publications/enisa-threat-landscape-for-ransomware-attacks)"@en ;
    rdfs:isDefinedBy risk: ;
    sw:term_status "accepted"@en ;
    skos:broader dpv:Detriment ;
    skos:inScheme risk:risk-consequences-classes ;
    skos:prefLabel "System Failure"@en .

risk:SystemIntrusion a rdfs:Class,
        skos:Concept,
        dpv:Consequence ;
    dct:contributor "Harshvardhan J. Pandit" ;
    dct:created "2022-08-17"^^xsd:date ;
    dct:source "(ENISA Reference Incident Classification Taxonomy 2018,https://www.enisa.europa.eu/publications/reference-incident-classification-taxonomy/)"@en ;
    rdfs:isDefinedBy risk: ;
    sw:term_status "accepted"@en ;
    skos:broader dpv:Detriment ;
    skos:inScheme risk:risk-consequences-classes ;
    skos:prefLabel "System Intrusion"@en .

risk:SystemMalfunction a rdfs:Class,
        skos:Concept,
        dpv:Consequence ;
    dct:contributor "Harshvardhan J. Pandit" ;
    dct:created "2022-08-17"^^xsd:date ;
    dct:source "(ISO/IEC 27005:2018,https://www.iso.org/standard/75281.html)"@en ;
    rdfs:isDefinedBy risk: ;
    sw:term_status "accepted"@en ;
    skos:broader dpv:Detriment ;
    skos:inScheme risk:risk-consequences-classes ;
    skos:prefLabel "System Malfunction"@en .

risk:Taxonomies a rdfs:Class,
        skos:Concept,
        risk:RiskAnalysis ;
    dct:contributor "Harshvardhan J. Pandit" ;
    dct:created "2022-08-18"^^xsd:date ;
    dct:source "(IEC 31010:2019,https://www.iso.org/standard/72140.html)"@en ;
    rdfs:isDefinedBy risk: ;
    sw:term_status "accepted"@en ;
    skos:broader risk:QualitativeRiskAnalysis ;
    skos:definition "A taxonomy based on experience or on concepts and models that can be used to help identify risks or controls."@en ;
    skos:inScheme risk:risk-assessment-classes ;
    skos:prefLabel "Taxonomies"@en .

risk:Terrorism a rdfs:Class,
        skos:Concept,
        dpv:Impact ;
    dct:contributor "Harshvardhan J. Pandit" ;
    dct:created "2022-08-17"^^xsd:date ;
    dct:source "(ISO/IEC 27005:2018,https://www.iso.org/standard/75281.html)"@en ;
    rdfs:isDefinedBy risk: ;
    sw:term_status "accepted"@en ;
    skos:broader dpv:Harm ;
    skos:inScheme risk:risk-consequences-classes ;
    skos:prefLabel "Terrorism"@en .

risk:Theft a rdfs:Class,
        skos:Concept,
        dpv:Impact ;
    dct:contributor "Harshvardhan J. Pandit" ;
    dct:created "2022-08-17"^^xsd:date ;
    dct:source "(ISO/IEC 27005:2018,https://www.iso.org/standard/75281.html)"@en ;
    rdfs:isDefinedBy risk: ;
    sw:term_status "accepted"@en ;
    skos:broader dpv:MaterialDamage ;
    skos:inScheme risk:risk-consequences-classes ;
    skos:prefLabel "Theft"@en .

risk:TheftEquipment a rdfs:Class,
        skos:Concept,
        dpv:Impact ;
    dct:contributor "Harshvardhan J. Pandit" ;
    dct:created "2022-08-17"^^xsd:date ;
    dct:source "(ISO/IEC 27005:2018,https://www.iso.org/standard/75281.html)"@en ;
    rdfs:isDefinedBy risk: ;
    sw:term_status "accepted"@en ;
    skos:broader dpv:MaterialDamage ;
    skos:inScheme risk:risk-consequences-classes ;
    skos:prefLabel "Theft of Equipment"@en .

risk:TheftMedia a rdfs:Class,
        skos:Concept,
        dpv:Impact ;
    dct:contributor "Harshvardhan J. Pandit" ;
    dct:created "2022-08-17"^^xsd:date ;
    dct:source "(ISO/IEC 27005:2018,https://www.iso.org/standard/75281.html)"@en ;
    rdfs:isDefinedBy risk: ;
    sw:term_status "accepted"@en ;
    skos:broader dpv:MaterialDamage ;
    skos:inScheme risk:risk-consequences-classes ;
    skos:prefLabel "Theft of Media"@en .

risk:ThirdPartyOperationDisruption a rdfs:Class,
        skos:Concept,
        dpv:Consequence ;
    dct:contributor "Harshvardhan J. Pandit" ;
    dct:created "2022-08-17"^^xsd:date ;
    dct:source "(ISO/IEC 27005:2018,https://www.iso.org/standard/75281.html)"@en ;
    rdfs:isDefinedBy risk: ;
    sw:term_status "accepted"@en ;
    skos:broader dpv:Detriment ;
    skos:inScheme risk:risk-consequences-classes ;
    skos:prefLabel "Third Party Operation Disruption"@en .

risk:Toxicological a rdfs:Class,
        skos:Concept,
        risk:RiskAnalysis ;
    dct:contributor "Harshvardhan J. Pandit" ;
    dct:created "2022-08-18"^^xsd:date ;
    dct:source "(IEC 31010:2019,https://www.iso.org/standard/72140.html)"@en ;
    rdfs:isDefinedBy risk: ;
    sw:term_status "accepted"@en ;
    skos:broader risk:QuantitativeRiskAnalysis ;
    skos:definition "A series of steps taken to obtain a measure for the risk to humans or ecological systems due to exposure to chemicals."@en ;
    skos:inScheme risk:risk-assessment-classes ;
    skos:prefLabel "Toxicological Risk Assessment"@en .

risk:UnauthorisedAccesstoPremises a rdfs:Class,
        skos:Concept,
        dpv:Consequence ;
    dct:contributor "Harshvardhan J. Pandit" ;
    dct:created "2022-08-17"^^xsd:date ;
    dct:source "(ISO/IEC 27005:2018,https://www.iso.org/standard/75281.html)"@en ;
    rdfs:isDefinedBy risk: ;
    sw:term_status "accepted"@en ;
    skos:broader dpv:Detriment ;
    skos:inScheme risk:risk-consequences-classes ;
    skos:prefLabel "Unauthorised Access to Premises"@en .

risk:UnauthorisedCodeAccess a rdfs:Class,
        skos:Concept,
        dpv:Consequence ;
    dct:contributor "Harshvardhan J. Pandit" ;
    dct:created "2022-08-17"^^xsd:date ;
    dct:source "(ENISA Methodology for Sectoral Cybersecurity Assessments,https://www.enisa.europa.eu/publications/methodology-for-a-sectoral-cybersecurity-assessment)"@en ;
    rdfs:isDefinedBy risk: ;
    sw:term_status "accepted"@en ;
    skos:broader dpv:Detriment ;
    skos:inScheme risk:risk-consequences-classes ;
    skos:prefLabel "Unauthorised Code Access"@en .

risk:UnauthorisedCodeDisclosure a rdfs:Class,
        skos:Concept,
        dpv:Consequence ;
    dct:contributor "Harshvardhan J. Pandit" ;
    dct:created "2022-08-17"^^xsd:date ;
    dct:source "(ENISA Methodology for Sectoral Cybersecurity Assessments,https://www.enisa.europa.eu/publications/methodology-for-a-sectoral-cybersecurity-assessment)"@en ;
    rdfs:isDefinedBy risk: ;
    sw:term_status "accepted"@en ;
    skos:broader dpv:Detriment ;
    skos:inScheme risk:risk-consequences-classes ;
    skos:prefLabel "Unauthorised Code Disclosure"@en .

risk:UnauthorisedCodeModification a rdfs:Class,
        skos:Concept,
        dpv:Consequence ;
    dct:contributor "Harshvardhan J. Pandit" ;
    dct:created "2022-08-17"^^xsd:date ;
    dct:source "(ENISA Methodology for Sectoral Cybersecurity Assessments,https://www.enisa.europa.eu/publications/methodology-for-a-sectoral-cybersecurity-assessment)"@en ;
    rdfs:isDefinedBy risk: ;
    sw:term_status "accepted"@en ;
    skos:broader dpv:Damage ;
    skos:inScheme risk:risk-consequences-classes ;
    skos:prefLabel "Unauthorised Code Modification"@en .

risk:UnauthorisedDataAccess a rdfs:Class,
        skos:Concept,
        dpv:Consequence ;
    dct:contributor "Harshvardhan J. Pandit" ;
    dct:created "2022-08-17"^^xsd:date ;
    dct:source "(ENISA Reference Incident Classification Taxonomy 2018,https://www.enisa.europa.eu/publications/reference-incident-classification-taxonomy/)"@en ;
    rdfs:isDefinedBy risk: ;
    sw:term_status "accepted"@en ;
    skos:broader dpv:Detriment ;
    skos:inScheme risk:risk-consequences-classes ;
    skos:prefLabel "Unauthorised Data Access"@en .

risk:UnauthorisedDataDisclosure a rdfs:Class,
        skos:Concept,
        dpv:Consequence ;
    dct:contributor "Harshvardhan J. Pandit" ;
    dct:created "2022-08-17"^^xsd:date ;
    dct:source "(ISO/IEC 27005:2018,https://www.iso.org/standard/75281.html)"@en ;
    rdfs:isDefinedBy risk: ;
    sw:term_status "accepted"@en ;
    skos:broader dpv:Detriment ;
    skos:inScheme risk:risk-consequences-classes ;
    skos:prefLabel "Unauthorised Data Disclosure"@en .

risk:UnauthorisedDataModification a rdfs:Class,
        skos:Concept,
        dpv:Impact ;
    dct:contributor "Harshvardhan J. Pandit" ;
    dct:created "2022-08-17"^^xsd:date ;
    dct:source "(ENISA Reference Incident Classification Taxonomy 2018,https://www.enisa.europa.eu/publications/reference-incident-classification-taxonomy/)"@en ;
    rdfs:isDefinedBy risk: ;
    sw:term_status "accepted"@en ;
    skos:broader dpv:NonMaterialDamage ;
    skos:inScheme risk:risk-consequences-classes ;
    skos:prefLabel "Unauthorised Data Modification"@en .

risk:UnauthorisedImpersonation a rdfs:Class,
        skos:Concept,
        dpv:Impact ;
    dct:contributor "Harshvardhan J. Pandit" ;
    dct:created "2022-08-17"^^xsd:date ;
    dct:source "(ISO/IEC 27005:2018,https://www.iso.org/standard/75281.html)"@en ;
    rdfs:isDefinedBy risk: ;
    sw:term_status "accepted"@en ;
    skos:broader dpv:NonMaterialDamage ;
    skos:inScheme risk:risk-consequences-classes ;
    skos:prefLabel "Unauthorised Impersonation"@en .

risk:UnauthorisedInformationDisclosure a rdfs:Class,
        skos:Concept,
        dpv:Consequence ;
    dct:contributor "Harshvardhan J. Pandit" ;
    dct:created "2022-08-17"^^xsd:date ;
    dct:source "(ENISA Reference Incident Classification Taxonomy 2018,https://www.enisa.europa.eu/publications/reference-incident-classification-taxonomy/)"@en ;
    rdfs:isDefinedBy risk: ;
    sw:term_status "accepted"@en ;
    skos:broader dpv:Detriment ;
    skos:inScheme risk:risk-consequences-classes ;
    skos:prefLabel "Unauthorised Information Disclosure"@en .

risk:UnauthorisedReIdentification a rdfs:Class,
        skos:Concept,
        dpv:Consequence ;
    dct:contributor "Georg P Krog" ;
    dct:created "2022-08-19"^^xsd:date ;
    rdfs:isDefinedBy risk: ;
    sw:term_status "accepted"@en ;
    skos:broader dpv:Consequence ;
    skos:inScheme risk:risk-consequences-classes ;
    skos:prefLabel "Unauthorised Re-Identification"@en .

risk:UnauthorisedResourceUse a rdfs:Class,
        skos:Concept,
        dpv:Consequence ;
    dct:contributor "Harshvardhan J. Pandit" ;
    dct:created "2022-08-17"^^xsd:date ;
    dct:source "(ISO/IEC 27005:2018,https://www.iso.org/standard/75281.html)"@en ;
    rdfs:isDefinedBy risk: ;
    sw:term_status "accepted"@en ;
    skos:broader dpv:Detriment ;
    skos:inScheme risk:risk-consequences-classes ;
    skos:prefLabel "Unauthorised Resource Use"@en .

risk:UnauthorisedSystemAccess a rdfs:Class,
        skos:Concept,
        dpv:Consequence ;
    dct:contributor "Harshvardhan J. Pandit" ;
    dct:created "2022-08-17"^^xsd:date ;
    dct:source "(ISO/IEC 27005:2018,https://www.iso.org/standard/75281.html)"@en ;
    rdfs:isDefinedBy risk: ;
    sw:term_status "accepted"@en ;
    skos:broader dpv:Detriment ;
    skos:inScheme risk:risk-consequences-classes ;
    skos:prefLabel "Unauthorised System Access"@en .

risk:UnauthorisedSystemModification a rdfs:Class,
        skos:Concept,
        dpv:Consequence ;
    dct:contributor "Harshvardhan J. Pandit" ;
    dct:created "2022-08-17"^^xsd:date ;
    dct:source "(ENISA Methodology for Sectoral Cybersecurity Assessments,https://www.enisa.europa.eu/publications/methodology-for-a-sectoral-cybersecurity-assessment)"@en ;
    rdfs:isDefinedBy risk: ;
    sw:term_status "accepted"@en ;
    skos:broader dpv:Damage ;
    skos:inScheme risk:risk-consequences-classes ;
    skos:prefLabel "Unauthorised System Modification"@en .

risk:UnknownVulnerabilityExploited a rdfs:Class,
        skos:Concept,
        dpv:Consequence ;
    dct:contributor "Harshvardhan J. Pandit" ;
    dct:created "2022-08-17"^^xsd:date ;
    dct:source "(ENISA Reference Incident Classification Taxonomy 2018,https://www.enisa.europa.eu/publications/reference-incident-classification-taxonomy/)"@en ;
    rdfs:isDefinedBy risk: ;
    sw:term_status "accepted"@en ;
    skos:broader dpv:Detriment ;
    skos:inScheme risk:risk-consequences-classes ;
    skos:prefLabel "Unknown Vulnerability Exploited"@en .

risk:UnwantedCodeDeletion a rdfs:Class,
        skos:Concept,
        dpv:Consequence ;
    dct:contributor "Harshvardhan J. Pandit" ;
    dct:created "2022-08-17"^^xsd:date ;
    dct:source "(ENISA Methodology for Sectoral Cybersecurity Assessments,https://www.enisa.europa.eu/publications/methodology-for-a-sectoral-cybersecurity-assessment)"@en ;
    rdfs:isDefinedBy risk: ;
    sw:term_status "accepted"@en ;
    skos:broader dpv:Damage ;
    skos:inScheme risk:risk-consequences-classes ;
    skos:prefLabel "Unwanted Code Deletion"@en .

risk:UnwantedDataDeletion a rdfs:Class,
        skos:Concept,
        dpv:Consequence ;
    dct:contributor "Harshvardhan J. Pandit" ;
    dct:created "2022-08-17"^^xsd:date ;
    dct:source "(ISO/IEC 27005:2018,https://www.iso.org/standard/75281.html)"@en ;
    rdfs:isDefinedBy risk: ;
    sw:term_status "accepted"@en ;
    skos:broader dpv:Damage ;
    skos:inScheme risk:risk-consequences-classes ;
    skos:prefLabel "Unwanted Data Deletion"@en .

risk:UnwantedDisclosureData a rdfs:Class,
        skos:Concept,
        dpv:Consequence ;
    dct:contributor "Harshvardhan J. Pandit" ;
    dct:created "2022-08-17"^^xsd:date ;
    dct:source "(ISO/IEC 27005:2018,https://www.iso.org/standard/75281.html)"@en ;
    rdfs:isDefinedBy risk: ;
    sw:term_status "accepted"@en ;
    skos:broader dpv:Detriment ;
    skos:inScheme risk:risk-consequences-classes ;
    skos:prefLabel "Unwanted Disclosure of Data"@en .

risk:VaR a rdfs:Class,
        skos:Concept,
        risk:RiskAnalysis ;
    dct:contributor "Harshvardhan J. Pandit" ;
    dct:created "2022-08-18"^^xsd:date ;
    dct:source "(IEC 31010:2019,https://www.iso.org/standard/72140.html)"@en ;
    rdfs:isDefinedBy risk: ;
    sw:term_status "accepted"@en ;
    skos:broader risk:QuantitativeRiskAnalysis ;
    skos:definition "Financial measure of risk that uses an assumed probability distribution of losses in a stable market condition to calculate the value of a loss that might occur with a specified probability within a defined time span."@en ;
    skos:inScheme risk:risk-assessment-classes ;
    skos:prefLabel "Value At Risk (VaR)"@en .

risk:Vandalism a rdfs:Class,
        skos:Concept,
        dpv:Consequence ;
    dct:contributor "Harshvardhan J. Pandit" ;
    dct:created "2022-08-17"^^xsd:date ;
    dct:source "(ENISA Threat Taxonomy 2016,https://www.enisa.europa.eu/topics/threat-risk-management/threats-and-trends/enisa-threat-landscape/threat-taxonomy/view)"@en ;
    rdfs:isDefinedBy risk: ;
    sw:term_status "accepted"@en ;
    skos:broader dpv:Damage ;
    skos:inScheme risk:risk-consequences-classes ;
    skos:prefLabel "Vandalism"@en .

risk:VeryHighLikelihood a rdfs:Class,
        skos:Concept,
        dpv:Likelihood ;
    dct:contributor "Harshvardhan J. Pandit" ;
    dct:created "2022-08-18"^^xsd:date ;
    rdf:value "0.9,xsd:decimal" ;
    rdfs:isDefinedBy risk: ;
    sw:term_status "accepted"@en ;
    skos:broader risk:5LikelihoodLevels,
        risk:7LikelihoodLevels ;
    skos:definition "Level where Likelihood is Very High"@en ;
    skos:inScheme risk:risk-levels-classes ;
    skos:prefLabel "Very High Likelihood"@en ;
    skos:scopeNote "The suggested quantitative value for this concept is 0.9 on a scale of 0 to 1"@en .

risk:VeryHighRisk a rdfs:Class,
        skos:Concept,
        dpv:RiskLevel ;
    dct:contributor "Harshvardhan J. Pandit" ;
    dct:created "2022-08-18"^^xsd:date ;
    rdf:value "0.9,xsd:decimal" ;
    rdfs:isDefinedBy risk: ;
    sw:term_status "accepted"@en ;
    skos:broader risk:5RiskLevels,
        risk:7RiskLevels ;
    skos:definition "Level where Risk is Very High"@en ;
    skos:inScheme risk:risk-levels-classes ;
    skos:prefLabel "Very High Risk"@en ;
    skos:scopeNote "The suggested quantitative value for this concept is 0.9 on a scale of 0 to 1"@en .

risk:VeryHighSeverity a rdfs:Class,
        skos:Concept,
        dpv:Severity ;
    dct:contributor "Harshvardhan J. Pandit" ;
    dct:created "2022-08-18"^^xsd:date ;
    rdf:value "0.9,xsd:decimal" ;
    rdfs:isDefinedBy risk: ;
    sw:term_status "accepted"@en ;
    skos:broader risk:5SeverityLevels,
        risk:7SeverityLevels ;
    skos:definition "Level where Severity is Very High"@en ;
    skos:inScheme risk:risk-levels-classes ;
    skos:prefLabel "Very High Severity"@en ;
    skos:scopeNote "The suggested quantitative value for this concept is 0.9 on a scale of 0 to 1"@en .

risk:VeryLowLikelihood a rdfs:Class,
        skos:Concept,
        dpv:Likelihood ;
    dct:contributor "Harshvardhan J. Pandit" ;
    dct:created "2022-08-18"^^xsd:date ;
    rdf:value "0.1,xsd:decimal" ;
    rdfs:isDefinedBy risk: ;
    sw:term_status "accepted"@en ;
    skos:broader risk:5LikelihoodLevels,
        risk:7LikelihoodLevels ;
    skos:definition "Level where Likelihood is Very Low"@en ;
    skos:inScheme risk:risk-levels-classes ;
    skos:prefLabel "Very Low Likelihood"@en ;
    skos:scopeNote "The suggested quantitative value for this concept is 0.1 on a scale of 0 to 1"@en .

risk:VeryLowRisk a rdfs:Class,
        skos:Concept,
        dpv:RiskLevel ;
    dct:contributor "Harshvardhan J. Pandit" ;
    dct:created "2022-08-18"^^xsd:date ;
    rdf:value "0.1,xsd:decimal" ;
    rdfs:isDefinedBy risk: ;
    sw:term_status "accepted"@en ;
    skos:broader risk:5RiskLevels,
        risk:7RiskLevels ;
    skos:definition "Level where Risk is Very Low"@en ;
    skos:inScheme risk:risk-levels-classes ;
    skos:prefLabel "Very Low Risk"@en ;
    skos:scopeNote "The suggested quantitative value for this concept is 0.1 on a scale of 0 to 1"@en .

risk:VeryLowSeverity a rdfs:Class,
        skos:Concept,
        dpv:Severity ;
    dct:contributor "Harshvardhan J. Pandit" ;
    dct:created "2022-08-18"^^xsd:date ;
    rdf:value "0.1,xsd:decimal" ;
    rdfs:isDefinedBy risk: ;
    sw:term_status "accepted"@en ;
    skos:broader risk:5SeverityLevels,
        risk:7SeverityLevels ;
    skos:definition "Level where Severity is Very Low"@en ;
    skos:inScheme risk:risk-levels-classes ;
    skos:prefLabel "Very Low Severity"@en ;
    skos:scopeNote "The suggested quantitative value for this concept is 0.1 on a scale of 0 to 1"@en .

risk:ViolationCodeConduct a rdfs:Class,
        skos:Concept,
        dpv:Consequence ;
    dct:contributor "Harshvardhan J. Pandit" ;
    dct:created "2022-08-17"^^xsd:date ;
    dct:source "(ISO/IEC 27005:2018,https://www.iso.org/standard/75281.html)"@en ;
    rdfs:isDefinedBy risk: ;
    sw:term_status "accepted"@en ;
    skos:broader dpv:Damage ;
    skos:inScheme risk:risk-consequences-classes ;
    skos:prefLabel "Violation of Code of Conduct"@en .

risk:ViolationContractualObligations a rdfs:Class,
        skos:Concept,
        dpv:Consequence ;
    dct:contributor "Harshvardhan J. Pandit" ;
    dct:created "2022-08-17"^^xsd:date ;
    dct:source "(ISO/IEC 27005:2018,https://www.iso.org/standard/75281.html)"@en ;
    rdfs:isDefinedBy risk: ;
    sw:term_status "accepted"@en ;
    skos:broader dpv:Damage ;
    skos:inScheme risk:risk-consequences-classes ;
    skos:prefLabel "Violation of Contractual Obligations"@en .

risk:ViolationEthicalCode a rdfs:Class,
        skos:Concept,
        dpv:Consequence ;
    dct:contributor "Harshvardhan J. Pandit" ;
    dct:created "2022-08-17"^^xsd:date ;
    dct:source "(ISO/IEC 27005:2018,https://www.iso.org/standard/75281.html)"@en ;
    rdfs:isDefinedBy risk: ;
    sw:term_status "accepted"@en ;
    skos:broader dpv:Damage ;
    skos:inScheme risk:risk-consequences-classes ;
    skos:prefLabel "Violation of Ethical Code"@en .

risk:ViolationOfRights a rdfs:Class,
        skos:Concept,
        dpv:Impact ;
    dct:contributor "Georg P Krog, Harshvardhan J. Pandit" ;
    dct:created "2022-08-18"^^xsd:date ;
    rdfs:isDefinedBy risk: ;
    sw:term_status "accepted"@en ;
    skos:broader dpv:Harm ;
    skos:inScheme risk:risk-consequences-classes ;
    skos:prefLabel "Violation of Rights"@en .

risk:ViolationRegulatoryObligations a rdfs:Class,
        skos:Concept,
        dpv:Consequence ;
    dct:contributor "Harshvardhan J. Pandit" ;
    dct:created "2022-08-17"^^xsd:date ;
    dct:source "(ISO/IEC 27005:2018,https://www.iso.org/standard/75281.html)"@en ;
    rdfs:isDefinedBy risk: ;
    sw:term_status "accepted"@en ;
    skos:broader dpv:Damage ;
    skos:inScheme risk:risk-consequences-classes ;
    skos:prefLabel "Violation of Regulatory Obligations"@en .

risk:ViolationStatutoryObligations a rdfs:Class,
        skos:Concept,
        dpv:Consequence ;
    dct:contributor "Harshvardhan J. Pandit" ;
    dct:created "2022-08-17"^^xsd:date ;
    dct:source "(ISO/IEC 27005:2018,https://www.iso.org/standard/75281.html)"@en ;
    rdfs:isDefinedBy risk: ;
    sw:term_status "accepted"@en ;
    skos:broader dpv:Damage ;
    skos:inScheme risk:risk-consequences-classes ;
    skos:prefLabel "Violation of Statutory Obligations"@en .

risk:VulnerabilityCreated a rdfs:Class,
        skos:Concept,
        dpv:Consequence ;
    dct:contributor "Harshvardhan J. Pandit" ;
    dct:created "2022-08-17"^^xsd:date ;
    dct:source "(ISO/IEC 27005:2018,https://www.iso.org/standard/75281.html)"@en ;
    rdfs:isDefinedBy risk: ;
    sw:term_status "accepted"@en ;
    skos:broader dpv:Detriment ;
    skos:inScheme risk:risk-consequences-classes ;
    skos:prefLabel "Vulnerability Created"@en .

risk:VulnerabilityExploited a rdfs:Class,
        skos:Concept,
        dpv:Consequence ;
    dct:contributor "Harshvardhan J. Pandit" ;
    dct:created "2022-08-17"^^xsd:date ;
    dct:source "(ENISA Reference Incident Classification Taxonomy 2018,https://www.enisa.europa.eu/publications/reference-incident-classification-taxonomy/)"@en ;
    rdfs:isDefinedBy risk: ;
    sw:term_status "accepted"@en ;
    skos:broader dpv:Detriment ;
    skos:inScheme risk:risk-consequences-classes ;
    skos:prefLabel "Vulnerability Exploited"@en .

<https://w3id.org/dpv/risk> a owl:Ontology ;
    dct:conformsTo "http://www.w3.org/2000/01/rdf-schema",
        "http://www.w3.org/2004/02/skos/core" ;
    dct:contributor "Georg P Krog",
        "Harshvardhan J. Pandit" ;
    dct:created "2022-08-14"@en ;
    dct:creator "Beatriz Esteves"@en,
        "Georg P Krog"@en,
        "Harshvardhan J. Pandit"@en,
        "Julian Flake"@en,
        "Paul Ryan"@en ;
    dct:description "Extension to the Data Privacy Vocabulary (DPV) providing concepts for representing information about risk assessment and risk management"@en ;
    dct:identifier "https://w3id.org/dpv/risk" ;
    dct:language "de" ;
    dct:license <https://www.w3.org/copyright/document-license-2023/> ;
    dct:modified "2024-01-01"@en ;
    dct:title "Risk Concepts"@en ;
    vann:preferredNamespacePrefix "risk" ;
    vann:preferredNamespaceUri "https://w3id.org/dpv/risk#" ;
    schema:version "0.8.2" .

dpv:RiskAssessment rdfs:superClassOf risk:RiskAnalysis ;
    skos:narrower risk:RiskAnalysis .

dpv:MaterialDamage skos:narrower risk:LossAssets,
        risk:LossFunds,
        risk:LossGoods,
        risk:Theft,
        risk:TheftEquipment,
        risk:TheftMedia .

dpv:Likelihood skos:narrower risk:3LikelihoodLevels,
        risk:5LikelihoodLevels,
        risk:7LikelihoodLevels .

dpv:RiskLevel skos:narrower risk:3RiskLevels,
        risk:5RiskLevels,
        risk:7RiskLevels .

dpv:Severity skos:narrower risk:3SeverityLevels,
        risk:5SeverityLevels,
        risk:7SeverityLevels .

dpv:Damage skos:narrower risk:CorruptionData,
        risk:DamageByThirdParty,
        risk:DataBreach,
        risk:EquipmentFailure,
        risk:FinancialLoss,
        risk:IllegalProcessingData,
        risk:InterceptionCommunications,
        risk:PublicOrderBreach,
        risk:UnauthorisedCodeModification,
        risk:UnauthorisedSystemModification,
        risk:UnwantedCodeDeletion,
        risk:UnwantedDataDeletion,
        risk:Vandalism,
        risk:ViolationCodeConduct,
        risk:ViolationContractualObligations,
        risk:ViolationEthicalCode,
        risk:ViolationRegulatoryObligations,
        risk:ViolationStatutoryObligations .

risk:risk-controls-classes a skos:ConceptScheme .

dpv:NonMaterialDamage skos:narrower risk:CompromiseAccountSecurity,
        risk:CopyrightViolation,
        risk:CyberSpying,
        risk:CyberStalking,
        risk:Eavesdropping,
        risk:LossCompetitiveAdvantage,
        risk:LossControlOverData,
        risk:LossCustomers,
        risk:LossData,
        risk:LossProprietaryInformation,
        risk:LossResources,
        risk:LossSuppliers,
        risk:LossTechnologicalAdvantage,
        risk:PersonnelAbsence,
        risk:PhysicalSpying,
        risk:PhysicalStalking,
        risk:RansomwareAttack,
        risk:RemoteSpying,
        risk:Spying,
        risk:Stalking,
        risk:UnauthorisedDataModification,
        risk:UnauthorisedImpersonation .

dpv:RiskMitigationMeasure skos:narrower risk:ControlConsequence,
        risk:ControlMonitors,
        risk:ControlRiskSource,
        risk:ReduceLikelihood,
        risk:ReduceSeverity,
        risk:ShareRisk .

dpv:Harm skos:narrower risk:AbusiveContentUtilisation,
        risk:AttackonPrivateLife,
        risk:Blackmail,
        risk:ChildViolence,
        risk:Coercion,
        risk:CompromiseAccount,
        risk:CompromiseAccountCredentials,
        risk:DangertoCustomers,
        risk:DangertoPersonnel,
        risk:Discrimination,
        risk:EnvironmentalSafetyEndangerment,
        risk:Extorsion,
        risk:Fraud,
        risk:HarmfulSpeech,
        risk:IdentityFraud,
        risk:IdentityTheft,
        risk:Injury,
        risk:LimitationOfRights,
        risk:PersonalSafetyEndangerment,
        risk:PhishingScam,
        risk:PhysicalAssault,
        risk:PreventExercisingOfRights,
        risk:PsychologicalHarm,
        risk:Sabotage,
        risk:Scam,
        risk:SexualViolence,
        risk:Spam,
        risk:Spoofing,
        risk:Terrorism,
        risk:ViolationOfRights .

risk:risk-levels-classes a skos:ConceptScheme .

risk:risk-methodology-classes a skos:ConceptScheme .

risk:risk-assessment-classes a skos:ConceptScheme .

dpv:Detriment skos:narrower risk:AuthorisationFailure,
        risk:BruteForceAuthorisations,
        risk:BusinessPerformanceImpairment,
        risk:Businessdisruption,
        risk:ConfidentialityBreach,
        risk:CostAcquisition,
        risk:CostBackup,
        risk:CostConfiguration,
        risk:CostInstallation,
        risk:CostJudicialPenalties,
        risk:CostJudicialProceedings,
        risk:CostOperationInterruption,
        risk:CostSuspendedOperations,
        risk:Cryptojacking,
        risk:DenialServiceAttack,
        risk:DetrimentToRecovery,
        risk:DistributedDenialServiceAttack,
        risk:EquipmentMalfunction,
        risk:ErrornousSystemUse,
        risk:FinancialEquipmentCosts,
        risk:FinancialInvestigationCosts,
        risk:FinancialPersonnelCosts,
        risk:FinancialRepairCosts,
        risk:GovernmentCrisis,
        risk:HumanErrors,
        risk:IdentityDispute,
        risk:IncreaseInternalCost,
        risk:IndustrialCrisis,
        risk:InternalOperationDisruption,
        risk:KnownVulnerabilityExploited,
        risk:LawEnforcementAdverseEffects,
        risk:LossCredibility,
        risk:LossCustomerConfidence,
        risk:LossGoodwill,
        risk:LossNegotiatingCapacity,
        risk:LossOpportunity,
        risk:LossReputation,
        risk:LossTrust,
        risk:MaliciousCodeAttack,
        risk:MalwareAttack,
        risk:MisinformationDisinformation,
        risk:MisuseBreachedInformation,
        risk:OrganisationDisruption,
        risk:ReplacementCosts,
        risk:RetrievalDeletedData,
        risk:RetrievalDiscardedEquipment,
        risk:ServiceInterruption,
        risk:SystemFailure,
        risk:SystemIntrusion,
        risk:SystemMalfunction,
        risk:ThirdPartyOperationDisruption,
        risk:UnauthorisedAccesstoPremises,
        risk:UnauthorisedCodeAccess,
        risk:UnauthorisedCodeDisclosure,
        risk:UnauthorisedDataAccess,
        risk:UnauthorisedDataDisclosure,
        risk:UnauthorisedInformationDisclosure,
        risk:UnauthorisedResourceUse,
        risk:UnauthorisedSystemAccess,
        risk:UnknownVulnerabilityExploited,
        risk:UnwantedDisclosureData,
        risk:VulnerabilityCreated,
        risk:VulnerabilityExploited .

risk:RiskManagement skos:narrower risk:ACSC-ISM,
        risk:ANSI-ISA-62443-3-2-2020,
        risk:BSI-200-2,
        risk:CCRACII,
        risk:CORAS,
        risk:CRAMM,
        risk:EBIOS,
        risk:ERM-IF,
        risk:ETSI-TS-102-165-1,
        risk:EU-ITSRM,
        risk:FAIR,
        risk:FAIR-Privacy,
        risk:GCSOS,
        risk:HITRUST-CSF,
        risk:IMO-MSC-FAL1-CIRC3,
        risk:IRAM2,
        risk:IS-BM,
        risk:ISACA-RISK-IT,
        risk:ISAMM,
        risk:ISO-IEC-27005-2018,
        risk:ISRAM,
        risk:IT-Grundschutz,
        risk:MAGERIT,
        risk:MEHARI,
        risk:MONARC,
        risk:NIST-SP-800-30,
        risk:NIST-SP-800-37,
        risk:NIST-SP-800-39,
        risk:NIST-SP-800-82,
        risk:O-RA,
        risk:OCTAVE,
        risk:OCTAVE-ALLEGRO,
        risk:OCTAVE-FORTE,
        risk:OCTAVE-S .

dpv:Impact skos:narrower risk:BusinessImpact,
        risk:CitizensImpact,
        risk:ComplianceImpact,
        risk:EconomicDisadvantage,
        risk:HealthLifeImpact,
        risk:ImpactOnDataSubject,
        risk:ImpacttoRights,
        risk:PrivacyImpact,
        risk:ReputationTrustImpact,
        risk:SocialDisadvantage .

risk:risk-matrix-classes a skos:ConceptScheme .

dpv:Consequence skos:narrower risk:ConsequenceForDataSubject,
        risk:ConsequenceOnDataSecurity,
        risk:SecurityBreach,
        risk:UnauthorisedReIdentification .

risk:risk-consequences-classes a skos:ConceptScheme .

