@prefix dcam: <http://purl.org/dc/dcam/> .
@prefix dcat: <http://www.w3.org/ns/dcat#> .
@prefix dct: <http://purl.org/dc/terms/> .
@prefix dex: <https://w3id.org/dpv/examples#> .
@prefix dpv: <https://w3id.org/dpv#> .
@prefix foaf: <http://xmlns.com/foaf/0.1/> .
@prefix owl: <http://www.w3.org/2002/07/owl#> .
@prefix rdf: <http://www.w3.org/1999/02/22-rdf-syntax-ns#> .
@prefix rdfs: <http://www.w3.org/2000/01/rdf-schema#> .
@prefix schema: <https://schema.org/> .
@prefix skos: <http://www.w3.org/2004/02/skos/core#> .
@prefix sw: <http://www.w3.org/2003/06/sw-vocab-status/ns#> .
@prefix vann: <http://purl.org/vocab/vann/> .
@prefix xsd: <http://www.w3.org/2001/XMLSchema#> .

dcat:Resource a rdfs:Class,
        owl:Class ;
    skos:prefLabel "dcat:Resource"@en ;
    skos:scopeNote "A dataset, data service, or any other resource associated with Right Exercise - such as for providing a copy of data"@en .

dpv:AcademicResearch a rdfs:Class,
        owl:Class,
        dpv:Purpose ;
    dct:contributor "Harshvardhan J. Pandit, Javier Fernandez, Axel Polleres, Elmar Kiesling, Fajar Ekaputra, Simon Steyskal" ;
    dct:created "2019-04-05"^^xsd:date ;
    rdfs:subClassOf dpv:ResearchAndDevelopment ;
    sw:term_status "accepted"@en ;
    skos:definition "Purposes associated with conducting or assisting with research conducted in an academic context e.g. within universities"@en ;
    skos:prefLabel "Academic Research"@en ;
    skos:related "svpu:Education"@en .

dpv:AcademicScientificOrganisation a rdfs:Class,
        owl:Class ;
    dct:contributor "Harshvardhan J. Pandit" ;
    dct:created "2022-02-02"^^xsd:date ;
    dct:modified "2020-10-05"^^xsd:date ;
    dct:source "(ADMS controlled vocabulary,http://purl.org/adms)"@en ;
    rdfs:subClassOf dpv:Organisation ;
    sw:term_status "accepted"@en ;
    skos:definition "Organisations related to academia or scientific pursuits e.g. Universities, Schools, Research Bodies"@en ;
    skos:prefLabel "Academic or Scientific Organisation"@en .

dpv:Access a rdfs:Class,
        owl:Class,
        dpv:Processing ;
    dct:contributor "Harshvardhan J. Pandit, Georg P Krog" ;
    dct:created "2022-06-15"^^xsd:date ;
    rdfs:subClassOf dpv:Use ;
    sw:term_status "accepted"@en ;
    skos:definition "to access data"@en ;
    skos:prefLabel "Access"@en .

dpv:AccessControlMethod a rdfs:Class,
        owl:Class,
        dpv:TechnicalMeasure ;
    dct:contributor "Axel Polleres, Rob Brennan, Harshvardhan J. Pandit, Mark Lizar" ;
    dct:created "2019-04-05"^^xsd:date ;
    vann:example dex:E0016 ;
    rdfs:subClassOf dpv:TechnicalMeasure ;
    sw:term_status "accepted"@en ;
    skos:definition "Methods which restrict access to a place or resource"@en ;
    skos:prefLabel "Access Control Method"@en .

dpv:AccountManagement a rdfs:Class,
        owl:Class,
        dpv:Purpose ;
    dct:contributor "Georg P Krog, Harshvardhan J. Pandit, Beatriz Esteves" ;
    dct:created "2021-09-08"^^xsd:date ;
    rdfs:subClassOf dpv:Purpose ;
    sw:term_status "accepted"@en ;
    skos:definition "Account Management refers to purposes associated with account management, such as to create, provide, maintain, and manage accounts"@en ;
    skos:prefLabel "Account Management"@en .

dpv:Acquire a rdfs:Class,
        owl:Class,
        dpv:Processing ;
    dct:created "2019-05-07"^^xsd:date ;
    dct:source "(GDPR Art.4-2,https://eur-lex.europa.eu/eli/reg/2016/679/art_4/par_2/oj)"@en ;
    rdfs:subClassOf dpv:Obtain ;
    sw:term_status "accepted"@en ;
    skos:definition "to come into possession or control of the data"@en ;
    skos:prefLabel "Acquire"@en .

dpv:ActiveRight a rdfs:Class,
        owl:Class,
        dpv:Right ;
    dct:contributor "Harshvardhan J Pandit, Beatriz Esteves, Georg P Krog, Paul Ryan" ;
    dct:created "2022-10-22"^^xsd:date ;
    rdfs:subClassOf dpv:Right ;
    sw:term_status "accepted"@en ;
    skos:definition "The right(s) applicable, provided, or expected that need to be (actively) exercised"@en ;
    skos:prefLabel "Active Right"@en ;
    skos:scopeNote "Active rights require the entity to expressly exercise them. For example, a Data Subject exercising their right to withdraw their consent."@en .

dpv:ActivityCompleted a rdfs:Class,
        owl:Class,
        dpv:ActivityStatus ;
    dct:contributor "Harshvardhan J. Pandit" ;
    dct:created "2022-05-18"^^xsd:date ;
    rdfs:subClassOf dpv:ActivityStatus ;
    sw:term_status "accepted"@en ;
    skos:definition "State of an activity that has completed i.e. is fully in the past"@en ;
    skos:prefLabel "Activity Completed"@en .

dpv:ActivityHalted a rdfs:Class,
        owl:Class,
        dpv:ActivityStatus ;
    dct:contributor "Harshvardhan J. Pandit" ;
    dct:created "2022-05-18"^^xsd:date ;
    rdfs:subClassOf dpv:ActivityStatus ;
    sw:term_status "accepted"@en ;
    skos:definition "State of an activity that was occuring in the past, and has been halted or paused or stoped"@en ;
    skos:prefLabel "Activity Halted"@en .

dpv:ActivityMonitoring a rdfs:Class,
        owl:Class,
        dpv:TechnicalMeasure ;
    dct:contributor "Harshvardhan J. Pandit" ;
    dct:created "2022-08-17"^^xsd:date ;
    dct:source "(ENISA Reference Incident Classification Taxonomy 2018,https://www.enisa.europa.eu/publications/reference-incident-classification-taxonomy/)"@en ;
    rdfs:subClassOf dpv:TechnicalMeasure ;
    sw:term_status "accepted"@en ;
    skos:definition "Monitoring of activities including assessing whether they have been successfully initiated and completed"@en ;
    skos:prefLabel "Activity Monitoring"@en .

dpv:ActivityNotCompleted a rdfs:Class,
        owl:Class,
        dpv:ActivityStatus ;
    dct:contributor "Harshvardhan J. Pandit" ;
    dct:created "2022-11-30"^^xsd:date ;
    rdfs:subClassOf dpv:ActivityStatus ;
    sw:term_status "accepted"@en ;
    skos:definition "State of an activity that could not be completed, but has reached some end state"@en ;
    skos:prefLabel "Acitivity Not Completed"@en ;
    skos:scopeNote "This relates to a 'Stop' state as distinct from a 'Halt' state. It makes no comments on whether the Acitivity can be resumed or continued towards completion."@en .

dpv:ActivityOngoing a rdfs:Class,
        owl:Class,
        dpv:ActivityStatus ;
    dct:contributor "Harshvardhan J. Pandit" ;
    dct:created "2022-05-18"^^xsd:date ;
    rdfs:subClassOf dpv:ActivityStatus ;
    sw:term_status "accepted"@en ;
    skos:definition "State of an activity occuring in continuation i.e. currently ongoing"@en ;
    skos:prefLabel "Activity Ongoing"@en .

dpv:ActivityProposed a rdfs:Class,
        owl:Class,
        dpv:ActivityStatus ;
    dct:contributor "Harshvardhan J. Pandit" ;
    dct:created "2022-05-18"^^xsd:date ;
    rdfs:subClassOf dpv:ActivityStatus ;
    sw:term_status "accepted"@en ;
    skos:definition "State of an activity being proposed or planned i.e. yet to occur"@en ;
    skos:prefLabel "Activity Proposed"@en .

dpv:ActivityStatus a rdfs:Class,
        owl:Class ;
    dct:contributor "Harshvardhan J. Pandit" ;
    dct:created "2022-05-18"^^xsd:date ;
    rdfs:subClassOf dpv:Status ;
    sw:term_status "accepted"@en ;
    skos:definition "Status associated with activity operations and lifecycles"@en ;
    skos:prefLabel "Activity Status"@en .

dpv:Adapt a rdfs:Class,
        owl:Class,
        dpv:Processing ;
    dct:created "2019-05-07"^^xsd:date ;
    dct:source "(GDPR Art.4-2,https://eur-lex.europa.eu/eli/reg/2016/679/art_4/par_2/oj)"@en ;
    rdfs:subClassOf dpv:Transform ;
    sw:term_status "accepted"@en ;
    skos:definition "to modify the data, often rewritten into a new form for a new use"@en ;
    skos:prefLabel "Adapt"@en .

dpv:Adult a rdfs:Class,
        owl:Class,
        dpv:DataSubject ;
    dct:contributor "Georg Krog" ;
    dct:created "2022-03-30"^^xsd:date ;
    rdfs:subClassOf dpv:DataSubject ;
    sw:term_status "accepted"@en ;
    skos:definition "A natural person that is not a child i.e. has attained some legally specified age of adulthood"@en ;
    skos:prefLabel "Adult"@en .

dpv:Advertising a rdfs:Class,
        owl:Class,
        dpv:Purpose ;
    dct:contributor "Georg P Krog, Harshvardhan J. Pandit, Beatriz Esteves" ;
    dct:created "2020-11-04"^^xsd:date ;
    rdfs:subClassOf dpv:Marketing ;
    sw:term_status "accepted"@en ;
    skos:definition "Purposes associated with conducting advertising i.e. process or artefact used to call attention to a product, service, etc. through announcements, notices, or other forms of communication"@en ;
    skos:prefLabel "Advertising"@en ;
    skos:scopeNote "Advertising is a subset of Marketing. Advertising by itself does not indicate 'personalisation' i.e. personalised ads."@en .

dpv:AlgorithmicLogic a rdfs:Class,
        owl:Class ;
    dct:contributor "Harshvardhan J. Pandit" ;
    dct:created "2022-01-26"^^xsd:date ;
    dct:modified "2023-12-10"^^xsd:date ;
    rdfs:subClassOf dpv:ProcessingContext ;
    sw:term_status "accepted"@en ;
    skos:definition "The algorithmic logic applied or used"@en ;
    skos:prefLabel "Algorithmic Logic"@en ;
    skos:scopeNote "Algorithmic Logic is intended as a broad concept for explaining the use of algorithms and automated decisions making within Processing. To describe the actual algorithm, see the Algorithm concept."@en .

dpv:Align a rdfs:Class,
        owl:Class,
        dpv:Processing ;
    dct:created "2019-05-07"^^xsd:date ;
    dct:source "(GDPR Art.4-2,https://eur-lex.europa.eu/eli/reg/2016/679/art_4/par_2/oj)"@en ;
    rdfs:subClassOf dpv:Transform ;
    sw:term_status "accepted"@en ;
    skos:definition "to adjust the data to be in relation to another data"@en ;
    skos:prefLabel "Align"@en .

dpv:Alter a rdfs:Class,
        owl:Class,
        dpv:Processing ;
    dct:created "2019-05-07"^^xsd:date ;
    dct:source "(GDPR Art.4-2,https://eur-lex.europa.eu/eli/reg/2016/679/art_4/par_2/oj)"@en ;
    rdfs:subClassOf dpv:Transform ;
    sw:term_status "accepted"@en ;
    skos:definition "to change the data without changing it into something else"@en ;
    skos:prefLabel "Alter"@en .

dpv:Analyse a rdfs:Class,
        owl:Class,
        dpv:Processing ;
    dct:created "2019-05-07"^^xsd:date ;
    dct:source "(SPECIAL Project,https://specialprivacy.ercim.eu/vocabs/processing)"@en ;
    rdfs:subClassOf dpv:Use ;
    sw:term_status "accepted"@en ;
    skos:definition "to study or examine the data in detail"@en ;
    skos:prefLabel "Analyse"@en ;
    skos:related "svpr:Analyse"@en .

dpv:Anonymisation a rdfs:Class,
        owl:Class,
        dpv:TechnicalMeasure ;
    dct:contributor "Axel Polleres, Rob Brennan, Harshvardhan J. Pandit, Mark Lizar" ;
    dct:created "2019-04-05"^^xsd:date ;
    dct:modified "2022-11-24"^^xsd:date ;
    dct:source "(ISO 29100:2011,https://www.iso.org/standard/45123.html)"@en ;
    rdfs:subClassOf dpv:Deidentification ;
    sw:term_status "modified"@en ;
    skos:definition "Anonymisation is the process by which data is irreversibly altered in such a way that a data subject can no longer be identified directly or indirectly, either by the entity holding the data alone or in collaboration with other entities and information sources"@en ;
    skos:prefLabel "Anonymisation"@en .

dpv:Anonymise a rdfs:Class,
        owl:Class,
        dpv:Processing ;
    dct:created "2019-05-07"^^xsd:date ;
    dct:source "(SPECIAL Project,https://specialprivacy.ercim.eu/vocabs/processing)"@en ;
    rdfs:subClassOf dpv:Transform ;
    sw:term_status "accepted"@en ;
    skos:definition "to irreversibly alter personal data in such a way that an unique data subject can no longer be identified directly or indirectly or in combination with other data"@en ;
    skos:prefLabel "Anonymise"@en ;
    skos:related "svpr:Anonymise"@en .

dpv:AnonymisedData a rdfs:Class,
        owl:Class ;
    dct:contributor "Piero Bonatti" ;
    dct:created "2022-01-19"^^xsd:date ;
    rdfs:subClassOf dpv:NonPersonalData ;
    sw:term_status "accepted"@en ;
    skos:definition "Personal Data that has been (fully and completely) anonymised so that it is no longer considered Personal Data"@en ;
    skos:prefLabel "Anonymised Data"@en ;
    skos:scopeNote "It is advised to carefully consider indicating data is fully or completely anonymised by determining whether the data by itself or in combination with other data can identify a person. Failing this condition, the data should be denoted as PseudonymisedData. To indicate data is anonymised only for a specified entity (e.g. within an organisation), the concept ContextuallyAnonymisedData (as subclass of PseudonymisedData) should be used instead of AnonymisedData."@en .

dpv:AntiTerrorismOperations a rdfs:Class,
        owl:Class,
        dpv:Purpose ;
    dct:contributor "Harshvardhan J. Pandit" ;
    dct:created "2022-04-20"^^xsd:date ;
    rdfs:subClassOf dpv:EnforceSecurity ;
    sw:term_status "accepted"@en ;
    skos:definition "Purposes associated with activities that detect, prevent, mitigate, or perform other activities for anti-terrorism"@en ;
    skos:prefLabel "Anti-Terrorism Operations"@en .

dpv:Applicant a rdfs:Class,
        owl:Class,
        dpv:DataSubject ;
    dct:contributor "Harshvardhan J. Pandit, Georg P. Krog, Julian Flake, Paul Ryan, Beatriz Esteves" ;
    dct:created "2022-04-06"^^xsd:date ;
    rdfs:subClassOf dpv:DataSubject ;
    sw:term_status "accepted"@en ;
    skos:definition "Data subjects that are applicants in some context"@en ;
    skos:prefLabel "Applicant"@en .

dpv:Assess a rdfs:Class,
        owl:Class,
        dpv:Processing ;
    dct:contributor "Harshvardhan J. Pandit, Georg P Krog" ;
    dct:created "2022-06-15"^^xsd:date ;
    rdfs:subClassOf dpv:Use ;
    sw:term_status "accepted"@en ;
    skos:definition "to assess data for some criteria"@en ;
    skos:prefLabel "Assess"@en .

dpv:Assessment a rdfs:Class,
        owl:Class,
        dpv:OrganisationalMeasure ;
    dct:contributor "Harshvardhan J. Pandit" ;
    dct:created "2021-09-08"^^xsd:date ;
    rdfs:subClassOf dpv:OrganisationalMeasure ;
    sw:term_status "accepted"@en ;
    skos:definition "The document, plan, or process for assessment or determination towards a purpose e.g. assessment of legality or impact assessments"@en ;
    skos:prefLabel "Assessment"@en .

dpv:AssetManagementProcedures a rdfs:Class,
        owl:Class,
        dpv:OrganisationalMeasure ;
    dct:contributor "Harshvardhan J. Pandit" ;
    dct:created "2022-08-17"^^xsd:date ;
    dct:source "(ENISA 5G Cybersecurity Standards,https://www.enisa.europa.eu/publications/5g-cybersecurity-standards)"@en ;
    rdfs:subClassOf dpv:GovernanceProcedures ;
    sw:term_status "accepted"@en ;
    skos:definition "Procedures related to management of assets"@en ;
    skos:prefLabel "Asset Management Procedures"@en .

dpv:AssistiveAutomation a rdfs:Class,
        owl:Class,
        dpv:Automation ;
    dct:created "2023-12-10"^^xsd:date ;
    rdfs:subClassOf dpv:Automation ;
    sw:term_status "accepted"@en ;
    skos:definition "The system assists an operator"@en ;
    skos:prefLabel "Assistive Automation"@en ;
    skos:scopeNote "Human Involvement is implied here, specifically the ability to make decisions regarding operations, but also possibly for intervention, oversight, and verification"@en .

dpv:AsylumSeeker a rdfs:Class,
        owl:Class,
        dpv:DataSubject ;
    dct:contributor "Georg P Krog" ;
    dct:created "2022-06-15"^^xsd:date ;
    rdfs:subClassOf dpv:VulnerableDataSubject ;
    sw:term_status "accepted"@en ;
    skos:definition "Data subjects that are asylum seekers"@en ;
    skos:prefLabel "Asylum Seeker"@en .

dpv:AsymmetricCryptography a rdfs:Class,
        owl:Class,
        dpv:TechnicalMeasure ;
    dct:contributor "Harshvardhan J. Pandit" ;
    dct:created "2022-08-17"^^xsd:date ;
    dct:source "(ENISA Reference Incident Classification Taxonomy 2018,https://www.enisa.europa.eu/publications/reference-incident-classification-taxonomy/)"@en ;
    rdfs:subClassOf dpv:CryptographicMethods ;
    sw:term_status "accepted"@en ;
    skos:definition "Use of public-key cryptography or asymmetric cryptography involving a public and private pair of keys"@en ;
    skos:prefLabel "Asymmetric Cryptography"@en .

dpv:AsymmetricEncryption a rdfs:Class,
        owl:Class,
        dpv:TechnicalMeasure ;
    dct:contributor "Harshvardhan J. Pandit" ;
    dct:created "2022-08-17"^^xsd:date ;
    dct:source "(ENISA Data Pseudonymisation: Advanced Techniques and Use Cases,https://www.enisa.europa.eu/publications/data-pseudonymisation-advanced-techniques-and-use-cases)"@en ;
    rdfs:subClassOf dpv:Encryption ;
    sw:term_status "accepted"@en ;
    skos:definition "Use of asymmetric cryptography to encrypt data"@en ;
    skos:prefLabel "Asymmetric Encryption"@en .

dpv:AuditApproved a rdfs:Class,
        owl:Class,
        dpv:AuditStatus ;
    dct:contributor "Harshvardhan J. Pandit" ;
    dct:created "2022-05-18"^^xsd:date ;
    rdfs:subClassOf dpv:AuditStatus ;
    sw:term_status "accepted"@en ;
    skos:definition "State of being approved through the audit"@en ;
    skos:prefLabel "Audit Approved"@en .

dpv:AuditConditionallyApproved a rdfs:Class,
        owl:Class,
        dpv:AuditStatus ;
    dct:contributor "Paul Ryan" ;
    dct:created "2022-06-29"^^xsd:date ;
    rdfs:subClassOf dpv:AuditStatus ;
    sw:term_status "accepted"@en ;
    skos:definition "State of being conditionally approved through the audit"@en ;
    skos:prefLabel "Audit Conditionally Approved"@en ;
    skos:scopeNote "A \"conditional approval\" is intended to reflect states where the audit has identified further changes which must be implemented before considering the audit has been 'passed', without requiring another audit to validate them. This is distinct from the case where an audit has state 'rejected', which means changes must be made and submitted for review. The requirements of a 'conditional acceptance' are expected to be minor or not significant enough to warrant another audit to review them."@en .

dpv:AuditNotRequired a rdfs:Class,
        owl:Class,
        dpv:AuditStatus ;
    dct:contributor "Harshvardhan J. Pandit" ;
    dct:created "2022-05-18"^^xsd:date ;
    rdfs:subClassOf dpv:AuditStatus ;
    sw:term_status "accepted"@en ;
    skos:definition "State where an audit is determined as not being required"@en ;
    skos:prefLabel "Audit Not Required"@en .

dpv:AuditRejected a rdfs:Class,
        owl:Class,
        dpv:AuditStatus ;
    dct:contributor "Harshvardhan J. Pandit" ;
    dct:created "2022-05-18"^^xsd:date ;
    rdfs:subClassOf dpv:AuditStatus ;
    sw:term_status "accepted"@en ;
    skos:definition "State of not being approved or being rejected through the audit"@en ;
    skos:prefLabel "Audit Rejected"@en .

dpv:AuditRequested a rdfs:Class,
        owl:Class,
        dpv:AuditStatus ;
    dct:contributor "Harshvardhan J. Pandit" ;
    dct:created "2022-05-18"^^xsd:date ;
    rdfs:subClassOf dpv:AuditStatus ;
    sw:term_status "accepted"@en ;
    skos:definition "State of an audit being requested whose outcome is not yet known"@en ;
    skos:prefLabel "Audit Requested"@en .

dpv:AuditRequired a rdfs:Class,
        owl:Class,
        dpv:AuditStatus ;
    dct:contributor "Harshvardhan J. Pandit" ;
    dct:created "2022-05-18"^^xsd:date ;
    rdfs:subClassOf dpv:AuditStatus ;
    sw:term_status "accepted"@en ;
    skos:definition "State where an audit is determined as being required but has not been conducted"@en ;
    skos:prefLabel "Audit Required"@en .

dpv:AuditStatus a rdfs:Class,
        owl:Class ;
    dct:contributor "Harshvardhan J. Pandit" ;
    dct:created "2022-05-18"^^xsd:date ;
    rdfs:subClassOf dpv:Status ;
    sw:term_status "accepted"@en ;
    skos:definition "Status associated with Auditing or Investigation"@en ;
    skos:prefLabel "Audit Status"@en .

dpv:Authentication-ABC a rdfs:Class,
        owl:Class,
        dpv:TechnicalMeasure ;
    dct:contributor "Harshvardhan J. Pandit" ;
    dct:created "2022-08-17"^^xsd:date ;
    dct:source "(ENISA Data Protection Engineering,https://www.enisa.europa.eu/publications/data-protection-engineering)"@en ;
    rdfs:subClassOf dpv:CryptographicAuthentication ;
    sw:term_status "accepted"@en ;
    skos:definition "Use of Attribute Based Credentials (ABC) to perform and manage authentication"@en ;
    skos:prefLabel "Authentication using ABC"@en .

dpv:Authentication-PABC a rdfs:Class,
        owl:Class,
        dpv:TechnicalMeasure ;
    dct:contributor "Harshvardhan J. Pandit" ;
    dct:created "2022-08-17"^^xsd:date ;
    dct:source "(ENISA Data Protection Engineering,https://www.enisa.europa.eu/publications/data-protection-engineering)"@en ;
    rdfs:subClassOf dpv:CryptographicAuthentication ;
    sw:term_status "accepted"@en ;
    skos:definition "Use of Privacy-enhancing Attribute Based Credentials (ABC) to perform and manage authentication"@en ;
    skos:prefLabel "Authentication using PABC"@en .

dpv:AuthenticationProtocols a rdfs:Class,
        owl:Class,
        dpv:TechnicalMeasure ;
    dct:contributor "Axel Polleres, Rob Brennan, Harshvardhan J. Pandit, Mark Lizar" ;
    dct:created "2019-04-05"^^xsd:date ;
    rdfs:subClassOf dpv:TechnicalMeasure ;
    sw:term_status "accepted"@en ;
    skos:definition "Protocols involving validation of identity i.e. authentication of a person or information"@en ;
    skos:prefLabel "Authentication Protocols"@en .

dpv:AuthorisationProcedure a rdfs:Class,
        owl:Class,
        dpv:OrganisationalMeasure ;
    dct:contributor "Axel Polleres, Rob Brennan, Harshvardhan J. Pandit, Mark Lizar" ;
    dct:created "2019-04-05"^^xsd:date ;
    rdfs:subClassOf dpv:OrganisationalMeasure ;
    sw:term_status "accepted"@en ;
    skos:definition "Procedures for determining authorisation through permission or authority"@en ;
    skos:prefLabel "Authorisation Procedure"@en ;
    skos:scopeNote "non-technical authorisation procedures: How is it described on an organisational level, who gets access to the data"@en .

dpv:AuthorisationProtocols a rdfs:Class,
        owl:Class,
        dpv:TechnicalMeasure ;
    dct:contributor "Harshvardhan J. Pandit" ;
    dct:created "2022-08-17"^^xsd:date ;
    dct:source "(ENISA Reference Incident Classification Taxonomy 2018,https://www.enisa.europa.eu/publications/reference-incident-classification-taxonomy/)"@en ;
    rdfs:subClassOf dpv:TechnicalMeasure ;
    sw:term_status "accepted"@en ;
    skos:definition "Protocols involving authorisation of roles or profiles to determine permission, rights, or privileges"@en ;
    skos:prefLabel "Authorisation Protocols"@en .

dpv:Authority a rdfs:Class,
        owl:Class ;
    dct:contributor "Georg Krog, Paul Ryan, Harshvardhan Pandit" ;
    dct:created "2020-11-04"^^xsd:date ;
    rdfs:subClassOf dpv:GovernmentalOrganisation ;
    rdfs:superClassOf dpv:DataProtectionAuthority,
        dpv:NationalAuthority,
        dpv:RegionalAuthority,
        dpv:SupraNationalAuthority ;
    sw:term_status "accepted"@en ;
    skos:definition "An authority with the power to create or enforce laws, or determine their compliance."@en ;
    skos:prefLabel "Authority"@en .

dpv:AutomatedDecisionMaking a rdfs:Class,
        owl:Class ;
    dct:contributor "Harshvardhan J. Pandit, Piero Bonatti" ;
    dct:created "2020-11-04"^^xsd:date ;
    dct:modified "2022-09-07"^^xsd:date ;
    dct:source "(GDPR Art.4-2,https://eur-lex.europa.eu/eli/reg/2016/679/art_4/par_2/oj)"@en ;
    rdfs:subClassOf dpv:DecisionMaking ;
    sw:term_status "accepted"@en ;
    skos:definition "Processing that involves automated decision making"@en ;
    skos:prefLabel "Automated Decision Making"@en ;
    skos:scopeNote "Automated decision making can be defined as “the ability to make decisions by technological means without human involvement.” (“Guidelines on Automated individual decision-making and Profiling for the purposes of Regulation 2016/679 (wp251rev.01)”, 2018, p. 8)"@en .

dpv:Automation a rdfs:Class,
        owl:Class ;
    dct:created "2023-12-10"^^xsd:date ;
    vann:example dex:E0013 ;
    rdfs:subClassOf dpv:ProcessingContext ;
    sw:term_status "accepted"@en ;
    skos:definition "Indication of degree or level of automation associated with specified context"@en ;
    skos:prefLabel "Automation"@en .

dpv:Autonomous a rdfs:Class,
        owl:Class,
        dpv:Automation ;
    dct:created "2023-12-10"^^xsd:date ;
    dct:source "(ISO/IEC 22989:2022 Artificial intelligence concepts and terminology,https://www.iso.org/standard/74296.html)"@en ;
    rdfs:subClassOf dpv:Automation ;
    sw:term_status "accepted"@en ;
    skos:definition "The system is capable of modifying its operation domain or its goals without external intervention, control or oversight"@en ;
    skos:prefLabel "Autonomous"@en ;
    skos:scopeNote "Though Autonomous, such operations can still be associated with dpv:HumanInvolved e.g. for inputs, oversight or verification"@en .

dpv:BackgroundChecks a rdfs:Class,
        owl:Class,
        dpv:OrganisationalMeasure ;
    dct:contributor "Harshvardhan J. Pandit" ;
    dct:created "2022-08-17"^^xsd:date ;
    dct:source "(ENISA 5G Cybersecurity Standards,https://www.enisa.europa.eu/publications/5g-cybersecurity-standards)"@en ;
    rdfs:subClassOf dpv:SecurityProcedure ;
    sw:term_status "accepted"@en ;
    skos:definition "Procedure where the background of an entity is assessed to identity vulnerabilities and threats due to their current or intended role"@en ;
    skos:prefLabel "Background Checks"@en .

dpv:Benefit a rdfs:Class,
        owl:Class,
        dpv:Impact ;
    dct:contributor "Harshvardhan J. Pandit, Julian Flake, Georg P Krog, Fajar Ekaputra, Beatriz Esteves, Axel Polleres" ;
    dct:created "2022-03-23"^^xsd:date ;
    rdfs:subClassOf dpv:Impact ;
    sw:term_status "accepted"@en ;
    skos:definition "Impact(s) that acts as or causes benefits"@en ;
    skos:prefLabel "Benefit"@en .

dpv:BiometricAuthentication a rdfs:Class,
        owl:Class,
        dpv:TechnicalMeasure ;
    dct:contributor "Harshvardhan J. Pandit" ;
    dct:created "2022-08-17"^^xsd:date ;
    dct:source "(ENISA Reference Incident Classification Taxonomy 2018,https://www.enisa.europa.eu/publications/reference-incident-classification-taxonomy/)"@en ;
    rdfs:subClassOf dpv:AuthenticationProtocols ;
    sw:term_status "accepted"@en ;
    skos:definition "Use of biometric data for authentication"@en ;
    skos:prefLabel "Biometric Authentication"@en .

dpv:Certification a rdfs:Class,
        owl:Class,
        dpv:OrganisationalMeasure ;
    dct:contributor "Axel Polleres, Rob Brennan, Harshvardhan J. Pandit, Mark Lizar" ;
    dct:created "2019-04-05"^^xsd:date ;
    rdfs:subClassOf dpv:CertificationSeal ;
    sw:term_status "accepted"@en ;
    skos:definition "Certification mechanisms, seals, and marks for the purpose of demonstrating compliance"@en ;
    skos:prefLabel "Certification"@en .

dpv:CertificationSeal a rdfs:Class,
        owl:Class,
        dpv:OrganisationalMeasure ;
    dct:contributor "Axel Polleres, Rob Brennan, Harshvardhan J. Pandit, Mark Lizar" ;
    dct:created "2019-04-05"^^xsd:date ;
    rdfs:subClassOf dpv:OrganisationalMeasure ;
    sw:term_status "accepted"@en ;
    skos:definition "Certifications, seals, and marks indicating compliance to regulations or practices"@en ;
    skos:prefLabel "Certification and Seal"@en .

dpv:Child a rdfs:Class,
        owl:Class,
        dpv:DataSubject ;
    dct:contributor "Harshvardhan J. Pandit" ;
    dct:created "2020-11-25"^^xsd:date ;
    dct:modified "2022-06-22"^^xsd:date ;
    rdfs:subClassOf dpv:DataSubject ;
    sw:term_status "accepted"@en ;
    skos:definition "A 'child' is a natural legal person who is below a certain legal age depending on the legal jurisdiction."@en ;
    skos:prefLabel "Child"@en ;
    skos:scopeNote "The legality of age defining a child varies by jurisdiction. In addition, 'child' is distinct from a 'minor'. For example, the legal age for consumption of alcohol can be 21, which makes a person of age 20 a 'minor' in this context. In other cases, 'minor' and 'child' are used interchangeably to refer to a person below some legally defined age."@en .

dpv:Citizen a rdfs:Class,
        owl:Class,
        dpv:DataSubject ;
    dct:contributor "Harshvardhan J. Pandit, Georg P. Krog, Julian Flake, Paul Ryan, Beatriz Esteves" ;
    dct:created "2022-04-06"^^xsd:date ;
    rdfs:subClassOf dpv:DataSubject ;
    sw:term_status "accepted"@en ;
    skos:definition "Data subjects that are citizens (for a jurisdiction)"@en ;
    skos:prefLabel "Citizen"@en .

dpv:City a rdfs:Class,
        owl:Class ;
    dct:contributor "Harshvardhan J. Pandit" ;
    dct:created "2022-10-22"^^xsd:date ;
    rdfs:subClassOf dpv:Region ;
    sw:term_status "accepted"@en ;
    skos:definition "A region consisting of urban population and commerce"@en ;
    skos:prefLabel "City"@en .

dpv:Client a rdfs:Class,
        owl:Class,
        dpv:DataSubject ;
    dct:contributor "Harshvardhan J. Pandit, Georg P. Krog, Julian Flake, Paul Ryan, Beatriz Esteves" ;
    dct:created "2022-04-06"^^xsd:date ;
    rdfs:subClassOf dpv:Customer ;
    sw:term_status "accepted"@en ;
    skos:definition "Data subjects that are clients or recipients of services"@en ;
    skos:prefLabel "Client"@en .

dpv:CloudLocation a rdfs:Class,
        owl:Class,
        dpv:Location ;
    dct:contributor "Harshvardhan J. Pandit" ;
    dct:created "2022-06-15"^^xsd:date ;
    dct:modified "2020-10-05"^^xsd:date ;
    rdfs:subClassOf dpv:RemoteLocation ;
    sw:term_status "accepted"@en ;
    skos:definition "Location that is in the 'cloud' i.e. a logical location operated over the internet"@en ;
    skos:prefLabel "Cloud Location"@en .

dpv:CodeOfConduct a rdfs:Class,
        owl:Class,
        dpv:OrganisationalMeasure ;
    dct:contributor "Axel Polleres, Rob Brennan, Harshvardhan J. Pandit, Mark Lizar" ;
    dct:created "2019-04-05"^^xsd:date ;
    rdfs:subClassOf dpv:GuidelinesPrinciple ;
    sw:term_status "accepted"@en ;
    skos:definition "A set of rules or procedures outlining the norms and practices for conducting activities"@en ;
    skos:prefLabel "Code of Conduct"@en .

dpv:Collect a rdfs:Class,
        owl:Class,
        dpv:Processing ;
    dct:created "2019-05-07"^^xsd:date ;
    dct:source "(GDPR Art.4-2,https://eur-lex.europa.eu/eli/reg/2016/679/art_4/par_2/oj), (SPECIAL Project,https://specialprivacy.ercim.eu/vocabs/processing)"@en ;
    vann:example dex:E0018 ;
    rdfs:subClassOf dpv:Obtain ;
    sw:term_status "accepted"@en ;
    skos:definition "to gather data from someone"@en ;
    skos:prefLabel "Collect"@en ;
    skos:related "svpr:Collect"@en .

dpv:CollectedData a rdfs:Class,
        owl:Class ;
    dct:created "2023-12-10"^^xsd:date ;
    rdfs:subClassOf dpv:Data ;
    rdfs:superClassOf dpv:CollectedPersonalData ;
    sw:term_status "accepted"@en ;
    skos:definition "Data that has been obtained by collecting it from a source"@en ;
    skos:prefLabel "Collected Data"@en .

dpv:CollectedPersonalData a rdfs:Class,
        owl:Class ;
    dct:contributor "Harshvardhan J. Pandit" ;
    dct:created "2022-03-30"^^xsd:date ;
    dct:modified "2023-12-10"^^xsd:date ;
    rdfs:subClassOf dpv:CollectedData,
        dpv:PersonalData ;
    sw:term_status "accepted"@en ;
    skos:definition "Personal Data that has been collected from another source such as the Data Subject"@en ;
    skos:prefLabel "Collected Personal Data"@en ;
    skos:scopeNote "To indicate the source of data, use the DataSource concept with the hasDataSource relation"@en .

dpv:Combine a rdfs:Class,
        owl:Class,
        dpv:Processing ;
    dct:created "2019-05-07"^^xsd:date ;
    dct:source "(GDPR Art.4-2,https://eur-lex.europa.eu/eli/reg/2016/679/art_4/par_2/oj), (SPECIAL Project,https://specialprivacy.ercim.eu/vocabs/processing)"@en ;
    rdfs:subClassOf dpv:Transform ;
    sw:term_status "accepted"@en ;
    skos:definition "to join or merge data"@en ;
    skos:prefLabel "Combine"@en ;
    skos:related "svpr:Aggregate"@en .

dpv:CommercialResearch a rdfs:Class,
        owl:Class,
        dpv:Purpose ;
    dct:contributor "Harshvardhan J. Pandit, Javier Fernandez, Axel Polleres, Elmar Kiesling, Fajar Ekaputra, Simon Steyskal" ;
    dct:created "2019-04-05"^^xsd:date ;
    rdfs:subClassOf dpv:ResearchAndDevelopment ;
    sw:term_status "accepted"@en ;
    skos:definition "Purposes associated with conducting research in a commercial setting or with intention to commercialise e.g. in a company or sponsored by a company"@en ;
    skos:prefLabel "Commercial Research"@en ;
    skos:related "svpu:Develop"@en .

dpv:CommerciallyConfidentialData a rdfs:Class,
        owl:Class ;
    dct:source "DGA 6.5(c)"@en ;
    rdfs:subClassOf dpv:Data ;
    sw:term_status "accepted"@en ;
    skos:definition "Data protected through Commercial Confidentiality Agreements"@en ;
    skos:prefLabel "CommerciallyConfidentialData"@en .

dpv:CommunicationForCustomerCare a rdfs:Class,
        owl:Class,
        dpv:Purpose ;
    dct:contributor "Georg P Krog, Harshvardhan J. Pandit, Beatriz Esteves" ;
    dct:created "2020-11-04"^^xsd:date ;
    rdfs:subClassOf dpv:CommunicationManagement,
        dpv:CustomerCare ;
    sw:term_status "accepted"@en ;
    skos:definition "Customer Care Communication refers to purposes associated with communicating with customers for assisting them, resolving issues, ensuring satisfaction, etc. in relation to services provided"@en ;
    skos:prefLabel "Communication for Customer Care"@en .

dpv:CommunicationManagement a rdfs:Class,
        owl:Class,
        dpv:Purpose ;
    dct:contributor "Georg P Krog, Paul Ryan, David Hickey, Harshvardhan J. Pandit" ;
    dct:created "2021-09-01"^^xsd:date ;
    rdfs:subClassOf dpv:Purpose ;
    sw:term_status "accepted"@en ;
    skos:definition "Communication Management refers to purposes associated with providing or managing communication activities e.g. to send an email for notifying some information"@en ;
    skos:prefLabel "Communication Management"@en ;
    skos:scopeNote "This purpose by itself does not sufficiently and clearly indicate what the communication is about. As such, it is recommended to combine it with another purpose to indicate the application. For example, Communication of Payment."@en .

dpv:ComplianceIndeterminate a rdfs:Class,
        owl:Class,
        dpv:ComplianceStatus ;
    dct:contributor "Harshvardhan J. Pandit" ;
    dct:created "2022-09-07"^^xsd:date ;
    rdfs:subClassOf dpv:ComplianceStatus ;
    sw:term_status "accepted"@en ;
    skos:definition "State where the status of compliance has not been fully assessed, evaluated, or determined"@en ;
    skos:prefLabel "Compliance Indeterminate"@en .

dpv:ComplianceMonitoring a rdfs:Class,
        owl:Class,
        dpv:OrganisationalMeasure ;
    dct:contributor "Harshvardhan J. Pandit" ;
    dct:created "2022-08-17"^^xsd:date ;
    dct:source "(ENISA 5G Cybersecurity Standards,https://www.enisa.europa.eu/publications/5g-cybersecurity-standards)"@en ;
    rdfs:subClassOf dpv:GovernanceProcedures ;
    sw:term_status "accepted"@en ;
    skos:definition "Monitoring of compliance (e.g. internal policy, regulations)"@en ;
    skos:prefLabel "Compliance Monitoring"@en .

dpv:ComplianceStatus a rdfs:Class,
        owl:Class ;
    dct:contributor "Harshvardhan J. Pandit" ;
    dct:created "2022-05-18"^^xsd:date ;
    rdfs:subClassOf dpv:Status ;
    rdfs:superClassOf dpv:Lawfulness ;
    sw:term_status "accepted"@en ;
    skos:definition "Status associated with Compliance with some norms, objectives, or requirements"@en ;
    skos:prefLabel "Compliance Status"@en .

dpv:ComplianceUnknown a rdfs:Class,
        owl:Class,
        dpv:ComplianceStatus ;
    dct:contributor "Harshvardhan J. Pandit" ;
    dct:created "2022-09-07"^^xsd:date ;
    rdfs:subClassOf dpv:ComplianceStatus ;
    sw:term_status "accepted"@en ;
    skos:definition "State where the status of compliance is unknown"@en ;
    skos:prefLabel "Compliance Unknown"@en .

dpv:ComplianceViolation a rdfs:Class,
        owl:Class,
        dpv:ComplianceStatus ;
    dct:contributor "Harshvardhan J. Pandit" ;
    dct:created "2022-05-18"^^xsd:date ;
    dct:modified "2022-09-07"^^xsd:date ;
    rdfs:subClassOf dpv:ComplianceStatus ;
    sw:term_status "accepted"@en ;
    skos:definition "State where compliance cannot be achieved due to requirements being violated"@en ;
    skos:prefLabel "Compliance Violation"@en ;
    skos:scopeNote "Changed from \"violation of compliance\" for consistency with other terms"@en .

dpv:Compliant a rdfs:Class,
        owl:Class,
        dpv:ComplianceStatus ;
    dct:contributor "Harshvardhan J. Pandit" ;
    dct:created "2022-05-18"^^xsd:date ;
    rdfs:subClassOf dpv:ComplianceStatus ;
    sw:term_status "accepted"@en ;
    skos:definition "State of being fully compliant"@en ;
    skos:prefLabel "Compliant"@en .

dpv:ConditionalAutomation a rdfs:Class,
        owl:Class,
        dpv:Automation ;
    dct:created "2023-12-10"^^xsd:date ;
    rdfs:subClassOf dpv:Automation ;
    sw:term_status "accepted"@en ;
    skos:definition "Sustained and specific performance by a system, with an external agent ready to take over when necessary"@en ;
    skos:prefLabel "Conditional Automation"@en ;
    skos:scopeNote "Human Involvement is implied here, e.g. for intervention, input, decisions"@en .

dpv:ConfidentialData a rdfs:Class,
        owl:Class ;
    dct:source "DGA 5.10"@en ;
    rdfs:subClassOf dpv:Data ;
    sw:term_status "accepted"@en ;
    skos:definition "Data deemed confidential"@en ;
    skos:prefLabel "ConfidentialData"@en .

dpv:ConformanceStatus a rdfs:Class,
        owl:Class ;
    dct:contributor "Harshvardhan J. Pandit" ;
    dct:created "2022-10-22"^^xsd:date ;
    rdfs:subClassOf dpv:Status ;
    sw:term_status "accepted"@en ;
    skos:definition "Status associated with conformance to a standard, guideline, code, or recommendation"@en ;
    skos:prefLabel "Conformance Status"@en .

dpv:Conformant a rdfs:Class,
        owl:Class,
        dpv:ConformanceStatus ;
    dct:contributor "Harshvardhan J. Pandit" ;
    dct:created "2022-10-22"^^xsd:date ;
    rdfs:subClassOf dpv:ConformanceStatus ;
    sw:term_status "accepted"@en ;
    skos:definition "State of being conformant"@en ;
    skos:prefLabel "Conformant"@en .

dpv:Consent a rdfs:Class,
        owl:Class,
        dpv:LegalBasis ;
    dct:contributor "Harshvardhan J. Pandit" ;
    dct:created "2021-04-07"^^xsd:date ;
    vann:example dex:E0019,
        dex:E0022,
        dex:E0023,
        dex:E0024,
        dex:E0025,
        dex:E0026 ;
    rdfs:subClassOf dpv:LegalBasis ;
    sw:term_status "accepted"@en ;
    skos:definition "Consent of the Data Subject for specified processing"@en ;
    skos:prefLabel "Consent"@en .

dpv:ConsentExpired a rdfs:Class,
        owl:Class,
        dpv:ConsentStatus ;
    dct:contributor "Georg P Krog, Harshvardhan J. Pandit, Paul Ryan, Julian Flake" ;
    dct:created "2022-06-22"^^xsd:date ;
    dct:source "(GConsent,https://w3id.org/GConsent)"@en ;
    rdfs:subClassOf dpv:ConsentStatusInvalidForProcessing ;
    sw:term_status "accepted"@en ;
    skos:definition "The state where the temporal or contextual validity of consent has 'expired'"@en ;
    skos:prefLabel "Consent Expired"@en ;
    skos:scopeNote "An example of this state is when the obtained consent has been assigned a duration - which has lapsed or 'expired', making it invalid to be used further for processing data"@en .

dpv:ConsentGiven a rdfs:Class,
        owl:Class,
        dpv:ConsentStatus ;
    dct:contributor "Georg P Krog, Harshvardhan J. Pandit, Paul Ryan, Julian Flake" ;
    dct:created "2022-06-22"^^xsd:date ;
    dct:source "(GConsent,https://w3id.org/GConsent)"@en ;
    rdfs:subClassOf dpv:ConsentStatusValidForProcessing ;
    sw:term_status "accepted"@en ;
    skos:definition "The state where consent has been given"@en ;
    skos:prefLabel "Consent Given"@en ;
    skos:scopeNote "An example of this state is when the individual clicks on a button, ticks a checkbox, verbally agrees - or any other form that communicates their decision agreeing to the processing of data"@en .

dpv:ConsentInvalidated a rdfs:Class,
        owl:Class,
        dpv:ConsentStatus ;
    dct:contributor "Georg P Krog, Harshvardhan J. Pandit, Paul Ryan, Julian Flake" ;
    dct:created "2022-06-22"^^xsd:date ;
    dct:source "(GConsent,https://w3id.org/GConsent)"@en ;
    rdfs:subClassOf dpv:ConsentStatusInvalidForProcessing ;
    sw:term_status "accepted"@en ;
    skos:definition "The state where consent has been deemed to be invalid"@en ;
    skos:prefLabel "Consent Invalidated"@en ;
    skos:scopeNote "An example of this state is where an investigating authority or a court finds the collected consent did not meet requirements, and 'invalidates' both prior and future uses of it to carry out processing"@en .

dpv:ConsentNotice a rdfs:Class,
        owl:Class,
        dpv:OrganisationalMeasure ;
    dct:contributor "Georg P Krog, Harshvardhan J. Pandit, Paul Ryan, Julian Flake" ;
    dct:created "2022-06-21"^^xsd:date ;
    rdfs:subClassOf dpv:PrivacyNotice ;
    sw:term_status "accepted"@en ;
    skos:definition "A Notice for information provision associated with Consent"@en ;
    skos:prefLabel "Consent Notice"@en .

dpv:ConsentRecord a rdfs:Class,
        owl:Class,
        dpv:OrganisationalMeasure ;
    dct:contributor "Georg P Krog, Harshvardhan J. Pandit, Paul Ryan, Julian Flake" ;
    dct:created "2022-06-22"^^xsd:date ;
    vann:example dex:E0019 ;
    rdfs:subClassOf dpv:DataProcessingRecord ;
    sw:term_status "accepted"@en ;
    skos:definition "A Record of Consent or Consent related activities"@en ;
    skos:prefLabel "Consent Record"@en .

dpv:ConsentRefused a rdfs:Class,
        owl:Class,
        dpv:ConsentStatus ;
    dct:contributor "Georg P Krog, Harshvardhan J. Pandit, Paul Ryan, Julian Flake" ;
    dct:created "2022-06-22"^^xsd:date ;
    dct:source "(GConsent,https://w3id.org/GConsent)"@en ;
    rdfs:subClassOf dpv:ConsentStatusInvalidForProcessing ;
    sw:term_status "accepted"@en ;
    skos:definition "The state where consent has been refused"@en ;
    skos:prefLabel "Consent Refused"@en ;
    skos:scopeNote "An example of this state is when the individual clicks on a 'disagree' or 'reject' or 'refuse' button, or leaves a checkbox unticked"@en .

dpv:ConsentRequestDeferred a rdfs:Class,
        owl:Class,
        dpv:ConsentStatus ;
    dct:contributor "Georg P Krog, Harshvardhan J. Pandit, Paul Ryan, Julian Flake" ;
    dct:created "2022-06-22"^^xsd:date ;
    dct:source "(GConsent,https://w3id.org/GConsent)"@en ;
    rdfs:subClassOf dpv:ConsentStatusInvalidForProcessing ;
    sw:term_status "accepted"@en ;
    skos:definition "State where a request for consent has been deferred without a decision"@en ;
    skos:prefLabel "Consent Request Deferred"@en ;
    skos:scopeNote "An example of this state is when the individual closes or dismisses a notice without making a decision. This state is intended for making the distinction between a notice being provided (as a consent request) and the individual interacting with the notice without making a decision - where the 'ignoring of a notice' is taken as consent being neither given nor refused"@en .

dpv:ConsentRequested a rdfs:Class,
        owl:Class,
        dpv:ConsentStatus ;
    dct:contributor "Georg P Krog, Harshvardhan J. Pandit, Paul Ryan, Julian Flake" ;
    dct:created "2022-06-22"^^xsd:date ;
    dct:source "(GConsent,https://w3id.org/GConsent)"@en ;
    rdfs:subClassOf dpv:ConsentStatusInvalidForProcessing ;
    sw:term_status "accepted"@en ;
    skos:definition "State where a request for consent has been made and is awaiting a decision"@en ;
    skos:prefLabel "Consent Requested"@en ;
    skos:scopeNote "An example of this state is when a notice has been presented to the individual but they have not made a decision"@en .

dpv:ConsentRevoked a rdfs:Class,
        owl:Class,
        dpv:ConsentStatus ;
    dct:contributor "Georg P Krog, Harshvardhan J. Pandit, Paul Ryan, Julian Flake" ;
    dct:created "2022-06-22"^^xsd:date ;
    dct:source "(GConsent,https://w3id.org/GConsent)"@en ;
    rdfs:subClassOf dpv:ConsentStatusInvalidForProcessing ;
    sw:term_status "accepted"@en ;
    skos:definition "The state where the consent is revoked by an entity other than the data subject and which prevents it from being further used as a valid state"@en ;
    skos:prefLabel "Consent Revoked"@en ;
    skos:scopeNote "An example of this state is when a Data Controller stops utilising previously obtaining consent, such as when that service no longer exists"@en .

dpv:ConsentStatus a rdfs:Class,
        owl:Class ;
    dct:contributor "Georg P Krog, Harshvardhan J. Pandit, Paul Ryan, Julian Flake" ;
    dct:created "2022-06-22"^^xsd:date ;
    dct:source "(GConsent,https://w3id.org/GConsent)"@en ;
    vann:example dex:E0019,
        dex:E0024,
        dex:E0025,
        dex:E0026 ;
    rdfs:subClassOf dpv:Status ;
    sw:term_status "accepted"@en ;
    skos:definition "The state or status of 'consent' that provides information reflecting its operational status and validity for processing data"@en ;
    skos:prefLabel "Consent Status"@en ;
    skos:scopeNote "States are useful as information artefacts to implement them in controlling processing, and to reflect the process and flow of obtaining and maintaining consent. For example, a database table that stores consent states for specific processing and can be queried to obtain them in an efficient manner. States are also useful in investigations to determine the use and validity of consenting practices"@en .

dpv:ConsentStatusInvalidForProcessing a rdfs:Class,
        owl:Class,
        dpv:ConsentStatus ;
    dct:contributor "Georg P Krog, Harshvardhan J. Pandit, Paul Ryan, Julian Flake" ;
    dct:created "2022-06-22"^^xsd:date ;
    dct:source "(GConsent,https://w3id.org/GConsent)"@en ;
    rdfs:subClassOf dpv:ConsentStatus ;
    sw:term_status "accepted"@en ;
    skos:definition "States of consent that cannot be used as valid justifications for processing data"@en ;
    skos:prefLabel "Consent Status Invalid for Processing"@en ;
    skos:scopeNote "This identifies the stages associated with consent that should not be used to process data"@en .

dpv:ConsentStatusValidForProcessing a rdfs:Class,
        owl:Class,
        dpv:ConsentStatus ;
    dct:contributor "Georg P Krog, Harshvardhan J. Pandit, Paul Ryan, Julian Flake" ;
    dct:created "2022-06-22"^^xsd:date ;
    dct:source "(GConsent,https://w3id.org/GConsent)"@en ;
    rdfs:subClassOf dpv:ConsentStatus ;
    sw:term_status "accepted"@en ;
    skos:definition "States of consent that can be used as valid justifications for processing data"@en ;
    skos:prefLabel "Consent Status Valid for Processing"@en ;
    skos:scopeNote "Practically, given consent is the only valid state for processing"@en .

dpv:ConsentUnknown a rdfs:Class,
        owl:Class,
        dpv:ConsentStatus ;
    dct:contributor "Georg P Krog, Harshvardhan J. Pandit, Paul Ryan, Julian Flake" ;
    dct:created "2022-06-22"^^xsd:date ;
    dct:source "(GConsent,https://w3id.org/GConsent)"@en ;
    rdfs:subClassOf dpv:ConsentStatusInvalidForProcessing ;
    sw:term_status "accepted"@en ;
    skos:definition "State where information about consent is not available or is unknown"@en ;
    skos:prefLabel "Consent Unknown"@en ;
    skos:scopeNote "Consent states can be unknown, for example, when information is not available, or cannot be trusted, or is known to be inaccurate"@en .

dpv:ConsentWithdrawn a rdfs:Class,
        owl:Class,
        dpv:ConsentStatus ;
    dct:contributor "Georg P Krog, Harshvardhan J. Pandit, Paul Ryan, Julian Flake" ;
    dct:created "2022-06-22"^^xsd:date ;
    dct:source "(GConsent,https://w3id.org/GConsent)"@en ;
    rdfs:subClassOf dpv:ConsentStatusInvalidForProcessing ;
    sw:term_status "accepted"@en ;
    skos:definition "The state where the consent is withdrawn or revoked specifically by the data subject and which prevents it from being further used as a valid state"@en ;
    skos:prefLabel "Consent Withdrawn"@en ;
    skos:scopeNote "This state can be considered a form of 'revocation' of consent, where the revocation can only be performed by the data subject. Therefore we suggest using ConsentRevoked when it is a non-data-subject entity, and ConsentWithdrawn when it is the data subject"@en .

dpv:Consequence a rdfs:Class,
        owl:Class ;
    dct:contributor "Harshvardhan J. Pandit" ;
    dct:created "2022-01-26"^^xsd:date ;
    vann:example dex:E0029 ;
    rdfs:superClassOf dpv:ConsequenceAsSideEffect,
        dpv:ConsequenceOfFailure,
        dpv:ConsequenceOfSuccess,
        dpv:Impact ;
    sw:term_status "accepted"@en ;
    skos:definition "The consequence(s) possible or arising from specified context"@en ;
    skos:prefLabel "Consequence"@en .

dpv:ConsequenceAsSideEffect a rdfs:Class,
        owl:Class ;
    dct:contributor "Harshvardhan J. Pandit" ;
    dct:created "2022-03-30"^^xsd:date ;
    rdfs:subClassOf dpv:Consequence ;
    sw:term_status "accepted"@en ;
    skos:definition "The consequence(s) possible or arising as a side-effect of specified context"@en ;
    skos:prefLabel "Consequence as Side-Effect"@en .

dpv:ConsequenceOfFailure a rdfs:Class,
        owl:Class ;
    dct:contributor "Harshvardhan J. Pandit, Georg P Krog" ;
    dct:created "2022-03-23"^^xsd:date ;
    rdfs:subClassOf dpv:Consequence ;
    sw:term_status "accepted"@en ;
    skos:definition "The consequence(s) possible or arising from failure of specified context"@en ;
    skos:prefLabel "Consequence of Failure"@en .

dpv:ConsequenceOfSuccess a rdfs:Class,
        owl:Class ;
    dct:contributor "Harshvardhan J. Pandit, Georg P Krog" ;
    dct:created "2022-03-23"^^xsd:date ;
    rdfs:subClassOf dpv:Consequence ;
    sw:term_status "accepted"@en ;
    skos:definition "The consequence(s) possible or arising from success of specified context"@en ;
    skos:prefLabel "Consequence of Success"@en .

dpv:Consult a rdfs:Class,
        owl:Class,
        dpv:Processing ;
    dct:created "2019-05-07"^^xsd:date ;
    dct:source "(GDPR Art.4-2,https://eur-lex.europa.eu/eli/reg/2016/679/art_4/par_2/oj), (SPECIAL Project,https://specialprivacy.ercim.eu/vocabs/processing)"@en ;
    rdfs:subClassOf dpv:Use ;
    sw:term_status "accepted"@en ;
    skos:definition "to consult or query data"@en ;
    skos:prefLabel "Consult"@en ;
    skos:related "svpr:Query"@en .

dpv:Consultation a rdfs:Class,
        owl:Class,
        dpv:OrganisationalMeasure ;
    dct:contributor "Georg P Krog, Harshvardhan J. Pandit, Paul Ryan" ;
    dct:created "2020-11-04"^^xsd:date ;
    rdfs:subClassOf dpv:OrganisationalMeasure ;
    sw:term_status "accepted"@en ;
    skos:definition "Consultation is a process of receiving feedback, advice, or opinion from an external agency"@en ;
    skos:prefLabel "Consultation"@en .

dpv:ConsultationWithAuthority a rdfs:Class,
        owl:Class,
        dpv:OrganisationalMeasure ;
    dct:contributor "Georg P Krog, Harshvardhan J. Pandit, Paul Ryan" ;
    dct:created "2020-11-04"^^xsd:date ;
    rdfs:subClassOf dpv:Consultation ;
    sw:term_status "accepted"@en ;
    skos:definition "Consultation with an authority or authoritative entity"@en ;
    skos:prefLabel "Consultation with Authority"@en .

dpv:ConsultationWithDPO a rdfs:Class,
        owl:Class,
        dpv:OrganisationalMeasure ;
    dct:contributor "Harshvardhan J. Pandit, Georg P Krog" ;
    dct:created "2022-06-15"^^xsd:date ;
    rdfs:subClassOf dpv:Consultation ;
    sw:term_status "accepted"@en ;
    skos:definition "Consultation with Data Protection Officer(s)"@en ;
    skos:prefLabel "Consultation with DPO"@en .

dpv:ConsultationWithDataSubject a rdfs:Class,
        owl:Class,
        dpv:OrganisationalMeasure ;
    dct:contributor "Harshvardhan J. Pandit, Georg P Krog" ;
    dct:created "2022-06-15"^^xsd:date ;
    rdfs:subClassOf dpv:Consultation ;
    sw:term_status "accepted"@en ;
    skos:definition "Consultation with data subject(s) or their representative(s)"@en ;
    skos:prefLabel "Consultation with Data Subject"@en .

dpv:ConsultationWithDataSubjectRepresentative a rdfs:Class,
        owl:Class,
        dpv:OrganisationalMeasure ;
    dct:contributor "Harshvardhan J. Pandit, Georg P Krog" ;
    dct:created "2022-10-22"^^xsd:date ;
    rdfs:subClassOf dpv:ConsultationWithDataSubject ;
    sw:term_status "accepted"@en ;
    skos:definition "Consultation with representative of data subject(s)"@en ;
    skos:prefLabel "Consultation with Data Subject Representative"@en .

dpv:Consumer a rdfs:Class,
        owl:Class,
        dpv:DataSubject ;
    dct:contributor "Harshvardhan J. Pandit, Georg P. Krog, Julian Flake, Paul Ryan, Beatriz Esteves" ;
    dct:created "2022-04-06"^^xsd:date ;
    rdfs:subClassOf dpv:DataSubject ;
    sw:term_status "accepted"@en ;
    skos:definition "Data subjects that consume goods or services for direct use"@en ;
    skos:prefLabel "Consumer"@en .

dpv:Context a rdfs:Class,
        owl:Class ;
    dct:contributor "Harshvardhan J. Pandit, Javier Fernandez, Axel Polleres, Elmar Kiesling, Fajar Ekaputra, Simon Steyskal" ;
    dct:created "2019-04-05"^^xsd:date ;
    dct:modified "2022-06-15"^^xsd:date ;
    vann:example dex:E0028 ;
    rdfs:superClassOf dpv:Duration,
        dpv:Frequency,
        dpv:Importance,
        dpv:Justification,
        dpv:Necessity,
        dpv:ProcessingContext,
        dpv:Scope,
        dpv:Status ;
    sw:term_status "accepted"@en ;
    skos:definition "Contextually relevant information"@en ;
    skos:prefLabel "Context"@en ;
    skos:scopeNote "Context is a catch-all concept for information of relevance not possible to represent through other core concepts. DPV offers specific contextual concepts such as Necessity, Frequency, and Duration. More can be created by extending Context within use-cases."@en .

dpv:ContinousFrequency a rdfs:Class,
        owl:Class,
        dpv:Frequency ;
    dct:contributor "Harshvardhan J. Pandit" ;
    dct:created "2022-06-15"^^xsd:date ;
    dct:modified "2020-10-05"^^xsd:date ;
    rdfs:subClassOf dpv:Frequency ;
    sw:term_status "accepted"@en ;
    skos:definition "Frequency where occurences are continous"@en ;
    skos:prefLabel "Continous Frequency"@en .

dpv:Contract a rdfs:Class,
        owl:Class,
        dpv:LegalBasis ;
    dct:contributor "Harshvardhan J. Pandit" ;
    dct:created "2021-04-07"^^xsd:date ;
    rdfs:subClassOf dpv:LegalAgreement ;
    sw:term_status "accepted"@en ;
    skos:definition "Creation, completion, fulfilment, or performance of a contract involving specified processing of data or technologies"@en ;
    skos:prefLabel "Contract"@en .

dpv:ContractPerformance a rdfs:Class,
        owl:Class,
        dpv:LegalBasis ;
    dct:contributor "Georg P Krog, Harshvardhan J. Pandit, Paul Ryan" ;
    dct:created "2021-04-07"^^xsd:date ;
    rdfs:subClassOf dpv:Contract ;
    sw:term_status "accepted"@en ;
    skos:definition "Fulfilment or performance of a contract involving specified processing"@en ;
    skos:prefLabel "Contract Performance"@en .

dpv:ContractualTerms a rdfs:Class,
        owl:Class,
        dpv:OrganisationalMeasure ;
    dct:contributor "Axel Polleres, Rob Brennan, Harshvardhan J. Pandit, Mark Lizar" ;
    dct:created "2019-04-05"^^xsd:date ;
    rdfs:subClassOf dpv:LegalAgreement ;
    sw:term_status "accepted"@en ;
    skos:definition "Contractual terms governing data handling within or with an entity"@en ;
    skos:prefLabel "Contractual Terms"@en .

dpv:ControllerProcessorAgreement a rdfs:Class,
        owl:Class,
        dpv:OrganisationalMeasure ;
    dct:contributor "Georg P Krog, Harshvardhan J. Pandit, Beatriz Esteves, Paul Ryan, Julian Flake" ;
    dct:created "2022-01-26"^^xsd:date ;
    vann:example dex:E0020,
        dex:E0021 ;
    rdfs:subClassOf dpv:DataProcessingAgreement ;
    sw:term_status "accepted"@en ;
    skos:definition "An agreement outlining conditions, criteria, obligations, responsibilities, and specifics for carrying out processing of personal data between a Data Controller and a Data Processor"@en ;
    skos:prefLabel "Controller-Processor Agreement"@en .

dpv:Copy a rdfs:Class,
        owl:Class,
        dpv:Processing ;
    dct:created "2019-05-07"^^xsd:date ;
    dct:source "(SPECIAL Project,https://specialprivacy.ercim.eu/vocabs/processing)"@en ;
    rdfs:subClassOf dpv:Processing ;
    sw:term_status "accepted"@en ;
    skos:definition "to produce an exact reproduction of the data"@en ;
    skos:prefLabel "Copy"@en ;
    skos:related "svpr:Copy"@en .

dpv:CounterMoneyLaundering a rdfs:Class,
        owl:Class,
        dpv:Purpose ;
    dct:contributor "Harshvardhan J. Pandit" ;
    dct:created "2022-04-20"^^xsd:date ;
    rdfs:subClassOf dpv:FraudPreventionAndDetection ;
    sw:term_status "accepted"@en ;
    skos:definition "Purposes associated with detection, prevention, and mitigation of mitigate money laundering"@en ;
    skos:prefLabel "Counter Money Laundering"@en .

dpv:Country a rdfs:Class,
        owl:Class ;
    dct:contributor "Harshvardhan J. Pandit, Georg P Krog" ;
    dct:created "2022-01-19"^^xsd:date ;
    rdfs:subClassOf dpv:Location ;
    rdfs:superClassOf dpv:Region,
        dpv:ThirdCountry ;
    sw:term_status "accepted"@en ;
    skos:definition "A political entity indicative of a sovereign or non-sovereign territorial state comprising of distinct geographical areas"@en ;
    skos:prefLabel "Country"@en ;
    skos:scopeNote "The definition of country is not intended for political interpretation. DPVCG welcomes alternate definitions based in existing sources with global scope, such as UN or ISO."@en .

dpv:CredentialManagement a rdfs:Class,
        owl:Class,
        dpv:OrganisationalMeasure ;
    dct:contributor "Georg P Krog" ;
    dct:created "2022-06-15"^^xsd:date ;
    rdfs:subClassOf dpv:AuthorisationProcedure ;
    sw:term_status "accepted"@en ;
    skos:definition "Management of credentials and their use in authorisations"@en ;
    skos:prefLabel "Credential Management"@en .

dpv:CreditChecking a rdfs:Class,
        owl:Class,
        dpv:Purpose ;
    dct:contributor "Harshvardhan J. Pandit" ;
    dct:created "2022-04-20"^^xsd:date ;
    rdfs:subClassOf dpv:CustomerSolvencyMonitoring ;
    sw:term_status "accepted"@en ;
    skos:definition "Purposes associated with monitoring, performing, or assessing credit worthiness or solvency"@en ;
    skos:prefLabel "Credit Checking"@en .

dpv:CryptographicAuthentication a rdfs:Class,
        owl:Class,
        dpv:TechnicalMeasure ;
    dct:contributor "Harshvardhan J. Pandit" ;
    dct:created "2022-08-17"^^xsd:date ;
    dct:source "(ENISA Reference Incident Classification Taxonomy 2018,https://www.enisa.europa.eu/publications/reference-incident-classification-taxonomy/)"@en ;
    rdfs:subClassOf dpv:AuthenticationProtocols,
        dpv:CryptographicMethods ;
    sw:term_status "accepted"@en ;
    skos:definition "Use of cryptography for authentication"@en ;
    skos:prefLabel "Cryptographic Authentication"@en .

dpv:CryptographicKeyManagement a rdfs:Class,
        owl:Class,
        dpv:TechnicalMeasure ;
    dct:contributor "Harshvardhan J. Pandit" ;
    dct:created "2022-08-17"^^xsd:date ;
    dct:source "(ENISA Reference Incident Classification Taxonomy 2018,https://www.enisa.europa.eu/publications/reference-incident-classification-taxonomy/)"@en ;
    rdfs:subClassOf dpv:CryptographicMethods ;
    sw:term_status "accepted"@en ;
    skos:definition "Management of cryptographic keys, including their generation, storage, assessment, and safekeeping"@en ;
    skos:prefLabel "Cryptographic Key Management"@en .

dpv:CryptographicMethods a rdfs:Class,
        owl:Class,
        dpv:TechnicalMeasure ;
    dct:contributor "Harshvardhan J. Pandit" ;
    dct:created "2022-08-17"^^xsd:date ;
    dct:source "(ENISA Reference Incident Classification Taxonomy 2018,https://www.enisa.europa.eu/publications/reference-incident-classification-taxonomy/)"@en ;
    rdfs:subClassOf dpv:TechnicalMeasure ;
    sw:term_status "accepted"@en ;
    skos:definition "Use of cryptographic methods to perform tasks"@en ;
    skos:prefLabel "Cryptographic Methods"@en .

dpv:Customer a rdfs:Class,
        owl:Class,
        dpv:DataSubject ;
    dct:contributor "Harshvardhan J. Pandit, Georg P. Krog, Julian Flake, Paul Ryan, Beatriz Esteves" ;
    dct:created "2022-04-06"^^xsd:date ;
    rdfs:subClassOf dpv:DataSubject ;
    sw:term_status "accepted"@en ;
    skos:definition "Data subjects that purchase goods or services"@en ;
    skos:prefLabel "Customer"@en ;
    skos:scopeNote "note: for B2B relations where customers are organisations, this concept only applies for data subjects"@en .

dpv:CustomerCare a rdfs:Class,
        owl:Class,
        dpv:Purpose ;
    dct:contributor "Harshvardhan J. Pandit, Javier Fernandez, Axel Polleres, Elmar Kiesling, Fajar Ekaputra, Simon Steyskal" ;
    dct:created "2019-04-05"^^xsd:date ;
    rdfs:subClassOf dpv:CustomerManagement ;
    sw:term_status "accepted"@en ;
    skos:definition "Customer Care refers to purposes associated with purposes for providing assistance, resolving issues, ensuring satisfaction, etc. in relation to services provided"@en ;
    skos:prefLabel "Customer Care"@en ;
    skos:related "svpu:Feedback"@en .

dpv:CustomerClaimsManagement a rdfs:Class,
        owl:Class,
        dpv:Purpose ;
    dct:contributor "Georg P Krog, Harshvardhan J. Pandit, Beatriz" ;
    dct:created "2021-09-08"^^xsd:date ;
    dct:source "(Belgian DPA ROPA Template, https://www.privacycommission.be/nl/model-voor-een-register-van-de-verwerkingsactiviteiten)"@en ;
    rdfs:subClassOf dpv:CustomerManagement ;
    sw:term_status "accepted"@en ;
    skos:definition "Customer Claims Management refers to purposes associated with managing claims, including repayment of monies owed"@en ;
    skos:prefLabel "Customer Claims Management"@en .

dpv:CustomerManagement a rdfs:Class,
        owl:Class,
        dpv:Purpose ;
    dct:contributor "Georg P Krog, Harshvardhan J. Pandit, Beatriz" ;
    dct:created "2021-09-08"^^xsd:date ;
    rdfs:subClassOf dpv:Purpose ;
    sw:term_status "accepted"@en ;
    skos:definition "Customer Management refers to purposes associated with managing activities related with past, current, and future customers"@en ;
    skos:prefLabel "Customer Management"@en .

dpv:CustomerOrderManagement a rdfs:Class,
        owl:Class,
        dpv:Purpose ;
    dct:contributor "Georg P Krog, Harshvardhan J. Pandit, Beatriz" ;
    dct:created "2021-09-08"^^xsd:date ;
    dct:source "(Belgian DPA ROPA Template, https://www.privacycommission.be/nl/model-voor-een-register-van-de-verwerkingsactiviteiten)"@en ;
    rdfs:subClassOf dpv:CustomerManagement ;
    sw:term_status "accepted"@en ;
    skos:definition "Customer Order Management refers to purposes associated with managing customer orders i.e. processing of an order related to customer's purchase of good or services"@en ;
    skos:prefLabel "Customer Order Management"@en .

dpv:CustomerRelationshipManagement a rdfs:Class,
        owl:Class,
        dpv:Purpose ;
    dct:contributor "Georg P Krog, Harshvardhan J. Pandit, Beatriz" ;
    dct:created "2021-09-08"^^xsd:date ;
    rdfs:subClassOf dpv:CustomerManagement ;
    sw:term_status "accepted"@en ;
    skos:definition "Customer Relationship Management refers to purposes associated with managing and analysing interactions with past, current, and potential customers"@en ;
    skos:prefLabel "Customer Relationship Management"@en .

dpv:CustomerSolvencyMonitoring a rdfs:Class,
        owl:Class,
        dpv:Purpose ;
    dct:contributor "Georg P Krog, Harshvardhan J. Pandit, Beatriz" ;
    dct:created "2021-09-08"^^xsd:date ;
    dct:source "(Belgian DPA ROPA Template, https://www.privacycommission.be/nl/model-voor-een-register-van-de-verwerkingsactiviteiten)"@en ;
    rdfs:subClassOf dpv:CustomerManagement ;
    sw:term_status "accepted"@en ;
    skos:definition "Customer Solvency Monitoring refers to purposes associated with monitor solvency of customers for financial diligence"@en ;
    skos:prefLabel "Customer Solvency Monitoring"@en .

dpv:CybersecurityAssessment a rdfs:Class,
        owl:Class,
        dpv:OrganisationalMeasure ;
    dct:contributor "Harshvardhan J. Pandit" ;
    dct:created "2022-08-17"^^xsd:date ;
    dct:source "(ENISA 5G Cybersecurity Standards,https://www.enisa.europa.eu/publications/5g-cybersecurity-standards)"@en ;
    rdfs:subClassOf dpv:Assessment,
        dpv:SecurityAssessment ;
    sw:term_status "accepted"@en ;
    skos:definition "Assessment of cybersecurity capabilities in terms of vulnerabilities and effectiveness of controls"@en ;
    skos:prefLabel "Cybersecurity Assessment"@en .

dpv:CybersecurityTraining a rdfs:Class,
        owl:Class,
        dpv:OrganisationalMeasure ;
    dct:contributor "Harshvardhan J. Pandit" ;
    dct:created "2022-08-17"^^xsd:date ;
    dct:source "(ENISA Reference Incident Classification Taxonomy 2018,https://www.enisa.europa.eu/publications/reference-incident-classification-taxonomy/)"@en ;
    rdfs:subClassOf dpv:StaffTraining ;
    sw:term_status "accepted"@en ;
    skos:definition "Training methods related to cybersecurity"@en ;
    skos:prefLabel "Cybersecurity Training"@en .

dpv:DPIA a rdfs:Class,
        owl:Class,
        dpv:OrganisationalMeasure ;
    dct:contributor "Georg P Krog, Harshvardhan J. Pandit, Paul Ryan" ;
    dct:created "2020-11-04"^^xsd:date ;
    rdfs:subClassOf dpv:ImpactAssessment ;
    sw:term_status "accepted"@en ;
    skos:definition "A DPIA involves determining the potential and actual impact of processing activities on individuals or groups of individuals"@en ;
    skos:prefLabel "Data Protection Impact Assessment (DPIA)"@en ;
    skos:scopeNote "Top class: Impact Assessment, and DPIA is sub-class"@en .

dpv:Damage a rdfs:Class,
        owl:Class,
        dpv:Impact ;
    dct:contributor "Harshvardhan J. Pandit" ;
    dct:created "2022-03-30"^^xsd:date ;
    rdfs:subClassOf dpv:Impact ;
    sw:term_status "accepted"@en ;
    skos:definition "Impact that acts as or causes damages"@en ;
    skos:prefLabel "Damage"@en .

dpv:Data a rdfs:Class,
        owl:Class ;
    dct:contributor "Harshvardhan J. Pandit" ;
    dct:created "2022-01-19"^^xsd:date ;
    rdfs:superClassOf dpv:CollectedData,
        dpv:CommerciallyConfidentialData,
        dpv:ConfidentialData,
        dpv:DerivedData,
        dpv:GeneratedData,
        dpv:IncorrectData,
        dpv:InferredData,
        dpv:IntellectualPropertyData,
        dpv:NonPersonalData,
        dpv:ObservedData,
        dpv:PersonalData,
        dpv:SensitiveData,
        dpv:StatisticallyConfidentialData,
        dpv:UnverifiedData,
        dpv:VerifiedData ;
    sw:term_status "accepted"@en ;
    skos:definition "A broad concept representing  'data' or 'information'"@en ;
    skos:prefLabel "Data"@en .

dpv:DataBackupProtocols a rdfs:Class,
        owl:Class,
        dpv:TechnicalMeasure ;
    dct:contributor "Georg P Krog" ;
    dct:created "2022-06-15"^^xsd:date ;
    rdfs:subClassOf dpv:TechnicalMeasure ;
    sw:term_status "accepted"@en ;
    skos:definition "Protocols or plans for backing up of data"@en ;
    skos:prefLabel "Data Backup Protocols"@en .

dpv:DataController a rdfs:Class,
        owl:Class ;
    dct:contributor "Axel Polleres, Javier Fernández" ;
    dct:created "2019-04-05"^^xsd:date ;
    dct:modified "2020-11-04"^^xsd:date ;
    dct:source "(GDPR Art.4-7g,https://eur-lex.europa.eu/eli/reg/2016/679/art_4/par_7/oj)"@en ;
    vann:example dex:E0019,
        dex:E0020 ;
    rdfs:subClassOf dpv:LegalEntity ;
    rdfs:superClassOf dpv:JointDataControllers ;
    sw:term_status "accepted"@en ;
    skos:definition "The individual or organisation that decides (or controls) the purpose(s) of processing personal data."@en ;
    skos:prefLabel "Data Controller"@en ;
    skos:scopeNote "The terms 'Controller', 'Data Controller', and 'PII Controller' refer to the same concept"@en .

dpv:DataControllerContract a rdfs:Class,
        owl:Class,
        dpv:LegalBasis ;
    dct:created "2023-12-10"^^xsd:date ;
    rdfs:subClassOf dpv:Contract ;
    sw:term_status "accepted"@en ;
    skos:definition "Creation, completion, fulfilment, or performance of a contract, with Data Controllers as parties being Joint Data Controllers, and involving specified processing"@en ;
    skos:prefLabel "Data Controller Contract"@en .

dpv:DataControllerDataSource a rdfs:Class,
        owl:Class,
        dpv:DataSource ;
    dct:created "2023-10-12"^^xsd:date ;
    rdfs:subClassOf dpv:DataSource ;
    sw:term_status "accepted"@en ;
    skos:definition "Data Sourced from Data Controller(s), e.g. a Controller inferring data or generating data"@en ;
    skos:prefLabel "Data Controller as Data Source"@en .

dpv:DataExporter a rdfs:Class,
        owl:Class ;
    dct:contributor "David Hickey, Georg Krog, Paul Ryan, Harshvardhan Pandit" ;
    dct:created "2021-09-08"^^xsd:date ;
    dct:source "(EDPB Recommendations 01/2020 on Data Transfers, https://edpb.europa.eu/our-work-tools/our-documents/recommendations/recommendations-012020-measures-supplement-transfer_en)"@en ;
    rdfs:subClassOf dpv:LegalEntity ;
    sw:term_status "accepted"@en ;
    skos:definition "An entity that 'exports' data where exporting is considered a form of data transfer"@en ;
    skos:prefLabel "Data Exporter"@en ;
    skos:scopeNote "The term 'Data Exporter' is used by the EU-EDPB as the entity that transfer data across borders. While the EDPB refers to the jurisdictional border of EU, the term within DPV can be used to denote any 'export' or transfer or transmission of data and is thus a broader concept than the EDPB's definition."@en .

dpv:DataImporter a rdfs:Class,
        owl:Class ;
    dct:contributor "David Hickey, Georg Krog, Paul Ryan, Harshvardhan Pandit" ;
    dct:created "2021-09-08"^^xsd:date ;
    dct:source "(EDPB Recommendations 01/2020 on Data Transfers, https://edpb.europa.eu/our-work-tools/our-documents/recommendations/recommendations-012020-measures-supplement-transfer_en)"@en ;
    rdfs:subClassOf dpv:Recipient ;
    sw:term_status "accepted"@en ;
    skos:definition "An entity that 'imports' data where importing is considered a form of data transfer"@en ;
    skos:prefLabel "Data Importer"@en ;
    skos:scopeNote "The term 'Data Importer' is used by the EU-EDPB as the entity that receives transferred data across borders. While the EDPB refers to the jurisdictional border of EU, the term within DPV can be used to denote any 'import' or reception of transfer or transmission of data and is thus a broader concept than the EDPB's definition."@en .

dpv:DataProcessingAgreement a rdfs:Class,
        owl:Class,
        dpv:OrganisationalMeasure ;
    dct:contributor "Georg P Krog, Harshvardhan J. Pandit, Beatriz Esteves, Paul Ryan, Julian Flake" ;
    dct:created "2022-01-26"^^xsd:date ;
    rdfs:subClassOf dpv:LegalAgreement ;
    sw:term_status "accepted"@en ;
    skos:definition "An agreement outlining conditions, criteria, obligations, responsibilities, and specifics for carrying out processing of data"@en ;
    skos:prefLabel "Data Processing Agreement"@en ;
    skos:scopeNote "For specific role-based data processing agreements, see concepts for Processors and JointDataController agreements."@en .

dpv:DataProcessingRecord a rdfs:Class,
        owl:Class,
        dpv:OrganisationalMeasure ;
    dct:contributor "Harshvardhan J. Pandit" ;
    dct:created "2021-09-08"^^xsd:date ;
    rdfs:subClassOf dpv:RecordsOfActivities ;
    sw:term_status "accepted"@en ;
    skos:definition "Record of data processing, whether ex-ante or ex-post"@en ;
    skos:prefLabel "Data Processing Record"@en .

dpv:DataProcessor a rdfs:Class,
        owl:Class ;
    dct:contributor "Harshvardhan J. Pandit" ;
    dct:created "2019-06-04"^^xsd:date ;
    dct:source "(GDPR Art.4-8,https://eur-lex.europa.eu/eli/reg/2016/679/art_4/par_8/oj)"@en ;
    vann:example dex:E0011 ;
    rdfs:subClassOf dpv:Recipient ;
    rdfs:superClassOf dpv:DataSubProcessor ;
    sw:term_status "accepted"@en ;
    skos:definition "A ‘processor’ means a natural or legal person, public authority, agency or other body which processes data on behalf of the controller."@en ;
    skos:prefLabel "Data Processor"@en .

dpv:DataProcessorContract a rdfs:Class,
        owl:Class,
        dpv:LegalBasis ;
    dct:created "2023-12-10"^^xsd:date ;
    rdfs:subClassOf dpv:Contract ;
    sw:term_status "accepted"@en ;
    skos:definition "Creation, completion, fulfilment, or performance of a contract, with the Data Controller and Data Processor as parties, and involving specified processing"@en ;
    skos:prefLabel "Data Processor Contract"@en .

dpv:DataProtectionAuthority a rdfs:Class,
        owl:Class ;
    dct:contributor "Georg Krog, Paul Ryan, Harshvardhan Pandit" ;
    dct:created "2020-11-04"^^xsd:date ;
    rdfs:subClassOf dpv:Authority ;
    sw:term_status "accepted"@en ;
    skos:definition "An authority tasked with overseeing legal compliance regarding privacy and data protection laws."@en ;
    skos:prefLabel "Data Protection Authority"@en .

dpv:DataProtectionOfficer a rdfs:Class,
        owl:Class ;
    dct:contributor "Georg Krog, Paul Ryan" ;
    dct:created "2020-11-04"^^xsd:date ;
    dct:modified "2021-12-08"^^xsd:date ;
    dct:source "(GDPR Art.37,https://eur-lex.europa.eu/eli/reg/2016/679/art_37/oj)"@en ;
    rdfs:subClassOf dpv:Representative ;
    sw:term_status "accepted"@en ;
    skos:definition "An entity within or authorised by an organisation to monitor internal compliance, inform and advise on data protection obligations and act as a contact point for data subjects and the supervisory authority."@en ;
    skos:prefLabel "Data Protection Officer"@en .

dpv:DataProtectionTraining a rdfs:Class,
        owl:Class,
        dpv:OrganisationalMeasure ;
    dct:contributor "Harshvardhan J. Pandit" ;
    dct:created "2022-08-17"^^xsd:date ;
    dct:source "(ENISA 5G Cybersecurity Standards,https://www.enisa.europa.eu/publications/5g-cybersecurity-standards)"@en ;
    rdfs:subClassOf dpv:StaffTraining ;
    sw:term_status "accepted"@en ;
    skos:definition "Training intended to increase knowledge regarding data protection"@en ;
    skos:prefLabel "Data Protection Training"@en .

dpv:DataPublishedByDataSubject a rdfs:Class,
        owl:Class,
        dpv:DataSubjectDataSource ;
    dct:contributor "Julian Flake" ;
    dct:created "2022-08-24"^^xsd:date ;
    dct:modified "2023-12-10"^^xsd:date ;
    rdfs:subClassOf dpv:DataSubjectDataSource ;
    sw:term_status "accepted"@en ;
    skos:definition "Data is published by the data subject"@en ;
    skos:prefLabel "Data published by Data Subject"@en ;
    skos:scopeNote "This refers to where that data was made publicly available by the data subject. An example of this would be a social media profile that the data subject has made publicly accessible."@en .

dpv:DataRedaction a rdfs:Class,
        owl:Class,
        dpv:TechnicalMeasure ;
    dct:contributor "Harshvardhan J. Pandit" ;
    dct:created "2020-10-01"^^xsd:date ;
    rdfs:subClassOf dpv:DataSanitisationTechnique ;
    sw:term_status "accepted"@en ;
    skos:definition "Removal of sensitive information from a data or document"@en ;
    skos:prefLabel "Data Redaction"@en .

dpv:DataSanitisationTechnique a rdfs:Class,
        owl:Class,
        dpv:TechnicalMeasure ;
    dct:contributor "Harshvardhan J. Pandit" ;
    dct:created "2022-08-17"^^xsd:date ;
    dct:source "(ENISA Reference Incident Classification Taxonomy 2018,https://www.enisa.europa.eu/publications/reference-incident-classification-taxonomy/)"@en ;
    rdfs:subClassOf dpv:TechnicalMeasure ;
    sw:term_status "accepted"@en ;
    skos:definition "Cleaning or any removal or re-organisation of elements in data based on selective criteria"@en ;
    skos:prefLabel "Data Sanitisation Technique"@en .

dpv:DataSource a rdfs:Class,
        owl:Class ;
    dct:contributor "Georg P Krog, Harshvardhan J. Pandit, Beatriz Esteves" ;
    dct:created "2020-11-04"^^xsd:date ;
    vann:example dex:E0012,
        dex:E0020 ;
    rdfs:subClassOf dpv:ProcessingContext ;
    sw:term_status "accepted"@en ;
    skos:definition "The source or origin of data"@en ;
    skos:prefLabel "Data Source"@en ;
    skos:scopeNote "Source' is the direct point of data collection; 'origin' would indicate the original/others points of where the data originates from."@en .

dpv:DataSubProcessor a rdfs:Class,
        owl:Class ;
    dct:contributor "Harshvardhan J. Pandit" ;
    dct:created "2020-11-25"^^xsd:date ;
    rdfs:subClassOf dpv:DataProcessor ;
    sw:term_status "accepted"@en ;
    skos:definition "A 'sub-processor' is a processor engaged by another processor"@en ;
    skos:prefLabel "Data Sub-Processor"@en ;
    skos:scopeNote "A 'Sub-Processor' is always a 'Processor' with the distinction of not directly being appointed by the 'Controller'"@en .

dpv:DataSubject a rdfs:Class,
        owl:Class ;
    dct:contributor "Axel Polleres, Javier Fernández" ;
    dct:created "2019-04-05"^^xsd:date ;
    dct:modified "2020-11-04"^^xsd:date ;
    dct:source "(GDPR Art.4-1g,https://eur-lex.europa.eu/eli/reg/2016/679/art_4/par_1/oj)"@en ;
    rdfs:subClassOf dpv:LegalEntity ;
    sw:term_status "accepted"@en ;
    skos:definition "The individual (or category of individuals) whose personal data is being processed"@en ;
    skos:prefLabel "Data Subject"@en ;
    skos:scopeNote "The term 'data subject' is specific to the GDPR, but is functionally equivalent to the term 'individual associated with data' and the ISO/IEC term 'PII Principle'"@en .

dpv:DataSubjectContract a rdfs:Class,
        owl:Class,
        dpv:LegalBasis ;
    dct:created "2023-12-10"^^xsd:date ;
    rdfs:subClassOf dpv:Contract ;
    sw:term_status "accepted"@en ;
    skos:definition "Creation, completion, fulfilment, or performance of a contract, with the Data Controller and Data Subject as parties, and involving specified processing"@en ;
    skos:prefLabel "Data Subject Contract"@en .

dpv:DataSubjectDataSource a rdfs:Class,
        owl:Class,
        dpv:DataSource ;
    dct:created "2023-10-12"^^xsd:date ;
    rdfs:subClassOf dpv:DataSource ;
    sw:term_status "accepted"@en ;
    skos:definition "Data Sourced from Data Subject(s), e.g. when data is collected via a form or observed from their activities"@en ;
    skos:prefLabel "Data Subject as Data Source"@en .

dpv:DataSubjectRight a rdfs:Class,
        owl:Class,
        dpv:Right ;
    dct:contributor "Beatriz Esteves, Georg P Krog, Harshvardhan Pandit" ;
    dct:created "2020-11-18"^^xsd:date ;
    rdfs:subClassOf dpv:Right ;
    sw:term_status "accepted"@en ;
    skos:definition "The rights applicable or provided to a Data Subject"@en ;
    skos:prefLabel "Data Subject Right"@en ;
    skos:scopeNote "Based on use of definitions, the notion of 'Data Subject Right' can be equivalent to 'Individual Right' or 'Right of a Person'"@en .

dpv:DataSubjectScale a rdfs:Class,
        owl:Class ;
    dct:contributor "Harshvardhan J. Pandit, Georg P Krog, Rana Saniei" ;
    dct:created "2022-06-15"^^xsd:date ;
    rdfs:subClassOf dpv:Scale ;
    sw:term_status "accepted"@en ;
    skos:definition "Scale of Data Subject(s)"@en ;
    skos:prefLabel "Data Subject Scale"@en .

dpv:DataTransferImpactAssessment a rdfs:Class,
        owl:Class,
        dpv:OrganisationalMeasure ;
    dct:contributor "Georg P Krog, Harshvardhan J. Pandit, Paul Ryan" ;
    dct:created "2021-09-08"^^xsd:date ;
    rdfs:subClassOf dpv:ImpactAssessment ;
    sw:term_status "accepted"@en ;
    skos:definition "Impact Assessment for conducting data transfers"@en ;
    skos:prefLabel "Data Transfer Impact Assessment"@en .

dpv:DataTransferLegalBasis a rdfs:Class,
        owl:Class,
        dpv:LegalBasis ;
    dct:contributor "David Hickey, Georg P Krogg" ;
    dct:created "2021-09-08"^^xsd:date ;
    rdfs:subClassOf dpv:LegalBasis ;
    sw:term_status "accepted"@en ;
    skos:definition "Specific or special categories and instances of legal basis intended for justifying data transfers"@en ;
    skos:prefLabel "Data Transfer Legal Basis"@en .

dpv:DataVolume a rdfs:Class,
        owl:Class ;
    dct:contributor "Harshvardhan J. Pandit, Georg P Krog, Rana Saniei" ;
    dct:created "2022-06-15"^^xsd:date ;
    rdfs:subClassOf dpv:Scale ;
    sw:term_status "accepted"@en ;
    skos:definition "Volume or Scale of Data"@en ;
    skos:prefLabel "Data Volume"@en .

dpv:DecentralisedLocations a rdfs:Class,
        owl:Class,
        dpv:LocationFixture ;
    dct:contributor "Harshvardhan J. Pandit" ;
    dct:created "2022-06-15"^^xsd:date ;
    dct:modified "2020-10-05"^^xsd:date ;
    rdfs:subClassOf dpv:LocationFixture ;
    sw:term_status "accepted"@en ;
    skos:definition "Location that is spread across multiple separate areas with no distinction between their importance"@en ;
    skos:prefLabel "Decentralised Locations"@en .

dpv:DecisionMaking a rdfs:Class,
        owl:Class ;
    dct:contributor "Harshvardhan J. Pandit" ;
    dct:created "2022-09-07"^^xsd:date ;
    rdfs:subClassOf dpv:ProcessingContext ;
    rdfs:superClassOf dpv:AutomatedDecisionMaking ;
    sw:term_status "accepted"@en ;
    skos:definition "Processing that involves decision making"@en ;
    skos:prefLabel "Decision Making"@en .

dpv:Deidentification a rdfs:Class,
        owl:Class,
        dpv:TechnicalMeasure ;
    dct:contributor "Axel Polleres, Rob Brennan, Harshvardhan J. Pandit, Mark Lizar" ;
    dct:created "2019-04-05"^^xsd:date ;
    dct:modified "2022-11-24"^^xsd:date ;
    dct:source "(NISTIR 8053,https://nvlpubs.nist.gov/nistpubs/ir/2015/NIST.IR.8053.pdf)"@en ;
    rdfs:subClassOf dpv:DataSanitisationTechnique ;
    sw:term_status "modified"@en ;
    skos:definition "Removal of identity or information to reduce identifiability"@en ;
    skos:prefLabel "De-Identification"@en .

dpv:DeliveryOfGoods a rdfs:Class,
        owl:Class,
        dpv:Purpose ;
    dct:contributor "Harshvardhan J. Pandit, Javier Fernandez, Axel Polleres, Elmar Kiesling, Fajar Ekaputra, Simon Steyskal" ;
    dct:created "2019-04-05"^^xsd:date ;
    rdfs:subClassOf dpv:RequestedServiceProvision ;
    sw:term_status "accepted"@en ;
    skos:definition "Purposes associated with delivering goods and services requested or asked by consumer"@en ;
    skos:prefLabel "Delivery of Goods"@en ;
    skos:related "svpu:Delivery"@en .

dpv:Derive a rdfs:Class,
        owl:Class,
        dpv:Processing ;
    dct:created "2019-05-07"^^xsd:date ;
    dct:source "(SPECIAL Project,https://specialprivacy.ercim.eu/vocabs/processing)"@en ;
    vann:example dex:E0014 ;
    rdfs:subClassOf dpv:Obtain ;
    sw:term_status "accepted"@en ;
    skos:definition "to create new derivative data from the original data"@en ;
    skos:prefLabel "Derive"@en ;
    skos:related "svpr:Derive"@en ;
    skos:scopeNote "Derive indicates data is present or obtainable from existing data. For data that is created without such existence, see Infer."@en .

dpv:DerivedData a rdfs:Class,
        owl:Class ;
    dct:created "2023-12-10"^^xsd:date ;
    rdfs:subClassOf dpv:Data ;
    rdfs:superClassOf dpv:DerivedPersonalData ;
    sw:term_status "accepted"@en ;
    skos:definition "Data that has been obtained through derivations of other data"@en ;
    skos:prefLabel "Derived Data"@en .

dpv:DerivedPersonalData a rdfs:Class,
        owl:Class ;
    dct:contributor "Elmar Kiesling; Harshvardhan J. Pandit, Fajar Ekaputra" ;
    dct:created "2019-05-07"^^xsd:date ;
    dct:modified "2023-12-10"^^xsd:date ;
    dct:source "(DPVCG, https://www.w3.org/community/dpvcg/)"@en ;
    rdfs:subClassOf dpv:DerivedData,
        dpv:PersonalData ;
    rdfs:superClassOf dpv:InferredPersonalData ;
    sw:term_status "accepted"@en ;
    skos:definition "Personal Data that is obtained or derived from other data"@en ;
    skos:prefLabel "Derived Personal Data"@en ;
    skos:related "svd:Derived"@en ;
    skos:scopeNote "Derived Data is data that is obtained through processing of existing data, e.g. deriving first name from full name. To indicate data that is derived but which was not present or evident within the source data, InferredPersonalData should be used."@en .

dpv:DesignStandard a rdfs:Class,
        owl:Class,
        dpv:OrganisationalMeasure ;
    dct:contributor "Axel Polleres, Rob Brennan, Harshvardhan J. Pandit, Mark Lizar" ;
    dct:created "2019-04-05"^^xsd:date ;
    rdfs:subClassOf dpv:GuidelinesPrinciple ;
    sw:term_status "accepted"@en ;
    skos:definition "A set of rules or guidelines outlining criterias for design"@en ;
    skos:prefLabel "Design Standard"@en .

dpv:Destruct a rdfs:Class,
        owl:Class,
        dpv:Processing ;
    dct:created "2019-05-07"^^xsd:date ;
    dct:source "(GDPR Art.4-2,https://eur-lex.europa.eu/eli/reg/2016/679/art_4/par_2/oj)"@en ;
    rdfs:subClassOf dpv:Remove ;
    sw:term_status "accepted"@en ;
    skos:definition "to process data in a way it no longer exists or cannot be repaired"@en ;
    skos:prefLabel "Destruct"@en .

dpv:DeterministicPseudonymisation a rdfs:Class,
        owl:Class,
        dpv:TechnicalMeasure ;
    dct:contributor "Harshvardhan J. Pandit" ;
    dct:created "2022-08-17"^^xsd:date ;
    dct:source "(ENISA Data Pseudonymisation: Advanced Techniques and Use Cases,https://www.enisa.europa.eu/publications/data-pseudonymisation-advanced-techniques-and-use-cases)"@en ;
    rdfs:subClassOf dpv:Pseudonymisation ;
    sw:term_status "accepted"@en ;
    skos:definition "Pseudonymisation achieved through a deterministic function"@en ;
    skos:prefLabel "Deterministic Pseudonymisation"@en .

dpv:Detriment a rdfs:Class,
        owl:Class,
        dpv:Impact ;
    dct:contributor "Harshvardhan J. Pandit, Julian Flake, Georg P Krog, Fajar Ekaputra, Beatriz Esteves" ;
    dct:created "2022-03-23"^^xsd:date ;
    rdfs:subClassOf dpv:Impact ;
    sw:term_status "accepted"@en ;
    skos:definition "Impact that acts as or causes detriments"@en ;
    skos:prefLabel "Detriment"@en .

dpv:DifferentialPrivacy a rdfs:Class,
        owl:Class,
        dpv:TechnicalMeasure ;
    dct:contributor "Harshvardhan J. Pandit" ;
    dct:created "2022-08-17"^^xsd:date ;
    dct:source "(ENISA Data Protection Engineering,https://www.enisa.europa.eu/publications/data-protection-engineering)"@en ;
    rdfs:subClassOf dpv:CryptographicMethods ;
    sw:term_status "accepted"@en ;
    skos:definition "Utilisation of differential privacy where information is shared as patterns or groups to withhold individual elements"@en ;
    skos:prefLabel "Differential Privacy"@en .

dpv:DigitalRightsManagement a rdfs:Class,
        owl:Class,
        dpv:TechnicalMeasure ;
    dct:contributor "Harshvardhan J. Pandit" ;
    dct:created "2022-08-17"^^xsd:date ;
    dct:source "(ENISA Reference Incident Classification Taxonomy 2018,https://www.enisa.europa.eu/publications/reference-incident-classification-taxonomy/)"@en ;
    rdfs:subClassOf dpv:TechnicalMeasure ;
    sw:term_status "accepted"@en ;
    skos:definition "Management of access, use, and other operations associated with digital content"@en ;
    skos:prefLabel "Digital Rights Management"@en .

dpv:DigitalSignatures a rdfs:Class,
        owl:Class,
        dpv:TechnicalMeasure ;
    dct:contributor "Harshvardhan J. Pandit" ;
    dct:created "2022-08-17"^^xsd:date ;
    dct:source "(ENISA Reference Incident Classification Taxonomy 2018,https://www.enisa.europa.eu/publications/reference-incident-classification-taxonomy/)"@en ;
    rdfs:subClassOf dpv:CryptographicMethods ;
    sw:term_status "accepted"@en ;
    skos:definition "Expression and authentication of identity through digital information containing cryptographic signatures"@en ;
    skos:prefLabel "Digital Signatures"@en .

dpv:DirectMarketing a rdfs:Class,
        owl:Class,
        dpv:Purpose ;
    dct:contributor "Georg P Krog, Harshvardhan J. Pandit, Beatriz Esteves" ;
    dct:created "2020-11-04"^^xsd:date ;
    rdfs:subClassOf dpv:Marketing ;
    sw:term_status "accepted"@en ;
    skos:definition "Purposes associated with conducting direct marketing i.e. marketing communicated directly to the individual"@en ;
    skos:prefLabel "Direct Marketing"@en .

dpv:DisasterRecoveryProcedures a rdfs:Class,
        owl:Class,
        dpv:OrganisationalMeasure ;
    dct:contributor "Harshvardhan J. Pandit" ;
    dct:created "2022-08-17"^^xsd:date ;
    dct:source "(ENISA 5G Cybersecurity Standards,https://www.enisa.europa.eu/publications/5g-cybersecurity-standards)"@en ;
    rdfs:subClassOf dpv:GovernanceProcedures ;
    sw:term_status "accepted"@en ;
    skos:definition "Procedures related to management of disasters and recovery"@en ;
    skos:prefLabel "Disaster Recovery Procedures"@en .

dpv:Disclose a rdfs:Class,
        owl:Class,
        dpv:Processing ;
    dct:created "2019-05-07"^^xsd:date ;
    dct:source "(GDPR Art.4-2,https://eur-lex.europa.eu/eli/reg/2016/679/art_4/par_2/oj)"@en ;
    rdfs:subClassOf dpv:Processing ;
    sw:term_status "accepted"@en ;
    skos:definition "to make data known"@en ;
    skos:prefLabel "Disclose"@en .

dpv:DiscloseByTransmission a rdfs:Class,
        owl:Class,
        dpv:Processing ;
    dct:created "2019-05-07"^^xsd:date ;
    dct:source "(GDPR Art.4-2,https://eur-lex.europa.eu/eli/reg/2016/679/art_4/par_2/oj)"@en ;
    rdfs:subClassOf dpv:Disclose ;
    sw:term_status "accepted"@en ;
    skos:definition "to disclose data by means of transmission"@en ;
    skos:prefLabel "Disclose by Transmission"@en .

dpv:DisputeManagement a rdfs:Class,
        owl:Class,
        dpv:Purpose ;
    dct:contributor "Georg P Krog, Harshvardhan J. Pandit, Beatriz Esteves" ;
    dct:created "2021-09-08"^^xsd:date ;
    dct:source "(Belgian DPA ROPA Template, https://www.privacycommission.be/nl/model-voor-een-register-van-de-verwerkingsactiviteiten)"@en ;
    rdfs:subClassOf dpv:OrganisationGovernance ;
    sw:term_status "accepted"@en ;
    skos:definition "Purposes associated with activities that manage disputes by natural persons, private bodies, or public authorities relevant to organisation"@en ;
    skos:prefLabel "Dispute Management"@en .

dpv:Disseminate a rdfs:Class,
        owl:Class,
        dpv:Processing ;
    dct:created "2019-05-07"^^xsd:date ;
    dct:source "(GDPR Art.4-2,https://eur-lex.europa.eu/eli/reg/2016/679/art_4/par_2/oj)"@en ;
    rdfs:subClassOf dpv:Disclose ;
    sw:term_status "accepted"@en ;
    skos:definition "to spread data throughout"@en ;
    skos:prefLabel "Disseminate"@en .

dpv:DistributedSystemSecurity a rdfs:Class,
        owl:Class,
        dpv:TechnicalMeasure ;
    dct:contributor "Harshvardhan J. Pandit" ;
    dct:created "2022-08-17"^^xsd:date ;
    dct:source "(ENISA Reference Incident Classification Taxonomy 2018,https://www.enisa.europa.eu/publications/reference-incident-classification-taxonomy/)"@en ;
    rdfs:subClassOf dpv:SecurityMethod ;
    sw:term_status "accepted"@en ;
    skos:definition "Security implementations provided using or over a distributed system"@en ;
    skos:prefLabel "Distributed System Security"@en .

dpv:DocumentRandomisedPseudonymisation a rdfs:Class,
        owl:Class,
        dpv:TechnicalMeasure ;
    dct:contributor "Harshvardhan J. Pandit" ;
    dct:created "2022-08-17"^^xsd:date ;
    dct:source "(ENISA Data Pseudonymisation: Advanced Techniques and Use Cases,https://www.enisa.europa.eu/publications/data-pseudonymisation-advanced-techniques-and-use-cases)"@en ;
    rdfs:subClassOf dpv:Pseudonymisation ;
    sw:term_status "accepted"@en ;
    skos:definition "Use of randomised pseudonymisation where the same elements are assigned different values in the same document or database"@en ;
    skos:prefLabel "Document Randomised Pseudonymisation"@en .

dpv:DocumentSecurity a rdfs:Class,
        owl:Class,
        dpv:TechnicalMeasure ;
    dct:contributor "Harshvardhan J. Pandit" ;
    dct:created "2022-08-17"^^xsd:date ;
    dct:source "(ENISA Reference Incident Classification Taxonomy 2018,https://www.enisa.europa.eu/publications/reference-incident-classification-taxonomy/)"@en ;
    rdfs:subClassOf dpv:SecurityMethod ;
    sw:term_status "accepted"@en ;
    skos:definition "Security measures enacted over documents to protect against tampering or restrict access"@en ;
    skos:prefLabel "Document Security"@en .

dpv:Duration a rdfs:Class,
        owl:Class ;
    dct:contributor "Harshvardhan J. Pandit" ;
    dct:created "2022-02-09"^^xsd:date ;
    vann:example dex:E0011,
        dex:E0019 ;
    rdfs:subClassOf dpv:Context ;
    rdfs:superClassOf dpv:FixedOccurencesDuration,
        dpv:StorageDuration,
        dpv:TemporalDuration,
        dpv:UntilEventDuration,
        dpv:UntilTimeDuration ;
    sw:term_status "accepted"@en ;
    skos:definition "The duration or temporal limitation"@en ;
    skos:prefLabel "Duration"@en .

dpv:EconomicUnion a rdfs:Class,
        owl:Class ;
    dct:contributor "Harshvardhan J. Pandit" ;
    dct:created "2022-01-19"^^xsd:date ;
    rdfs:subClassOf dpv:Location ;
    sw:term_status "accepted"@en ;
    skos:definition "A political union of two or more countries based on economic or trade agreements"@en ;
    skos:prefLabel "Economic Union"@en .

dpv:EducationalTraining a rdfs:Class,
        owl:Class,
        dpv:OrganisationalMeasure ;
    dct:contributor "Harshvardhan J. Pandit" ;
    dct:created "2022-08-17"^^xsd:date ;
    dct:source "(ENISA Reference Incident Classification Taxonomy 2018,https://www.enisa.europa.eu/publications/reference-incident-classification-taxonomy/)"@en ;
    rdfs:subClassOf dpv:StaffTraining ;
    sw:term_status "accepted"@en ;
    skos:definition "Training methods that are intended to provide education on topic(s)"@en ;
    skos:prefLabel "Educational Training"@en .

dpv:EffectivenessDeterminationProcedures a rdfs:Class,
        owl:Class,
        dpv:OrganisationalMeasure ;
    dct:contributor "Harshvardhan J. Pandit" ;
    dct:created "2022-08-17"^^xsd:date ;
    dct:source "(ENISA 5G Cybersecurity Standards,https://www.enisa.europa.eu/publications/5g-cybersecurity-standards)"@en ;
    rdfs:subClassOf dpv:Assessment ;
    sw:term_status "accepted"@en ;
    skos:definition "Procedures intended to determine effectiveness of other measures"@en ;
    skos:prefLabel "Effectiveness Determination Procedures"@en .

dpv:ElderlyDataSubject a rdfs:Class,
        owl:Class,
        dpv:DataSubject ;
    dct:contributor "Georg P Krog" ;
    dct:created "2022-06-15"^^xsd:date ;
    rdfs:subClassOf dpv:VulnerableDataSubject ;
    sw:term_status "accepted"@en ;
    skos:definition "Data subjects that are considered elderly (i.e. based on age)"@en ;
    skos:prefLabel "Elderly Data Subject"@en .

dpv:Employee a rdfs:Class,
        owl:Class,
        dpv:DataSubject ;
    dct:contributor "Harshvardhan J. Pandit, Georg P. Krog, Julian Flake, Paul Ryan, Beatriz Esteves" ;
    dct:created "2022-04-06"^^xsd:date ;
    rdfs:subClassOf dpv:DataSubject ;
    sw:term_status "accepted"@en ;
    skos:definition "Data subjects that are employees"@en ;
    skos:prefLabel "Employee"@en .

dpv:Encryption a rdfs:Class,
        owl:Class,
        dpv:TechnicalMeasure ;
    dct:contributor "Axel Polleres, Rob Brennan, Harshvardhan J. Pandit, Mark Lizar" ;
    dct:created "2019-04-05"^^xsd:date ;
    vann:example dex:E0016 ;
    rdfs:subClassOf dpv:TechnicalMeasure ;
    sw:term_status "accepted"@en ;
    skos:definition "Technical measures consisting of encryption"@en ;
    skos:prefLabel "Encryption"@en .

dpv:EncryptionAtRest a rdfs:Class,
        owl:Class,
        dpv:TechnicalMeasure ;
    dct:contributor "Axel Polleres, Rob Brennan, Harshvardhan J. Pandit, Mark Lizar" ;
    dct:created "2019-04-05"^^xsd:date ;
    rdfs:subClassOf dpv:Encryption ;
    sw:term_status "accepted"@en ;
    skos:definition "Encryption of data when being stored (persistent encryption)"@en ;
    skos:prefLabel "Encryption at Rest"@en .

dpv:EncryptionInTransfer a rdfs:Class,
        owl:Class,
        dpv:TechnicalMeasure ;
    dct:contributor "Axel Polleres, Rob Brennan, Harshvardhan J. Pandit, Mark Lizar" ;
    dct:created "2019-04-05"^^xsd:date ;
    rdfs:subClassOf dpv:Encryption ;
    sw:term_status "accepted"@en ;
    skos:definition "Encryption of data in transit e.g. when being transferred from one location to another, including sharing"@en ;
    skos:prefLabel "Encryption in Transfer"@en .

dpv:EncryptionInUse a rdfs:Class,
        owl:Class,
        dpv:TechnicalMeasure ;
    dct:contributor "Harshvardhan J. Pandit" ;
    dct:created "2022-10-22"^^xsd:date ;
    rdfs:subClassOf dpv:Encryption ;
    sw:term_status "accepted"@en ;
    skos:definition "Encryption of data when it is being used"@en ;
    skos:prefLabel "Encryption in Use"@en .

dpv:EndToEndEncryption a rdfs:Class,
        owl:Class,
        dpv:TechnicalMeasure ;
    dct:contributor "Harshvardhan J. Pandit" ;
    dct:created "2022-08-17"^^xsd:date ;
    dct:source "(ENISA Data Protection Engineering,https://www.enisa.europa.eu/publications/data-protection-engineering)"@en ;
    rdfs:subClassOf dpv:Encryption ;
    sw:term_status "accepted"@en ;
    skos:definition "Encrypted communications where data is encrypted by the sender and decrypted by the intended receiver to prevent access to any third party"@en ;
    skos:prefLabel "End-to-End Encryption (E2EE)"@en .

dpv:EndlessDuration a rdfs:Class,
        owl:Class,
        dpv:Duration ;
    dct:contributor "Harshvardhan J. Pandit" ;
    dct:created "2022-06-15"^^xsd:date ;
    dct:modified "2020-10-05"^^xsd:date ;
    rdfs:subClassOf dpv:Duration ;
    sw:term_status "accepted"@en ;
    skos:definition "Duration that is (known or intended to be) open ended or without an end"@en ;
    skos:prefLabel "Endless Duration"@en .

dpv:EnforceAccessControl a rdfs:Class,
        owl:Class,
        dpv:Purpose ;
    dct:contributor "Harshvardhan J. Pandit, Javier Fernandez, Axel Polleres, Elmar Kiesling, Fajar Ekaputra, Simon Steyskal" ;
    dct:created "2019-04-05"^^xsd:date ;
    rdfs:subClassOf dpv:EnforceSecurity ;
    sw:term_status "accepted"@en ;
    skos:definition "Purposes associated with conducting or enforcing access control as a form of security"@en ;
    skos:prefLabel "Enforce Access Control"@en ;
    skos:related "svpu:Login"@en ;
    skos:scopeNote "Was previously \"Access Control\". Prefixed to distinguish from Technical Measure."@en .

dpv:EnforceSecurity a rdfs:Class,
        owl:Class,
        dpv:Purpose ;
    dct:contributor "Harshvardhan J. Pandit, Javier Fernandez, Axel Polleres, Elmar Kiesling, Fajar Ekaputra, Simon Steyskal" ;
    dct:created "2019-04-05"^^xsd:date ;
    rdfs:subClassOf dpv:Purpose ;
    sw:term_status "accepted"@en ;
    skos:definition "Purposes associated with ensuring and enforcing security for data, personnel, or other related matters"@en ;
    skos:prefLabel "Enforce Security"@en ;
    skos:scopeNote "Was previous \"Security\". Prefixed to distinguish from TechOrg measures."@en .

dpv:EnterIntoContract a rdfs:Class,
        owl:Class,
        dpv:LegalBasis ;
    dct:contributor "Georg P Krog, Harshvardhan J. Pandit, Paul Ryan" ;
    dct:created "2021-04-07"^^xsd:date ;
    rdfs:subClassOf dpv:Contract ;
    sw:term_status "accepted"@en ;
    skos:definition "Processing necessary to enter into contract"@en ;
    skos:prefLabel "Enter Into Contract"@en .

dpv:Entity a rdfs:Class,
        owl:Class ;
    dct:contributor "Harshvardhan J. Pandit" ;
    dct:created "2022-02-02"^^xsd:date ;
    vann:example dex:E0027 ;
    rdfs:superClassOf dpv:LegalEntity,
        dpv:NaturalPerson,
        dpv:OrganisationalUnit ;
    sw:term_status "accepted"@en ;
    skos:definition "A human or non-human 'thing' that constitutes as an entity"@en ;
    skos:prefLabel "Entity"@en .

dpv:Erase a rdfs:Class,
        owl:Class,
        dpv:Processing ;
    dct:created "2019-05-07"^^xsd:date ;
    dct:source "(GDPR Art.4-2,https://eur-lex.europa.eu/eli/reg/2016/679/art_4/par_2/oj)"@en ;
    rdfs:subClassOf dpv:Remove ;
    sw:term_status "accepted"@en ;
    skos:definition "to delete data"@en ;
    skos:prefLabel "Erase"@en .

dpv:EstablishContractualAgreement a rdfs:Class,
        owl:Class,
        dpv:Purpose ;
    dct:contributor "Georg P Krog, Harshvardhan J. Pandit" ;
    dct:created "2022-11-09"^^xsd:date ;
    rdfs:subClassOf dpv:Purpose ;
    sw:term_status "accepted"@en ;
    skos:definition "Purposes associated with carrying out data processing to establish an agreement, such as for entering into a contract"@en ;
    skos:prefLabel "Establish Contractual Agreement"@en .

dpv:EvaluationOfIndividuals a rdfs:Class,
        owl:Class,
        dpv:EvaluationScoring ;
    dct:contributor "Harshvardhan J. Pandit" ;
    dct:created "2022-10-22"^^xsd:date ;
    dct:modified "2022-11-30"^^xsd:date ;
    dct:source "(GDPR Art.4-2,https://eur-lex.europa.eu/eli/reg/2016/679/art_4/par_2/oj)"@en ;
    rdfs:subClassOf dpv:EvaluationScoring ;
    sw:term_status "accepted"@en ;
    skos:definition "Processing that involves evaluation of individuals"@en ;
    skos:prefLabel "Evaluation of Individuals"@en .

dpv:EvaluationScoring a rdfs:Class,
        owl:Class ;
    dct:contributor "Harshvardhan J. Pandit, Piero Bonatti" ;
    dct:created "2020-11-04"^^xsd:date ;
    dct:source "(GDPR Art.4-2,https://eur-lex.europa.eu/eli/reg/2016/679/art_4/par_2/oj)"@en ;
    rdfs:subClassOf dpv:ProcessingContext ;
    sw:term_status "accepted"@en ;
    skos:definition "Processing that involves evaluation and scoring of individuals"@en ;
    skos:prefLabel "Evaluation and Scoring"@en .

dpv:ExplicitlyExpressedConsent a rdfs:Class,
        owl:Class,
        dpv:LegalBasis ;
    dct:contributor "Georg P Krog, Harshvardhan J. Pandit, Paul Ryan, Julian Flake" ;
    dct:created "2022-06-21"^^xsd:date ;
    rdfs:subClassOf dpv:ExpressedConsent ;
    sw:term_status "accepted"@en ;
    skos:definition "Consent that is expressed through an explicit action solely conveying a consenting decision"@en ;
    skos:prefLabel "Explicitly Expressed Consent"@en ;
    skos:scopeNote "Explicitly expressed consent is a more specific form of Expressed consent where the action taken must 'explicitly' relate to only the consent decision. Expressed consent where the consenting is part of other matters therefore cannot satisfy the requirements of explicitly expressed consent. An example of explicit action expressing the consenting decision is a button on a web form where the form only relates to consent, or it is accompanied with suitable text that reiterates what the consenting decision is about"@en .

dpv:ExpressedConsent a rdfs:Class,
        owl:Class,
        dpv:LegalBasis ;
    dct:contributor "Georg P Krog, Harshvardhan J. Pandit, Paul Ryan, Julian Flake" ;
    dct:created "2022-06-21"^^xsd:date ;
    rdfs:subClassOf dpv:InformedConsent ;
    sw:term_status "accepted"@en ;
    skos:definition "Consent that is expressed through an action intended to convey a consenting decision"@en ;
    skos:prefLabel "Expressed Consent"@en ;
    skos:scopeNote "Expressed consent requires the individual take a specific and unambigious action that directly indicates their consent. This action may be a part of other processes such as setting preferences, or agreeing to a contract, or other matters not relating to consent. An example of expressed consent is interacting with a checkbox within a dashboard or clicking a button on a web form"@en .

dpv:FederatedLocations a rdfs:Class,
        owl:Class,
        dpv:LocationFixture ;
    dct:contributor "Harshvardhan J. Pandit" ;
    dct:created "2022-06-15"^^xsd:date ;
    dct:modified "2020-10-05"^^xsd:date ;
    rdfs:subClassOf dpv:LocationFixture ;
    sw:term_status "accepted"@en ;
    skos:definition "Location that is federated across multiple separate areas with designation of a primary or central location"@en ;
    skos:prefLabel "Federated Locations"@en .

dpv:FileSystemSecurity a rdfs:Class,
        owl:Class,
        dpv:TechnicalMeasure ;
    dct:contributor "Harshvardhan J. Pandit" ;
    dct:created "2022-08-17"^^xsd:date ;
    dct:source "(ENISA Reference Incident Classification Taxonomy 2018,https://www.enisa.europa.eu/publications/reference-incident-classification-taxonomy/)"@en ;
    rdfs:subClassOf dpv:SecurityMethod ;
    sw:term_status "accepted"@en ;
    skos:definition "Security implemented over a file system"@en ;
    skos:prefLabel "File System Security"@en .

dpv:Filter a rdfs:Class,
        owl:Class,
        dpv:Processing ;
    dct:contributor "Harshvardhan J. Pandit, Georg P Krog" ;
    dct:created "2022-06-15"^^xsd:date ;
    rdfs:subClassOf dpv:Transform ;
    sw:term_status "accepted"@en ;
    skos:definition "to filter or keep data for some criteria"@en ;
    skos:prefLabel "Filter"@en .

dpv:FixedLocation a rdfs:Class,
        owl:Class,
        dpv:LocationFixture ;
    dct:contributor "Harshvardhan J. Pandit" ;
    dct:created "2022-06-15"^^xsd:date ;
    dct:modified "2020-10-05"^^xsd:date ;
    rdfs:subClassOf dpv:LocationFixture ;
    sw:term_status "accepted"@en ;
    skos:definition "Location that is fixed i.e. known to occur at a specific place"@en ;
    skos:prefLabel "Fixed Location"@en .

dpv:FixedMultipleLocations a rdfs:Class,
        owl:Class,
        dpv:LocationFixture ;
    dct:contributor "Harshvardhan J. Pandit" ;
    dct:created "2022-06-15"^^xsd:date ;
    dct:modified "2020-10-05"^^xsd:date ;
    rdfs:subClassOf dpv:FixedLocation ;
    sw:term_status "accepted"@en ;
    skos:definition "Location that is fixed with multiple places e.g. multiple cities"@en ;
    skos:prefLabel "Fixed Multiple Locations"@en .

dpv:FixedOccurencesDuration a rdfs:Class,
        owl:Class ;
    dct:contributor "Harshvardhan J. Pandit" ;
    dct:created "2022-06-15"^^xsd:date ;
    dct:modified "2020-10-05"^^xsd:date ;
    rdfs:subClassOf dpv:Duration ;
    sw:term_status "accepted"@en ;
    skos:definition "Duration that takes place a fixed number of times e.g. 3 times"@en ;
    skos:prefLabel "Fixed Occurences Duration"@en .

dpv:FixedSingularLocation a rdfs:Class,
        owl:Class,
        dpv:LocationFixture ;
    dct:contributor "Harshvardhan J. Pandit" ;
    dct:created "2022-06-15"^^xsd:date ;
    dct:modified "2020-10-05"^^xsd:date ;
    rdfs:subClassOf dpv:FixedLocation ;
    sw:term_status "accepted"@en ;
    skos:definition "Location that is fixed at a specific place e.g. a city"@en ;
    skos:prefLabel "Fixed Singular Location"@en .

dpv:ForProfitOrganisation a rdfs:Class,
        owl:Class ;
    dct:contributor "Harshvardhan J. Pandit" ;
    dct:created "2022-02-02"^^xsd:date ;
    dct:modified "2020-10-05"^^xsd:date ;
    rdfs:subClassOf dpv:Organisation ;
    sw:term_status "accepted"@en ;
    skos:definition "An organisation that aims to achieve profit as its primary goal"@en ;
    skos:prefLabel "For-Profit Organisation"@en .

dpv:FraudPreventionAndDetection a rdfs:Class,
        owl:Class,
        dpv:Purpose ;
    dct:contributor "Harshvardhan J. Pandit, Javier Fernandez, Axel Polleres, Elmar Kiesling, Fajar Ekaputra, Simon Steyskal" ;
    dct:created "2019-04-05"^^xsd:date ;
    rdfs:subClassOf dpv:EnforceSecurity ;
    sw:term_status "accepted"@en ;
    skos:definition "Purposes associated with fraud detection, prevention, and mitigation"@en ;
    skos:prefLabel "Fraud Prevention and Detection"@en ;
    skos:related "svpu:Government"@en .

dpv:Frequency a rdfs:Class,
        owl:Class ;
    dct:contributor "Harshvardhan J. Pandit" ;
    dct:created "2022-02-16"^^xsd:date ;
    rdfs:subClassOf dpv:Context ;
    sw:term_status "accepted"@en ;
    skos:definition "The frequency or information about periods and repetitions in terms of recurrence."@en ;
    skos:prefLabel "Frequency"@en .

dpv:FulfilmentOfContractualObligation a rdfs:Class,
        owl:Class,
        dpv:Purpose ;
    dct:contributor "Georg P Krog, Harshvardhan J. Pandit" ;
    dct:created "2022-11-09"^^xsd:date ;
    rdfs:subClassOf dpv:FulfilmentOfObligation ;
    sw:term_status "accepted"@en ;
    skos:definition "Purposes associated with carrying out data processing to fulfill a contractual obligation"@en ;
    skos:prefLabel "Fulfilment of Contractual Obligation"@en .

dpv:FulfilmentOfObligation a rdfs:Class,
        owl:Class,
        dpv:Purpose ;
    dct:contributor "Georg P Krog, Harshvardhan J. Pandit" ;
    dct:created "2022-11-09"^^xsd:date ;
    rdfs:subClassOf dpv:Purpose ;
    sw:term_status "accepted"@en ;
    skos:definition "Purposes associated with carrying out data processing to fulfill an obligation"@en ;
    skos:prefLabel "Fulfilment of Obligation"@en .

dpv:FullAutomation a rdfs:Class,
        owl:Class,
        dpv:Automation ;
    dct:created "2023-12-10"^^xsd:date ;
    rdfs:subClassOf dpv:Automation ;
    sw:term_status "accepted"@en ;
    skos:definition "The system is capable of performing its entire mission without external intervention"@en ;
    skos:prefLabel "Full Automation"@en ;
    skos:scopeNote "Though Fully Automated such operations can still be associated with dpv:HumanInvolved e.g. for inputs, oversight or verification"@en .

dpv:FullyRandomisedPseudonymisation a rdfs:Class,
        owl:Class,
        dpv:TechnicalMeasure ;
    dct:contributor "Harshvardhan J. Pandit" ;
    dct:created "2022-08-17"^^xsd:date ;
    dct:source "(ENISA Data Pseudonymisation: Advanced Techniques and Use Cases,https://www.enisa.europa.eu/publications/data-pseudonymisation-advanced-techniques-and-use-cases)"@en ;
    rdfs:subClassOf dpv:Pseudonymisation ;
    sw:term_status "accepted"@en ;
    skos:definition "Use of randomised pseudonymisation where the same elements are assigned different values each time they occur"@en ;
    skos:prefLabel "Fully Randomised Pseudonymisation"@en .

dpv:Generate a rdfs:Class,
        owl:Class,
        dpv:Processing ;
    dct:contributor "Harshvardhan J. Pandit" ;
    dct:created "2022-04-20"^^xsd:date ;
    rdfs:subClassOf dpv:Obtain ;
    sw:term_status "accepted"@en ;
    skos:definition "to generate or create data"@en ;
    skos:prefLabel "Generate"@en .

dpv:GeneratedData a rdfs:Class,
        owl:Class ;
    dct:created "2023-12-10"^^xsd:date ;
    rdfs:subClassOf dpv:Data ;
    rdfs:superClassOf dpv:SyntheticData ;
    sw:term_status "accepted"@en ;
    skos:definition "Data that has been obtained through generation or creation as a source"@en ;
    skos:prefLabel "Generated Data"@en .

dpv:GeneratedPersonalData a rdfs:Class,
        owl:Class ;
    dct:contributor "Harshvardhan J. Pandit" ;
    dct:created "2022-03-30"^^xsd:date ;
    dct:modified "2023-12-10"^^xsd:date ;
    rdfs:subClassOf dpv:InferredData,
        dpv:PersonalData ;
    rdfs:superClassOf dpv:InferredPersonalData ;
    sw:term_status "accepted"@en ;
    skos:definition "Personal Data that is generated or brought into existence without relation to existing data i.e. it is not derived or inferred from other data"@en ;
    skos:prefLabel "Generated Personal Data"@en ;
    skos:scopeNote "Generated Data is used to indicate data that is produced and is not derived or inferred from other data"@en .

dpv:GeographicCoverage a rdfs:Class,
        owl:Class ;
    dct:contributor "Harshvardhan J. Pandit, Georg P Krog, Paul Ryan" ;
    dct:created "2022-06-15"^^xsd:date ;
    rdfs:subClassOf dpv:Scale ;
    sw:term_status "accepted"@en ;
    skos:definition "Indicate of scale in terms of geographic coverage"@en ;
    skos:prefLabel "Geographic Coverage"@en .

dpv:GlobalScale a rdfs:Class,
        owl:Class,
        dpv:GeographicCoverage ;
    dct:contributor "Harshvardhan J. Pandit" ;
    dct:created "2022-06-15"^^xsd:date ;
    rdfs:subClassOf dpv:GeographicCoverage ;
    sw:term_status "accepted"@en ;
    skos:definition "Geographic coverage spanning the entire globe"@en ;
    skos:prefLabel "Global Scale"@en .

dpv:GovernanceProcedures a rdfs:Class,
        owl:Class,
        dpv:OrganisationalMeasure ;
    dct:contributor "Harshvardhan J. Pandit" ;
    dct:created "2022-08-17"^^xsd:date ;
    dct:source "(ENISA 5G Cybersecurity Standards,https://www.enisa.europa.eu/publications/5g-cybersecurity-standards)"@en ;
    rdfs:subClassOf dpv:OrganisationalMeasure ;
    sw:term_status "accepted"@en ;
    skos:definition "Procedures related to governance (e.g. organisation, unit, team, process, system)"@en ;
    skos:prefLabel "Governance Procedures"@en .

dpv:GovernmentalOrganisation a rdfs:Class,
        owl:Class ;
    dct:contributor "Harshvardhan J. Pandit" ;
    dct:created "2022-02-02"^^xsd:date ;
    dct:modified "2020-10-05"^^xsd:date ;
    rdfs:subClassOf dpv:Organisation ;
    rdfs:superClassOf dpv:Authority ;
    sw:term_status "accepted"@en ;
    skos:definition "An organisation managed or part of government"@en ;
    skos:prefLabel "Governmental Organisation"@en .

dpv:GuardianOfDataSubject a rdfs:Class,
        owl:Class,
        dpv:DataSubject ;
    dct:contributor "Georg P Krog" ;
    dct:created "2022-08-03"^^xsd:date ;
    rdfs:subClassOf dpv:DataSubject ;
    sw:term_status "accepted"@en ;
    skos:definition "Guardian(s) of data subjects such as children"@en ;
    skos:prefLabel "Guardian(s) of Data Subject"@en .

dpv:GuidelinesPrinciple a rdfs:Class,
        owl:Class,
        dpv:OrganisationalMeasure ;
    dct:contributor "Axel Polleres, Rob Brennan, Harshvardhan J. Pandit, Mark Lizar" ;
    dct:created "2019-04-05"^^xsd:date ;
    rdfs:subClassOf dpv:OrganisationalMeasure ;
    sw:term_status "accepted"@en ;
    skos:definition "Guidelines or Principles regarding processing and operational measures"@en ;
    skos:prefLabel "GuidelinesPrinciple"@en .

dpv:HardwareSecurityProtocols a rdfs:Class,
        owl:Class,
        dpv:TechnicalMeasure ;
    dct:contributor "Harshvardhan J. Pandit" ;
    dct:created "2022-08-17"^^xsd:date ;
    dct:source "(ENISA Reference Incident Classification Taxonomy 2018,https://www.enisa.europa.eu/publications/reference-incident-classification-taxonomy/)"@en ;
    rdfs:subClassOf dpv:SecurityMethod ;
    sw:term_status "accepted"@en ;
    skos:definition "Security protocols implemented at or within hardware"@en ;
    skos:prefLabel "Hardware Security Protocols"@en .

dpv:Harm a rdfs:Class,
        owl:Class,
        dpv:Impact ;
    dct:contributor "Harshvardhan J. Pandit, Julian Flake, Georg P Krog, Fajar Ekaputra, Beatriz Esteves" ;
    dct:created "2022-08-13"^^xsd:date ;
    vann:example dex:E0029 ;
    rdfs:subClassOf dpv:Damage ;
    sw:term_status "changed"@en ;
    skos:definition "Impact that acts as or causes harms"@en ;
    skos:prefLabel "Harm"@en .

dpv:HashFunctions a rdfs:Class,
        owl:Class,
        dpv:TechnicalMeasure ;
    dct:contributor "Harshvardhan J. Pandit" ;
    dct:created "2022-08-17"^^xsd:date ;
    dct:source "(ENISA Reference Incident Classification Taxonomy 2018,https://www.enisa.europa.eu/publications/reference-incident-classification-taxonomy/)"@en ;
    rdfs:subClassOf dpv:CryptographicMethods ;
    sw:term_status "accepted"@en ;
    skos:definition "Use of hash functions to map information or to retrieve a prior categorisation"@en ;
    skos:prefLabel "Hash Functions"@en .

dpv:HashMessageAuthenticationCode a rdfs:Class,
        owl:Class,
        dpv:TechnicalMeasure ;
    dct:contributor "Harshvardhan J. Pandit" ;
    dct:created "2022-08-17"^^xsd:date ;
    dct:source "(ENISA 5G Cybersecurity Standards,https://www.enisa.europa.eu/publications/5g-cybersecurity-standards)"@en ;
    rdfs:subClassOf dpv:CryptographicAuthentication ;
    sw:term_status "accepted"@en ;
    skos:definition "Use of HMAC where message authentication code (MAC) utilise a cryptographic hash function and a secret cryptographic key"@en ;
    skos:prefLabel "Hash-based Message Authentication Code (HMAC)"@en .

dpv:HighAutomation a rdfs:Class,
        owl:Class,
        dpv:Automation ;
    dct:created "2023-12-10"^^xsd:date ;
    rdfs:subClassOf dpv:Automation ;
    sw:term_status "accepted"@en ;
    skos:definition "The system performs parts of its mission without external intervention"@en ;
    skos:prefLabel "High Automation"@en ;
    skos:scopeNote "Human Involvement is implied here, e.g. for intervention, input, decisions"@en .

dpv:HomomorphicEncryption a rdfs:Class,
        owl:Class,
        dpv:TechnicalMeasure ;
    dct:contributor "Harshvardhan J. Pandit" ;
    dct:created "2022-08-17"^^xsd:date ;
    dct:source "(ENISA Reference Incident Classification Taxonomy 2018,https://www.enisa.europa.eu/publications/reference-incident-classification-taxonomy/)"@en ;
    rdfs:subClassOf dpv:CryptographicMethods ;
    sw:term_status "accepted"@en ;
    skos:definition "Use of Homomorphic encryption that permits computations on encrypted data without decrypting it"@en ;
    skos:prefLabel "Homomorphic Encryption"@en .

dpv:HugeDataVolume a rdfs:Class,
        owl:Class,
        dpv:DataVolume ;
    dct:contributor "Harshvardhan J. Pandit" ;
    dct:created "2022-06-15"^^xsd:date ;
    rdfs:subClassOf dpv:DataVolume ;
    sw:term_status "accepted"@en ;
    skos:definition "Data volume that is considered huge or more than large within the context"@en ;
    skos:prefLabel "Huge Data Volume"@en .

dpv:HugeScaleOfDataSubjects a rdfs:Class,
        owl:Class,
        dpv:DataSubjectScale ;
    dct:contributor "Harshvardhan J. Pandit" ;
    dct:created "2022-06-15"^^xsd:date ;
    rdfs:subClassOf dpv:DataSubjectScale ;
    sw:term_status "accepted"@en ;
    skos:definition "Scale of data subjects considered huge or more than large within the context"@en ;
    skos:prefLabel "Huge Scale Of Data Subjects"@en .

dpv:HumanInvolved a rdfs:Class,
        owl:Class,
        dpv:HumanInvolvement ;
    dct:created "2022-09-03"^^xsd:date ;
    dct:modified "2023-12-10"^^xsd:date ;
    rdfs:subClassOf dpv:HumanInvolvement ;
    sw:term_status "accepted"@en ;
    skos:definition "Humans are involved in the specified context"@en ;
    skos:prefLabel "Human involved"@en ;
    skos:scopeNote "This concept only indicates that humans are involved. For specific involvement, see specialised concepts e.g. involved for input, oversight."@en .

dpv:HumanInvolvement a rdfs:Class,
        owl:Class ;
    dct:contributor "Harshvardhan J. Pandit" ;
    dct:created "2022-01-26"^^xsd:date ;
    dct:modified "2023-12-10"^^xsd:date ;
    rdfs:subClassOf dpv:ProcessingContext ;
    sw:term_status "accepted"@en ;
    skos:definition "The involvement of humans in specified context"@en ;
    skos:prefLabel "Human Involvement"@en ;
    skos:scopeNote "Human Involvement here broadly refers to any involvement by a human in the context of carrying out processing. This may include verification of outcomes, providing input data for making decisions, or overseeing activities. To indicate whether humans are involved or not, see relevant concepts of dpv:HumanInvolved and dpv:HumanNotInvolved. The term 'Human in the loop' and its varieties are absent from DPV due to their contradictory and non-compatible use across different sources."@en .

dpv:HumanInvolvementForControl a rdfs:Class,
        owl:Class,
        dpv:HumanInvolvement ;
    dct:created "2022-09-04"^^xsd:date ;
    dct:modified "2023-12-10"^^xsd:date ;
    rdfs:subClassOf dpv:HumanInvolvement ;
    sw:term_status "accepted"@en ;
    skos:definition "Human involvement for the purposes of exercising control over the specified operations in context"@en ;
    skos:prefLabel "Human Involvement for control"@en ;
    skos:scopeNote "Control is a broad term that can be applied to various stages and operations. It maps to None, Assistive, and Partial automation models."@en .

dpv:HumanInvolvementForDecision a rdfs:Class,
        owl:Class,
        dpv:HumanInvolvement ;
    dct:created "2022-09-06"^^xsd:date ;
    dct:modified "2023-12-10"^^xsd:date ;
    rdfs:subClassOf dpv:HumanInvolvement ;
    sw:term_status "accepted"@en ;
    skos:definition "Human involvement for the purposes of exercising decisions over the specified operations in context"@en ;
    skos:prefLabel "Human Involvement for decision"@en ;
    skos:scopeNote "Decisions are about exercising control over the operation, and are distinct from input (data or parameters)."@en .

dpv:HumanInvolvementForInput a rdfs:Class,
        owl:Class,
        dpv:HumanInvolvement ;
    dct:contributor "Harshvardhan J. Pandit" ;
    dct:created "2022-09-07"^^xsd:date ;
    dct:modified "2023-12-10"^^xsd:date ;
    rdfs:subClassOf dpv:HumanInvolvement ;
    sw:term_status "accepted"@en ;
    skos:definition "Human involvement for the purposes of providing inputs to the specified context"@en ;
    skos:prefLabel "Human Involvement for Input"@en ;
    skos:scopeNote "Inputs can be in the form of data or other resources."@en .

dpv:HumanInvolvementForIntervention a rdfs:Class,
        owl:Class,
        dpv:HumanInvolvement ;
    dct:created "2022-09-05"^^xsd:date ;
    dct:modified "2023-12-10"^^xsd:date ;
    rdfs:subClassOf dpv:HumanInvolvement ;
    sw:term_status "accepted"@en ;
    skos:definition "Human involvement for the purposes of exercising interventions over the specified operations in context"@en ;
    skos:prefLabel "Human Involvement for intervention"@en ;
    skos:scopeNote "Intervention indicates the ability to intervene in operations, which can be at various stages. It maps to Conditional and High automation models."@en .

dpv:HumanInvolvementForOversight a rdfs:Class,
        owl:Class,
        dpv:HumanInvolvement ;
    dct:contributor "Harshvardhan J. Pandit" ;
    dct:created "2022-09-07"^^xsd:date ;
    dct:modified "2023-12-10"^^xsd:date ;
    rdfs:subClassOf dpv:HumanInvolvement ;
    sw:term_status "accepted"@en ;
    skos:definition "Human involvement for the purposes of having oversight over the specified context regarding its operations, inputs, or outputs"@en ;
    skos:prefLabel "Human Involvement for Oversight"@en ;
    skos:scopeNote "Oversight by itself does not indicate the ability to intervene or control the operations."@en .

dpv:HumanInvolvementForVerification a rdfs:Class,
        owl:Class,
        dpv:HumanInvolvement ;
    dct:contributor "Harshvardhan J. Pandit" ;
    dct:created "2022-09-07"^^xsd:date ;
    dct:modified "2023-12-10"^^xsd:date ;
    rdfs:subClassOf dpv:HumanInvolvement ;
    sw:term_status "accepted"@en ;
    skos:definition "Human involvement for the purposes of verification of specified context to ensure its operations, inputs, or outputs are correct or are acceptable."@en ;
    skos:prefLabel "Human Involvement for Verification"@en ;
    skos:scopeNote "Verification by itself does not imply ability to Control, Intervene, or having Oversight."@en .

dpv:HumanNotInvolved a rdfs:Class,
        owl:Class,
        dpv:HumanInvolvement ;
    dct:created "2023-12-10"^^xsd:date ;
    rdfs:subClassOf dpv:HumanInvolvement ;
    sw:term_status "accepted"@en ;
    skos:definition "Humans are not involved in the specified context"@en ;
    skos:prefLabel "Human not involved"@en ;
    skos:scopeNote "This maps to Autonomous and Full Automation models if no humans are involved."@en .

dpv:HumanResourceManagement a rdfs:Class,
        owl:Class,
        dpv:Purpose ;
    dct:contributor "Paul Ryan, David Hickey, Georg P Krog, Harshvardhan J. Pandit, Beatriz Esteves" ;
    dct:created "2021-09-01"^^xsd:date ;
    dct:source "(Belgian DPA ROPA Template, https://www.privacycommission.be/nl/model-voor-een-register-van-de-verwerkingsactiviteiten)"@en ;
    rdfs:subClassOf dpv:Purpose ;
    sw:term_status "accepted"@en ;
    skos:definition "Purposes associated with managing humans and 'human resources' within the organisation for effective and efficient operations."@en ;
    skos:prefLabel "Human Resource Management"@en ;
    skos:scopeNote "HR is a broad concept. Its management includes, amongst others - recruiting employees and intermediaries e.g. brokers, independent representatives; payroll administration, remunerations, commissions, and wages; and application of social legislation."@en .

dpv:IdentifyingPersonalData a rdfs:Class,
        owl:Class ;
    rdfs:subClassOf dpv:PersonalData ;
    sw:term_status "accepted"@en ;
    skos:definition "Personal Data that explicitly and by itself is sufficient to identify a person"@en ;
    skos:prefLabel "Identifying Personal Data"@en ;
    skos:scopeNote "DPV does not use PII ('Personally Identifiable Information') as it has varying and conflicting definitions across sources. Instead the concept 'identifying personal data' is intended to provide a clear categorisation of its interpretation. Where multiple data categories can be combined to create an 'identifying' category e.g. fingerprinting, this concept represents the combined category."@en .

dpv:IdentityManagementMethod a rdfs:Class,
        owl:Class,
        dpv:OrganisationalMeasure ;
    dct:contributor "Harshvardhan J. Pandit" ;
    dct:created "2022-08-17"^^xsd:date ;
    dct:source "(ENISA Reference Incident Classification Taxonomy 2018,https://www.enisa.europa.eu/publications/reference-incident-classification-taxonomy/)"@en ;
    rdfs:subClassOf dpv:AuthorisationProcedure ;
    sw:term_status "accepted"@en ;
    skos:definition "Management of identity and identity-based processes"@en ;
    skos:prefLabel "Identity Management Method"@en .

dpv:IdentityVerification a rdfs:Class,
        owl:Class,
        dpv:Purpose ;
    dct:contributor "Harshvardhan J. Pandit, Javier Fernandez, Axel Polleres, Elmar Kiesling, Fajar Ekaputra, Simon Steyskal" ;
    dct:created "2019-04-05"^^xsd:date ;
    rdfs:subClassOf dpv:EnforceSecurity ;
    sw:term_status "accepted"@en ;
    skos:definition "Purposes associated with verifying or authorising identity as a form of security"@en ;
    skos:prefLabel "Identity Verification"@en .

dpv:Immigrant a rdfs:Class,
        owl:Class,
        dpv:DataSubject ;
    dct:contributor "Harshvardhan J. Pandit, Georg P. Krog, Julian Flake, Paul Ryan, Beatriz Esteves" ;
    dct:created "2022-04-06"^^xsd:date ;
    rdfs:subClassOf dpv:DataSubject ;
    sw:term_status "accepted"@en ;
    skos:definition "Data subjects that are immigrants (for a jurisdiction)"@en ;
    skos:prefLabel "Immigrant"@en .

dpv:Impact a rdfs:Class,
        owl:Class ;
    dct:contributor "Harshvardhan J. Pandit, Julian Flake, Georg P Krog, Fajar Ekaputra, Beatriz Esteves" ;
    dct:created "2022-03-23"^^xsd:date ;
    vann:example dex:E0029 ;
    rdfs:subClassOf dpv:Consequence ;
    sw:term_status "accepted"@en ;
    skos:definition "The impact(s) possible or arising as a consequence from specified context"@en ;
    skos:prefLabel "Impact"@en ;
    skos:scopeNote "Impact is a stronger notion of consequence in terms of influence, change, or effect on something e.g. for impact assessments"@en .

dpv:ImpactAssessment a rdfs:Class,
        owl:Class,
        dpv:OrganisationalMeasure ;
    dct:contributor "Georg P Krog, Harshvardhan J. Pandit, Paul Ryan" ;
    dct:created "2020-11-04"^^xsd:date ;
    rdfs:subClassOf dpv:Assessment ;
    sw:term_status "accepted"@en ;
    skos:definition "Calculating or determining the likelihood of impact of an existing or proposed process, which can involve risks or detriments."@en ;
    skos:prefLabel "Impact Assessment"@en .

dpv:ImpliedConsent a rdfs:Class,
        owl:Class,
        dpv:LegalBasis ;
    dct:contributor "Georg P Krog, Harshvardhan J. Pandit, Paul Ryan, Julian Flake" ;
    dct:created "2022-06-21"^^xsd:date ;
    rdfs:subClassOf dpv:InformedConsent ;
    sw:term_status "accepted"@en ;
    skos:definition "Consent that is implied indirectly through an action not associated solely with conveying a consenting decision"@en ;
    skos:prefLabel "Implied Consent"@en ;
    skos:scopeNote "Implied consent is expected to also be Informed Consent. An example is a CCTV notice outside a monitored area that informs the individuals that by walking in they would be consenting to the use of camera for surveillance."@en .

dpv:Importance a rdfs:Class,
        owl:Class ;
    dct:contributor "Harshvardhan J. Pandit, Paul Ryan, Georg P Krog, Julian Flake, Beatriz Esteves" ;
    dct:created "2022-02-09"^^xsd:date ;
    rdfs:subClassOf dpv:Context ;
    sw:term_status "accepted"@en ;
    skos:definition "An indication of 'importance' within a context"@en ;
    skos:prefLabel "Importance"@en ;
    skos:scopeNote "Importance can be used to express importance, desirability, relevance, or significance as a context."@en .

dpv:ImproveExistingProductsAndServices a rdfs:Class,
        owl:Class,
        dpv:Purpose ;
    dct:contributor "Harshvardhan J. Pandit, Javier Fernandez, Axel Polleres, Elmar Kiesling, Fajar Ekaputra, Simon Steyskal" ;
    dct:created "2019-04-05"^^xsd:date ;
    rdfs:subClassOf dpv:OptimisationForController ;
    sw:term_status "accepted"@en ;
    skos:definition "Purposes associated with improving existing products and services"@en ;
    skos:prefLabel "Improve Existing Products and Services"@en .

dpv:ImproveInternalCRMProcesses a rdfs:Class,
        owl:Class,
        dpv:Purpose ;
    dct:contributor "Harshvardhan J. Pandit, Javier Fernandez, Axel Polleres, Elmar Kiesling, Fajar Ekaputra, Simon Steyskal" ;
    dct:created "2019-04-05"^^xsd:date ;
    rdfs:subClassOf dpv:CustomerRelationshipManagement,
        dpv:OptimisationForController ;
    sw:term_status "accepted"@en ;
    skos:definition "Purposes associated with improving customer-relationship management (CRM) processes"@en ;
    skos:prefLabel "Improve Internal CRM Processes"@en .

dpv:IncidentManagementProcedures a rdfs:Class,
        owl:Class,
        dpv:OrganisationalMeasure ;
    dct:contributor "Harshvardhan J. Pandit" ;
    dct:created "2022-08-17"^^xsd:date ;
    dct:source "(ENISA 5G Cybersecurity Standards,https://www.enisa.europa.eu/publications/5g-cybersecurity-standards)"@en ;
    rdfs:subClassOf dpv:GovernanceProcedures ;
    sw:term_status "accepted"@en ;
    skos:definition "Procedures related to management of incidents"@en ;
    skos:prefLabel "Incident Management Procedures"@en .

dpv:IncidentReportingCommunication a rdfs:Class,
        owl:Class,
        dpv:OrganisationalMeasure ;
    dct:contributor "Harshvardhan J. Pandit" ;
    dct:created "2022-08-17"^^xsd:date ;
    dct:source "(ENISA 5G Cybersecurity Standards,https://www.enisa.europa.eu/publications/5g-cybersecurity-standards)"@en ;
    rdfs:subClassOf dpv:GovernanceProcedures ;
    sw:term_status "accepted"@en ;
    skos:definition "Procedures related to management of incident reporting"@en ;
    skos:prefLabel "Incident Reporting Communication"@en .

dpv:IncorrectData a rdfs:Class,
        owl:Class ;
    dct:contributor "Harshvardhan J. Pandit" ;
    dct:created "2022-11-02"^^xsd:date ;
    rdfs:subClassOf dpv:Data ;
    sw:term_status "accepted"@en ;
    skos:definition "Data that is known to be incorrect or inconsistent with some requirements"@en ;
    skos:prefLabel "Incorrect Data"@en .

dpv:IncreaseServiceRobustness a rdfs:Class,
        owl:Class,
        dpv:Purpose ;
    dct:contributor "Harshvardhan J. Pandit, Javier Fernandez, Axel Polleres, Elmar Kiesling, Fajar Ekaputra, Simon Steyskal" ;
    dct:created "2019-04-05"^^xsd:date ;
    rdfs:subClassOf dpv:OptimisationForController ;
    sw:term_status "accepted"@en ;
    skos:definition "Purposes associated with improving robustness and resilience of services"@en ;
    skos:prefLabel "Increase Service Robustness"@en .

dpv:IndeterminateDuration a rdfs:Class,
        owl:Class,
        dpv:Duration ;
    dct:contributor "Harshvardhan J. Pandit" ;
    dct:created "2022-11-30"^^xsd:date ;
    rdfs:subClassOf dpv:Duration ;
    sw:term_status "accepted"@en ;
    skos:definition "Duration that is indeterminate or cannot be determined"@en ;
    skos:prefLabel "Indeterminate Duration"@en ;
    skos:scopeNote "Indeterminate means (exact or otherwise) information about the duration cannot be determined, which is distinct from 'EndlessDuration' where it is known (or decided) that the duration is open-ended or without an end."@en .

dpv:IndustryConsortium a rdfs:Class,
        owl:Class ;
    dct:contributor "Harshvardhan J. Pandit" ;
    dct:created "2022-02-02"^^xsd:date ;
    dct:modified "2020-10-05"^^xsd:date ;
    dct:source "(ADMS controlled vocabulary,http://purl.org/adms)"@en ;
    rdfs:subClassOf dpv:Organisation ;
    sw:term_status "accepted"@en ;
    skos:definition "A consortium established and comprising on industry organisations"@en ;
    skos:prefLabel "Industry Consortium"@en .

dpv:Infer a rdfs:Class,
        owl:Class,
        dpv:Processing ;
    dct:contributor "Harshvardhan J. Pandit" ;
    dct:created "2022-04-20"^^xsd:date ;
    dct:modified "2022-10-14"^^xsd:date ;
    vann:example dex:E0014 ;
    rdfs:subClassOf dpv:Derive ;
    sw:term_status "accepted"@en ;
    skos:definition "to infer data from existing data"@en ;
    skos:prefLabel "Infer"@en ;
    skos:scopeNote "Infer indicates data that is derived without it being present or obtainable from existing data. For data that is presented, and is 'extracted' or 'obtained' from existing data, see Derive."@en .

dpv:InferredData a rdfs:Class,
        owl:Class ;
    dct:created "2023-12-10"^^xsd:date ;
    rdfs:subClassOf dpv:Data ;
    rdfs:superClassOf dpv:GeneratedPersonalData ;
    sw:term_status "accepted"@en ;
    skos:definition "Data that has been obtained through inferences of other data"@en ;
    skos:prefLabel "Inferred Data"@en .

dpv:InferredPersonalData a rdfs:Class,
        owl:Class ;
    dct:contributor "Harshvardhan J. Pandit" ;
    dct:created "2022-01-19"^^xsd:date ;
    dct:modified "2023-12-10"^^xsd:date ;
    rdfs:subClassOf dpv:DerivedPersonalData,
        dpv:GeneratedPersonalData ;
    sw:term_status "accepted"@en ;
    skos:definition "Personal Data that is obtained through inference from other data"@en ;
    skos:prefLabel "Inferred Personal Data"@en ;
    skos:scopeNote "Inferred Data is derived data generated from existing data, but which did not originally exist within it, e.g. inferring demographics from browsing history."@en .

dpv:InformationFlowControl a rdfs:Class,
        owl:Class,
        dpv:TechnicalMeasure ;
    dct:contributor "Harshvardhan J. Pandit" ;
    dct:created "2022-08-17"^^xsd:date ;
    dct:source "(ENISA Reference Incident Classification Taxonomy 2018,https://www.enisa.europa.eu/publications/reference-incident-classification-taxonomy/)"@en ;
    rdfs:subClassOf dpv:TechnicalMeasure ;
    sw:term_status "accepted"@en ;
    skos:definition "Use of measures to control information flows"@en ;
    skos:prefLabel "Information Flow Control"@en .

dpv:InformationSecurityPolicy a rdfs:Class,
        owl:Class,
        dpv:OrganisationalMeasure ;
    dct:contributor "Harshvardhan J. Pandit" ;
    dct:created "2022-08-17"^^xsd:date ;
    dct:source "(ENISA 5G Cybersecurity Standards,https://www.enisa.europa.eu/publications/5g-cybersecurity-standards)"@en ;
    rdfs:subClassOf dpv:Policy ;
    sw:term_status "accepted"@en ;
    skos:definition "Policy regarding security of information"@en ;
    skos:prefLabel "Information Security Policy"@en .

dpv:InformedConsent a rdfs:Class,
        owl:Class,
        dpv:LegalBasis ;
    dct:contributor "Georg P Krog, Harshvardhan J. Pandit, Paul Ryan, Julian Flake" ;
    dct:created "2022-06-21"^^xsd:date ;
    rdfs:subClassOf dpv:Consent ;
    sw:term_status "accepted"@en ;
    skos:definition "Consent that is informed i.e. with the requirement to provide sufficient information to make a consenting decision"@en ;
    skos:prefLabel "Informed Consent"@en ;
    skos:scopeNote "The specifics for what information should be provided or made available will depend on the context, use-case, or relevant legal requirements"@en .

dpv:InnovativeUseOfExistingTechnology a rdfs:Class,
        owl:Class,
        dpv:InnovativeUseOfTechnology ;
    dct:created "2023-12-10"^^xsd:date ;
    rdfs:subClassOf dpv:InnovativeUseOfTechnology ;
    sw:term_status "accepted"@en ;
    skos:definition "Involvement of existing technologies used in an innovative manner"@en ;
    skos:prefLabel "Innovative Use of Existing Technologies"@en .

dpv:InnovativeUseOfNewTechnologies a rdfs:Class,
        owl:Class,
        dpv:InnovativeUseOfTechnology ;
    dct:contributor "Harshvardhan J. Pandit, Piero Bonatti" ;
    dct:created "2020-11-04"^^xsd:date ;
    dct:modified "2023-12-10"^^xsd:date ;
    dct:source "(GDPR Art.4-2,https://eur-lex.europa.eu/eli/reg/2016/679/art_4/par_2/oj)"@en ;
    rdfs:subClassOf dpv:InnovativeUseOfTechnology ;
    sw:term_status "accepted"@en ;
    skos:definition "Involvement of a new (innovative) technologies"@en ;
    skos:prefLabel "Innovative Use of New Technologies"@en ;
    skos:scopeNote "New technologies are by definition considered innovative"@en .

dpv:InnovativeUseOfTechnology a rdfs:Class,
        owl:Class ;
    dct:created "2023-12-10"^^xsd:date ;
    rdfs:subClassOf dpv:ProcessingContext ;
    sw:term_status "accepted"@en ;
    skos:definition "Indicates that technology is being used in an innovative manner"@en ;
    skos:prefLabel "Innovative use of Technology"@en ;
    skos:scopeNote "Innovative here refers to 'state of the art' rather than the implementing entity, and can be for either new technology or new uses of existing technology"@en .

dpv:IntellectualPropertyData a rdfs:Class,
        owl:Class ;
    dct:source "DGA 5.10"@en ;
    rdfs:subClassOf dpv:Data ;
    sw:term_status "accepted"@en ;
    skos:definition "Data protected by Intellectual Property rights and regulations"@en ;
    skos:prefLabel "IntellectualPropertyData"@en .

dpv:InternalResourceOptimisation a rdfs:Class,
        owl:Class,
        dpv:Purpose ;
    dct:contributor "Harshvardhan J. Pandit, Javier Fernandez, Axel Polleres, Elmar Kiesling, Fajar Ekaputra, Simon Steyskal" ;
    dct:created "2019-04-05"^^xsd:date ;
    rdfs:subClassOf dpv:OptimisationForController ;
    sw:term_status "accepted"@en ;
    skos:definition "Purposes associated with optimisation of internal resource availability and usage for organisation"@en ;
    skos:prefLabel "Internal Resource Optimisation"@en .

dpv:InternationalOrganisation a rdfs:Class,
        owl:Class ;
    dct:contributor "Julian Flake, Georg P. Krog" ;
    dct:created "2022-03-23"^^xsd:date ;
    dct:modified "2020-10-05"^^xsd:date ;
    dct:source "(GDPR Art.4-26,https://eur-lex.europa.eu/eli/reg/2016/679/art_4/par_26/oj)"@en ;
    rdfs:subClassOf dpv:Organisation ;
    sw:term_status "accepted"@en ;
    skos:definition "An organisation and its subordinate bodies governed by public international law, or any other body which is set up by, or on the basis of, an agreement between two or more countries"@en ;
    skos:prefLabel "International Organisation"@en .

dpv:IntrusionDetectionSystem a rdfs:Class,
        owl:Class,
        dpv:TechnicalMeasure ;
    dct:contributor "Harshvardhan J. Pandit" ;
    dct:created "2022-08-17"^^xsd:date ;
    dct:source "(ENISA Reference Incident Classification Taxonomy 2018,https://www.enisa.europa.eu/publications/reference-incident-classification-taxonomy/)"@en ;
    rdfs:subClassOf dpv:SecurityMethod ;
    sw:term_status "accepted"@en ;
    skos:definition "Use of measures to detect intrusions and other unauthorised attempts to gain access to a system"@en ;
    skos:prefLabel "Intrusion Detection System"@en .

dpv:JobApplicant a rdfs:Class,
        owl:Class,
        dpv:DataSubject ;
    dct:contributor "Harshvardhan J. Pandit, Georg P. Krog, Julian Flake, Paul Ryan, Beatriz Esteves" ;
    dct:created "2022-04-06"^^xsd:date ;
    rdfs:subClassOf dpv:DataSubject ;
    sw:term_status "accepted"@en ;
    skos:definition "Data subjects that apply for jobs or employments"@en ;
    skos:prefLabel "Job Applicant"@en .

dpv:JointDataControllers a rdfs:Class,
        owl:Class ;
    dct:contributor "Georg Krog, Harshvardhan Pandit" ;
    dct:created "2022-02-02"^^xsd:date ;
    rdfs:subClassOf dpv:DataController ;
    sw:term_status "accepted"@en ;
    skos:definition "A group of Data Controllers that jointly determine the purposes and means of processing"@en ;
    skos:prefLabel "Joint Data Controllers"@en ;
    skos:scopeNote "While Joint Data Controllers operate together, they are made up of individually distinct legal entities. To indicate the membership of this group, hasDataController should be used to denote each Data Controller. The concept of Joint Data Controllers also allows specifying a single group as the 'Controller' and to specify role and responsibilities within that group for each entity using DPV's concepts (e.g. isImplementedByEntity)"@en .

dpv:JointDataControllersAgreement a rdfs:Class,
        owl:Class,
        dpv:OrganisationalMeasure ;
    dct:contributor "Georg P Krog, Harshvardhan J. Pandit, Beatriz Esteves, Paul Ryan, Julian Flake" ;
    dct:created "2022-01-26"^^xsd:date ;
    rdfs:subClassOf dpv:DataProcessingAgreement ;
    sw:term_status "accepted"@en ;
    skos:definition "An agreement outlining conditions, criteria, obligations, responsibilities, and specifics for carrying out processing of personal data between Controllers within a Joint Controllers relationship"@en ;
    skos:prefLabel "Joint Data Controllers Agreement"@en .

dpv:Justification a rdfs:Class,
        owl:Class ;
    dct:contributor "Harshvardhan J. Pandit" ;
    dct:created "2022-06-15"^^xsd:date ;
    rdfs:subClassOf dpv:Context ;
    sw:term_status "accepted"@en ;
    skos:definition "A form of documentation providing reaosns, explanations, or justifications"@en ;
    skos:prefLabel "Justification"@en .

dpv:LargeDataVolume a rdfs:Class,
        owl:Class,
        dpv:DataVolume ;
    dct:contributor "Harshvardhan J. Pandit" ;
    dct:created "2022-06-15"^^xsd:date ;
    rdfs:subClassOf dpv:DataVolume ;
    sw:term_status "accepted"@en ;
    skos:definition "Data volume that is considered large within the context"@en ;
    skos:prefLabel "Large Data Volume"@en .

dpv:LargeScaleOfDataSubjects a rdfs:Class,
        owl:Class,
        dpv:DataSubjectScale ;
    dct:contributor "Harshvardhan J. Pandit" ;
    dct:created "2022-06-15"^^xsd:date ;
    rdfs:subClassOf dpv:DataSubjectScale ;
    sw:term_status "accepted"@en ;
    skos:definition "Scale of data subjects considered large within the context"@en ;
    skos:prefLabel "Large Scale Of Data Subjects"@en .

dpv:LargeScaleProcessing a rdfs:Class,
        owl:Class,
        dpv:ProcessingScale ;
    dct:contributor "Harshvardhan J. Pandit, Piero Bonatti" ;
    dct:created "2020-11-04"^^xsd:date ;
    dct:modified "2022-09-07"^^xsd:date ;
    dct:source "(GDPR Art.4-2,https://eur-lex.europa.eu/eli/reg/2016/679/art_4/par_2/oj)"@en ;
    rdfs:subClassOf dpv:ProcessingScale ;
    sw:term_status "accepted"@en ;
    skos:definition "Processing that takes place at large scales (as specified by some criteria)"@en ;
    skos:prefLabel "Large Scale Processing"@en ;
    skos:scopeNote "The exact definition of what constitutes \"large scale\" depends on use of jurisdictional, domain-specific, or other forms of externally defined criterias. Where possible, this should be reflected by extending this term with the appropriate context."@en .

dpv:Law a rdfs:Class,
        owl:Class ;
    dct:contributor "Harshvardhan J. Pandit" ;
    dct:created "2022-01-19"^^xsd:date ;
    rdfs:subClassOf rdfs:Class ;
    sw:term_status "accepted"@en ;
    skos:definition "A law is a set of rules created by government or authorities"@en ;
    skos:prefLabel "Law"@en .

dpv:Lawful a rdfs:Class,
        owl:Class,
        dpv:Lawfulness ;
    dct:contributor "Harshvardhan J. Pandit" ;
    dct:created "2022-10-19"^^xsd:date ;
    rdfs:subClassOf dpv:Lawfulness ;
    sw:term_status "accepted"@en ;
    skos:definition "State of being lawful or legally compliant"@en ;
    skos:prefLabel "Lawful"@en .

dpv:Lawfulness a rdfs:Class,
        owl:Class ;
    dct:contributor "Harshvardhan J. Pandit" ;
    dct:created "2022-10-19"^^xsd:date ;
    rdfs:subClassOf dpv:ComplianceStatus ;
    sw:term_status "accepted"@en ;
    skos:definition "Status associated with expressing lawfullness or legal compliance"@en ;
    skos:prefLabel "Lawfulness"@en .

dpv:LawfulnessUnkown a rdfs:Class,
        owl:Class,
        dpv:Lawfulness ;
    dct:contributor "Harshvardhan J. Pandit" ;
    dct:created "2022-10-19"^^xsd:date ;
    rdfs:subClassOf dpv:Lawfulness ;
    sw:term_status "accepted"@en ;
    skos:definition "State of the lawfulness not being known"@en ;
    skos:prefLabel "Lawfulness Unknown"@en .

dpv:LegalAgreement a rdfs:Class,
        owl:Class,
        dpv:OrganisationalMeasure ;
    dct:contributor "Axel Polleres, Rob Brennan, Harshvardhan J. Pandit, Mark Lizar" ;
    dct:created "2019-04-05"^^xsd:date ;
    rdfs:subClassOf dpv:OrganisationalMeasure ;
    sw:term_status "accepted"@en ;
    skos:definition "A legally binding agreement"@en ;
    skos:prefLabel "Legal Agreement"@en .

dpv:LegalBasis a rdfs:Class,
        owl:Class ;
    dct:created "2019-04-05"^^xsd:date ;
    dct:modified "2020-11-04"^^xsd:date ;
    vann:example dex:E0022,
        dex:E0023 ;
    sw:term_status "accepted"@en ;
    skos:definition "Legal basis used to justify processing of data or use of technology in accordance with a law"@en ;
    skos:prefLabel "Legal Basis"@en ;
    skos:scopeNote "Legal basis (plural: legal bases) are defined by legislations and regulations, whose applicability is usually restricted to specific jurisdictions which can be represented using dpv:hasJurisdiction or dpv:hasLaw. Legal basis can be used without such declarations, e.g. 'Consent', however their interpretation will require association with a law, e.g. 'EU GDPR'."@en .

dpv:LegalCompliance a rdfs:Class,
        owl:Class,
        dpv:Purpose ;
    dct:contributor "Georg P Krog, Harshvardhan J. Pandit, Beatriz Esteves" ;
    dct:created "2020-11-04"^^xsd:date ;
    dct:modified "2022-11-09"^^xsd:date ;
    rdfs:subClassOf dpv:FulfilmentOfObligation ;
    sw:term_status "accepted"@en ;
    skos:definition "Purposes associated with carrying out data processing to fulfill a legal or statutory obligation"@en ;
    skos:prefLabel "Legal Compliance"@en ;
    skos:scopeNote "This purpose only refers to processing that is additionally required in order to fulfill the obligations and requirements associated with a law. For example, the use of consent would have its own separate purposes, with this purpose addressing a legal requirement for maintaining consent record (along with RecordManagement). This purpose will typically be used with Legal Obligation as the legal basis."@en .

dpv:LegalEntity a rdfs:Class,
        owl:Class ;
    dct:contributor "Harshvardhan J. Pandit" ;
    dct:created "2019-04-05"^^xsd:date ;
    rdfs:subClassOf dpv:Entity ;
    rdfs:superClassOf dpv:DataController,
        dpv:DataExporter,
        dpv:DataSubject,
        dpv:Organisation,
        dpv:Recipient,
        dpv:Representative ;
    sw:term_status "accepted"@en ;
    skos:definition "A human or non-human 'thing' that constitutes as an entity and which is recognised and defined in law"@en ;
    skos:prefLabel "Legal Entity"@en .

dpv:LegalMeasure a rdfs:Class,
        owl:Class ;
    dct:created "2023-12-10"^^xsd:date ;
    dct:modified "2023-12-10"^^xsd:date ;
    rdfs:subClassOf dpv:TechnicalOrganisationalMeasure ;
    sw:term_status "accepted"@en ;
    skos:definition "Legal measures used to safeguard and ensure good practices in connection with data and technologies"@en ;
    skos:prefLabel "Legal Measure"@en .

dpv:LegalObligation a rdfs:Class,
        owl:Class,
        dpv:LegalBasis ;
    dct:contributor "Harshvardhan J. Pandit" ;
    dct:created "2021-04-07"^^xsd:date ;
    rdfs:subClassOf dpv:LegalBasis ;
    sw:term_status "accepted"@en ;
    skos:definition "Legal Obligation to conduct the specified processing"@en ;
    skos:prefLabel "Legal Obligation"@en .

dpv:LegitimateInterest a rdfs:Class,
        owl:Class,
        dpv:LegalBasis ;
    dct:contributor "Harshvardhan J. Pandit" ;
    dct:created "2021-05-19"^^xsd:date ;
    rdfs:subClassOf dpv:LegalBasis ;
    sw:term_status "accepted"@en ;
    skos:definition "Legitimate Interests of a Party as justification for specified processing"@en ;
    skos:prefLabel "Legitimate Interest"@en .

dpv:LegitimateInterestAssessment a rdfs:Class,
        owl:Class,
        dpv:OrganisationalMeasure ;
    dct:contributor "Georg P Krog, Harshvardhan J. Pandit, Paul Ryan" ;
    dct:created "2021-09-08"^^xsd:date ;
    rdfs:subClassOf dpv:Assessment ;
    sw:term_status "accepted"@en ;
    skos:definition "Indicates an assessment regarding the use of legitimate interest as a lawful basis by the data controller"@en ;
    skos:prefLabel "Legitimate Interest Assessment"@en .

dpv:LegitimateInterestOfController a rdfs:Class,
        owl:Class,
        dpv:LegalBasis ;
    dct:contributor "Georg P Krog, Harshvardhan J. Pandit, Paul Ryan" ;
    dct:created "2021-05-19"^^xsd:date ;
    rdfs:subClassOf dpv:LegitimateInterest ;
    sw:term_status "accepted"@en ;
    skos:definition "Legitimate Interests of a Data Controller in conducting specified processing"@en ;
    skos:prefLabel "Legitimate Interest of Controller"@en .

dpv:LegitimateInterestOfDataSubject a rdfs:Class,
        owl:Class,
        dpv:LegalBasis ;
    dct:contributor "Georg P Krog" ;
    dct:created "2022-10-22"^^xsd:date ;
    rdfs:subClassOf dpv:LegitimateInterest ;
    sw:term_status "accepted"@en ;
    skos:definition "Legitimate Interests of the Data Subject in conducting specified processing"@en ;
    skos:prefLabel "Legitimate Interest of Data Subject"@en .

dpv:LegitimateInterestOfThirdParty a rdfs:Class,
        owl:Class,
        dpv:LegalBasis ;
    dct:contributor "Georg P Krog, Harshvardhan J. Pandit, Paul Ryan" ;
    dct:created "2021-05-19"^^xsd:date ;
    rdfs:subClassOf dpv:LegitimateInterest ;
    sw:term_status "accepted"@en ;
    skos:definition "Legitimate Interests of a Third Party in conducting specified processing"@en ;
    skos:prefLabel "Legitimate Interest of Third Party"@en .

dpv:Likelihood a rdfs:Class,
        owl:Class ;
    dct:contributor "Harshvardhan J. Pandit" ;
    dct:created "2022-07-22"^^xsd:date ;
    sw:term_status "accepted"@en ;
    skos:definition "The likelihood or probability or chance of something taking place or occuring"@en ;
    skos:prefLabel "Likelihood"@en ;
    skos:scopeNote "Likelihood can be expressed in a subjective manner, such as 'Unlikely', or in a quantitative manner such as \"Twice in a Day\" (frequency per period). The suggestion is to use quantitative values, or to associate them with subjective terms used so as to enable accurate interpretations and interoperability. See the concepts related to Frequency and Duration for possible uses as a combination to express Likelihood."@en .

dpv:LocalEnvironmentScale a rdfs:Class,
        owl:Class,
        dpv:GeographicCoverage ;
    dct:contributor "Harshvardhan J. Pandit" ;
    dct:created "2022-06-15"^^xsd:date ;
    rdfs:subClassOf dpv:GeographicCoverage ;
    sw:term_status "accepted"@en ;
    skos:definition "Geographic coverage spanning a specific environment within the locality"@en ;
    skos:prefLabel "Local Environment Scale"@en ;
    skos:scopeNote "For example, geographic scale of an event take place in a specific building or room"@en .

dpv:LocalLocation a rdfs:Class,
        owl:Class,
        dpv:Location ;
    dct:contributor "Harshvardhan J. Pandit" ;
    dct:created "2022-06-15"^^xsd:date ;
    dct:modified "2020-10-05"^^xsd:date ;
    rdfs:subClassOf dpv:LocationLocality ;
    sw:term_status "accepted"@en ;
    skos:definition "Location is local"@en ;
    skos:prefLabel "Local Location"@en .

dpv:LocalityScale a rdfs:Class,
        owl:Class,
        dpv:GeographicCoverage ;
    dct:contributor "Harshvardhan J. Pandit" ;
    dct:created "2022-06-15"^^xsd:date ;
    rdfs:subClassOf dpv:GeographicCoverage ;
    sw:term_status "accepted"@en ;
    skos:definition "Geographic coverage spanning a specific locality"@en ;
    skos:prefLabel "Locality Scale"@en ;
    skos:scopeNote "For example, geographic scale of a city or an area within a city"@en .

dpv:Location a rdfs:Class,
        owl:Class ;
    dct:contributor "Harshvardhan J. Pandit, Georg P Krog" ;
    dct:created "2022-01-19"^^xsd:date ;
    vann:example dex:E0011 ;
    rdfs:subClassOf rdfs:Class ;
    rdfs:superClassOf dpv:Country,
        dpv:EconomicUnion,
        dpv:StorageLocation,
        dpv:SupraNationalUnion ;
    sw:term_status "accepted"@en ;
    skos:definition "A location is a position, site, or area where something is located"@en ;
    skos:prefLabel "Location"@en ;
    skos:scopeNote "Location may be geographic, physical, or virtual."@en .

dpv:LocationFixture a rdfs:Class,
        owl:Class ;
    dct:contributor "Harshvardhan J. Pandit" ;
    dct:created "2022-06-15"^^xsd:date ;
    rdfs:subClassOf rdfs:Class ;
    sw:term_status "accepted"@en ;
    skos:definition "The fixture of location refers to whether the location is fixed"@en ;
    skos:prefLabel "Location Fixture"@en .

dpv:LocationLocality a rdfs:Class,
        owl:Class,
        dpv:Location ;
    dct:contributor "Harshvardhan J. Pandit" ;
    dct:created "2022-06-15"^^xsd:date ;
    dct:modified "2022-10-04"^^xsd:date ;
    rdfs:subClassOf dpv:Location ;
    sw:term_status "accepted"@en ;
    skos:definition "Locality refers to whether the specified location is local within some context, e.g. for the user"@en ;
    skos:prefLabel "Location Locality"@en .

dpv:LoggingPolicies a rdfs:Class,
        owl:Class,
        dpv:OrganisationalMeasure ;
    dct:contributor "Harshvardhan J. Pandit" ;
    dct:created "2022-08-17"^^xsd:date ;
    dct:source "(ENISA 5G Cybersecurity Standards,https://www.enisa.europa.eu/publications/5g-cybersecurity-standards)"@en ;
    rdfs:subClassOf dpv:GovernanceProcedures ;
    sw:term_status "accepted"@en ;
    skos:definition "Policy for logging of information"@en ;
    skos:prefLabel "Logging Policies"@en .

dpv:MaintainCreditCheckingDatabase a rdfs:Class,
        owl:Class,
        dpv:Purpose ;
    dct:contributor "Harshvardhan J. Pandit, Georg P Krog" ;
    dct:created "2022-06-15"^^xsd:date ;
    rdfs:subClassOf dpv:CreditChecking ;
    sw:term_status "accepted"@en ;
    skos:definition "Purposes associated with maintaining a Credit Checking Database"@en ;
    skos:prefLabel "Maintain Credit Checking Database"@en .

dpv:MaintainCreditRatingDatabase a rdfs:Class,
        owl:Class,
        dpv:Purpose ;
    dct:contributor "Harshvardhan J. Pandit, Georg P Krog" ;
    dct:created "2022-06-15"^^xsd:date ;
    rdfs:subClassOf dpv:CreditChecking ;
    sw:term_status "accepted"@en ;
    skos:definition "Purposes associated with maintaining a Credit Rating Database"@en ;
    skos:prefLabel "Maintain Credit Rating Database"@en .

dpv:MaintainFraudDatabase a rdfs:Class,
        owl:Class,
        dpv:Purpose ;
    dct:contributor "Harshvardhan J. Pandit, Georg P Krog" ;
    dct:created "2022-06-15"^^xsd:date ;
    rdfs:subClassOf dpv:FraudPreventionAndDetection ;
    sw:term_status "accepted"@en ;
    skos:definition "Purposes associated with maintaining a database related to identifying and identified fraud risks and fraud incidents"@en ;
    skos:prefLabel "Maintain Fraud Database"@en .

dpv:MakeAvailable a rdfs:Class,
        owl:Class,
        dpv:Processing ;
    dct:created "2019-05-07"^^xsd:date ;
    dct:source "(GDPR Art.4-2,https://eur-lex.europa.eu/eli/reg/2016/679/art_4/par_2/oj)"@en ;
    rdfs:subClassOf dpv:Disclose ;
    sw:term_status "accepted"@en ;
    skos:definition "to transform or publish data to be used"@en ;
    skos:prefLabel "Make Available"@en .

dpv:Marketing a rdfs:Class,
        owl:Class,
        dpv:Purpose ;
    dct:contributor "Georg P Krog, Harshvardhan J. Pandit, Beatriz Esteves" ;
    dct:created "2020-11-04"^^xsd:date ;
    rdfs:subClassOf dpv:Purpose ;
    sw:term_status "accepted"@en ;
    skos:definition "Purposes associated with conducting marketing in relation to organisation or products or services e.g. promoting, selling, and distributing"@en ;
    skos:prefLabel "Marketing"@en ;
    skos:scopeNote "Was commercial interest, changed to consider Marketing a separate Purpose category by itself"@en .

dpv:Match a rdfs:Class,
        owl:Class,
        dpv:Processing ;
    dct:contributor "Harshvardhan J. Pandit" ;
    dct:created "2022-04-20"^^xsd:date ;
    dct:source "(A29WP WP 248 rev.01 Guideliens on DPIA,https://ec.europa.eu/newsroom/article29/items/611236)"@en ;
    rdfs:subClassOf dpv:Use ;
    sw:term_status "accepted"@en ;
    skos:definition "to combine, compare, or match data from different sources"@en ;
    skos:prefLabel "Match"@en .

dpv:MaterialDamage a rdfs:Class,
        owl:Class,
        dpv:Impact ;
    dct:contributor "Harshvardhan J. Pandit" ;
    dct:created "2022-03-30"^^xsd:date ;
    rdfs:subClassOf dpv:Damage ;
    sw:term_status "accepted"@en ;
    skos:definition "Impact that acts as or causes material damages"@en ;
    skos:prefLabel "Material Damage"@en .

dpv:MediumDataVolume a rdfs:Class,
        owl:Class,
        dpv:DataVolume ;
    dct:contributor "Harshvardhan J. Pandit, Georg P Krog, Paul Ryan" ;
    dct:created "2022-06-15"^^xsd:date ;
    rdfs:subClassOf dpv:DataVolume ;
    sw:term_status "accepted"@en ;
    skos:definition "Data volume that is considered medium i.e. neither large nor small within the context"@en ;
    skos:prefLabel "Medium Data Volume"@en .

dpv:MediumScaleOfDataSubjects a rdfs:Class,
        owl:Class,
        dpv:DataSubjectScale ;
    dct:contributor "Harshvardhan J. Pandit, Georg P Krog, Paul Ryan" ;
    dct:created "2022-06-15"^^xsd:date ;
    rdfs:subClassOf dpv:DataSubjectScale ;
    sw:term_status "accepted"@en ;
    skos:definition "Scale of data subjects considered medium i.e. neither large nor small within the context"@en ;
    skos:prefLabel "Medium Scale Of Data Subjects"@en .

dpv:MediumScaleProcessing a rdfs:Class,
        owl:Class,
        dpv:ProcessingScale ;
    dct:contributor "Harshvardhan J. Pandit" ;
    dct:created "2022-09-07"^^xsd:date ;
    rdfs:subClassOf dpv:ProcessingScale ;
    sw:term_status "accepted"@en ;
    skos:definition "Processing that takes place at medium scales (as specified by some criteria)"@en ;
    skos:prefLabel "Medium Scale Processing"@en .

dpv:Member a rdfs:Class,
        owl:Class,
        dpv:DataSubject ;
    dct:contributor "Harshvardhan J. Pandit, Georg P. Krog, Julian Flake, Paul Ryan, Beatriz Esteves" ;
    dct:created "2022-04-06"^^xsd:date ;
    rdfs:subClassOf dpv:DataSubject ;
    sw:term_status "accepted"@en ;
    skos:definition "Data subjects that are members of a group, organisation, or other collectives"@en ;
    skos:prefLabel "Member"@en .

dpv:MemberPartnerManagement a rdfs:Class,
        owl:Class,
        dpv:Purpose ;
    dct:contributor "Paul Ryan, Georg P Krog, David Hickey, Harshvardhan J. Pandit" ;
    dct:created "2021-09-01"^^xsd:date ;
    dct:source "(Belgian DPA ROPA Template, https://www.privacycommission.be/nl/model-voor-een-register-van-de-verwerkingsactiviteiten)"@en ;
    rdfs:subClassOf dpv:OrganisationGovernance ;
    sw:term_status "accepted"@en ;
    skos:definition "Purposes associated with maintaining a registry of shareholders, members, or partners for governance, administration, and management functions"@en ;
    skos:prefLabel "Members and Partners Management"@en .

dpv:MentallyVulnerableDataSubject a rdfs:Class,
        owl:Class,
        dpv:DataSubject ;
    dct:contributor "Georg P Krog" ;
    dct:created "2022-06-15"^^xsd:date ;
    rdfs:subClassOf dpv:VulnerableDataSubject ;
    sw:term_status "accepted"@en ;
    skos:definition "Data subjects that are considered mentally vulnerable"@en ;
    skos:prefLabel "Mentally Vulnerable Data Subject"@en .

dpv:MessageAuthenticationCodes a rdfs:Class,
        owl:Class,
        dpv:TechnicalMeasure ;
    dct:contributor "Harshvardhan J. Pandit" ;
    dct:created "2022-08-17"^^xsd:date ;
    dct:source "(ENISA Reference Incident Classification Taxonomy 2018,https://www.enisa.europa.eu/publications/reference-incident-classification-taxonomy/)"@en ;
    rdfs:subClassOf dpv:CryptographicAuthentication ;
    sw:term_status "accepted"@en ;
    skos:definition "Use of cryptographic methods to authenticate messages"@en ;
    skos:prefLabel "Message Authentication Codes (MAC)"@en .

dpv:MobilePlatformSecurity a rdfs:Class,
        owl:Class,
        dpv:TechnicalMeasure ;
    dct:contributor "Harshvardhan J. Pandit" ;
    dct:created "2022-08-17"^^xsd:date ;
    dct:source "(ENISA Reference Incident Classification Taxonomy 2018,https://www.enisa.europa.eu/publications/reference-incident-classification-taxonomy/)"@en ;
    rdfs:subClassOf dpv:SecurityMethod ;
    sw:term_status "accepted"@en ;
    skos:definition "Security implemented over a mobile platform"@en ;
    skos:prefLabel "Mobile Platform Security"@en .

dpv:Modify a rdfs:Class,
        owl:Class,
        dpv:Processing ;
    dct:contributor "Harshvardhan J. Pandit, Georg P Krog" ;
    dct:created "2022-06-15"^^xsd:date ;
    rdfs:subClassOf dpv:Alter ;
    sw:term_status "accepted"@en ;
    skos:definition "to modify or change data"@en ;
    skos:prefLabel "Modify"@en .

dpv:Monitor a rdfs:Class,
        owl:Class,
        dpv:Processing ;
    dct:contributor "Harshvardhan J. Pandit, Georg P Krog" ;
    dct:created "2022-06-15"^^xsd:date ;
    rdfs:subClassOf dpv:Consult ;
    sw:term_status "accepted"@en ;
    skos:definition "to monitor data for some criteria"@en ;
    skos:prefLabel "Monitor"@en .

dpv:MonitoringPolicies a rdfs:Class,
        owl:Class,
        dpv:OrganisationalMeasure ;
    dct:contributor "Harshvardhan J. Pandit" ;
    dct:created "2022-08-17"^^xsd:date ;
    dct:source "(ENISA 5G Cybersecurity Standards,https://www.enisa.europa.eu/publications/5g-cybersecurity-standards)"@en ;
    rdfs:subClassOf dpv:GovernanceProcedures ;
    sw:term_status "accepted"@en ;
    skos:definition "Policy for monitoring (e.g. progress, performance)"@en ;
    skos:prefLabel "Monitoring Policies"@en .

dpv:MonotonicCounterPseudonymisation a rdfs:Class,
        owl:Class,
        dpv:TechnicalMeasure ;
    dct:contributor "Harshvardhan J. Pandit" ;
    dct:created "2022-08-17"^^xsd:date ;
    dct:modified "2022-10-13"^^xsd:date ;
    dct:source "(ENISA Data Pseudonymisation: Advanced Techniques and Use Cases,https://www.enisa.europa.eu/publications/data-pseudonymisation-advanced-techniques-and-use-cases)"@en ;
    rdfs:subClassOf dpv:Pseudonymisation ;
    sw:term_status "modified"@en ;
    skos:definition "A simple pseudonymisation method where identifiers are substituted by a number chosen by a monotonic counter"@en ;
    skos:prefLabel "Monotonic Counter Pseudonymisation"@en .

dpv:Move a rdfs:Class,
        owl:Class,
        dpv:Processing ;
    dct:created "2019-05-07"^^xsd:date ;
    dct:source "(SPECIAL Project,https://specialprivacy.ercim.eu/vocabs/processing)"@en ;
    rdfs:subClassOf dpv:Transfer ;
    sw:term_status "accepted"@en ;
    skos:definition "to move data from one location to another including deleting the original copy"@en ;
    skos:prefLabel "Move"@en ;
    skos:related "svpr:Move"@en .

dpv:MultiFactorAuthentication a rdfs:Class,
        owl:Class,
        dpv:TechnicalMeasure ;
    dct:contributor "Harshvardhan J. Pandit" ;
    dct:created "2022-08-17"^^xsd:date ;
    dct:source "(ENISA Reference Incident Classification Taxonomy 2018,https://www.enisa.europa.eu/publications/reference-incident-classification-taxonomy/)"@en ;
    rdfs:subClassOf dpv:AuthenticationProtocols ;
    sw:term_status "accepted"@en ;
    skos:definition "An authentication system that uses two or more methods to authenticate"@en ;
    skos:prefLabel "Multi-Factor Authentication (MFA)"@en .

dpv:MultiNationalScale a rdfs:Class,
        owl:Class,
        dpv:GeographicCoverage ;
    dct:contributor "Harshvardhan J. Pandit" ;
    dct:created "2022-06-15"^^xsd:date ;
    rdfs:subClassOf dpv:GeographicCoverage ;
    sw:term_status "accepted"@en ;
    skos:definition "Geographic coverage spanning multiple nations"@en ;
    skos:prefLabel "Multi National Scale"@en .

dpv:NDA a rdfs:Class,
        owl:Class,
        dpv:OrganisationalMeasure ;
    dct:contributor "Axel Polleres, Rob Brennan, Harshvardhan J. Pandit, Mark Lizar" ;
    dct:created "2019-04-05"^^xsd:date ;
    rdfs:subClassOf dpv:LegalAgreement ;
    sw:term_status "accepted"@en ;
    skos:definition "Non-disclosure Agreements e.g. preserving confidentiality of information"@en ;
    skos:prefLabel "Non-Disclosure Agreement (NDA)"@en .

dpv:NationalAuthority a rdfs:Class,
        owl:Class ;
    dct:contributor "Harshvardhan J. Pandit" ;
    dct:created "2022-02-02"^^xsd:date ;
    dct:source "(ADMS controlled vocabulary,http://purl.org/adms)"@en ;
    rdfs:subClassOf dpv:Authority ;
    sw:term_status "accepted"@en ;
    skos:definition "An authority tasked with overseeing legal compliance for a nation"@en ;
    skos:prefLabel "National Authority"@en .

dpv:NationalScale a rdfs:Class,
        owl:Class,
        dpv:GeographicCoverage ;
    dct:contributor "Harshvardhan J. Pandit" ;
    dct:created "2022-06-15"^^xsd:date ;
    rdfs:subClassOf dpv:GeographicCoverage ;
    sw:term_status "accepted"@en ;
    skos:definition "Geographic coverage spanning a nation"@en ;
    skos:prefLabel "National Scale"@en .

dpv:NaturalPerson a rdfs:Class,
        owl:Class ;
    dct:contributor "Harshvardhan J. Pandit" ;
    dct:created "2022-02-09"^^xsd:date ;
    rdfs:subClassOf dpv:Entity ;
    sw:term_status "accepted"@en ;
    skos:definition "A human"@en ;
    skos:prefLabel "Natural Person"@en .

dpv:NearlyGlobalScale a rdfs:Class,
        owl:Class,
        dpv:GeographicCoverage ;
    dct:contributor "Harshvardhan J. Pandit" ;
    dct:created "2022-06-15"^^xsd:date ;
    rdfs:subClassOf dpv:GeographicCoverage ;
    sw:term_status "accepted"@en ;
    skos:definition "Geographic coverage nearly spanning the entire globe"@en ;
    skos:prefLabel "Nearly Global Scale"@en .

dpv:Necessity a rdfs:Class,
        owl:Class ;
    dct:contributor "Harshvardhan J. Pandit, Paul Ryan, Georg P Krog, Julian Flake, Beatriz Esteves" ;
    dct:created "2022-02-12"^^xsd:date ;
    vann:example dex:E0028 ;
    rdfs:subClassOf dpv:Context ;
    sw:term_status "accepted"@en ;
    skos:definition "An indication of 'necessity' within a context"@en ;
    skos:prefLabel "Necessity"@en ;
    skos:scopeNote "Necessity can be used to express need, essentiality, requirement, or compulsion."@en .

dpv:NetworkProxyRouting a rdfs:Class,
        owl:Class,
        dpv:TechnicalMeasure ;
    dct:contributor "Harshvardhan J. Pandit" ;
    dct:created "2022-08-17"^^xsd:date ;
    dct:source "(ENISA Data Protection Engineering,https://www.enisa.europa.eu/publications/data-protection-engineering)"@en ;
    rdfs:subClassOf dpv:SecurityMethod ;
    sw:term_status "accepted"@en ;
    skos:definition "Use of network routing using proxy"@en ;
    skos:prefLabel "Network Proxy Routing"@en .

dpv:NetworkSecurityProtocols a rdfs:Class,
        owl:Class,
        dpv:TechnicalMeasure ;
    dct:contributor "Harshvardhan J. Pandit" ;
    dct:created "2022-08-17"^^xsd:date ;
    dct:source "(ENISA Reference Incident Classification Taxonomy 2018,https://www.enisa.europa.eu/publications/reference-incident-classification-taxonomy/)"@en ;
    rdfs:subClassOf dpv:SecurityMethod ;
    sw:term_status "accepted"@en ;
    skos:definition "Security implemented at or over networks protocols"@en ;
    skos:prefLabel "Network Security Protocols"@en .

dpv:NonCitizen a rdfs:Class,
        owl:Class,
        dpv:DataSubject ;
    dct:contributor "Harshvardhan J. Pandit, Georg P. Krog, Julian Flake, Paul Ryan, Beatriz Esteves" ;
    dct:created "2022-04-06"^^xsd:date ;
    rdfs:subClassOf dpv:DataSubject ;
    sw:term_status "accepted"@en ;
    skos:definition "Data subjects that are not citizens (for a jurisdiction)"@en ;
    skos:prefLabel "Non-Citizen"@en .

dpv:NonCommercialResearch a rdfs:Class,
        owl:Class,
        dpv:Purpose ;
    dct:contributor "Harshvardhan J. Pandit, Javier Fernandez, Axel Polleres, Elmar Kiesling, Fajar Ekaputra, Simon Steyskal" ;
    dct:created "2019-04-05"^^xsd:date ;
    rdfs:subClassOf dpv:ResearchAndDevelopment ;
    sw:term_status "accepted"@en ;
    skos:definition "Purposes associated with conducting research in a non-commercial setting e.g. for a non-profit-organisation (NGO)"@en ;
    skos:prefLabel "Non-Commercial Research"@en .

dpv:NonCompliant a rdfs:Class,
        owl:Class,
        dpv:ComplianceStatus ;
    dct:contributor "Harshvardhan J. Pandit" ;
    dct:created "2022-05-18"^^xsd:date ;
    dct:modified "2022-09-07"^^xsd:date ;
    rdfs:subClassOf dpv:ComplianceStatus ;
    sw:term_status "accepted"@en ;
    skos:definition "State of non-compliance where objectives have not been met, but have not been violated"@en ;
    skos:prefLabel "Non Compliant"@en ;
    skos:scopeNote "Changed from not compliant for consistency in commonly used terms"@en .

dpv:NonConformant a rdfs:Class,
        owl:Class,
        dpv:ConformanceStatus ;
    dct:contributor "Harshvardhan J. Pandit" ;
    dct:created "2022-10-22"^^xsd:date ;
    rdfs:subClassOf dpv:ConformanceStatus ;
    sw:term_status "accepted"@en ;
    skos:definition "State of being non-conformant"@en ;
    skos:prefLabel "NonConformant"@en .

dpv:NonGovernmentalOrganisation a rdfs:Class,
        owl:Class ;
    dct:contributor "Harshvardhan J. Pandit" ;
    dct:created "2022-02-02"^^xsd:date ;
    dct:modified "2020-10-05"^^xsd:date ;
    dct:source "(ADMS controlled vocabulary,http://purl.org/adms)"@en ;
    rdfs:subClassOf dpv:Organisation ;
    sw:term_status "accepted"@en ;
    skos:definition "An organisation not part of or independent from the government"@en ;
    skos:prefLabel "Non-Governmental Organisation"@en .

dpv:NonMaterialDamage a rdfs:Class,
        owl:Class,
        dpv:Impact ;
    dct:contributor "Harshvardhan J. Pandit" ;
    dct:created "2022-03-30"^^xsd:date ;
    rdfs:subClassOf dpv:Damage ;
    sw:term_status "accepted"@en ;
    skos:definition "Impact that acts as or causes non-material damages"@en ;
    skos:prefLabel "Non-Material Damage"@en .

dpv:NonPersonalData a rdfs:Class,
        owl:Class ;
    dct:contributor "Harshvardhan J. Pandit" ;
    dct:created "2022-01-19"^^xsd:date ;
    rdfs:subClassOf dpv:Data ;
    rdfs:superClassOf dpv:AnonymisedData ;
    sw:term_status "accepted"@en ;
    skos:definition "Data that is not Personal Data"@en ;
    skos:prefLabel "Non-Personal Data"@en ;
    skos:scopeNote "The term NonPersonalData is provided to distinguish between PersonalData and other data, e.g. for indicating which data is regulated by privacy laws. To specify personal data that has been anonymised, the concept AnonymisedData should be used as the anonymisation process has a risk of not being fully effective and such anonymous data may be found to be personal data depending on circumstances."@en .

dpv:NonPersonalDataProcess a rdfs:Class,
        owl:Class ;
    dct:contributor "Harshvardhan J. Pandit" ;
    rdfs:subClassOf dpv:Process ;
    sw:term_status "accepted"@en ;
    skos:definition "An action, activity, or method involving non-personal data, and asserting that no personal data is involved"@en ;
    skos:prefLabel "Non-Personal Data Process"@en ;
    skos:scopeNote "Use of personal data within NonPersonalDataProcess should be considered a violation of the explicit constraint that no personal data is involved."@en .

dpv:NonProfitOrganisation a rdfs:Class,
        owl:Class ;
    dct:contributor "Harshvardhan J. Pandit" ;
    dct:created "2022-02-02"^^xsd:date ;
    dct:modified "2020-10-05"^^xsd:date ;
    dct:source "(ADMS controlled vocabulary,http://purl.org/adms)"@en ;
    rdfs:subClassOf dpv:Organisation ;
    sw:term_status "accepted"@en ;
    skos:definition "An organisation that does not aim to achieve profit as its primary goal"@en ;
    skos:prefLabel "Non-Profit Organisation"@en .

dpv:NonPublicDataSource a rdfs:Class,
        owl:Class,
        dpv:DataSource ;
    dct:contributor "Georg P Krog, Harshvardhan J. Pandit, Beatriz Esteves, Paul Ryan, Julian Flake" ;
    dct:created "2022-01-26"^^xsd:date ;
    rdfs:subClassOf dpv:DataSource ;
    sw:term_status "accepted"@en ;
    skos:definition "A source of data that is not publicly accessible or available"@en ;
    skos:prefLabel "Non-Public Data Source"@en .

dpv:NotAutomated a rdfs:Class,
        owl:Class,
        dpv:Automation ;
    dct:created "2023-12-10"^^xsd:date ;
    rdfs:subClassOf dpv:Automation ;
    sw:term_status "accepted"@en ;
    skos:definition "The operator fully controls the system"@en ;
    skos:prefLabel "Not Automated"@en ;
    skos:scopeNote "Human Involvement is necessary here as there is no automation"@en .

dpv:NotRequired a rdfs:Class,
        owl:Class,
        dpv:Necessity ;
    dct:contributor "Harshvardhan J. Pandit, Paul Ryan, Georg P Krog, Julian Flake, Beatriz Esteves" ;
    dct:created "2022-02-15"^^xsd:date ;
    rdfs:subClassOf dpv:Necessity ;
    sw:term_status "accepted"@en ;
    skos:definition "Indication of neither being required nor optional i.e. not relevant or needed"@en ;
    skos:prefLabel "Not Required"@en .

dpv:Notice a rdfs:Class,
        owl:Class,
        dpv:OrganisationalMeasure ;
    dct:contributor "Paul Ryan, David Hickey, Georg P Krog, Harshvardhan J. Pandit" ;
    dct:created "2021-09-08"^^xsd:date ;
    vann:example dex:E0025 ;
    rdfs:subClassOf dpv:OrganisationalMeasure ;
    sw:term_status "accepted"@en ;
    skos:definition "A notice is an artefact for providing information, choices, or controls"@en ;
    skos:prefLabel "Notice"@en .

dpv:Obligation a rdfs:Class,
        owl:Class,
        dpv:Rule ;
    dct:contributor "Harshvardhan J. Pandit, Georg P Krog, Beatriz Esteves, Paul Ryan" ;
    dct:created "2022-10-19"^^xsd:date ;
    rdfs:subClassOf dpv:Rule ;
    sw:term_status "accepted"@en ;
    skos:definition "A rule describing an obligation for performing an activity"@en ;
    skos:prefLabel "Obligation"@en .

dpv:Observe a rdfs:Class,
        owl:Class,
        dpv:Processing ;
    dct:contributor "Harshvardhan J. Pandit, Georg P Krog" ;
    dct:created "2022-06-15"^^xsd:date ;
    rdfs:subClassOf dpv:Obtain ;
    sw:term_status "accepted"@en ;
    skos:definition "to obtain data through observation"@en ;
    skos:prefLabel "Observe"@en .

dpv:ObservedData a rdfs:Class,
        owl:Class ;
    dct:created "2023-12-10"^^xsd:date ;
    rdfs:subClassOf dpv:Data ;
    rdfs:superClassOf dpv:ObservedPersonalData ;
    sw:term_status "accepted"@en ;
    skos:definition "Data that has been obtained through observations of a source"@en ;
    skos:prefLabel "Observed Data"@en .

dpv:ObservedPersonalData a rdfs:Class,
        owl:Class ;
    dct:contributor "Georg P Krog" ;
    dct:created "2022-08-24"^^xsd:date ;
    dct:modified "2023-12-10"^^xsd:date ;
    rdfs:subClassOf dpv:ObservedData,
        dpv:PersonalData ;
    sw:term_status "accepted"@en ;
    skos:definition "Personal Data that has been collected through observation of the Data Subject(s)"@en ;
    skos:prefLabel "Observed Personal Data"@en .

dpv:Obtain a rdfs:Class,
        owl:Class,
        dpv:Processing ;
    dct:created "2019-05-07"^^xsd:date ;
    dct:source "(GDPR Art.4-2,https://eur-lex.europa.eu/eli/reg/2016/679/art_4/par_2/oj)"@en ;
    rdfs:subClassOf dpv:Processing ;
    sw:term_status "accepted"@en ;
    skos:definition "to solicit or gather data from someone"@en ;
    skos:prefLabel "Obtain"@en .

dpv:OfficialAuthorityOfController a rdfs:Class,
        owl:Class,
        dpv:LegalBasis ;
    dct:contributor "Georg P Krog, Harshvardhan J. Pandit, Paul Ryan" ;
    dct:created "2021-05-05"^^xsd:date ;
    rdfs:subClassOf dpv:LegalBasis ;
    sw:term_status "accepted"@en ;
    skos:definition "Processing necessary or authorised through the official authority granted to or vested in the Data Controller"@en ;
    skos:prefLabel "Official Authority of Controller"@en .

dpv:OftenFrequency a rdfs:Class,
        owl:Class,
        dpv:Frequency ;
    dct:contributor "Harshvardhan J. Pandit" ;
    dct:created "2022-06-15"^^xsd:date ;
    dct:modified "2020-10-05"^^xsd:date ;
    rdfs:subClassOf dpv:Frequency ;
    sw:term_status "accepted"@en ;
    skos:definition "Frequency where occurences are often or frequent, but not continous"@en ;
    skos:prefLabel "Often Frequency"@en .

dpv:OperatingSystemSecurity a rdfs:Class,
        owl:Class,
        dpv:TechnicalMeasure ;
    dct:contributor "Harshvardhan J. Pandit" ;
    dct:created "2022-08-17"^^xsd:date ;
    dct:source "(ENISA Reference Incident Classification Taxonomy 2018,https://www.enisa.europa.eu/publications/reference-incident-classification-taxonomy/)"@en ;
    rdfs:subClassOf dpv:SecurityMethod ;
    sw:term_status "accepted"@en ;
    skos:definition "Security implemented at or through operating systems"@en ;
    skos:prefLabel "Operating System Security"@en .

dpv:OptimisationForConsumer a rdfs:Class,
        owl:Class,
        dpv:Purpose ;
    dct:contributor "Harshvardhan J. Pandit, Javier Fernandez, Axel Polleres, Elmar Kiesling, Fajar Ekaputra, Simon Steyskal" ;
    dct:created "2019-04-05"^^xsd:date ;
    rdfs:subClassOf dpv:ServiceOptimisation ;
    sw:term_status "accepted"@en ;
    skos:definition "Purposes associated with optimisation of activities and services for consumer or user"@en ;
    skos:prefLabel "Optimisation for Consumer"@en ;
    skos:related "svpu:Custom"@en ;
    skos:scopeNote "The term optmisation here refers to the efficiency of the service in terms of technical provision (or similar means) with benefits for everybody. Personalisation implies making changes that benefit the current user or persona."@en .

dpv:OptimisationForController a rdfs:Class,
        owl:Class,
        dpv:Purpose ;
    dct:contributor "Harshvardhan J. Pandit, Javier Fernandez, Axel Polleres, Elmar Kiesling, Fajar Ekaputra, Simon Steyskal" ;
    dct:created "2019-04-05"^^xsd:date ;
    rdfs:subClassOf dpv:ServiceOptimisation ;
    sw:term_status "accepted"@en ;
    skos:definition "Purposes associated with optimisation of activities and services for provider or controller"@en ;
    skos:prefLabel "Optimisation for Controller"@en .

dpv:OptimiseUserInterface a rdfs:Class,
        owl:Class,
        dpv:Purpose ;
    dct:contributor "Harshvardhan J. Pandit, Javier Fernandez, Axel Polleres, Elmar Kiesling, Fajar Ekaputra, Simon Steyskal" ;
    dct:created "2019-04-05"^^xsd:date ;
    rdfs:subClassOf dpv:OptimisationForConsumer ;
    sw:term_status "accepted"@en ;
    skos:definition "Purposes associated with optimisation of interfaces presented to the user"@en ;
    skos:prefLabel "Optimise User Interface"@en .

dpv:Optional a rdfs:Class,
        owl:Class,
        dpv:Necessity ;
    dct:contributor "Harshvardhan J. Pandit, Paul Ryan, Georg P Krog, Julian Flake, Beatriz Esteves" ;
    dct:created "2022-02-14"^^xsd:date ;
    rdfs:subClassOf dpv:Necessity ;
    sw:term_status "accepted"@en ;
    skos:definition "Indication of 'optional' or 'voluntary'"@en ;
    skos:prefLabel "Optional"@en .

dpv:Organisation a rdfs:Class,
        owl:Class ;
    dct:contributor "Harshvardhan J. Pandit" ;
    dct:created "2022-02-02"^^xsd:date ;
    rdfs:subClassOf dpv:LegalEntity ;
    rdfs:superClassOf dpv:AcademicScientificOrganisation,
        dpv:ForProfitOrganisation,
        dpv:GovernmentalOrganisation,
        dpv:IndustryConsortium,
        dpv:InternationalOrganisation,
        dpv:NonGovernmentalOrganisation,
        dpv:NonProfitOrganisation ;
    sw:term_status "accepted"@en ;
    skos:definition "A general term reflecting a company or a business or a group acting as a unit"@en ;
    skos:prefLabel "Organisation"@en .

dpv:OrganisationComplianceManagement a rdfs:Class,
        owl:Class,
        dpv:Purpose ;
    dct:contributor "Paul Ryan, Georg P Krog, David Hickey, Harshvardhan J. Pandit" ;
    dct:created "2021-09-01"^^xsd:date ;
    rdfs:subClassOf dpv:OrganisationGovernance ;
    sw:term_status "accepted"@en ;
    skos:definition "Purposes associated with managing compliance for organisation in relation to internal policies"@en ;
    skos:prefLabel "Organisation Compliance Management"@en ;
    skos:scopeNote "Note that this concept relates to internal organisational compliance. The concept LegalCompliance should be used for external legal or regulatory compliance."@en .

dpv:OrganisationGovernance a rdfs:Class,
        owl:Class,
        dpv:Purpose ;
    dct:contributor "Paul Ryan, Georg P Krog, David Hickey, Harshvardhan J. Pandit" ;
    dct:created "2021-09-01"^^xsd:date ;
    dct:source "(Belgian DPA ROPA Template, https://www.privacycommission.be/nl/model-voor-een-register-van-de-verwerkingsactiviteiten)"@en ;
    rdfs:subClassOf dpv:Purpose ;
    sw:term_status "accepted"@en ;
    skos:definition "Purposes associated with conducting activities and functions for governance of an organisation"@en ;
    skos:prefLabel "Organisation Governance"@en .

dpv:OrganisationRiskManagement a rdfs:Class,
        owl:Class,
        dpv:Purpose ;
    dct:contributor "Paul Ryan, Georg P Krog, David Hickey, Harshvardhan J. Pandit" ;
    dct:created "2021-09-01"^^xsd:date ;
    rdfs:subClassOf dpv:OrganisationGovernance ;
    sw:term_status "accepted"@en ;
    skos:definition "Purposes associated with managing risk for organisation's activities"@en ;
    skos:prefLabel "Organisation Risk Management"@en .

dpv:OrganisationalMeasure a rdfs:Class,
        owl:Class ;
    dct:contributor "Axel Polleres, Rob Brennan, Harshvardhan J. Pandit, Mark Lizar" ;
    dct:created "2019-04-05"^^xsd:date ;
    dct:modified "2023-12-10"^^xsd:date ;
    rdfs:subClassOf dpv:TechnicalOrganisationalMeasure ;
    sw:term_status "accepted"@en ;
    skos:definition "Organisational measures used to safeguard and ensure good practices in connection with data and technologies"@en ;
    skos:prefLabel "Organisational Measure"@en .

dpv:OrganisationalUnit a rdfs:Class,
        owl:Class ;
    dct:contributor "Harshvardhan J. Pandit, Paul Ryan" ;
    dct:created "2022-03-23"^^xsd:date ;
    rdfs:subClassOf dpv:Entity ;
    sw:term_status "accepted"@en ;
    skos:definition "Entity within an organisation that does not constitute as a separate legal entity"@en ;
    skos:prefLabel "Organisational Unit"@en .

dpv:Organise a rdfs:Class,
        owl:Class,
        dpv:Processing ;
    dct:created "2019-05-07"^^xsd:date ;
    dct:source "(GDPR Art.4-2,https://eur-lex.europa.eu/eli/reg/2016/679/art_4/par_2/oj)"@en ;
    rdfs:subClassOf dpv:Processing ;
    sw:term_status "accepted"@en ;
    skos:definition "to organize data for arranging or classifying"@en ;
    skos:prefLabel "Organise"@en .

dpv:PIA a rdfs:Class,
        owl:Class,
        dpv:OrganisationalMeasure ;
    dct:contributor "Georg P Krog, Harshvardhan J. Pandit, Paul Ryan" ;
    dct:created "2020-11-04"^^xsd:date ;
    rdfs:subClassOf dpv:ImpactAssessment ;
    sw:term_status "accepted"@en ;
    skos:definition "Carrying out an impact assessment regarding privacy risks"@en ;
    skos:prefLabel "Privacy Impact Assessment"@en .

dpv:ParentOfDataSubject a rdfs:Class,
        owl:Class,
        dpv:DataSubject ;
    dct:contributor "Georg P Krog" ;
    dct:created "2022-08-03"^^xsd:date ;
    rdfs:subClassOf dpv:DataSubject ;
    sw:term_status "accepted"@en ;
    skos:definition "Parent(s) of data subjects such as children"@en ;
    skos:prefLabel "Parent(s) of Data Subject"@en .

dpv:PartialAutomation a rdfs:Class,
        owl:Class,
        dpv:Automation ;
    dct:created "2023-12-10"^^xsd:date ;
    rdfs:subClassOf dpv:Automation ;
    sw:term_status "accepted"@en ;
    skos:definition "Some sub-functions of the system are fully automated while the system remains under the control of an external agent"@en ;
    skos:prefLabel "Partial Automation"@en ;
    skos:scopeNote "Human Involvement is implied here, specifically the ability to Control operations, but also possibly for intervention, oversight, and verification"@en .

dpv:PartiallyCompliant a rdfs:Class,
        owl:Class,
        dpv:ComplianceStatus ;
    dct:contributor "Harshvardhan J. Pandit" ;
    dct:created "2022-05-18"^^xsd:date ;
    rdfs:subClassOf dpv:ComplianceStatus ;
    sw:term_status "accepted"@en ;
    skos:definition "State of partially being compliant i.e. only some objectives have been met, and others have not been in violation"@en ;
    skos:prefLabel "Partially Compliant"@en .

dpv:Participant a rdfs:Class,
        owl:Class,
        dpv:DataSubject ;
    dct:contributor "Harshvardhan J. Pandit, Georg P. Krog, Julian Flake, Paul Ryan, Beatriz Esteves" ;
    dct:created "2022-04-06"^^xsd:date ;
    rdfs:subClassOf dpv:DataSubject ;
    sw:term_status "accepted"@en ;
    skos:definition "Data subjects that participate in some context such as volunteers in a function"@en ;
    skos:prefLabel "Participant"@en .

dpv:PassiveRight a rdfs:Class,
        owl:Class,
        dpv:Right ;
    dct:contributor "Harshvardhan J Pandit, Beatriz Esteves, Georg P Krog, Paul Ryan" ;
    dct:created "2022-10-22"^^xsd:date ;
    rdfs:subClassOf dpv:Right ;
    sw:term_status "accepted"@en ;
    skos:definition "The right(s) applicable, provided, or expected that are always (passively) applicable"@en ;
    skos:prefLabel "Passive Right"@en ;
    skos:scopeNote "Passive rights do not require the entity to request or exercise them. They are considered to be always applicable. For example, the Right to Privacy (in EU) does not require an exercise for it to be fulfilled."@en .

dpv:PasswordAuthentication a rdfs:Class,
        owl:Class,
        dpv:TechnicalMeasure ;
    dct:contributor "Harshvardhan J. Pandit" ;
    dct:created "2022-08-17"^^xsd:date ;
    dct:source "(ENISA Reference Incident Classification Taxonomy 2018,https://www.enisa.europa.eu/publications/reference-incident-classification-taxonomy/)"@en ;
    rdfs:subClassOf dpv:AuthenticationProtocols ;
    sw:term_status "accepted"@en ;
    skos:definition "Use of passwords to perform authentication"@en ;
    skos:prefLabel "Password Authentication"@en .

dpv:Patient a rdfs:Class,
        owl:Class,
        dpv:DataSubject ;
    dct:contributor "Harshvardhan J. Pandit, Georg P. Krog, Julian Flake, Paul Ryan, Beatriz Esteves" ;
    dct:created "2022-04-06"^^xsd:date ;
    rdfs:subClassOf dpv:DataSubject ;
    sw:term_status "accepted"@en ;
    skos:definition "Data subjects that receive medican attention, treatment, care, advice, or other health related services"@en ;
    skos:prefLabel "Patient"@en .

dpv:PaymentManagement a rdfs:Class,
        owl:Class,
        dpv:Purpose ;
    dct:contributor "Georg P Krog, Harshvardhan J. Pandit, Beatriz Esteves" ;
    dct:created "2020-11-04"^^xsd:date ;
    rdfs:subClassOf dpv:ServiceProvision ;
    sw:term_status "accepted"@en ;
    skos:definition "Purposes associated with processing and managing payment in relation to service, including invoicing and records"@en ;
    skos:prefLabel "Payment Management"@en .

dpv:PenetrationTestingMethods a rdfs:Class,
        owl:Class,
        dpv:TechnicalMeasure ;
    dct:contributor "Harshvardhan J. Pandit" ;
    dct:created "2022-08-17"^^xsd:date ;
    dct:source "(ENISA Reference Incident Classification Taxonomy 2018,https://www.enisa.europa.eu/publications/reference-incident-classification-taxonomy/)"@en ;
    rdfs:subClassOf dpv:SecurityMethod ;
    sw:term_status "accepted"@en ;
    skos:definition "Use of penetration testing to identify weaknesses and vulnerabilities through simulations"@en ;
    skos:prefLabel "Penetration Testing Methods"@en .

dpv:Permission a rdfs:Class,
        owl:Class,
        dpv:Rule ;
    dct:contributor "Harshvardhan J. Pandit, Georg P Krog, Beatriz Esteves, Paul Ryan" ;
    dct:created "2022-10-19"^^xsd:date ;
    rdfs:subClassOf dpv:Rule ;
    sw:term_status "accepted"@en ;
    skos:definition "A rule describing a permission to perform an activity"@en ;
    skos:prefLabel "Permission"@en .

dpv:PersonalData a rdfs:Class,
        owl:Class ;
    dct:contributor "Harshvardhan Pandit" ;
    dct:created "2019-04-05"^^xsd:date ;
    dct:modified "2022-01-19"^^xsd:date ;
    dct:source "(GDPR Art.4-1g,https://eur-lex.europa.eu/eli/reg/2016/679/art_4/par_1/oj)"@en ;
    rdfs:subClassOf dpv:Data ;
    rdfs:superClassOf dpv:CollectedPersonalData,
        dpv:DerivedPersonalData,
        dpv:GeneratedPersonalData,
        dpv:IdentifyingPersonalData,
        dpv:ObservedPersonalData,
        dpv:PseudonymisedData,
        dpv:SensitivePersonalData ;
    sw:term_status "accepted"@en ;
    skos:definition "Data directly or indirectly associated or related to an individual."@en ;
    skos:prefLabel "Personal Data"@en ;
    skos:related "spl:AnyData"@en ;
    skos:scopeNote "This definition of personal data encompasses the concepts used in GDPR Art.4-1 for 'personal data' and ISO/IEC 2700 for 'personally identifiable information (PII)'."@en .

dpv:PersonalDataHandling a rdfs:Class,
        owl:Class ;
    dct:contributor "Axel Polleres, Javier Fernández" ;
    dct:created "2019-04-05"^^xsd:date ;
    dct:modified "2023-12-10"^^xsd:date ;
    vann:example dex:E0007,
        dex:E0008,
        dex:E0014,
        dex:E0018,
        dex:E0019,
        dex:E0020,
        dex:E0022,
        dex:E0028 ;
    rdfs:subClassOf dpv:Process ;
    sw:term_status "sunset"@en ;
    skos:definition "An abstract concept describing 'personal data handling'"@en ;
    skos:prefLabel "Personal Data Handling"@en ;
    skos:scopeNote "This concept will be deprecated in future updates. It is recommended to use dpv:PersonalDataProcess as the equivalent alternative which is better aligned with legal and operational terminology."@en .

dpv:PersonalDataProcess a rdfs:Class,
        owl:Class ;
    dct:contributor "Harshvardhan J. Pandit" ;
    rdfs:subClassOf dpv:Process ;
    sw:term_status "accepted"@en ;
    skos:definition "An action, activity, or method involving personal data"@en ;
    skos:prefLabel "Personal Data Process"@en .

dpv:Personalisation a rdfs:Class,
        owl:Class,
        dpv:Purpose ;
    dct:contributor "Harshvardhan J. Pandit" ;
    dct:created "2021-09-01"^^xsd:date ;
    rdfs:subClassOf dpv:Purpose ;
    sw:term_status "accepted"@en ;
    skos:definition "Purposes associated with creating and providing customisation based on attributes and/or needs of person(s) or context(s)."@en ;
    skos:prefLabel "Personalisation"@en ;
    skos:scopeNote "This term is a blanket purpose category for indicating personalisation of some other purpose, e.g. by creating a subclass of the other concept and Personalisation"@en .

dpv:PersonalisedAdvertising a rdfs:Class,
        owl:Class,
        dpv:Purpose ;
    dct:contributor "Georg P Krog, Harshvardhan J. Pandit, Beatriz Esteves" ;
    dct:created "2020-11-04"^^xsd:date ;
    rdfs:subClassOf dpv:Advertising,
        dpv:Personalisation ;
    sw:term_status "accepted"@en ;
    skos:definition "Purposes associated with creating and providing personalised advertising"@en ;
    skos:prefLabel "Personalised Advertising"@en .

dpv:PersonalisedBenefits a rdfs:Class,
        owl:Class,
        dpv:Purpose ;
    dct:contributor "Harshvardhan J. Pandit, Javier Fernandez, Axel Polleres, Elmar Kiesling, Fajar Ekaputra, Simon Steyskal" ;
    dct:created "2019-04-05"^^xsd:date ;
    rdfs:subClassOf dpv:ServicePersonalisation ;
    sw:term_status "accepted"@en ;
    skos:definition "Purposes associated with creating and providing personalised benefits for a service"@en ;
    skos:prefLabel "Personalised Benefits"@en .

dpv:PersonnelHiring a rdfs:Class,
        owl:Class,
        dpv:Purpose ;
    dct:contributor "Harshvardhan J. Pandit" ;
    dct:created "2022-04-20"^^xsd:date ;
    rdfs:subClassOf dpv:PersonnelManagement ;
    sw:term_status "accepted"@en ;
    skos:definition "Purposes associated with management and execution of hiring processes of personnel"@en ;
    skos:prefLabel "Personnel Hiring"@en .

dpv:PersonnelManagement a rdfs:Class,
        owl:Class,
        dpv:Purpose ;
    dct:contributor "Paul Ryan, Harshvardhan J. Pandit" ;
    dct:created "2022-03-30"^^xsd:date ;
    dct:source "(Belgian DPA ROPA Template, https://www.privacycommission.be/nl/model-voor-een-register-van-de-verwerkingsactiviteiten)"@en ;
    rdfs:subClassOf dpv:HumanResourceManagement ;
    sw:term_status "accepted"@en ;
    skos:definition "Purposes associated with management of personnel associated with the organisation e.g. evaluation and management of employees and intermediaries"@en ;
    skos:prefLabel "Personnel Management"@en .

dpv:PersonnelPayment a rdfs:Class,
        owl:Class,
        dpv:Purpose ;
    dct:contributor "Harshvardhan J. Pandit" ;
    dct:created "2022-04-20"^^xsd:date ;
    rdfs:subClassOf dpv:PersonnelManagement ;
    sw:term_status "accepted"@en ;
    skos:definition "Purposes associated with management and execution of payment of personnel"@en ;
    skos:prefLabel "Personnel Payment"@en .

dpv:PhysicalAccessControlMethod a rdfs:Class,
        owl:Class,
        dpv:TechnicalMeasure ;
    dct:contributor "Georg P Krog" ;
    dct:created "2022-06-15"^^xsd:date ;
    rdfs:subClassOf dpv:AccessControlMethod ;
    sw:term_status "accepted"@en ;
    skos:definition "Access control applied for physical access e.g. premises or equipment"@en ;
    skos:prefLabel "Physical Access Control Method"@en .

dpv:PhysicalMeasure a rdfs:Class,
        owl:Class ;
    dct:created "2023-12-10"^^xsd:date ;
    dct:modified "2023-12-10"^^xsd:date ;
    rdfs:subClassOf dpv:TechnicalOrganisationalMeasure ;
    sw:term_status "accepted"@en ;
    skos:definition "Physical measures used to safeguard and ensure good practices in connection with data and technologies"@en ;
    skos:prefLabel "Physical Measure"@en .

dpv:Policy a rdfs:Class,
        owl:Class,
        dpv:OrganisationalMeasure ;
    dct:contributor "Paul Ryan, David Hickey, Georg P Krog, Harshvardhan J. Pandit" ;
    dct:created "2021-09-08"^^xsd:date ;
    vann:example dex:E0017 ;
    rdfs:subClassOf dpv:OrganisationalMeasure ;
    sw:term_status "accepted"@en ;
    skos:definition "A guidance document outlining any of: procedures, plans, principles, decisions, intent, or protocols."@en ;
    skos:prefLabel "Policy"@en .

dpv:PostQuantumCryptography a rdfs:Class,
        owl:Class,
        dpv:TechnicalMeasure ;
    dct:contributor "Harshvardhan J. Pandit" ;
    dct:created "2022-08-17"^^xsd:date ;
    dct:source "(ENISA Reference Incident Classification Taxonomy 2018,https://www.enisa.europa.eu/publications/reference-incident-classification-taxonomy/)"@en ;
    rdfs:subClassOf dpv:CryptographicMethods ;
    sw:term_status "accepted"@en ;
    skos:definition "Use of algorithms that are intended to be secure against cryptanalytic attack by a quantum computer"@en ;
    skos:prefLabel "Post-Quantum Cryptography"@en .

dpv:PrimaryImportance a rdfs:Class,
        owl:Class,
        dpv:Importance ;
    dct:contributor "Harshvardhan J. Pandit, Paul Ryan, Georg P Krog, Julian Flake, Beatriz Esteves" ;
    dct:created "2022-02-10"^^xsd:date ;
    rdfs:subClassOf dpv:Importance ;
    sw:term_status "accepted"@en ;
    skos:definition "Indication of 'primary' or 'main' or 'core' importance"@en ;
    skos:prefLabel "Primary Importance"@en .

dpv:PrivacyByDefault a rdfs:Class,
        owl:Class,
        dpv:OrganisationalMeasure ;
    dct:contributor "Axel Polleres, Rob Brennan, Harshvardhan J. Pandit, Mark Lizar" ;
    dct:created "2019-04-05"^^xsd:date ;
    rdfs:subClassOf dpv:GuidelinesPrinciple ;
    sw:term_status "accepted"@en ;
    skos:definition "Practices regarding selecting appropriate data protection and privacy measures as the 'default' in an activity or service"@en ;
    skos:prefLabel "Privacy by Default"@en .

dpv:PrivacyByDesign a rdfs:Class,
        owl:Class,
        dpv:OrganisationalMeasure ;
    dct:contributor "Axel Polleres, Rob Brennan, Harshvardhan J. Pandit, Mark Lizar" ;
    dct:created "2019-04-05"^^xsd:date ;
    rdfs:subClassOf dpv:OrganisationalMeasure ;
    sw:term_status "accepted"@en ;
    skos:definition "Practices regarding incorporating data protection and privacy in the design of information and services"@en ;
    skos:prefLabel "Privacy by Design"@en .

dpv:PrivacyNotice a rdfs:Class,
        owl:Class,
        dpv:OrganisationalMeasure ;
    dct:contributor "Georg P Krog, Paul Ryan, David Hickey, Harshvardhan J. Pandit" ;
    dct:created "2021-09-08"^^xsd:date ;
    vann:example dex:E0018,
        dex:E0025 ;
    rdfs:subClassOf dpv:Notice ;
    sw:term_status "accepted"@en ;
    skos:definition "Represents a notice or document outlining information regarding privacy"@en ;
    skos:prefLabel "Privacy Notice"@en .

dpv:PrivacyPreservingProtocol a rdfs:Class,
        owl:Class,
        dpv:TechnicalMeasure ;
    dct:contributor "Harshvardhan J. Pandit" ;
    dct:created "2022-08-17"^^xsd:date ;
    dct:source "(ENISA Reference Incident Classification Taxonomy 2018,https://www.enisa.europa.eu/publications/reference-incident-classification-taxonomy/)"@en ;
    rdfs:subClassOf dpv:CryptographicMethods ;
    sw:term_status "accepted"@en ;
    skos:definition "Use of protocols designed with the intention of provided additional guarantees regarding privacy"@en ;
    skos:prefLabel "Privacy Preserving Protocol"@en .

dpv:PrivateInformationRetrieval a rdfs:Class,
        owl:Class,
        dpv:TechnicalMeasure ;
    dct:contributor "Harshvardhan J. Pandit" ;
    dct:created "2022-08-17"^^xsd:date ;
    dct:source "(ENISA Data Protection Engineering,https://www.enisa.europa.eu/publications/data-protection-engineering)"@en ;
    rdfs:subClassOf dpv:CryptographicMethods ;
    sw:term_status "accepted"@en ;
    skos:definition "Use of cryptographic methods to retrieve a record from a system without revealing which record is retrieved"@en ;
    skos:prefLabel "Private Information Retrieval"@en .

dpv:PrivateLocation a rdfs:Class,
        owl:Class,
        dpv:Location ;
    dct:contributor "Harshvardhan J. Pandit" ;
    dct:created "2022-10-22"^^xsd:date ;
    rdfs:subClassOf dpv:LocalLocation ;
    sw:term_status "accepted"@en ;
    skos:definition "Location that is not or cannot be accessed by the public and is controlled as a private space"@en ;
    skos:prefLabel "Private Location"@en .

dpv:Process a rdfs:Class,
        owl:Class ;
    dct:contributor "Harshvardhan J. Pandit" ;
    rdfs:superClassOf dpv:NonPersonalDataProcess,
        dpv:PersonalDataHandling,
        dpv:PersonalDataProcess ;
    sw:term_status "accepted"@en ;
    skos:definition "An action, activity, or method"@en ;
    skos:prefLabel "Process"@en .

dpv:Processing a rdfs:Class,
        owl:Class ;
    dct:contributor "Axel Polleres, Javier Fernández" ;
    dct:created "2019-04-05"^^xsd:date ;
    dct:modified "2020-11-04"^^xsd:date ;
    dct:source "(SPECIAL Project,https://specialprivacy.ercim.eu/)"@en ;
    vann:example dex:E0005,
        dex:E0011,
        dex:E0014 ;
    sw:term_status "accepted"@en ;
    skos:definition "Operations or 'processing' performed on data"@en ;
    skos:prefLabel "Processing"@en ;
    skos:related "spl:AnyProcessing"@en .

dpv:ProcessingCondition a rdfs:Class,
        owl:Class ;
    dct:created "2023-12-10"^^xsd:date ;
    rdfs:subClassOf dpv:ProcessingContext ;
    rdfs:superClassOf dpv:ProcessingDuration,
        dpv:ProcessingLocation,
        dpv:StorageCondition ;
    sw:term_status "accepted"@en ;
    skos:definition "Conditions required or followed regarding processing of data or use of technologies"@en ;
    skos:prefLabel "Processing Condition"@en .

dpv:ProcessingContext a rdfs:Class,
        owl:Class ;
    dct:contributor "Harshvardhan J. Pandit" ;
    dct:created "2022-02-09"^^xsd:date ;
    rdfs:subClassOf dpv:Context ;
    rdfs:superClassOf dpv:AlgorithmicLogic,
        dpv:Automation,
        dpv:DataSource,
        dpv:DecisionMaking,
        dpv:EvaluationScoring,
        dpv:HumanInvolvement,
        dpv:InnovativeUseOfTechnology,
        dpv:ProcessingCondition,
        dpv:Scale ;
    sw:term_status "accepted"@en ;
    skos:definition "Context or conditions within which processing takes place"@en ;
    skos:prefLabel "Processing Context"@en .

dpv:ProcessingDuration a rdfs:Class,
        owl:Class ;
    dct:created "2023-12-10"^^xsd:date ;
    rdfs:subClassOf dpv:ProcessingCondition ;
    sw:term_status "accepted"@en ;
    skos:definition "Conditions regarding Duration for processing of data or use of technologies"@en ;
    skos:prefLabel "Processing Duration"@en .

dpv:ProcessingLocation a rdfs:Class,
        owl:Class ;
    dct:created "2023-12-10"^^xsd:date ;
    rdfs:subClassOf dpv:ProcessingCondition ;
    sw:term_status "accepted"@en ;
    skos:definition "Conditions regarding Location for processing of data or use of technologies"@en ;
    skos:prefLabel "Processing Location"@en .

dpv:ProcessingScale a rdfs:Class,
        owl:Class ;
    dct:contributor "Harshvardhan J. Pandit, Piero Bonatti" ;
    dct:created "2022-09-07"^^xsd:date ;
    rdfs:subClassOf dpv:Scale ;
    sw:term_status "accepted"@en ;
    skos:definition "Scale of Processing"@en ;
    skos:prefLabel "Processing Scale"@en ;
    skos:scopeNote "The exact definition of what constitutes \"scale\" depends on use of jurisdictional, domain-specific, or other forms of externally defined criterias. Where possible, this should be reflected by extending the scales provided with the appropriate context."@en .

dpv:ProfessionalTraining a rdfs:Class,
        owl:Class,
        dpv:OrganisationalMeasure ;
    dct:contributor "Harshvardhan J. Pandit" ;
    dct:created "2022-08-17"^^xsd:date ;
    dct:source "(ENISA Reference Incident Classification Taxonomy 2018,https://www.enisa.europa.eu/publications/reference-incident-classification-taxonomy/)"@en ;
    rdfs:subClassOf dpv:StaffTraining ;
    sw:term_status "accepted"@en ;
    skos:definition "Training methods that are intended to provide professional knowledge and expertise"@en ;
    skos:prefLabel "Professional Training"@en .

dpv:Profiling a rdfs:Class,
        owl:Class,
        dpv:Processing ;
    dct:created "2019-05-07"^^xsd:date ;
    dct:source "(GDPR Art.4-2,https://eur-lex.europa.eu/eli/reg/2016/679/art_4/par_2/oj)"@en ;
    rdfs:subClassOf dpv:Use ;
    sw:term_status "accepted"@en ;
    skos:definition "to create a profile that describes or represents a person"@en ;
    skos:prefLabel "Profiling"@en .

dpv:Prohibition a rdfs:Class,
        owl:Class,
        dpv:Rule ;
    dct:contributor "Harshvardhan J. Pandit, Georg P Krog, Beatriz Esteves, Paul Ryan" ;
    dct:created "2022-10-19"^^xsd:date ;
    rdfs:subClassOf dpv:Rule ;
    sw:term_status "accepted"@en ;
    skos:definition "A rule describing a prohibition to perform an activity"@en ;
    skos:prefLabel "Prohibition"@en .

dpv:ProvideEventRecommendations a rdfs:Class,
        owl:Class,
        dpv:Purpose ;
    dct:contributor "Harshvardhan J. Pandit, Rudy Jacob" ;
    dct:created "2019-11-26"^^xsd:date ;
    dct:modified "2022-10-14"^^xsd:date ;
    dct:source "(SPECIAL Project,https://specialprivacy.ercim.eu/)"@en ;
    rdfs:subClassOf dpv:ProvidePersonalisedRecommendations ;
    sw:term_status "accepted"@en ;
    skos:definition "Purposes associated with creating and providing personalised recommendations for events"@en ;
    skos:prefLabel "Provide Event Recommendations"@en .

dpv:ProvidePersonalisedRecommendations a rdfs:Class,
        owl:Class,
        dpv:Purpose ;
    dct:contributor "Harshvardhan J. Pandit, Rudy Jacob" ;
    dct:created "2019-11-26"^^xsd:date ;
    dct:modified "2022-10-14"^^xsd:date ;
    dct:source "(SPECIAL Project,https://specialprivacy.ercim.eu/)"@en ;
    rdfs:subClassOf dpv:ServicePersonalisation ;
    sw:term_status "accepted"@en ;
    skos:definition "Purposes associated with creating and providing personalised recommendations"@en ;
    skos:prefLabel "Provide Personalised Recommendations"@en .

dpv:ProvideProductRecommendations a rdfs:Class,
        owl:Class,
        dpv:Purpose ;
    dct:contributor "Harshvardhan J. Pandit, Javier Fernandez, Axel Polleres, Elmar Kiesling, Fajar Ekaputra, Simon Steyskal" ;
    dct:created "2019-04-05"^^xsd:date ;
    dct:modified "2022-10-14"^^xsd:date ;
    rdfs:subClassOf dpv:ProvidePersonalisedRecommendations ;
    sw:term_status "accepted"@en ;
    skos:definition "Purposes associated with creating and providing product recommendations e.g. suggest similar products"@en ;
    skos:prefLabel "Provide Product Recommendations"@en ;
    skos:related "svpu:Marketing"@en .

dpv:Pseudonymisation a rdfs:Class,
        owl:Class,
        dpv:TechnicalMeasure ;
    dct:contributor "Axel Polleres, Rob Brennan, Harshvardhan J. Pandit, Mark Lizar" ;
    dct:created "2019-04-05"^^xsd:date ;
    dct:modified "2022-11-24"^^xsd:date ;
    dct:source "(GDPR Art.4-5,https://eur-lex.europa.eu/eli/reg/2016/679/art_4/par_5/oj)"@en ;
    rdfs:subClassOf dpv:Deidentification ;
    sw:term_status "modified"@en ;
    skos:definition "Pseudonymisation means the processing of personal data in such a manner that the personal data can no longer be attributed to a specific data subject without the use of additional information, provided that such additional information is kept separately and is subject to technical and organisational measures to ensure that the personal data are not attributed to an identified or identifiable natural person;"@en ;
    skos:prefLabel "Pseudonymisation"@en .

dpv:Pseudonymise a rdfs:Class,
        owl:Class,
        dpv:Processing ;
    dct:contributor "2022-10-14" ;
    dct:created "2019-05-07"^^xsd:date ;
    dct:source "(GDPR Art.4-2,https://eur-lex.europa.eu/eli/reg/2016/679/art_4/par_2/oj)"@en ;
    rdfs:subClassOf dpv:Transform ;
    sw:term_status "accepted"@en ;
    skos:definition "to replace personal identifiable information by artificial identifiers"@en ;
    skos:prefLabel "Pseudonymise"@en .

dpv:PseudonymisedData a rdfs:Class,
        owl:Class ;
    dct:contributor "Harshvardhan J. Pandit" ;
    dct:created "2022-01-19"^^xsd:date ;
    rdfs:subClassOf dpv:PersonalData ;
    sw:term_status "accepted"@en ;
    skos:definition "Personal Data that has undergone a pseudonymisation process or a partial (incomplete) anonymisation process such that it is still considered Personal Data"@en ;
    skos:prefLabel "Pseudonymised Data"@en .

dpv:PublicDataSource a rdfs:Class,
        owl:Class,
        dpv:DataSource ;
    dct:contributor "Georg P Krog, Harshvardhan J. Pandit, Beatriz Esteves, Paul Ryan, Julian Flake" ;
    dct:created "2022-01-26"^^xsd:date ;
    rdfs:subClassOf dpv:DataSource ;
    sw:term_status "accepted"@en ;
    skos:definition "A source of data that is publicly accessible or available"@en ;
    skos:prefLabel "Public Data Source"@en ;
    skos:scopeNote "The term 'Public' is used here in a broad sense. Actual consideration of what is 'Public Data' can vary based on several contextual or jurisdictional factors such as  definition of open, methods of access, permissions and licenses."@en .

dpv:PublicInterest a rdfs:Class,
        owl:Class,
        dpv:LegalBasis ;
    dct:contributor "Harshvardhan J. Pandit" ;
    dct:created "2021-04-21"^^xsd:date ;
    rdfs:subClassOf dpv:LegalBasis ;
    sw:term_status "accepted"@en ;
    skos:definition "Processing is necessary or beneficial for interest of the public or society at large"@en ;
    skos:prefLabel "Public Interest"@en .

dpv:PublicLocation a rdfs:Class,
        owl:Class,
        dpv:Location ;
    dct:contributor "Georg P Krog" ;
    dct:created "2022-10-22"^^xsd:date ;
    rdfs:subClassOf dpv:LocalLocation ;
    sw:term_status "accepted"@en ;
    skos:definition "Location that is or can be accessed by the public"@en ;
    skos:prefLabel "Public Location"@en .

dpv:PublicRelations a rdfs:Class,
        owl:Class,
        dpv:Purpose ;
    dct:contributor "Paul Ryan, Georg P Krog, David Hickey, Harshvardhan J. Pandit" ;
    dct:created "2021-09-01"^^xsd:date ;
    dct:source "(Belgian DPA ROPA Template, https://www.privacycommission.be/nl/model-voor-een-register-van-de-verwerkingsactiviteiten)"@en ;
    rdfs:subClassOf dpv:Marketing ;
    sw:term_status "accepted"@en ;
    skos:definition "Purposes associated with managing and conducting public relations processes, including creating goodwill for the organisation"@en ;
    skos:prefLabel "Public Relations"@en .

dpv:Purpose a rdfs:Class,
        owl:Class ;
    dct:contributor "Axel Polleres, Javier Fernández" ;
    dct:created "2019-04-05"^^xsd:date ;
    dct:modified "2023-12-10"^^xsd:date ;
    dct:source "(SPECIAL Project,https://specialprivacy.ercim.eu/)"@en ;
    vann:example dex:E0001,
        dex:E0002,
        dex:E0003,
        dex:E0004,
        dex:E0006,
        dex:E0009,
        dex:E0010,
        dex:E0014 ;
    sw:term_status "accepted"@en ;
    skos:definition "Purpose or Goal of processing data or using technology"@en ;
    skos:prefLabel "Purpose"@en ;
    skos:related "spl:AnyPurpose"@en ;
    skos:scopeNote "The purpose or goal here is intended to sufficiently describe the intention or objective of why the data or technology is being used, and should be broader than mere technical descriptions of achieving a capability. For example, \"Analyse Data\" is an abstract purpose with no indication of what the analyses is for as compared to a purpose such as \"Marketing\" or \"Service Provision\" which provide clarity and comprehension of the 'purpose' and can be enhanced with additional descriptions."@en .

dpv:QuantumCryptography a rdfs:Class,
        owl:Class,
        dpv:TechnicalMeasure ;
    dct:contributor "Harshvardhan J. Pandit" ;
    dct:created "2022-08-17"^^xsd:date ;
    dct:source "(ENISA Reference Incident Classification Taxonomy 2018,https://www.enisa.europa.eu/publications/reference-incident-classification-taxonomy/)"@en ;
    rdfs:subClassOf dpv:CryptographicMethods ;
    sw:term_status "accepted"@en ;
    skos:definition "Cryptographic methods that utilise quantum mechanical properties to perform cryptographic tasks"@en ;
    skos:prefLabel "Quantum Cryptography"@en .

dpv:Query a rdfs:Class,
        owl:Class,
        dpv:Processing ;
    dct:contributor "Harshvardhan J. Pandit" ;
    dct:created "2022-06-15"^^xsd:date ;
    rdfs:subClassOf dpv:Consult ;
    sw:term_status "accepted"@en ;
    skos:definition "to query or make enquiries over data"@en ;
    skos:prefLabel "Query"@en .

dpv:RNGPseudonymisation a rdfs:Class,
        owl:Class,
        dpv:TechnicalMeasure ;
    dct:contributor "Harshvardhan J. Pandit" ;
    dct:created "2022-08-17"^^xsd:date ;
    dct:modified "2022-10-13"^^xsd:date ;
    dct:source "(ENISA Data Pseudonymisation: Advanced Techniques and Use Cases,https://www.enisa.europa.eu/publications/data-pseudonymisation-advanced-techniques-and-use-cases)"@en ;
    rdfs:subClassOf dpv:Pseudonymisation ;
    sw:term_status "modified"@en ;
    skos:definition "A pseudonymisation method where identifiers are substituted by a number chosen by a Random Number Generator (RNG)"@en ;
    skos:prefLabel "RNG Pseudonymisation"@en .

dpv:RandomLocation a rdfs:Class,
        owl:Class,
        dpv:LocationFixture ;
    dct:contributor "Harshvardhan J. Pandit" ;
    dct:created "2022-06-15"^^xsd:date ;
    dct:modified "2020-10-05"^^xsd:date ;
    rdfs:subClassOf dpv:LocationFixture ;
    sw:term_status "accepted"@en ;
    skos:definition "Location that is random or unknown"@en ;
    skos:prefLabel "Random Location"@en .

dpv:Recipient a rdfs:Class,
        owl:Class ;
    dct:contributor "Axel Polleres, Javier Fernández" ;
    dct:created "2019-04-05"^^xsd:date ;
    dct:modified "2023-12-10"^^xsd:date ;
    dct:source "(SPECIAL Project,https://specialprivacy.ercim.eu/),(GDPR Art.4-9g,https://eur-lex.europa.eu/eli/reg/2016/679/art_4/par_9/oj)"@en ;
    vann:example dex:E0019 ;
    rdfs:subClassOf dpv:LegalEntity ;
    rdfs:superClassOf dpv:DataImporter,
        dpv:DataProcessor,
        dpv:ThirdParty ;
    sw:term_status "accepted"@en ;
    skos:definition "Entities that receive data"@en ;
    skos:prefLabel "Recipient"@en ;
    skos:related "spl:AnyRecipient"@en ;
    skos:scopeNote "Recipients indicate entities that receives data, for example personal data recipients can be a Third Party, Data Controller, or Data Processor."@en .

dpv:Record a rdfs:Class,
        owl:Class,
        dpv:Processing ;
    dct:created "2019-05-07"^^xsd:date ;
    dct:source "(GDPR Art.4-2,https://eur-lex.europa.eu/eli/reg/2016/679/art_4/par_2/oj)"@en ;
    rdfs:subClassOf dpv:Obtain ;
    sw:term_status "accepted"@en ;
    skos:definition "to make a record (especially media)"@en ;
    skos:prefLabel "Record"@en .

dpv:RecordManagement a rdfs:Class,
        owl:Class,
        dpv:Purpose ;
    dct:contributor "Paul Ryan, Georg P Krog, David Hickey, Harshvardhan J. Pandit" ;
    dct:created "2021-09-01"^^xsd:date ;
    rdfs:subClassOf dpv:Purpose ;
    sw:term_status "accepted"@en ;
    skos:definition "Purposes associated with manage creation, storage, and use of records relevant to operations, events, and processes e.g. to store logs or access requests"@en ;
    skos:prefLabel "Record Management"@en ;
    skos:scopeNote "This purpose relates specifiaclly for record creation and management. This can be combined or used along with other purposes to express intentions such as records for legal compliance or vendor payments."@en .

dpv:RecordsOfActivities a rdfs:Class,
        owl:Class,
        dpv:OrganisationalMeasure ;
    dct:contributor "Georg P Krog, Harshvardhan J. Pandit, Paul Ryan" ;
    dct:created "2021-09-08"^^xsd:date ;
    rdfs:subClassOf dpv:OrganisationalMeasure ;
    sw:term_status "accepted"@en ;
    skos:definition "Records of activities within some context such as maintainence tasks or governance functions"@en ;
    skos:prefLabel "Records of Activities"@en .

dpv:Region a rdfs:Class,
        owl:Class ;
    dct:contributor "Harshvardhan J. Pandit" ;
    dct:created "2022-01-19"^^xsd:date ;
    rdfs:subClassOf dpv:Country ;
    rdfs:superClassOf dpv:City ;
    sw:term_status "accepted"@en ;
    skos:definition "A region is an area or site that is considered a location"@en ;
    skos:prefLabel "Region"@en .

dpv:RegionalAuthority a rdfs:Class,
        owl:Class ;
    dct:contributor "Harshvardhan J. Pandit" ;
    dct:created "2022-02-02"^^xsd:date ;
    dct:source "(ADMS controlled vocabulary,http://purl.org/adms)"@en ;
    rdfs:subClassOf dpv:Authority ;
    sw:term_status "accepted"@en ;
    skos:definition "An authority tasked with overseeing legal compliance for a region"@en ;
    skos:prefLabel "Regional Authority"@en .

dpv:RegionalScale a rdfs:Class,
        owl:Class,
        dpv:GeographicCoverage ;
    dct:contributor "Harshvardhan J. Pandit" ;
    dct:created "2022-06-15"^^xsd:date ;
    rdfs:subClassOf dpv:GeographicCoverage ;
    sw:term_status "accepted"@en ;
    skos:definition "Geographic coverage spanning a specific region or regions"@en ;
    skos:prefLabel "Regional Scale"@en .

dpv:RegularityOfRecertification a rdfs:Class,
        owl:Class,
        dpv:OrganisationalMeasure ;
    dct:contributor "Axel Polleres, Rob Brennan, Harshvardhan J. Pandit, Mark Lizar" ;
    dct:created "2019-04-05"^^xsd:date ;
    rdfs:subClassOf dpv:OrganisationalMeasure ;
    sw:term_status "accepted"@en ;
    skos:definition "Policy regarding repetition or renewal of existing certification(s)"@en ;
    skos:prefLabel "Regularity of Re-certification"@en .

dpv:RemoteLocation a rdfs:Class,
        owl:Class,
        dpv:Location ;
    dct:contributor "Harshvardhan J. Pandit" ;
    dct:created "2022-06-15"^^xsd:date ;
    dct:modified "2020-10-05"^^xsd:date ;
    rdfs:subClassOf dpv:LocationLocality ;
    sw:term_status "accepted"@en ;
    skos:definition "Location is remote i.e. not local"@en ;
    skos:prefLabel "Remote Location"@en .

dpv:Remove a rdfs:Class,
        owl:Class,
        dpv:Processing ;
    dct:created "2019-05-07"^^xsd:date ;
    dct:source "(GDPR Art.4-2,https://eur-lex.europa.eu/eli/reg/2016/679/art_4/par_2/oj)"@en ;
    rdfs:subClassOf dpv:Processing ;
    sw:term_status "accepted"@en ;
    skos:definition "to destruct or erase data"@en ;
    skos:prefLabel "Remove"@en .

dpv:RenewedConsentGiven a rdfs:Class,
        owl:Class,
        dpv:ConsentStatus ;
    dct:contributor "Georg P Krog, Harshvardhan J. Pandit, Paul Ryan, Julian Flake" ;
    dct:created "2022-06-22"^^xsd:date ;
    dct:source "(GConsent,https://w3id.org/GConsent)"@en ;
    rdfs:subClassOf dpv:ConsentStatusValidForProcessing ;
    sw:term_status "accepted"@en ;
    skos:definition "The state where a previously given consent has been 'renewed' or 'refreshed' or 'reaffirmed' to form a new instance of given consent"@en ;
    skos:prefLabel "Renewed Consent Given"@en ;
    skos:scopeNote "An example of this state is when a previously given consent has expired, and the individual is presented a notice regarding continuing associated processing operations - to which they agree. This state can be useful to keep track of 'reconfirmed' or 'refreshed' consent within consent records, assist notices and contextual agents to create better consenting dialogues, and assist with specific legal obligations related to subsequent consenting"@en .

dpv:RepairImpairments a rdfs:Class,
        owl:Class,
        dpv:Purpose ;
    dct:contributor "Harshvardhan J. Pandit" ;
    dct:created "2022-08-24"^^xsd:date ;
    rdfs:subClassOf dpv:ServiceProvision ;
    sw:term_status "accepted"@en ;
    skos:definition "Purposes associated with identifying, rectifying, or otherwise undertaking activities intended to fix or repair impairments to existing functionalities"@en ;
    skos:prefLabel "Repair Impairments"@en ;
    skos:scopeNote "An example of identifying and rectifying impairments is the process of finding and fixing errors in products, commonly referred to as debugging"@en .

dpv:Representative a rdfs:Class,
        owl:Class ;
    dct:contributor "Georg Krog, Paul Ryan, Harshvardhan J. Pandit, Beatriz Esteves" ;
    dct:created "2020-11-04"^^xsd:date ;
    dct:source "(GDPR Art.27,https://eur-lex.europa.eu/eli/reg/2016/679/art_27/oj)"@en ;
    rdfs:subClassOf dpv:LegalEntity ;
    rdfs:superClassOf dpv:DataProtectionOfficer ;
    sw:term_status "accepted"@en ;
    skos:definition "A representative of a legal entity"@en ;
    skos:prefLabel "Representative"@en .

dpv:RequestAccepted a rdfs:Class,
        owl:Class,
        dpv:RequestStatus ;
    dct:contributor "Harshvardhan J. Pandit" ;
    dct:created "2022-11-30"^^xsd:date ;
    rdfs:subClassOf dpv:RequestStatus ;
    sw:term_status "accepted"@en ;
    skos:definition "State of a request being accepted towards fulfilment"@en ;
    skos:prefLabel "Request Accepted"@en .

dpv:RequestAcknowledged a rdfs:Class,
        owl:Class,
        dpv:RequestStatus ;
    dct:contributor "Harshvardhan J. Pandit" ;
    dct:created "2022-11-30"^^xsd:date ;
    rdfs:subClassOf dpv:RequestStatus ;
    sw:term_status "accepted"@en ;
    skos:definition "State of a request being acknowledged"@en ;
    skos:prefLabel "Request Acknowledged"@en .

dpv:RequestActionDelayed a rdfs:Class,
        owl:Class,
        dpv:RequestStatus ;
    dct:contributor "Harshvardhan J. Pandit" ;
    dct:created "2022-11-30"^^xsd:date ;
    rdfs:subClassOf dpv:RequestStatus ;
    sw:term_status "accepted"@en ;
    skos:definition "State of a request being delayed towards fulfilment"@en ;
    skos:prefLabel "Request Action Delayed"@en .

dpv:RequestFulfilled a rdfs:Class,
        owl:Class,
        dpv:RequestStatus ;
    dct:contributor "Harshvardhan J. Pandit" ;
    dct:created "2022-11-30"^^xsd:date ;
    rdfs:subClassOf dpv:RequestStatus ;
    sw:term_status "accepted"@en ;
    skos:definition "State of a request being fulfilled"@en ;
    skos:prefLabel "Request Fulfilled"@en .

dpv:RequestInitiated a rdfs:Class,
        owl:Class,
        dpv:RequestStatus ;
    dct:contributor "Harshvardhan J. Pandit" ;
    dct:created "2022-11-30"^^xsd:date ;
    rdfs:subClassOf dpv:RequestStatus ;
    sw:term_status "accepted"@en ;
    skos:definition "State of a request being initiated"@en ;
    skos:prefLabel "Request Initiated"@en .

dpv:RequestRejected a rdfs:Class,
        owl:Class,
        dpv:RequestStatus ;
    dct:contributor "Harshvardhan J. Pandit" ;
    dct:created "2022-11-30"^^xsd:date ;
    rdfs:subClassOf dpv:RequestStatus ;
    sw:term_status "accepted"@en ;
    skos:definition "State of a request being rejected towards non-fulfilment"@en ;
    skos:prefLabel "Request Rejected"@en .

dpv:RequestRequiredActionPerformed a rdfs:Class,
        owl:Class,
        dpv:RequestStatus ;
    dct:contributor "Harshvardhan J. Pandit" ;
    dct:created "2022-11-30"^^xsd:date ;
    rdfs:subClassOf dpv:RequestStatus ;
    sw:term_status "accepted"@en ;
    skos:definition "State of a request's required action having been performed by the other party"@en ;
    skos:prefLabel "Request Required Action Performed"@en .

dpv:RequestRequiresAction a rdfs:Class,
        owl:Class,
        dpv:RequestStatus ;
    dct:contributor "Harshvardhan J. Pandit" ;
    dct:created "2022-11-30"^^xsd:date ;
    rdfs:subClassOf dpv:RequestStatus ;
    sw:term_status "accepted"@en ;
    skos:definition "State of a request requiring an action to be performed from another party"@en ;
    skos:prefLabel "Request Requires Action"@en .

dpv:RequestStatus a rdfs:Class,
        owl:Class ;
    dct:contributor "Harshvardhan J. Pandit" ;
    dct:created "2022-11-30"^^xsd:date ;
    rdfs:subClassOf dpv:Status ;
    sw:term_status "accepted"@en ;
    skos:definition "Status associated with requests"@en ;
    skos:prefLabel "Request Status"@en .

dpv:RequestStatusQuery a rdfs:Class,
        owl:Class,
        dpv:RequestStatus ;
    dct:contributor "Harshvardhan J. Pandit" ;
    dct:created "2022-11-30"^^xsd:date ;
    rdfs:subClassOf dpv:RequestStatus ;
    sw:term_status "accepted"@en ;
    skos:definition "State of a request's status being queried"@en ;
    skos:prefLabel "Request Status Query"@en .

dpv:RequestUnfulfilled a rdfs:Class,
        owl:Class,
        dpv:RequestStatus ;
    dct:contributor "Harshvardhan J. Pandit" ;
    dct:created "2022-11-30"^^xsd:date ;
    rdfs:subClassOf dpv:RequestStatus ;
    sw:term_status "accepted"@en ;
    skos:definition "State of a request being unfulfilled"@en ;
    skos:prefLabel "Request Unfulfilled"@en .

dpv:RequestedServiceProvision a rdfs:Class,
        owl:Class,
        dpv:Purpose ;
    dct:contributor "Georg P Krog, Harshvardhan J. Pandit, Beatriz Esteves" ;
    dct:created "2021-09-08"^^xsd:date ;
    rdfs:subClassOf dpv:ServiceProvision ;
    sw:term_status "accepted"@en ;
    skos:definition "Purposes associated with delivering services as requested by user or consumer"@en ;
    skos:prefLabel "Requested Service Provision"@en ;
    skos:scopeNote "The use of 'request' here includes where an user explicitly asks for the service and also when an established contract requires the provision of the service"@en .

dpv:Required a rdfs:Class,
        owl:Class,
        dpv:Necessity ;
    dct:contributor "Harshvardhan J. Pandit, Paul Ryan, Georg P Krog, Julian Flake, Beatriz Esteves" ;
    dct:created "2022-02-13"^^xsd:date ;
    rdfs:subClassOf dpv:Necessity ;
    sw:term_status "accepted"@en ;
    skos:definition "Indication of 'required' or 'necessary'"@en ;
    skos:prefLabel "Required"@en .

dpv:ResearchAndDevelopment a rdfs:Class,
        owl:Class,
        dpv:Purpose ;
    dct:contributor "Harshvardhan J. Pandit, Javier Fernandez, Axel Polleres, Elmar Kiesling, Fajar Ekaputra, Simon Steyskal" ;
    dct:created "2019-04-05"^^xsd:date ;
    rdfs:subClassOf dpv:Purpose ;
    sw:term_status "accepted"@en ;
    skos:definition "Purposes associated with conducting research and development for new methods, products, or services"@en ;
    skos:prefLabel "Research and Development"@en .

dpv:Restrict a rdfs:Class,
        owl:Class,
        dpv:Processing ;
    dct:created "2019-05-07"^^xsd:date ;
    dct:source "(GDPR Art.4-2,https://eur-lex.europa.eu/eli/reg/2016/679/art_4/par_2/oj)"@en ;
    rdfs:subClassOf dpv:Transform ;
    sw:term_status "accepted"@en ;
    skos:definition "to apply a restriction on the processing of specific records"@en ;
    skos:prefLabel "Restrict"@en .

dpv:Retrieve a rdfs:Class,
        owl:Class,
        dpv:Processing ;
    dct:created "2019-05-07"^^xsd:date ;
    dct:source "(GDPR Art.4-2,https://eur-lex.europa.eu/eli/reg/2016/679/art_4/par_2/oj)"@en ;
    rdfs:subClassOf dpv:Use ;
    sw:term_status "accepted"@en ;
    skos:definition "to retrieve data, often in an automated manner"@en ;
    skos:prefLabel "Retrieve"@en .

dpv:ReviewImpactAssessment a rdfs:Class,
        owl:Class,
        dpv:OrganisationalMeasure ;
    dct:contributor "Harshvardhan J. Pandit, Georg P Krog" ;
    dct:created "2022-10-22"^^xsd:date ;
    rdfs:subClassOf dpv:ImpactAssessment,
        dpv:ReviewProcedure ;
    sw:term_status "accepted"@en ;
    skos:definition "Procedures to review impact assessments in terms of continued validity, adequacy for intended purposes, and conformance of processes with findings"@en ;
    skos:prefLabel "Review Impact Assessment"@en .

dpv:ReviewProcedure a rdfs:Class,
        owl:Class,
        dpv:OrganisationalMeasure ;
    dct:contributor "Harshvardhan J. Pandit, Georg P Krog" ;
    dct:created "2022-10-22"^^xsd:date ;
    rdfs:subClassOf dpv:OrganisationalMeasure ;
    sw:term_status "accepted"@en ;
    skos:definition "A procedure or process that reviews the correctness and validity of other measures and processes"@en ;
    skos:prefLabel "Review Procedure"@en .

dpv:Right a rdfs:Class,
        owl:Class ;
    dct:contributor "Harshvardhan J Pandit, Beatriz Esteves, Georg P Krog" ;
    dct:created "2020-11-18"^^xsd:date ;
    sw:term_status "accepted"@en ;
    skos:definition "The right(s) applicable, provided, or expected"@en ;
    skos:prefLabel "Right"@en ;
    skos:scopeNote "A 'right' is a legal, social, or ethical principle of freedom or entitlement which dictate the norms regarding what is allowed or owed. Rights as a concept encompass a broad area of norms and entities, and are not specific to Individuals or Data Protection / Privacy. For individual specific rights, see dpv:DataSubjectRight"@en .

dpv:RightExerciseActivity a rdfs:Class,
        owl:Class,
        dpv:OrganisationalMeasure ;
    dct:contributor "Harshvardhan J Pandit, Beatriz Esteves, Georg P Krog, Paul Ryan" ;
    dct:created "2022-11-02"^^xsd:date ;
    rdfs:subClassOf dpv:OrganisationalMeasure ;
    sw:term_status "accepted"@en ;
    skos:definition "An activity representing an exercising of an active right"@en ;
    skos:prefLabel "Right Exercise Activity"@en ;
    skos:scopeNote "There may be multiple activities associated with exercising and fulfilling rights. See the RightExerciseRecord concept for record-keeping of such activities in a cohesive manner."@en .

dpv:RightExerciseNotice a rdfs:Class,
        owl:Class,
        dpv:OrganisationalMeasure ;
    dct:contributor "Harshvardhan J Pandit, Beatriz Esteves, Georg P Krog, Paul Ryan" ;
    dct:created "2022-10-22"^^xsd:date ;
    rdfs:subClassOf dpv:OrganisationalMeasure ;
    sw:term_status "accepted"@en ;
    skos:definition "Information associated with exercising of an active right"@en ;
    skos:prefLabel "Right Exercise Notice"@en ;
    skos:scopeNote "This concept is intended for providing information regarding a right exercise. For specific instances of such exercises, see RightExerciseActivity and RightExerciseRecord."@en .

dpv:RightExerciseRecord a rdfs:Class,
        owl:Class,
        dpv:OrganisationalMeasure ;
    dct:contributor "Harshvardhan J Pandit, Beatriz Esteves, Georg P Krog, Paul Ryan" ;
    dct:created "2022-11-02"^^xsd:date ;
    rdfs:subClassOf dpv:Record ;
    sw:term_status "accepted"@en ;
    skos:definition "Record of a Right being exercised"@en ;
    skos:prefLabel "Right Exercise Record"@en ;
    skos:scopeNote "This concept represents a record of one or more right exercise activities, such as those associated with a single data subject or service or entity"@en .

dpv:RightFulfilmentNotice a rdfs:Class,
        owl:Class,
        dpv:OrganisationalMeasure ;
    dct:contributor "Harshvardhan J. Pandit, Beatriz Esteves" ;
    dct:created "2022-11-02"^^xsd:date ;
    rdfs:subClassOf dpv:Notice ;
    sw:term_status "accepted"@en ;
    skos:definition "Notice provided regarding fulfilment of a right"@en ;
    skos:prefLabel "Right Fulfilment Notice"@en ;
    skos:scopeNote "This notice is associated with situations where information is provided with the intention of progressing the fulfilment of a right. For example, a notice asking for more information regarding the scope of the right, or providing information on where to access the data provided under a right."@en .

dpv:RightNonFulfilmentNotice a rdfs:Class,
        owl:Class,
        dpv:OrganisationalMeasure ;
    dct:contributor "Harshvardhan J. Pandit, Beatriz Esteves" ;
    dct:created "2022-11-02"^^xsd:date ;
    rdfs:subClassOf dpv:Notice ;
    sw:term_status "accepted"@en ;
    skos:definition "Notice provided regarding non-fulfilment of a right"@en ;
    skos:prefLabel "Right Non-Fulfilment Notice"@en ;
    skos:scopeNote "This notice is associated with situations where information is provided with the intention of communicating non-fulfilment of a right. For example, to provide justifications on why a right could not be fulfilled or providing information about another entity  who should be approached for exercising this right."@en .

dpv:Risk a rdfs:Class,
        owl:Class ;
    dct:contributor "Harshvardhan J. Pandit" ;
    dct:created "2020-11-18"^^xsd:date ;
    vann:example dex:E0029 ;
    sw:term_status "accepted"@en ;
    skos:definition "A risk or possibility or uncertainty of negative effects, impacts, or consequences"@en ;
    skos:prefLabel "Risk"@en ;
    skos:scopeNote "Risks can be associated with one or more different concepts such as purpose, processing, personal data, technical or organisational measure"@en .

dpv:RiskLevel a rdfs:Class,
        owl:Class ;
    dct:contributor "Harshvardhan J. Pandit" ;
    dct:created "2022-07-20"^^xsd:date ;
    sw:term_status "accepted"@en ;
    skos:definition "The magnitude of a risk expressed as an indication to aid in its management"@en ;
    skos:prefLabel "Risk Level"@en ;
    skos:scopeNote "Risk Levels can be defined as a combination of different characteristics. For example, ISO 31073:2022 defines it as a combination of consequences and their likelihood. Another example would be the Risk Matrix where Risk Level is defined as a combination of Likelihood and Severity associated with the Risk."@en .

dpv:RiskManagementPlan a rdfs:Class,
        owl:Class,
        dpv:OrganisationalMeasure ;
    dct:contributor "Harshvardhan J. Pandit" ;
    dct:created "2022-08-18"^^xsd:date ;
    dct:source "(ISO 31073:2022,https://www.iso.org/standard/79637.html)"@en ;
    rdfs:subClassOf dpv:SecurityProcedure ;
    sw:term_status "accepted"@en ;
    skos:definition "A scheme within the risk management framework specifying the approach, the management components, and resources to be applied to the management of risk"@en ;
    skos:prefLabel "Risk Management Plan"@en .

dpv:RiskManagementPolicy a rdfs:Class,
        owl:Class,
        dpv:OrganisationalMeasure ;
    dct:contributor "Harshvardhan J. Pandit" ;
    dct:created "2022-08-18"^^xsd:date ;
    dct:source "(ISO 31073:2022,https://www.iso.org/standard/79637.html)"@en ;
    rdfs:subClassOf dpv:Policy,
        dpv:SecurityProcedure ;
    sw:term_status "accepted"@en ;
    skos:definition "A policy or statement of the overall intentions and direction of an organisation related to risk management"@en ;
    skos:prefLabel "Risk Management Policy"@en .

dpv:RiskMitigationMeasure a rdfs:Class,
        owl:Class ;
    dct:contributor "Georg P Krog, Harshvardhan J. Pandit, Paul Ryan" ;
    dct:created "2020-11-04"^^xsd:date ;
    vann:example dex:E0029 ;
    rdfs:subClassOf dpv:TechnicalOrganisationalMeasure ;
    sw:term_status "accepted"@en ;
    skos:definition "Measures intended to mitigate, minimise, or prevent risk."@en ;
    skos:prefLabel "Risk Mitigation Measure"@en .

dpv:Rule a rdfs:Class,
        owl:Class ;
    dct:contributor "Harshvardhan J. Pandit, Georg P Krog, Beatriz Esteves, Paul Ryan" ;
    dct:created "2022-10-19"^^xsd:date ;
    sw:term_status "accepted"@en ;
    skos:definition "A rule describing a process or control that directs or determines if and how an activity should be conducted"@en ;
    skos:prefLabel "Rule"@en .

dpv:Safeguard a rdfs:Class,
        owl:Class,
        dpv:OrganisationalMeasure ;
    dct:contributor "David Hickey, Paul Ryan, Georg P Krog, Harshvardhan J. Pandit" ;
    dct:created "2021-09-22"^^xsd:date ;
    rdfs:subClassOf dpv:OrganisationalMeasure ;
    sw:term_status "accepted"@en ;
    skos:definition "A safeguard is a precautionary measure for the protection against or mitigation of negative effects"@en ;
    skos:prefLabel "Safeguard"@en ;
    skos:scopeNote "This concept is relevant given the requirement to assert safeguards in cross-border data transfers"@en .

dpv:SafeguardForDataTransfer a rdfs:Class,
        owl:Class,
        dpv:OrganisationalMeasure ;
    dct:contributor "David Hickey, Paul Ryan, Georg P Krog, Harshvardhan J. Pandit" ;
    dct:created "2021-09-22"^^xsd:date ;
    rdfs:subClassOf dpv:Safeguard ;
    sw:term_status "accepted"@en ;
    skos:definition "Represents a safeguard used for data transfer. Can include technical or organisational measures."@en ;
    skos:prefLabel "Safeguard for Data Transfer"@en .

dpv:Scale a rdfs:Class,
        owl:Class ;
    dct:contributor "Harshvardhan J. Pandit, Georg P Krog, Rana Saniei" ;
    dct:created "2022-06-15"^^xsd:date ;
    rdfs:subClassOf dpv:ProcessingContext ;
    rdfs:superClassOf dpv:DataSubjectScale,
        dpv:DataVolume,
        dpv:GeographicCoverage,
        dpv:ProcessingScale ;
    sw:term_status "accepted"@en ;
    skos:definition "A measurement along some dimension"@en ;
    skos:prefLabel "Scale"@en ;
    skos:scopeNote "Scales are subjective concepts that need to be defined and interpreted within the context of their application. For example, what would be small within one context could be large within another."@en .

dpv:Scope a rdfs:Class,
        owl:Class ;
    dct:contributor "Harshvardhan J. Pandit" ;
    dct:created "2022-06-15"^^xsd:date ;
    rdfs:subClassOf dpv:Context ;
    sw:term_status "accepted"@en ;
    skos:definition "Indication of the extent or range or boundaries associated with(in) a context"@en ;
    skos:prefLabel "Scope"@en .

dpv:ScoringOfIndividuals a rdfs:Class,
        owl:Class,
        dpv:EvaluationScoring ;
    dct:contributor "Harshvardhan J. Pandit" ;
    dct:created "2022-10-22"^^xsd:date ;
    dct:modified "2022-11-30"^^xsd:date ;
    dct:source "(GDPR Art.4-2,https://eur-lex.europa.eu/eli/reg/2016/679/art_4/par_2/oj)"@en ;
    rdfs:subClassOf dpv:EvaluationScoring ;
    sw:term_status "accepted"@en ;
    skos:definition "Processing that involves scoring of individuals"@en ;
    skos:prefLabel "Scoring of Individuals"@en .

dpv:Screen a rdfs:Class,
        owl:Class,
        dpv:Processing ;
    dct:contributor "Harshvardhan J. Pandit, Georg P Krog" ;
    dct:created "2022-06-15"^^xsd:date ;
    rdfs:subClassOf dpv:Transform ;
    sw:term_status "accepted"@en ;
    skos:definition "to remove data for some criteria"@en ;
    skos:prefLabel "Screen"@en .

dpv:Seal a rdfs:Class,
        owl:Class,
        dpv:OrganisationalMeasure ;
    dct:contributor "Axel Polleres, Rob Brennan, Harshvardhan J. Pandit, Mark Lizar" ;
    dct:created "2019-04-05"^^xsd:date ;
    rdfs:subClassOf dpv:CertificationSeal ;
    sw:term_status "accepted"@en ;
    skos:definition "A seal or a mark indicating proof of certification to some certification or standard"@en ;
    skos:prefLabel "Seal"@en .

dpv:SearchFunctionalities a rdfs:Class,
        owl:Class,
        dpv:Purpose ;
    dct:contributor "Georg P Krog" ;
    dct:created "2022-11-09"^^xsd:date ;
    rdfs:subClassOf dpv:ServiceProvision ;
    sw:term_status "accepted"@en ;
    skos:definition "Purposes associated with providing searching, querying, or other forms of information retrieval related functionalities"@en ;
    skos:prefLabel "Search Functionalities"@en .

dpv:SecondaryImportance a rdfs:Class,
        owl:Class,
        dpv:Importance ;
    dct:contributor "Harshvardhan J. Pandit, Paul Ryan, Georg P Krog, Julian Flake, Beatriz Esteves" ;
    dct:created "2022-02-11"^^xsd:date ;
    rdfs:subClassOf dpv:Importance ;
    sw:term_status "accepted"@en ;
    skos:definition "Indication of 'secondary' or 'minor' or 'auxiliary' importance"@en ;
    skos:prefLabel "Secondary Importance"@en .

dpv:SecretSharingSchemes a rdfs:Class,
        owl:Class,
        dpv:TechnicalMeasure ;
    dct:contributor "Harshvardhan J. Pandit" ;
    dct:created "2022-08-17"^^xsd:date ;
    dct:source "(ENISA Data Pseudonymisation: Advanced Techniques and Use Cases,https://www.enisa.europa.eu/publications/data-pseudonymisation-advanced-techniques-and-use-cases)"@en ;
    rdfs:subClassOf dpv:CryptographicMethods ;
    sw:term_status "accepted"@en ;
    skos:definition "Use of secret sharing schemes where the secret can only be reconstructed through combination of sufficient number of individuals"@en ;
    skos:prefLabel "Secret Sharing Schemes"@en .

dpv:Sector a rdfs:Class,
        owl:Class ;
    dct:contributor "Harshvardhan J. Pandit, Javier Fernandez, Axel Polleres, Elmar Kiesling, Fajar Ekaputra, Simon Steyskal" ;
    dct:created "2019-04-05"^^xsd:date ;
    vann:example dex:E0010 ;
    sw:term_status "accepted"@en ;
    skos:definition "Sector describes the area of application or domain that indicates or restricts scope for interpretation and application of purpose e.g. Agriculture, Banking"@en ;
    skos:prefLabel "Sector"@en ;
    skos:scopeNote "There are various sector codes used commonly to indicate the domain of an organisation or business. Examples include NACE (EU), ISIC (UN), SIC and NAICS (USA)."@en .

dpv:SecureMultiPartyComputation a rdfs:Class,
        owl:Class,
        dpv:TechnicalMeasure ;
    dct:contributor "Harshvardhan J. Pandit" ;
    dct:created "2022-08-17"^^xsd:date ;
    dct:source "(ENISA Reference Incident Classification Taxonomy 2018,https://www.enisa.europa.eu/publications/reference-incident-classification-taxonomy/)"@en ;
    rdfs:subClassOf dpv:CryptographicMethods ;
    sw:term_status "accepted"@en ;
    skos:definition "Use of cryptographic methods for entities to jointly compute functions without revealing inputs"@en ;
    skos:prefLabel "Secure Multi-Party Computation"@en .

dpv:SecurityAssessment a rdfs:Class,
        owl:Class,
        dpv:OrganisationalMeasure ;
    dct:contributor "Harshvardhan J. Pandit" ;
    dct:created "2022-08-17"^^xsd:date ;
    dct:source "(ENISA 5G Cybersecurity Standards,https://www.enisa.europa.eu/publications/5g-cybersecurity-standards)"@en ;
    rdfs:subClassOf dpv:Assessment,
        dpv:SecurityProcedure ;
    sw:term_status "accepted"@en ;
    skos:definition "Assessment of security intended to identity gaps, vulnerabilities, risks, and effectiveness of controls"@en ;
    skos:prefLabel "Security Assessment"@en .

dpv:SecurityKnowledgeTraining a rdfs:Class,
        owl:Class,
        dpv:OrganisationalMeasure ;
    dct:contributor "Harshvardhan J. Pandit" ;
    dct:created "2022-08-17"^^xsd:date ;
    dct:source "(ENISA 5G Cybersecurity Standards,https://www.enisa.europa.eu/publications/5g-cybersecurity-standards)"@en ;
    rdfs:subClassOf dpv:StaffTraining ;
    sw:term_status "accepted"@en ;
    skos:definition "Training intended to increase knowledge regarding security"@en ;
    skos:prefLabel "Security Knowledge Training"@en .

dpv:SecurityMethod a rdfs:Class,
        owl:Class,
        dpv:TechnicalMeasure ;
    dct:contributor "Harshvardhan J. Pandit" ;
    dct:created "2022-08-24"^^xsd:date ;
    rdfs:subClassOf dpv:TechnicalMeasure ;
    sw:term_status "accepted"@en ;
    skos:definition "Methods that relate to creating and providing security"@en ;
    skos:prefLabel "Security Method"@en .

dpv:SecurityProcedure a rdfs:Class,
        owl:Class,
        dpv:OrganisationalMeasure ;
    dct:contributor "Harshvardhan J. Pandit" ;
    dct:created "2022-08-24"^^xsd:date ;
    rdfs:subClassOf dpv:OrganisationalMeasure ;
    sw:term_status "accepted"@en ;
    skos:definition "Procedures associated with assessing, implementing, and evaluating security"@en ;
    skos:prefLabel "Security Procedure"@en .

dpv:SecurityRoleProcedures a rdfs:Class,
        owl:Class,
        dpv:OrganisationalMeasure ;
    dct:contributor "Harshvardhan J. Pandit" ;
    dct:created "2022-08-17"^^xsd:date ;
    dct:source "(ENISA 5G Cybersecurity Standards,https://www.enisa.europa.eu/publications/5g-cybersecurity-standards)"@en ;
    rdfs:subClassOf dpv:SecurityProcedure ;
    sw:term_status "accepted"@en ;
    skos:definition "Procedures related to security roles"@en ;
    skos:prefLabel "Security Role Procedures"@en .

dpv:SellDataToThirdParties a rdfs:Class,
        owl:Class,
        dpv:Purpose ;
    dct:contributor "Harshvardhan J. Pandit, Javier Fernandez, Axel Polleres, Elmar Kiesling, Fajar Ekaputra, Simon Steyskal" ;
    dct:created "2019-04-05"^^xsd:date ;
    rdfs:subClassOf dpv:SellProducts ;
    sw:term_status "accepted"@en ;
    skos:definition "Purposes associated with selling or sharing data or information to third parties"@en ;
    skos:prefLabel "Sell Data to Third Parties"@en ;
    skos:scopeNote "Sell here means exchange, submit, or provide in return for direct or indirect compensation. Was subclass of commercial interest, changed to reflect selling something"@en .

dpv:SellInsightsFromData a rdfs:Class,
        owl:Class,
        dpv:Purpose ;
    dct:contributor "Harshvardhan J. Pandit, Javier Fernandez, Axel Polleres, Elmar Kiesling, Fajar Ekaputra, Simon Steyskal" ;
    dct:created "2019-04-05"^^xsd:date ;
    rdfs:subClassOf dpv:SellProducts ;
    sw:term_status "accepted"@en ;
    skos:definition "Purposes associated with selling or sharing insights obtained from analysis of data"@en ;
    skos:prefLabel "Sell Insights from Data"@en ;
    skos:scopeNote "Sell here means exchange, submit, or provide in return for direct or indirect compensation. Was subclass of commercial interest, changed to reflect selling something"@en .

dpv:SellProducts a rdfs:Class,
        owl:Class,
        dpv:Purpose ;
    dct:contributor "Georg P Krog, Harshvardhan J. Pandit, Beatriz Esteves" ;
    dct:created "2021-09-08"^^xsd:date ;
    rdfs:subClassOf dpv:ServiceProvision ;
    sw:term_status "accepted"@en ;
    skos:definition "Purposes associated with selling products or services"@en ;
    skos:prefLabel "Sell Products"@en ;
    skos:scopeNote "Sell here means exchange, submit, or provide in return for direct or indirect compensation."@en .

dpv:SellProductsToDataSubject a rdfs:Class,
        owl:Class,
        dpv:Purpose ;
    dct:contributor "Harshvardhan J. Pandit, Javier Fernandez, Axel Polleres, Elmar Kiesling, Fajar Ekaputra, Simon Steyskal" ;
    dct:created "2019-04-05"^^xsd:date ;
    rdfs:subClassOf dpv:SellProducts ;
    sw:term_status "accepted"@en ;
    skos:definition "Purposes associated with selling products or services to the user, consumer, or data subjects"@en ;
    skos:prefLabel "Sell Products to Data Subject"@en ;
    skos:scopeNote "Sell Products here refers to processing necessary to provide and complete a sale to customers. It should not be confused with providing services with a cost based on an established agreement."@en .

dpv:SensitiveData a rdfs:Class,
        owl:Class ;
    rdfs:subClassOf dpv:Data ;
    rdfs:superClassOf dpv:SensitiveNonPersonalData ;
    sw:term_status "accepted"@en ;
    skos:definition "Data deemed sensitive"@en ;
    skos:prefLabel "SensitiveData"@en .

dpv:SensitiveNonPersonalData a rdfs:Class,
        owl:Class ;
    dct:source "DGA 30(a)"@en ;
    rdfs:subClassOf dpv:SensitiveData ;
    sw:term_status "accepted"@en ;
    skos:definition "Non-personal data deemed sensitive"@en ;
    skos:prefLabel "SensitiveNonPersonalData"@en .

dpv:SensitivePersonalData a rdfs:Class,
        owl:Class ;
    dct:contributor "Harshvardhan J. Pandit" ;
    dct:created "2022-01-19"^^xsd:date ;
    vann:example dex:E0015 ;
    rdfs:subClassOf dpv:PersonalData ;
    rdfs:superClassOf dpv:SpecialCategoryPersonalData ;
    sw:term_status "accepted"@en ;
    skos:definition "Personal data that is considered 'sensitive' in terms of privacy and/or impact, and therefore requires additional considerations and/or protection"@en ;
    skos:prefLabel "Sensitive Personal Data"@en ;
    skos:scopeNote "Sensitivity' is a matter of context, and may be defined within legal frameworks. For GDPR, Special categories of personal data are considered a subset of sensitive data. To illustrate the difference between the two, consider the situation where Location data is collected, and which is considered 'sensitive' but not 'special'. As a probable rule, sensitive data require additional considerations whereas special category data requires additional legal basis / justifications."@en .

dpv:ServiceOptimisation a rdfs:Class,
        owl:Class,
        dpv:Purpose ;
    dct:contributor "Harshvardhan J. Pandit, Javier Fernandez, Axel Polleres, Elmar Kiesling, Fajar Ekaputra, Simon Steyskal" ;
    dct:created "2019-04-05"^^xsd:date ;
    rdfs:subClassOf dpv:ServiceProvision ;
    sw:term_status "accepted"@en ;
    skos:definition "Purposes associated with optimisation of services or activities"@en ;
    skos:prefLabel "Service Optimisation"@en ;
    skos:scopeNote "Subclass of ServiceProvision since optimisation is usually considered part of providing services"@en .

dpv:ServicePersonalisation a rdfs:Class,
        owl:Class,
        dpv:Purpose ;
    dct:contributor "Harshvardhan J. Pandit, Javier Fernandez, Axel Polleres, Elmar Kiesling, Fajar Ekaputra, Simon Steyskal" ;
    dct:created "2019-04-05"^^xsd:date ;
    rdfs:subClassOf dpv:Personalisation,
        dpv:ServiceProvision ;
    sw:term_status "accepted"@en ;
    skos:definition "Purposes associated with providing personalisation within services or product or activities"@en ;
    skos:prefLabel "Service Personalisation"@en .

dpv:ServiceProvision a rdfs:Class,
        owl:Class,
        dpv:Purpose ;
    dct:contributor "Harshvardhan J. Pandit, Javier Fernandez, Axel Polleres, Elmar Kiesling, Fajar Ekaputra, Simon Steyskal" ;
    dct:created "2019-04-05"^^xsd:date ;
    vann:example dex:E0018 ;
    rdfs:subClassOf dpv:Purpose ;
    sw:term_status "accepted"@en ;
    skos:definition "Purposes associated with providing service or product or activities"@en ;
    skos:prefLabel "Service Provision"@en .

dpv:ServiceRegistration a rdfs:Class,
        owl:Class,
        dpv:Purpose ;
    dct:contributor "Georg P Krog, Harshvardhan J. Pandit, Beatriz Esteves" ;
    dct:created "2020-11-04"^^xsd:date ;
    rdfs:subClassOf dpv:ServiceProvision ;
    sw:term_status "accepted"@en ;
    skos:definition "Purposes associated with registering users and collecting information required for providing a service"@en ;
    skos:prefLabel "Service Registration"@en ;
    skos:scopeNote "An example of service registration is to provide a form that collects information such as preferred language or media format for downloading a movie"@en .

dpv:ServiceUsageAnalytics a rdfs:Class,
        owl:Class,
        dpv:Purpose ;
    dct:contributor "Georg P Krog, Harshvardhan J. Pandit, Beatriz Esteves" ;
    dct:created "2020-11-04"^^xsd:date ;
    dct:modified "2022-10-05"^^xsd:date ;
    rdfs:subClassOf dpv:ServiceProvision ;
    sw:term_status "accepted"@en ;
    skos:definition "Purposes associated with conducting analysis and reporting related to usage of services or products"@en ;
    skos:prefLabel "Service Usage Analytics"@en ;
    skos:scopeNote "Was \"UsageAnalytics\", prefixed with Service to better reflect scope"@en .

dpv:Severity a rdfs:Class,
        owl:Class ;
    dct:contributor "Harshvardhan J. Pandit" ;
    dct:created "2022-07-21"^^xsd:date ;
    sw:term_status "accepted"@en ;
    skos:definition "The magnitude of being unwanted or having negative effects such as harmful impacts"@en ;
    skos:prefLabel "Severity"@en ;
    skos:scopeNote "Severity can be associated with Risk, or its Consequences and Impacts"@en .

dpv:Share a rdfs:Class,
        owl:Class,
        dpv:Processing ;
    dct:created "2019-05-07"^^xsd:date ;
    dct:source "(GDPR Art.4-2,https://eur-lex.europa.eu/eli/reg/2016/679/art_4/par_2/oj)"@en ;
    rdfs:subClassOf dpv:Disclose ;
    sw:term_status "accepted"@en ;
    skos:definition "to give data (or a portion of it) to others"@en ;
    skos:prefLabel "Share"@en .

dpv:SingleSignOn a rdfs:Class,
        owl:Class,
        dpv:TechnicalMeasure ;
    dct:contributor "Georg P Krog, Harshvardhan J. Pandit, Paul Ryan" ;
    dct:created "2020-11-04"^^xsd:date ;
    rdfs:subClassOf dpv:AuthenticationProtocols ;
    sw:term_status "accepted"@en ;
    skos:definition "Use of credentials or processes that enable using one set of credentials to authenticate multiple contexts."@en ;
    skos:prefLabel "Single Sign On"@en .

dpv:SingularDataVolume a rdfs:Class,
        owl:Class,
        dpv:DataVolume ;
    dct:contributor "Harshvardhan J. Pandit" ;
    dct:created "2022-06-15"^^xsd:date ;
    rdfs:subClassOf dpv:DataVolume ;
    sw:term_status "accepted"@en ;
    skos:definition "Data volume that is considered singular i.e. a specific instance or single item"@en ;
    skos:prefLabel "Singular Data Volume"@en .

dpv:SingularFrequency a rdfs:Class,
        owl:Class,
        dpv:Frequency ;
    dct:contributor "Harshvardhan J. Pandit" ;
    dct:created "2022-06-15"^^xsd:date ;
    dct:modified "2020-10-05"^^xsd:date ;
    rdfs:subClassOf dpv:Frequency ;
    sw:term_status "accepted"@en ;
    skos:definition "Frequency where occurences are singular i.e. they take place only once"@en ;
    skos:prefLabel "Singular Frequency"@en .

dpv:SingularScaleOfDataSubjects a rdfs:Class,
        owl:Class,
        dpv:DataSubjectScale ;
    dct:contributor "Harshvardhan J. Pandit" ;
    dct:created "2022-06-15"^^xsd:date ;
    rdfs:subClassOf dpv:DataSubjectScale ;
    sw:term_status "accepted"@en ;
    skos:definition "Scale of data subjects considered singular i.e. a specific data subject"@en ;
    skos:prefLabel "Singular Scale Of Data Subjects"@en .

dpv:SmallDataVolume a rdfs:Class,
        owl:Class,
        dpv:DataVolume ;
    dct:contributor "Harshvardhan J. Pandit" ;
    dct:created "2022-06-15"^^xsd:date ;
    rdfs:subClassOf dpv:DataVolume ;
    sw:term_status "accepted"@en ;
    skos:definition "Data volume that is considered small or limited within the context"@en ;
    skos:prefLabel "Small Data Volume"@en .

dpv:SmallScaleOfDataSubjects a rdfs:Class,
        owl:Class,
        dpv:DataSubjectScale ;
    dct:contributor "Harshvardhan J. Pandit" ;
    dct:created "2022-06-15"^^xsd:date ;
    rdfs:subClassOf dpv:DataSubjectScale ;
    sw:term_status "accepted"@en ;
    skos:definition "Scale of data subjects considered small or limited within the context"@en ;
    skos:prefLabel "Small Scale Of Data Subjects"@en .

dpv:SmallScaleProcessing a rdfs:Class,
        owl:Class,
        dpv:ProcessingScale ;
    dct:contributor "Harshvardhan J. Pandit" ;
    dct:created "2022-09-07"^^xsd:date ;
    rdfs:subClassOf dpv:ProcessingScale ;
    sw:term_status "accepted"@en ;
    skos:definition "Processing that takes place at small scales (as specified by some criteria)"@en ;
    skos:prefLabel "Small Scale Processing"@en .

dpv:SocialMediaMarketing a rdfs:Class,
        owl:Class,
        dpv:Purpose ;
    dct:contributor "Georg P Krog, Harshvardhan J. Pandit, Beatriz Esteves" ;
    dct:created "2020-11-04"^^xsd:date ;
    rdfs:subClassOf dpv:Marketing ;
    sw:term_status "accepted"@en ;
    skos:definition "Purposes associated with conducting marketing through social media"@en ;
    skos:prefLabel "Social Media Marketing"@en .

dpv:SpecialCategoryPersonalData a rdfs:Class,
        owl:Class ;
    dct:contributor "Elmar Kiesling; Harshvardhan J. Pandit, Fajar Ekaputra" ;
    dct:created "2019-05-07"^^xsd:date ;
    dct:modified "2022-01-19"^^xsd:date ;
    dct:source "(GDPR Art.9-1, https://eur-lex.europa.eu/eli/reg/2016/679/art_9/par_1/oj)"@en ;
    vann:example dex:E0015 ;
    rdfs:subClassOf dpv:SensitivePersonalData ;
    sw:term_status "accepted"@en ;
    skos:definition "Sensitive Personal Data whose use requires specific additional legal permission or justification"@en ;
    skos:prefLabel "Special Category Personal Data"@en ;
    skos:scopeNote "The term 'special category' is based on GDPR Art.9, but should not be considered as exlusive to it. DPV considers all Special Categories to also be Sensitive, but whose use is either prohibited or regulated and therefore requires additional legal basis for justification that is separate from that for general personal data."@en .

dpv:SporadicDataVolume a rdfs:Class,
        owl:Class,
        dpv:DataVolume ;
    dct:contributor "Harshvardhan J. Pandit" ;
    dct:created "2022-06-15"^^xsd:date ;
    rdfs:subClassOf dpv:DataVolume ;
    sw:term_status "accepted"@en ;
    skos:definition "Data volume that is considered sporadic or sparse within the context"@en ;
    skos:prefLabel "Sporadic Data Volume"@en .

dpv:SporadicFrequency a rdfs:Class,
        owl:Class,
        dpv:Frequency ;
    dct:contributor "Harshvardhan J. Pandit" ;
    dct:created "2022-06-15"^^xsd:date ;
    dct:modified "2020-10-05"^^xsd:date ;
    rdfs:subClassOf dpv:Frequency ;
    sw:term_status "accepted"@en ;
    skos:definition "Frequency where occurences are sporadic or infrequent or sparse"@en ;
    skos:prefLabel "Sporadic Frequency"@en .

dpv:SporadicScaleOfDataSubjects a rdfs:Class,
        owl:Class,
        dpv:DataSubjectScale ;
    dct:contributor "Harshvardhan J. Pandit" ;
    dct:created "2022-06-15"^^xsd:date ;
    rdfs:subClassOf dpv:DataSubjectScale ;
    sw:term_status "accepted"@en ;
    skos:definition "Scale of data subjects considered sporadic or sparse within the context"@en ;
    skos:prefLabel "Sporadic Scale Of Data Subjects"@en .

dpv:StaffTraining a rdfs:Class,
        owl:Class,
        dpv:OrganisationalMeasure ;
    dct:contributor "Axel Polleres, Rob Brennan, Harshvardhan J. Pandit, Mark Lizar" ;
    dct:created "2019-04-05"^^xsd:date ;
    vann:example dex:E0017 ;
    rdfs:subClassOf dpv:OrganisationalMeasure ;
    sw:term_status "accepted"@en ;
    skos:definition "Practices and policies regarding training of staff members"@en ;
    skos:prefLabel "Staff Training"@en .

dpv:StatisticallyConfidentialData a rdfs:Class,
        owl:Class ;
    dct:source "DGA 2(20)"@en ;
    rdfs:subClassOf dpv:Data ;
    sw:term_status "accepted"@en ;
    skos:definition "Data protected through Statistical Confidentiality regulations and agreements"@en ;
    skos:prefLabel "StatisticallyConfidentialData"@en .

dpv:Status a rdfs:Class,
        owl:Class ;
    dct:contributor "Harshvardhan J. Pandit" ;
    dct:created "2022-05-18"^^xsd:date ;
    rdfs:subClassOf dpv:Context ;
    rdfs:superClassOf dpv:ActivityStatus,
        dpv:AuditStatus,
        dpv:ComplianceStatus,
        dpv:ConformanceStatus,
        dpv:ConsentStatus,
        dpv:RequestStatus ;
    sw:term_status "accepted"@en ;
    skos:definition "The status or state of something"@en ;
    skos:prefLabel "Status"@en .

dpv:StorageCondition a rdfs:Class,
        owl:Class ;
    dct:contributor "Axel Polleres, Rob Brennan, Harshvardhan J. Pandit, Mark Lizar" ;
    dct:created "2019-04-05"^^xsd:date ;
    vann:example dex:E0011 ;
    rdfs:subClassOf dpv:ProcessingCondition ;
    rdfs:superClassOf dpv:StorageDeletion,
        dpv:StorageDuration,
        dpv:StorageLocation,
        dpv:StorageRestoration ;
    sw:term_status "accepted"@en ;
    skos:definition "Conditions required or followed regarding storage of data"@en ;
    skos:prefLabel "Storage Condition"@en .

dpv:StorageDeletion a rdfs:Class,
        owl:Class ;
    dct:contributor "Axel Polleres, Rob Brennan, Harshvardhan J. Pandit, Mark Lizar" ;
    dct:created "2019-04-05"^^xsd:date ;
    rdfs:subClassOf dpv:StorageCondition ;
    sw:term_status "accepted"@en ;
    skos:definition "Deletion or Erasure of data including any deletion guarantees"@en ;
    skos:prefLabel "Storage Deletion"@en .

dpv:StorageDuration a rdfs:Class,
        owl:Class ;
    dct:contributor "Axel Polleres, Rob Brennan, Harshvardhan J. Pandit, Mark Lizar" ;
    dct:created "2019-04-05"^^xsd:date ;
    rdfs:subClassOf dpv:Duration,
        dpv:StorageCondition ;
    sw:term_status "accepted"@en ;
    skos:definition "Duration or temporal limitation on storage of data"@en ;
    skos:prefLabel "Storage Duration"@en .

dpv:StorageLocation a rdfs:Class,
        owl:Class ;
    dct:contributor "Axel Polleres, Rob Brennan, Harshvardhan J. Pandit, Mark Lizar" ;
    dct:created "2019-04-05"^^xsd:date ;
    rdfs:subClassOf dpv:Location,
        dpv:StorageCondition ;
    sw:term_status "accepted"@en ;
    skos:definition "Location or geospatial scope where the data is stored"@en ;
    skos:prefLabel "Storage Location"@en .

dpv:StorageRestoration a rdfs:Class,
        owl:Class ;
    dct:contributor "Axel Polleres, Rob Brennan, Harshvardhan J. Pandit, Mark Lizar" ;
    dct:created "2019-04-05"^^xsd:date ;
    rdfs:subClassOf dpv:StorageCondition ;
    sw:term_status "accepted"@en ;
    skos:definition "Regularity and temporal span of data restoration/backup mechanisms that guarantee that data is preserved"@en ;
    skos:prefLabel "Storage Restoration"@en .

dpv:Store a rdfs:Class,
        owl:Class,
        dpv:Processing ;
    dct:created "2019-05-07"^^xsd:date ;
    dct:source "(GDPR Art.4-2,https://eur-lex.europa.eu/eli/reg/2016/679/art_4/par_2/oj)"@en ;
    rdfs:subClassOf dpv:Processing ;
    sw:term_status "accepted"@en ;
    skos:definition "to keep data for future use"@en ;
    skos:prefLabel "Store"@en .

dpv:Structure a rdfs:Class,
        owl:Class,
        dpv:Processing ;
    dct:created "2019-05-07"^^xsd:date ;
    dct:source "(GDPR Art.4-2,https://eur-lex.europa.eu/eli/reg/2016/679/art_4/par_2/oj)"@en ;
    rdfs:subClassOf dpv:Organise ;
    sw:term_status "accepted"@en ;
    skos:definition "to arrange data according to a structure"@en ;
    skos:prefLabel "Structure"@en .

dpv:Student a rdfs:Class,
        owl:Class,
        dpv:DataSubject ;
    dct:contributor "Harshvardhan J. Pandit, Georg P. Krog, Julian Flake, Paul Ryan, Beatriz Esteves" ;
    dct:created "2022-04-06"^^xsd:date ;
    rdfs:subClassOf dpv:DataSubject ;
    sw:term_status "accepted"@en ;
    skos:definition "Data subjects that are students"@en ;
    skos:prefLabel "Student"@en .

dpv:SubProcessorAgreement a rdfs:Class,
        owl:Class,
        dpv:OrganisationalMeasure ;
    dct:contributor "Georg P Krog, Harshvardhan J. Pandit, Beatriz Esteves, Paul Ryan, Julian Flake" ;
    dct:created "2022-01-26"^^xsd:date ;
    rdfs:subClassOf dpv:DataProcessingAgreement ;
    sw:term_status "accepted"@en ;
    skos:definition "An agreement outlining conditions, criteria, obligations, responsibilities, and specifics for carrying out processing of personal data between a Data Processor and a Data (Sub-)Processor"@en ;
    skos:prefLabel "Sub-Processor Agreement"@en .

dpv:Subscriber a rdfs:Class,
        owl:Class,
        dpv:DataSubject ;
    dct:contributor "Harshvardhan J. Pandit, Georg P. Krog, Julian Flake, Paul Ryan, Beatriz Esteves" ;
    dct:created "2022-04-06"^^xsd:date ;
    rdfs:subClassOf dpv:DataSubject ;
    sw:term_status "accepted"@en ;
    skos:definition "Data subjects that subscribe to service(s)"@en ;
    skos:prefLabel "Subscriber"@en ;
    skos:scopeNote "note: subscriber can be customer or consumer"@en .

dpv:SupraNationalAuthority a rdfs:Class,
        owl:Class ;
    dct:contributor "Harshvardhan J. Pandit" ;
    dct:created "2022-02-02"^^xsd:date ;
    dct:source "(ADMS controlled vocabulary,http://purl.org/adms)"@en ;
    rdfs:subClassOf dpv:Authority ;
    sw:term_status "accepted"@en ;
    skos:definition "An authority tasked with overseeing legal compliance for a supra-national union e.g. EU"@en ;
    skos:prefLabel "Supra-National Authority"@en .

dpv:SupraNationalUnion a rdfs:Class,
        owl:Class ;
    dct:contributor "Harshvardhan J. Pandit" ;
    dct:created "2022-01-19"^^xsd:date ;
    rdfs:subClassOf dpv:Location ;
    sw:term_status "accepted"@en ;
    skos:definition "A political union of two or more countries with an establishment of common authority"@en ;
    skos:prefLabel "Supranational Union"@en .

dpv:SymmetricCryptography a rdfs:Class,
        owl:Class,
        dpv:TechnicalMeasure ;
    dct:contributor "Harshvardhan J. Pandit" ;
    dct:created "2022-08-17"^^xsd:date ;
    dct:source "(ENISA Reference Incident Classification Taxonomy 2018,https://www.enisa.europa.eu/publications/reference-incident-classification-taxonomy/)"@en ;
    rdfs:subClassOf dpv:CryptographicMethods ;
    sw:term_status "accepted"@en ;
    skos:definition "Use of cryptography where the same keys are utilised for encryption and decryption of information"@en ;
    skos:prefLabel "Symmetric Cryptography"@en .

dpv:SymmetricEncryption a rdfs:Class,
        owl:Class,
        dpv:TechnicalMeasure ;
    dct:contributor "Harshvardhan J. Pandit" ;
    dct:created "2022-08-17"^^xsd:date ;
    dct:source "(ENISA Data Pseudonymisation: Advanced Techniques and Use Cases,https://www.enisa.europa.eu/publications/data-pseudonymisation-advanced-techniques-and-use-cases)"@en ;
    rdfs:subClassOf dpv:Encryption ;
    sw:term_status "accepted"@en ;
    skos:definition "Use of symmetric cryptography to encrypt data"@en ;
    skos:prefLabel "Symmetric Encryption"@en .

dpv:SyntheticData a rdfs:Class,
        owl:Class ;
    dct:contributor "Harshvardhan J. Pandit" ;
    dct:created "2022-08-18"^^xsd:date ;
    dct:modified "2023-12-10"^^xsd:date ;
    dct:source "(ENISA Data Protection Engineering,https://www.enisa.europa.eu/publications/data-protection-engineering)"@en ;
    rdfs:subClassOf dpv:GeneratedData ;
    sw:term_status "accepted"@en ;
    skos:definition "Synthetic data reffers to artificially created data such that it is intended to resemble real data (personal or non-personal), but does not refer to any specific identified or identifiable individual, or to the real measure of an observable parameter in the case of non-personal data"@en ;
    skos:prefLabel "Synthetic Data"@en .

dpv:SystematicMonitoring a rdfs:Class,
        owl:Class,
        dpv:ProcessingContext ;
    dct:contributor "Harshvardhan J. Pandit, Piero Bonatti" ;
    dct:created "2020-11-04"^^xsd:date ;
    dct:source "(GDPR Art.4-2,https://eur-lex.europa.eu/eli/reg/2016/679/art_4/par_2/oj)"@en ;
    rdfs:subClassOf dpv:ProcessingContext ;
    sw:term_status "accepted"@en ;
    skos:definition "Processing that involves systematic monitoring of individuals"@en ;
    skos:prefLabel "Systematic Monitoring"@en .

dpv:TargetedAdvertising a rdfs:Class,
        owl:Class,
        dpv:Purpose ;
    dct:contributor "Harshvardhan J. Pandit" ;
    dct:created "2022-03-30"^^xsd:date ;
    rdfs:subClassOf dpv:PersonalisedAdvertising ;
    sw:term_status "accepted"@en ;
    skos:definition "Purposes associated with creating and providing pesonalised advertisement where the personalisation is targeted to a specific individual or group of individuals"@en ;
    skos:prefLabel "Targeted Advertising"@en .

dpv:TechnicalMeasure a rdfs:Class,
        owl:Class ;
    dct:contributor "Axel Polleres, Rob Brennan, Harshvardhan J. Pandit, Mark Lizar" ;
    dct:created "2019-04-05"^^xsd:date ;
    dct:modified "2023-12-10"^^xsd:date ;
    rdfs:subClassOf dpv:TechnicalOrganisationalMeasure ;
    sw:term_status "accepted"@en ;
    skos:definition "Technical measures used to safeguard and ensure good practices in connection with data and technologies"@en ;
    skos:prefLabel "Technical Measure"@en .

dpv:TechnicalOrganisationalMeasure a rdfs:Class,
        owl:Class ;
    dct:contributor "Bud Bruegger" ;
    dct:created "2019-04-05"^^xsd:date ;
    dct:modified "2023-12-10"^^xsd:date ;
    rdfs:superClassOf dpv:LegalMeasure,
        dpv:OrganisationalMeasure,
        dpv:PhysicalMeasure,
        dpv:RiskMitigationMeasure,
        dpv:TechnicalMeasure ;
    sw:term_status "accepted"@en ;
    skos:definition "Technical and Organisational measures used to safeguard and ensure good practices in connection with data and technologies"@en ;
    skos:prefLabel "Technical and Organisational Measure"@en .

dpv:TechnicalServiceProvision a rdfs:Class,
        owl:Class,
        dpv:Purpose ;
    dct:contributor "Harshvardhan J. Pandit" ;
    dct:created "2021-09-08"^^xsd:date ;
    rdfs:subClassOf dpv:ServiceProvision ;
    sw:term_status "accepted"@en ;
    skos:definition "Purposes associated with managing and providing technical processes and functions necessary for delivering services"@en ;
    skos:prefLabel "Technical Service Provision"@en .

dpv:Technology a rdfs:Class,
        owl:Class ;
    dct:contributor "Harshvardhan J. Pandit" ;
    dct:created "2022-01-26"^^xsd:date ;
    sw:term_status "accepted"@en ;
    skos:definition "The technology, technological implementation, or any techniques, skills, methods, and processes used or applied"@en ;
    skos:prefLabel "Technology"@en ;
    skos:scopeNote "Examples (non-exhaustive) include: Algorithm, Process, Method, Skill, Database, Cookies, Server, Device"@en .

dpv:TemporalDuration a rdfs:Class,
        owl:Class ;
    dct:contributor "Harshvardhan J. Pandit" ;
    dct:created "2022-06-15"^^xsd:date ;
    dct:modified "2020-10-05"^^xsd:date ;
    rdfs:subClassOf dpv:Duration ;
    sw:term_status "accepted"@en ;
    skos:definition "Duration that has a fixed temporal duration e.g. 6 months"@en ;
    skos:prefLabel "Temporal Duration"@en .

dpv:ThirdCountry a rdfs:Class,
        owl:Class ;
    dct:contributor "Harshvardhan J. Pandit" ;
    dct:created "2022-02-09"^^xsd:date ;
    rdfs:subClassOf dpv:Country ;
    sw:term_status "accepted"@en ;
    skos:definition "Represents a country outside applicable or compatible jurisdiction as outlined in law"@en ;
    skos:prefLabel "Third Country"@en .

dpv:ThirdParty a rdfs:Class,
        owl:Class ;
    dct:contributor "Harshvardhan J. Pandit" ;
    dct:created "2019-06-04"^^xsd:date ;
    dct:source "(GDPR Art.4-10,https://eur-lex.europa.eu/eli/reg/2016/679/art_4/par_10/oj)"@en ;
    rdfs:subClassOf dpv:Recipient ;
    sw:term_status "accepted"@en ;
    skos:definition "A ‘third party’ means a natural or legal person, public authority, agency or body other than the data subject, controller, processor and people who, under the direct authority of the controller or processor, are authorised to process personal data."@en ;
    skos:prefLabel "Third Party"@en .

dpv:ThirdPartyAgreement a rdfs:Class,
        owl:Class,
        dpv:OrganisationalMeasure ;
    dct:contributor "Harshvardhan J. Pandit" ;
    dct:created "2022-02-09"^^xsd:date ;
    rdfs:subClassOf dpv:DataProcessingAgreement ;
    sw:term_status "accepted"@en ;
    skos:definition "An agreement outlining conditions, criteria, obligations, responsibilities, and specifics for carrying out processing of personal data between a Data Controller or Processor and a Third Party"@en ;
    skos:prefLabel "Third-Party Agreement"@en .

dpv:ThirdPartyContract a rdfs:Class,
        owl:Class,
        dpv:LegalBasis ;
    dct:created "2023-12-10"^^xsd:date ;
    rdfs:subClassOf dpv:Contract ;
    sw:term_status "accepted"@en ;
    skos:definition "Creation, completion, fulfilment, or performance of a contract, with the Data Controller and Third Party as parties, and involving specified processing"@en ;
    skos:prefLabel "Third Party Contract"@en .

dpv:ThirdPartyDataSource a rdfs:Class,
        owl:Class,
        dpv:DataSource ;
    dct:created "2023-10-12"^^xsd:date ;
    rdfs:subClassOf dpv:DataSource ;
    sw:term_status "accepted"@en ;
    skos:definition "Data Sourced from a Third Party, e.g. when data is collected from an entity that is neither the Controller nor the Data Subject"@en ;
    skos:prefLabel "ThirdParty as Data Source"@en .

dpv:ThirdPartySecurityProcedures a rdfs:Class,
        owl:Class,
        dpv:OrganisationalMeasure ;
    dct:contributor "Harshvardhan J. Pandit" ;
    dct:created "2022-08-17"^^xsd:date ;
    dct:source "(ENISA 5G Cybersecurity Standards,https://www.enisa.europa.eu/publications/5g-cybersecurity-standards)"@en ;
    rdfs:subClassOf dpv:SecurityProcedure ;
    sw:term_status "accepted"@en ;
    skos:definition "Procedures related to security associated with Third Parties"@en ;
    skos:prefLabel "Third Party Security Procedures"@en .

dpv:Tourist a rdfs:Class,
        owl:Class,
        dpv:DataSubject ;
    dct:contributor "Harshvardhan J. Pandit, Georg P. Krog, Julian Flake, Paul Ryan, Beatriz Esteves" ;
    dct:created "2022-04-06"^^xsd:date ;
    rdfs:subClassOf dpv:DataSubject ;
    sw:term_status "accepted"@en ;
    skos:definition "Data subjects that are tourists i.e. not citizens and not immigrants"@en ;
    skos:prefLabel "Tourist"@en .

dpv:Transfer a rdfs:Class,
        owl:Class,
        dpv:Processing ;
    dct:created "2019-05-07"^^xsd:date ;
    dct:source "(SPECIAL Project,https://specialprivacy.ercim.eu/vocabs/processing)"@en ;
    vann:example dex:E0020 ;
    rdfs:subClassOf dpv:Processing ;
    sw:term_status "accepted"@en ;
    skos:definition "to move data from one place to another"@en ;
    skos:prefLabel "Transfer"@en ;
    skos:related "svpr:Transfer"@en .

dpv:Transform a rdfs:Class,
        owl:Class,
        dpv:Processing ;
    dct:created "2019-05-07"^^xsd:date ;
    dct:source "(GDPR Art.4-2,https://eur-lex.europa.eu/eli/reg/2016/679/art_4/par_2/oj)"@en ;
    rdfs:subClassOf dpv:Processing ;
    sw:term_status "accepted"@en ;
    skos:definition "to change the form or nature of data"@en ;
    skos:prefLabel "Transform"@en .

dpv:Transmit a rdfs:Class,
        owl:Class,
        dpv:Processing ;
    dct:created "2019-05-07"^^xsd:date ;
    dct:source "(GDPR Art.4-2,https://eur-lex.europa.eu/eli/reg/2016/679/art_4/par_2/oj)"@en ;
    rdfs:subClassOf dpv:Disclose ;
    sw:term_status "accepted"@en ;
    skos:definition "to send out data"@en ;
    skos:prefLabel "Transmit"@en .

dpv:TrustedComputing a rdfs:Class,
        owl:Class,
        dpv:TechnicalMeasure ;
    dct:contributor "Harshvardhan J. Pandit" ;
    dct:created "2022-08-17"^^xsd:date ;
    dct:source "(ENISA Reference Incident Classification Taxonomy 2018,https://www.enisa.europa.eu/publications/reference-incident-classification-taxonomy/)"@en ;
    rdfs:subClassOf dpv:CryptographicMethods ;
    sw:term_status "accepted"@en ;
    skos:definition "Use of cryptographic methods to restrict access and execution to trusted parties and code"@en ;
    skos:prefLabel "Trusted Computing"@en .

dpv:TrustedExecutionEnvironments a rdfs:Class,
        owl:Class,
        dpv:TechnicalMeasure ;
    dct:contributor "Harshvardhan J. Pandit" ;
    dct:created "2022-08-17"^^xsd:date ;
    dct:source "(ENISA Data Protection Engineering,https://www.enisa.europa.eu/publications/data-protection-engineering)"@en ;
    rdfs:subClassOf dpv:CryptographicMethods ;
    sw:term_status "accepted"@en ;
    skos:definition "Use of cryptographic methods to restrict access and execution to trusted parties and code within a dedicated execution environment"@en ;
    skos:prefLabel "Trusted Execution Environments"@en .

dpv:TrustedThirdPartyUtilisation a rdfs:Class,
        owl:Class,
        dpv:OrganisationalMeasure ;
    dct:contributor "Harshvardhan J. Pandit" ;
    dct:created "2022-08-17"^^xsd:date ;
    dct:source "(ENISA Data Pseudonymisation: Advanced Techniques and Use Cases,https://www.enisa.europa.eu/publications/data-pseudonymisation-advanced-techniques-and-use-cases)"@en ;
    rdfs:subClassOf dpv:SecurityProcedure ;
    sw:term_status "accepted"@en ;
    skos:definition "Utilisation of a trusted third party to provide or carry out a measure"@en ;
    skos:prefLabel "Trusted Third Party Utilisation"@en .

dpv:UninformedConsent a rdfs:Class,
        owl:Class,
        dpv:LegalBasis ;
    dct:contributor "Georg P Krog, Harshvardhan J. Pandit, Paul Ryan, Julian Flake" ;
    dct:created "2022-06-21"^^xsd:date ;
    rdfs:subClassOf dpv:Consent ;
    sw:term_status "accepted"@en ;
    skos:definition "Consent that is uninformed i.e. without requirement to provide sufficient information to make a consenting decision"@en ;
    skos:prefLabel "Uninformed Consent"@en .

dpv:Unlawful a rdfs:Class,
        owl:Class,
        dpv:Lawfulness ;
    dct:contributor "Harshvardhan J. Pandit" ;
    dct:created "2022-10-19"^^xsd:date ;
    rdfs:subClassOf dpv:Lawfulness ;
    sw:term_status "accepted"@en ;
    skos:definition "State of being unlawful or legally non-compliant"@en ;
    skos:prefLabel "Unlawful"@en .

dpv:UntilEventDuration a rdfs:Class,
        owl:Class ;
    dct:contributor "Harshvardhan J. Pandit" ;
    dct:created "2022-06-15"^^xsd:date ;
    dct:modified "2020-10-05"^^xsd:date ;
    rdfs:subClassOf dpv:Duration ;
    sw:term_status "accepted"@en ;
    skos:definition "Duration that takes place until a specific event occurs e.g. Account Closure"@en ;
    skos:prefLabel "Until Event Duration"@en .

dpv:UntilTimeDuration a rdfs:Class,
        owl:Class ;
    dct:contributor "Harshvardhan J. Pandit" ;
    dct:created "2022-06-15"^^xsd:date ;
    dct:modified "2020-10-05"^^xsd:date ;
    rdfs:subClassOf dpv:Duration ;
    sw:term_status "accepted"@en ;
    skos:definition "Duration that has a fixed end date e.g. 2022-12-31"@en ;
    skos:prefLabel "Until Time Duration"@en .

dpv:UnverifiedData a rdfs:Class,
        owl:Class ;
    dct:contributor "Harshvardhan J. Pandit" ;
    dct:created "2022-11-02"^^xsd:date ;
    rdfs:subClassOf dpv:Data ;
    sw:term_status "accepted"@en ;
    skos:definition "Data that has not been verified in terms of accuracy, inconsistency, or quality"@en ;
    skos:prefLabel "Unverified Data"@en .

dpv:UsageControl a rdfs:Class,
        owl:Class,
        dpv:TechnicalMeasure ;
    dct:contributor "Harshvardhan J. Pandit" ;
    dct:created "2022-08-17"^^xsd:date ;
    dct:source "(ENISA Reference Incident Classification Taxonomy 2018,https://www.enisa.europa.eu/publications/reference-incident-classification-taxonomy/)"@en ;
    rdfs:subClassOf dpv:AccessControlMethod ;
    sw:term_status "accepted"@en ;
    skos:definition "Management of usage, which is intended to be broader than access control and may cover trust, digital rights, or other relevant controls"@en ;
    skos:prefLabel "Usage Control"@en .

dpv:Use a rdfs:Class,
        owl:Class,
        dpv:Processing ;
    dct:created "2019-05-07"^^xsd:date ;
    dct:source "(GDPR Art.4-2,https://eur-lex.europa.eu/eli/reg/2016/679/art_4/par_2/oj)"@en ;
    rdfs:subClassOf dpv:Processing ;
    sw:term_status "accepted"@en ;
    skos:definition "to use data"@en ;
    skos:prefLabel "Use"@en .

dpv:UseSyntheticData a rdfs:Class,
        owl:Class,
        dpv:TechnicalMeasure ;
    dct:contributor "Harshvardhan J. Pandit" ;
    dct:created "2022-08-17"^^xsd:date ;
    dct:source "(ENISA Data Protection Engineering,https://www.enisa.europa.eu/publications/data-protection-engineering)"@en ;
    rdfs:subClassOf dpv:SecurityMethod ;
    sw:term_status "accepted"@en ;
    skos:definition "Use of synthetic data to preserve privacy, security, or other effects and side-effects"@en ;
    skos:prefLabel "Use of Synthetic Data"@en .

dpv:User a rdfs:Class,
        owl:Class,
        dpv:DataSubject ;
    dct:contributor "Harshvardhan J. Pandit, Georg P. Krog, Julian Flake, Paul Ryan, Beatriz Esteves" ;
    dct:created "2022-04-06"^^xsd:date ;
    rdfs:subClassOf dpv:DataSubject ;
    sw:term_status "accepted"@en ;
    skos:definition "Data subjects that use service(s)"@en ;
    skos:prefLabel "User"@en .

dpv:UserInterfacePersonalisation a rdfs:Class,
        owl:Class,
        dpv:Purpose ;
    dct:contributor "Harshvardhan J. Pandit, Javier Fernandez, Axel Polleres, Elmar Kiesling, Fajar Ekaputra, Simon Steyskal" ;
    dct:created "2019-04-05"^^xsd:date ;
    rdfs:subClassOf dpv:ServicePersonalisation ;
    sw:term_status "accepted"@en ;
    skos:definition "Purposes associated with personalisation of interfaces presented to the user"@en ;
    skos:prefLabel "User Interface Personalisation"@en ;
    skos:scopeNote "Examples of user-interface personalisation include changing the language to match the locale"@en .

dpv:VariableLocation a rdfs:Class,
        owl:Class,
        dpv:LocationFixture ;
    dct:contributor "Harshvardhan J. Pandit" ;
    dct:created "2022-06-15"^^xsd:date ;
    dct:modified "2020-10-05"^^xsd:date ;
    rdfs:subClassOf dpv:LocationFixture ;
    sw:term_status "accepted"@en ;
    skos:definition "Location that is known but is variable e.g. somewhere within a given area"@en ;
    skos:prefLabel "Variable Location"@en .

dpv:VendorManagement a rdfs:Class,
        owl:Class,
        dpv:Purpose ;
    dct:contributor "Paul Ryan, Georg P Krog, David Hickey, Harshvardhan J. Pandit" ;
    dct:created "2021-09-01"^^xsd:date ;
    dct:source "(Belgian DPA ROPA Template, https://www.privacycommission.be/nl/model-voor-een-register-van-de-verwerkingsactiviteiten)"@en ;
    rdfs:subClassOf dpv:Purpose ;
    sw:term_status "accepted"@en ;
    skos:definition "Purposes associated with manage orders, payment, evaluation, and prospecting related to vendors"@en ;
    skos:prefLabel "Vendor Management"@en .

dpv:VendorPayment a rdfs:Class,
        owl:Class,
        dpv:Purpose ;
    dct:contributor "Paul Ryan, Georg P Krog, David Hickey, Harshvardhan J. Pandit" ;
    dct:created "2021-09-01"^^xsd:date ;
    dct:source "(Belgian DPA ROPA Template, https://www.privacycommission.be/nl/model-voor-een-register-van-de-verwerkingsactiviteiten)"@en ;
    rdfs:subClassOf dpv:VendorManagement ;
    sw:term_status "accepted"@en ;
    skos:definition "Purposes associated with managing payment of vendors"@en ;
    skos:prefLabel "Vendor Payment"@en .

dpv:VendorRecordsManagement a rdfs:Class,
        owl:Class,
        dpv:Purpose ;
    dct:contributor "Paul Ryan, Georg P Krog, David Hickey, Harshvardhan J. Pandit" ;
    dct:created "2021-09-01"^^xsd:date ;
    dct:source "(Belgian DPA ROPA Template, https://www.privacycommission.be/nl/model-voor-een-register-van-de-verwerkingsactiviteiten)"@en ;
    rdfs:subClassOf dpv:VendorManagement ;
    sw:term_status "accepted"@en ;
    skos:definition "Purposes associated with managing records and orders related to vendors"@en ;
    skos:prefLabel "Vendor Records Management"@en .

dpv:VendorSelectionAssessment a rdfs:Class,
        owl:Class,
        dpv:Purpose ;
    dct:contributor "Paul Ryan, Georg P Krog, David Hickey, Harshvardhan J. Pandit" ;
    dct:created "2021-09-01"^^xsd:date ;
    dct:source "(Belgian DPA ROPA Template, https://www.privacycommission.be/nl/model-voor-een-register-van-de-verwerkingsactiviteiten)"@en ;
    rdfs:subClassOf dpv:VendorManagement ;
    sw:term_status "accepted"@en ;
    skos:definition "Purposes associated with managing selection, assessment, and evaluation related to vendors"@en ;
    skos:prefLabel "Vendor Selection Assessment"@en .

dpv:VerifiedData a rdfs:Class,
        owl:Class ;
    dct:contributor "Harshvardhan J. Pandit" ;
    dct:created "2022-11-02"^^xsd:date ;
    rdfs:subClassOf dpv:Data ;
    sw:term_status "accepted"@en ;
    skos:definition "Data that has been verified in terms of accuracy, consistency, or quality"@en ;
    skos:prefLabel "Verified Data"@en .

dpv:VirtualisationSecurity a rdfs:Class,
        owl:Class,
        dpv:TechnicalMeasure ;
    dct:contributor "Harshvardhan J. Pandit" ;
    dct:created "2022-08-17"^^xsd:date ;
    dct:source "(ENISA Reference Incident Classification Taxonomy 2018,https://www.enisa.europa.eu/publications/reference-incident-classification-taxonomy/)"@en ;
    rdfs:subClassOf dpv:SecurityMethod ;
    sw:term_status "accepted"@en ;
    skos:definition "Security implemented at or through virtualised environments"@en ;
    skos:prefLabel "Virtualisation Security"@en .

dpv:Visitor a rdfs:Class,
        owl:Class,
        dpv:DataSubject ;
    dct:contributor "Harshvardhan J. Pandit, Georg P. Krog, Julian Flake, Paul Ryan, Beatriz Esteves" ;
    dct:created "2022-04-06"^^xsd:date ;
    rdfs:subClassOf dpv:DataSubject ;
    sw:term_status "accepted"@en ;
    skos:definition "Data subjects that are temporary visitors"@en ;
    skos:prefLabel "Visitor"@en .

dpv:VitalInterest a rdfs:Class,
        owl:Class,
        dpv:LegalBasis ;
    dct:contributor "Harshvardhan J. Pandit" ;
    dct:created "2021-04-21"^^xsd:date ;
    rdfs:subClassOf dpv:LegalBasis ;
    sw:term_status "accepted"@en ;
    skos:definition "Processing is necessary or required to protect vital interests of a data subject or other natural person"@en ;
    skos:prefLabel "Vital Interest"@en .

dpv:VitalInterestOfDataSubject a rdfs:Class,
        owl:Class,
        dpv:LegalBasis ;
    dct:contributor "Georg P Krog, Harshvardhan J. Pandit, Paul Ryan" ;
    dct:created "2021-04-21"^^xsd:date ;
    rdfs:subClassOf dpv:VitalInterestOfNaturalPerson ;
    sw:term_status "accepted"@en ;
    skos:definition "Processing is necessary or required to protect vital interests of a data subject"@en ;
    skos:prefLabel "Vital Interest of Data Subject"@en .

dpv:VitalInterestOfNaturalPerson a rdfs:Class,
        owl:Class,
        dpv:LegalBasis ;
    dct:contributor "Georg P Krog, Harshvardhan J. Pandit, Paul Ryan" ;
    dct:created "2021-04-21"^^xsd:date ;
    rdfs:subClassOf dpv:VitalInterest ;
    sw:term_status "accepted"@en ;
    skos:definition "Processing is necessary or required to protect vital interests of a natural person"@en ;
    skos:prefLabel "Vital Interest of Natural Person"@en .

dpv:VulnerabilityTestingMethods a rdfs:Class,
        owl:Class,
        dpv:TechnicalMeasure ;
    dct:contributor "Harshvardhan J. Pandit" ;
    dct:created "2022-08-17"^^xsd:date ;
    dct:source "(ENISA Reference Incident Classification Taxonomy 2018,https://www.enisa.europa.eu/publications/reference-incident-classification-taxonomy/)"@en ;
    rdfs:subClassOf dpv:SecurityMethod ;
    sw:term_status "accepted"@en ;
    skos:definition "Methods that assess or discover vulnerabilities in a system"@en ;
    skos:prefLabel "Vulnerability Testing Methods"@en .

dpv:VulnerableDataSubject a rdfs:Class,
        owl:Class,
        dpv:DataSubject ;
    dct:contributor "Georg Krog, Paul Ryan, Harshvardhan Pandit" ;
    dct:created "2020-11-04"^^xsd:date ;
    rdfs:subClassOf dpv:DataSubject ;
    sw:term_status "accepted"@en ;
    skos:definition "Data Subjects which should be considered 'vulnerable' and therefore would require additional measures and safeguards"@en ;
    skos:prefLabel "Vulnerable Data Subject"@en ;
    skos:scopeNote "This concept denotes a Data Subject or a group are vulnerable, but not what vulnerability they possess or its context. This information can be provided additionally as comments, or as separate concepts and relations. Proposals for this are welcome."@en .

dpv:WebBrowserSecurity a rdfs:Class,
        owl:Class,
        dpv:TechnicalMeasure ;
    dct:contributor "Harshvardhan J. Pandit" ;
    dct:created "2022-08-17"^^xsd:date ;
    dct:source "(ENISA Reference Incident Classification Taxonomy 2018,https://www.enisa.europa.eu/publications/reference-incident-classification-taxonomy/)"@en ;
    rdfs:subClassOf dpv:SecurityMethod ;
    sw:term_status "accepted"@en ;
    skos:definition "Security implemented at or over web browsers"@en ;
    skos:prefLabel "WebBrowser Security"@en .

dpv:WebSecurityProtocols a rdfs:Class,
        owl:Class,
        dpv:TechnicalMeasure ;
    dct:contributor "Harshvardhan J. Pandit" ;
    dct:created "2022-08-17"^^xsd:date ;
    dct:source "(ENISA Reference Incident Classification Taxonomy 2018,https://www.enisa.europa.eu/publications/reference-incident-classification-taxonomy/)"@en ;
    rdfs:subClassOf dpv:SecurityMethod ;
    sw:term_status "accepted"@en ;
    skos:definition "Security implemented at or over web-based protocols"@en ;
    skos:prefLabel "Web Security Protocols"@en .

dpv:WirelessSecurityProtocols a rdfs:Class,
        owl:Class,
        dpv:TechnicalMeasure ;
    dct:contributor "Harshvardhan J. Pandit" ;
    dct:created "2022-08-17"^^xsd:date ;
    dct:source "(ENISA Reference Incident Classification Taxonomy 2018,https://www.enisa.europa.eu/publications/reference-incident-classification-taxonomy/)"@en ;
    rdfs:subClassOf dpv:SecurityMethod ;
    sw:term_status "accepted"@en ;
    skos:definition "Security implemented at or over wireless communication protocols"@en ;
    skos:prefLabel "Wireless Security Protocols"@en .

dpv:WithinDevice a rdfs:Class,
        owl:Class,
        dpv:Location ;
    dct:contributor "Harshvardhan J. Pandit" ;
    dct:created "2022-06-15"^^xsd:date ;
    dct:modified "2020-10-05"^^xsd:date ;
    rdfs:subClassOf dpv:LocalLocation ;
    sw:term_status "accepted"@en ;
    skos:definition "Location is local and entirely within a device, such as a smartphone"@en ;
    skos:prefLabel "Within Device"@en .

dpv:WithinPhysicalEnvironment a rdfs:Class,
        owl:Class,
        dpv:Location ;
    dct:contributor "Harshvardhan J. Pandit" ;
    dct:created "2020-10-06"^^xsd:date ;
    rdfs:subClassOf dpv:LocalLocation ;
    sw:term_status "accepted"@en ;
    skos:definition "Location is local and entirely within a physical environment, such as a room"@en ;
    skos:prefLabel "Within Physical Environment"@en .

dpv:WithinVirtualEnvironment a rdfs:Class,
        owl:Class,
        dpv:Location ;
    dct:contributor "Harshvardhan J. Pandit" ;
    dct:created "2020-10-06"^^xsd:date ;
    rdfs:subClassOf dpv:LocalLocation ;
    sw:term_status "accepted"@en ;
    skos:definition "Location is local and entirely within a virtual environment, such as a shared network directory"@en ;
    skos:prefLabel "Within Virtual Environment"@en .

dpv:ZeroKnowledgeAuthentication a rdfs:Class,
        owl:Class,
        dpv:TechnicalMeasure ;
    dct:contributor "Harshvardhan J. Pandit" ;
    dct:created "2022-08-17"^^xsd:date ;
    dct:source "(ENISA Data Protection Engineering,https://www.enisa.europa.eu/publications/data-protection-engineering)"@en ;
    rdfs:subClassOf dpv:AuthenticationProtocols,
        dpv:CryptographicMethods ;
    sw:term_status "accepted"@en ;
    skos:definition "Authentication using Zero-Knowledge proofs"@en ;
    skos:prefLabel "Zero Knowledge Authentication"@en .

dct:accessRights a rdf:Property,
        owl:ObjectProperty ;
    skos:prefLabel "dct:accessRights"@en ;
    skos:scopeNote "Specfiying constraints on access associated with Rights Exercising (e.g. User must log in) or access to provided data (e.g. access via link)"@en .

dct:format a rdf:Property,
        owl:ObjectProperty ;
    skos:prefLabel "dct:format"@en ;
    skos:scopeNote "Specifying the format of provided information, for example a CSV dataset"@en .

dct:hasPart a rdf:Property,
        owl:ObjectProperty ;
    dcam:domainIncludes dpv:RightExerciseRecord ;
    dcam:rangeIncludes dpv:RightExerciseActivity ;
    skos:prefLabel "dct:hasPart"@en ;
    skos:scopeNote "Specifying a RightExerciseRecord has RightExerciseActivity as part of its records"@en ;
    schema:domainIncludes dpv:RightExerciseRecord ;
    schema:rangeIncludes dpv:RightExerciseActivity .

dct:isPartOf a rdf:Property,
        owl:ObjectProperty ;
    dcam:domainIncludes dpv:RightExerciseActivity ;
    dcam:rangeIncludes dpv:RightExerciseRecord ;
    skos:prefLabel "dct:isPartOf"@en ;
    skos:scopeNote "Specifying a RightExerciseActivity is part of a RightExerciseRecord"@en ;
    schema:domainIncludes dpv:RightExerciseActivity ;
    schema:rangeIncludes dpv:RightExerciseRecord .

dct:valid a rdf:Property,
        owl:ObjectProperty ;
    skos:prefLabel "dct:valid"@en ;
    skos:scopeNote "Specfiying the temporal validity of an activity associated with Right Exercise. For example, limits on duration for providing or accessing provided information"@en .

foaf:page a rdf:Property,
        owl:ObjectProperty ;
    dcam:domainIncludes dpv:RightExerciseActivity ;
    skos:prefLabel "foaf:page"@en ;
    skos:scopeNote "Indicates a web page or document providing information or functionality associated with a Right Exercise"@en ;
    schema:domainIncludes dpv:RightExerciseActivity .

<https://w3id.org/dpv#dcat:Resource> dct:created "2022-11-02"^^xsd:date .

<https://w3id.org/dpv#dct:accessRights> dct:contributor "Harshvardhan J. Pandit" ;
    dct:created "2022-11-02"^^xsd:date .

<https://w3id.org/dpv#dct:format> dct:contributor "Harshvardhan J. Pandit" ;
    dct:created "2022-11-02"^^xsd:date .

<https://w3id.org/dpv#dct:hasPart> dct:contributor "Harshvardhan J. Pandit" ;
    dct:created "2022-11-02"^^xsd:date .

<https://w3id.org/dpv#dct:isPartOf> dct:contributor "Harshvardhan J. Pandit" ;
    dct:created "2022-11-02"^^xsd:date .

<https://w3id.org/dpv#dct:valid> dct:contributor "Harshvardhan J. Pandit" ;
    dct:created "2022-11-02"^^xsd:date .

<https://w3id.org/dpv#dpv:hasJustification> dct:contributor "Harshvardhan J. Pandit" ;
    dct:created "2022-11-02"^^xsd:date .

<https://w3id.org/dpv#dpv:hasRecipient> dct:contributor "Harshvardhan J. Pandit" ;
    dct:created "2022-11-02"^^xsd:date .

<https://w3id.org/dpv#dpv:hasStatus> dct:contributor "Harshvardhan J. Pandit" ;
    dct:created "2022-11-02"^^xsd:date .

<https://w3id.org/dpv#dpv:isAfter> dct:contributor "Harshvardhan J. Pandit" ;
    dct:created "2022-11-02"^^xsd:date .

<https://w3id.org/dpv#dpv:isBefore> dct:contributor "Harshvardhan J. Pandit" ;
    dct:created "2022-11-02"^^xsd:date .

<https://w3id.org/dpv#dpv:isImplementedByEntity> dct:contributor "Harshvardhan J. Pandit" ;
    dct:created "2022-11-02"^^xsd:date .

<https://w3id.org/dpv#foaf:page> dct:contributor "Harshvardhan J. Pandit" ;
    dct:created "2022-11-02"^^xsd:date .

dpv:hasAddress a rdf:Property,
        owl:ObjectProperty ;
    dcam:domainIncludes dpv:Entity ;
    dct:contributor "Harshvardhan J.Pandit, Georg P Krog, Paul Ryan, Beatriz Esteves" ;
    dct:created "2020-11-04"^^xsd:date ;
    sw:term_status "accepted"@en ;
    skos:definition "Specifies address of a legal entity such as street address or pin code"@en ;
    skos:prefLabel "has address"@en ;
    schema:domainIncludes dpv:Entity .

dpv:hasAlgorithmicLogic a rdf:Property,
        owl:ObjectProperty ;
    dcam:rangeIncludes dpv:AlgorithmicLogic ;
    dct:contributor "Georg P. Krog, Paul Ryan, Harshvardhan J. Pandit" ;
    dct:created "2020-11-04"^^xsd:date ;
    dct:modified "2022-06-15"^^xsd:date ;
    sw:term_status "accepted"@en ;
    skos:definition "Indicates the logic used in processing such as for automated decision making"@en ;
    skos:prefLabel "has algorithmic logic"@en ;
    schema:rangeIncludes dpv:AlgorithmicLogic .

dpv:hasApplicableLaw a rdf:Property,
        owl:ObjectProperty ;
    dcam:rangeIncludes dpv:Law ;
    dct:contributor "Harshvardhan J. Pandit" ;
    dct:created "2022-01-19"^^xsd:date ;
    sw:term_status "accepted"@en ;
    skos:definition "Indicates applicability of a Law"@en ;
    skos:prefLabel "has applicable law"@en ;
    schema:rangeIncludes dpv:Law .

dpv:hasAuthority a rdf:Property,
        owl:ObjectProperty ;
    dcam:rangeIncludes dpv:Authority ;
    dct:contributor "Harshvardhan J. Pandit, Georg P Krog" ;
    dct:created "2022-01-19"^^xsd:date ;
    sw:term_status "accepted"@en ;
    skos:definition "Indicates applicability of authority for a jurisdiction"@en ;
    skos:prefLabel "has authority"@en ;
    schema:rangeIncludes dpv:Authority .

dpv:hasConsentStatus a rdf:Property,
        owl:ObjectProperty ;
    dcam:rangeIncludes dpv:ConsentStatus ;
    dct:contributor "Georg P Krog, Harshvardhan J. Pandit, Paul Ryan, Julian Flake" ;
    dct:created "2022-06-21"^^xsd:date ;
    sw:term_status "accepted"@en ;
    skos:definition "Specifies the state or status of consent"@en ;
    skos:prefLabel "has consent status"@en ;
    schema:rangeIncludes dpv:ConsentStatus .

dpv:hasContact a rdf:Property,
        owl:ObjectProperty ;
    dcam:domainIncludes dpv:Entity ;
    dct:contributor "Harshvardhan J.Pandit, Georg P Krog, Paul Ryan, Beatriz Esteves" ;
    dct:created "2020-11-04"^^xsd:date ;
    sw:term_status "accepted"@en ;
    skos:definition "Specifies contact details of a legal entity such as phone  or email"@en ;
    skos:prefLabel "has contact"@en ;
    schema:domainIncludes dpv:Entity .

dpv:hasContext a rdf:Property,
        owl:ObjectProperty ;
    dcam:rangeIncludes dpv:Context ;
    dct:created "2019-04-05"^^xsd:date ;
    sw:term_status "accepted"@en ;
    skos:definition "Indicates a purpose is restricted to the specified context(s)"@en ;
    skos:prefLabel "has context"@en ;
    schema:rangeIncludes dpv:Context .

dpv:hasDataSource a rdf:Property,
        owl:ObjectProperty ;
    dcam:rangeIncludes dpv:DataSource ;
    dct:contributor "Georg P. Krog, Paul Ryan, Harshvardhan J. Pandit" ;
    dct:created "2020-11-04"^^xsd:date ;
    sw:term_status "accepted"@en ;
    skos:definition "Indicates the source or origin of data being processed"@en ;
    skos:prefLabel "has data source"@en ;
    schema:rangeIncludes dpv:DataSource .

dpv:hasDuration a rdf:Property,
        owl:ObjectProperty ;
    dcam:rangeIncludes dpv:Duration ;
    dct:contributor "Axel Polleres, Rob Brennan, Harshvardhan J. Pandit, Mark Lizar" ;
    dct:created "2019-04-05"^^xsd:date ;
    dct:source "(SPECIAL Project,https://specialprivacy.ercim.eu/)"@en ;
    sw:term_status "accepted"@en ;
    skos:definition "Indicates information about duration"@en ;
    skos:prefLabel "has duration"@en ;
    schema:rangeIncludes dpv:Duration .

dpv:hasFrequency a rdf:Property,
        owl:ObjectProperty ;
    dcam:rangeIncludes dpv:Frequency ;
    dct:contributor "Harshvardhan J. Pandit" ;
    dct:created "2022-02-16"^^xsd:date ;
    sw:term_status "accepted"@en ;
    skos:definition "Indicates the frequency with which something takes place"@en ;
    skos:prefLabel "has frequency"@en ;
    schema:rangeIncludes dpv:Frequency .

dpv:hasHumanInvolvement a rdf:Property,
        owl:ObjectProperty ;
    dcam:rangeIncludes dpv:HumanInvolvement ;
    dct:contributor "Georg P. Krog, Paul Ryan, Harshvardhan J. Pandit" ;
    dct:created "2020-11-04"^^xsd:date ;
    sw:term_status "accepted"@en ;
    skos:definition "Indicates Involvement of humans in processing such as within automated decision making process"@en ;
    skos:prefLabel "has human involvement"@en ;
    skos:scopeNote "Human involvement is also relevant to 'human in the loop'"@en ;
    schema:rangeIncludes dpv:HumanInvolvement .

dpv:hasIdentifier a rdf:Property,
        owl:ObjectProperty ;
    dct:contributor "Harshvardhan J.Pandit, Georg P Krog, Paul Ryan, Beatriz Esteves" ;
    dct:created "2020-11-25"^^xsd:date ;
    sw:term_status "accepted"@en ;
    skos:definition "Indicates an identifier associated for identification or reference"@en ;
    skos:prefLabel "has identifier"@en .

dpv:hasIndicationMethod a rdf:Property,
        owl:ObjectProperty ;
    dct:contributor "Georg P Krog, Harshvardhan J. Pandit, Paul Ryan, Julian Flake" ;
    dct:created "2022-06-21"^^xsd:date ;
    sw:term_status "accepted"@en ;
    skos:definition "Specifies the method by which an entity has indicated the specific context"@en ;
    skos:prefLabel "has indication method"@en .

dpv:hasJurisdiction a rdf:Property,
        owl:ObjectProperty ;
    dcam:rangeIncludes dpv:Location ;
    dct:contributor "Harshvardhan J. Pandit" ;
    dct:created "2022-01-19"^^xsd:date ;
    sw:term_status "accepted"@en ;
    skos:definition "Indicates applicability of specified jurisdiction"@en ;
    skos:prefLabel "has jurisdiction"@en ;
    schema:rangeIncludes dpv:Location .

dpv:hasJustification a rdf:Property,
        owl:ObjectProperty ;
    dcam:domainIncludes dpv:RightExerciseActivity ;
    dcam:rangeIncludes dpv:Justification ;
    dct:contributor "Harshvardhan J. Pandit" ;
    dct:created "2022-06-15"^^xsd:date ;
    sw:term_status "accepted"@en ;
    skos:definition "Indicates a justification for specified concept or context"@en ;
    skos:prefLabel "has justification"@en ;
    skos:scopeNote "Specifying a justification for non-fulfilment of Right Exercise"@en ;
    schema:domainIncludes dpv:RightExerciseActivity ;
    schema:rangeIncludes dpv:Justification .

dpv:hasLegalBasis a rdf:Property,
        owl:ObjectProperty ;
    dcam:rangeIncludes dpv:LegalBasis ;
    dct:contributor "Axel Polleres, Javier Fernández" ;
    dct:created "2019-04-04"^^xsd:date ;
    dct:modified "2020-11-04"^^xsd:date ;
    sw:term_status "accepted"@en ;
    skos:definition "Indicates use or applicability of a Legal Basis"@en ;
    skos:prefLabel "has legal basis"@en ;
    schema:rangeIncludes dpv:LegalBasis .

dpv:hasLikelihood a rdf:Property,
        owl:ObjectProperty ;
    dcam:rangeIncludes dpv:Likelihood ;
    dct:contributor "Harshvardhan J. Pandit, Georg P Krog, Paul Ryan, Julian Flake" ;
    dct:created "2022-07-20"^^xsd:date ;
    sw:term_status "accepted"@en ;
    skos:definition "Indicates the likelihood associated with a concept"@en ;
    skos:prefLabel "has likelihood"@en ;
    schema:rangeIncludes dpv:Likelihood .

dpv:hasName a rdf:Property,
        owl:ObjectProperty ;
    dcam:domainIncludes dpv:Entity ;
    dct:contributor "Harshvardhan J.Pandit, Georg P Krog, Paul Ryan, Beatriz Esteves" ;
    dct:created "2020-11-04"^^xsd:date ;
    sw:term_status "accepted"@en ;
    skos:definition "Specifies name of a legal entity"@en ;
    skos:prefLabel "has name"@en ;
    schema:domainIncludes dpv:Entity .

dpv:hasNonPersonalDataProcess a rdf:Property,
        owl:ObjectProperty ;
    dcam:rangeIncludes dpv:NonPersonalDataProcess ;
    dct:contributor "Harshvardhan J. Pandit" ;
    dct:created "2023-12-12"^^xsd:date ;
    sw:term_status "accepted"@en ;
    skos:definition "Indicates association with a Non-Personal Data Process"@en ;
    skos:prefLabel "has non-personal data process"@en ;
    schema:rangeIncludes dpv:NonPersonalDataProcess .

dpv:hasOutcome a rdf:Property,
        owl:ObjectProperty ;
    dct:contributor "Harshvardhan J. Pandit" ;
    dct:created "2022-05-18"^^xsd:date ;
    sw:term_status "accepted"@en ;
    skos:definition "Indicates an outcome of specified concept or context"@en ;
    skos:prefLabel "has outcome"@en .

dpv:hasPersonalDataHandling a rdf:Property,
        owl:ObjectProperty ;
    dcam:rangeIncludes dpv:PersonalDataHandling ;
    dct:contributor "Harshvardhan J. Pandit, Georg P Krog" ;
    dct:created "2022-01-19"^^xsd:date ;
    sw:term_status "accepted"@en ;
    skos:definition "Indicates association with Personal Data Handling"@en ;
    skos:prefLabel "has personal data handling"@en ;
    schema:rangeIncludes dpv:PersonalDataHandling .

dpv:hasPersonalDataProcess a rdf:Property,
        owl:ObjectProperty ;
    dcam:rangeIncludes dpv:PersonalDataProcess ;
    dct:contributor "Harshvardhan J. Pandit" ;
    dct:created "2023-12-11"^^xsd:date ;
    sw:term_status "accepted"@en ;
    skos:definition "Indicates association with a Personal Data Process"@en ;
    skos:prefLabel "has personal data process"@en ;
    schema:rangeIncludes dpv:PersonalDataProcess .

dpv:hasProcess a rdf:Property,
        owl:ObjectProperty ;
    dcam:rangeIncludes dpv:Process ;
    dct:contributor "Harshvardhan J. Pandit" ;
    dct:created "2023-12-10"^^xsd:date ;
    sw:term_status "accepted"@en ;
    skos:definition "Indicates association with a Process"@en ;
    skos:prefLabel "has process"@en ;
    schema:rangeIncludes dpv:Process .

dpv:hasProcessing a rdf:Property,
        owl:ObjectProperty ;
    dcam:rangeIncludes dpv:Processing ;
    dct:contributor "Axel Polleres, Javier Fernández, Harshvardhan J. Pandit, Mark Lizar, Bud Bruegger" ;
    dct:created "2019-04-04"^^xsd:date ;
    dct:modified "2020-11-04"^^xsd:date ;
    dct:source "(SPECIAL Project,https://specialprivacy.ercim.eu/)"@en ;
    sw:term_status "accepted"@en ;
    skos:definition "Indicates association with Processing"@en ;
    skos:prefLabel "has processing"@en ;
    schema:rangeIncludes dpv:Processing .

dpv:hasProcessingAutomation a rdf:Property,
        owl:ObjectProperty ;
    dcam:rangeIncludes dpv:AutomationOfProcessing ;
    dct:contributor "Harshvardhan J. Pandit" ;
    dct:created "2022-08-13"^^xsd:date ;
    sw:term_status "accepted"@en ;
    skos:definition "Indicates the use or extent of automation associated with processing"@en ;
    skos:prefLabel "has processing automation"@en ;
    schema:rangeIncludes dpv:AutomationOfProcessing .

dpv:hasPurpose a rdf:Property,
        owl:ObjectProperty ;
    dcam:rangeIncludes dpv:Purpose ;
    dct:contributor "Axel Polleres, Javier Fernández, Harshvardhan J. Pandit, Mark Lizar, Bud Bruegger" ;
    dct:created "2019-04-04"^^xsd:date ;
    dct:modified "2020-11-04"^^xsd:date ;
    dct:source "(SPECIAL Project,https://specialprivacy.ercim.eu/)"@en ;
    sw:term_status "accepted"@en ;
    skos:definition "Indicates association with Purpose"@en ;
    skos:prefLabel "has purpose"@en ;
    schema:rangeIncludes dpv:Purpose .

dpv:hasResidualRisk a rdf:Property,
        owl:ObjectProperty ;
    dcam:domainIncludes dpv:Risk ;
    dcam:rangeIncludes dpv:Risk ;
    dct:contributor "Harshvardhan J. Pandit, Georg P Krog, Paul Ryan, Julian Flake" ;
    dct:created "2022-07-20"^^xsd:date ;
    sw:term_status "accepted"@en ;
    skos:definition "Indicates the associated risk is the remaining or residual risk from applying mitigation measures or treatments to this risk"@en ;
    skos:prefLabel "has residual risk"@en ;
    schema:domainIncludes dpv:Risk ;
    schema:rangeIncludes dpv:Risk .

dpv:hasRight a rdf:Property,
        owl:ObjectProperty ;
    dcam:rangeIncludes dpv:Right ;
    dct:contributor "Harshvardhan J. Pandit" ;
    dct:created "2020-11-18"^^xsd:date ;
    sw:term_status "accepted"@en ;
    skos:definition "Indicates use or applicability of Right"@en ;
    skos:prefLabel "has right"@en ;
    schema:rangeIncludes dpv:Right .

dpv:hasRisk a rdf:Property,
        owl:ObjectProperty ;
    dcam:rangeIncludes dpv:Risk ;
    dct:contributor "Harshvardhan J. Pandit" ;
    dct:created "2020-11-18"^^xsd:date ;
    sw:term_status "accepted"@en ;
    skos:definition "Indicates applicability of Risk for this concept"@en ;
    skos:prefLabel "has risk"@en ;
    schema:rangeIncludes dpv:Risk .

dpv:hasRiskLevel a rdf:Property,
        owl:ObjectProperty ;
    dcam:domainIncludes dpv:Risk ;
    dcam:rangeIncludes dpv:RiskLevel ;
    dct:contributor "Harshvardhan J. Pandit, Georg P Krog, Paul Ryan, Julian Flake" ;
    dct:created "2022-07-20"^^xsd:date ;
    sw:term_status "accepted"@en ;
    skos:definition "Indicates the associated risk level associated with a risk"@en ;
    skos:prefLabel "has risk level"@en ;
    schema:domainIncludes dpv:Risk ;
    schema:rangeIncludes dpv:RiskLevel .

dpv:hasScope a rdf:Property,
        owl:ObjectProperty ;
    dcam:rangeIncludes dpv:Scope ;
    dct:contributor "Harshvardhan J. Pandit" ;
    dct:created "2022-06-15"^^xsd:date ;
    sw:term_status "accepted"@en ;
    skos:definition "Indicates the scope of specified concept or context"@en ;
    skos:prefLabel "has scope"@en ;
    schema:rangeIncludes dpv:Scope .

dpv:hasSector a rdf:Property,
        owl:ObjectProperty ;
    dcam:rangeIncludes dpv:Sector ;
    dct:created "2019-04-05"^^xsd:date ;
    sw:term_status "accepted"@en ;
    skos:definition "Indicates the purpose is associated with activities in the indicated (Economic) Sector(s)"@en ;
    skos:prefLabel "has sector"@en ;
    schema:rangeIncludes dpv:Sector .

dpv:hasSeverity a rdf:Property,
        owl:ObjectProperty ;
    dcam:rangeIncludes dpv:Severity ;
    dct:contributor "Harshvardhan J. Pandit, Georg P Krog, Paul Ryan, Julian Flake" ;
    dct:created "2022-07-20"^^xsd:date ;
    sw:term_status "accepted"@en ;
    skos:definition "Indicates the severity associated with a concept"@en ;
    skos:prefLabel "has severity"@en ;
    schema:rangeIncludes dpv:Severity .

dpv:hasStorageCondition a rdf:Property,
        owl:ObjectProperty ;
    dcam:rangeIncludes dpv:StorageCondition ;
    dct:contributor "Axel Polleres, Rob Brennan, Harshvardhan J. Pandit, Mark Lizar" ;
    dct:created "2022-08-13"^^xsd:date ;
    dct:source "(SPECIAL Project,https://specialprivacy.ercim.eu/)"@en ;
    sw:term_status "accepted"@en ;
    skos:definition "Indicates information about storage condition"@en ;
    skos:prefLabel "has storage condition"@en ;
    schema:rangeIncludes dpv:StorageCondition .

dpv:isAfter a rdf:Property,
        owl:ObjectProperty ;
    dcam:domainIncludes dpv:RightExerciseActivity ;
    dcam:rangeIncludes dpv:RightExerciseActivity ;
    dct:contributor "Georg P. Krog, Harshvardhan J. Pandit, Julian Flake" ;
    dct:created "2022-03-02"^^xsd:date ;
    sw:term_status "accepted"@en ;
    skos:definition "Indicates the specified concepts is 'after' this concept in some context"@en ;
    skos:prefLabel "is after"@en ;
    skos:scopeNote "Specifying a RightExerciseActivity occurs before another RightExerciseActivity"@en ;
    schema:domainIncludes dpv:RightExerciseActivity ;
    schema:rangeIncludes dpv:RightExerciseActivity .

dpv:isAuthorityFor a rdf:Property,
        owl:ObjectProperty ;
    dcam:domainIncludes dpv:Authority ;
    dct:contributor "Harshvardhan J. Pandit, Georg P Krog" ;
    dct:created "2022-01-19"^^xsd:date ;
    sw:term_status "accepted"@en ;
    skos:definition "Indicates area, scope, or applicability of an Authority"@en ;
    skos:prefLabel "is authority for"@en ;
    schema:domainIncludes dpv:Authority .

dpv:isBefore a rdf:Property,
        owl:ObjectProperty ;
    dcam:domainIncludes dpv:RightExerciseActivity ;
    dcam:rangeIncludes dpv:RightExerciseActivity ;
    dct:contributor "Georg P. Krog, Harshvardhan J. Pandit, Julian Flake" ;
    dct:created "2022-03-02"^^xsd:date ;
    sw:term_status "accepted"@en ;
    skos:definition "Indicates the specified concepts is 'before' this concept in some context"@en ;
    skos:prefLabel "is before"@en ;
    skos:scopeNote "Specifying a RightExerciseActivity occurs before another RightExerciseActivity"@en ;
    schema:domainIncludes dpv:RightExerciseActivity ;
    schema:rangeIncludes dpv:RightExerciseActivity .

dpv:isExercisedAt a rdf:Property,
        owl:ObjectProperty ;
    dcam:domainIncludes dpv:ActiveRight ;
    dcam:rangeIncludes dpv:RightExerciseNotice ;
    dct:contributor "Harshvardhan J. Pandit" ;
    dct:created "2022-10-22"^^xsd:date ;
    sw:term_status "accepted"@en ;
    skos:definition "Indicates context or information about exercising a right"@en ;
    skos:prefLabel "is exercised at"@en ;
    schema:domainIncludes dpv:ActiveRight ;
    schema:rangeIncludes dpv:RightExerciseNotice .

dpv:isImplementedByEntity a rdf:Property,
        owl:ObjectProperty ;
    dcam:domainIncludes dpv:RightExerciseActivity ;
    dcam:rangeIncludes dpv:Entity ;
    dct:contributor "Axel Polleres, Harshvardhan J. Pandit, Beatriz Esteves, Paul Ryan, Julian Flake" ;
    dct:created "2019-05-07"^^xsd:date ;
    dct:modified "2022-01-26"^^xsd:date ;
    sw:term_status "accepted"@en ;
    skos:definition "Indicates implementation details such as entities or agents"@en ;
    skos:prefLabel "is implemented by entity"@en ;
    skos:scopeNote "Indicates the Entity that implements or performs a Right Exercise Activity"@en,
        "The use of 'entity' is inclusive of entities (e.g. Data Processor) as well as 'agent' (e.g. DPO). For indicating technological implementation, the property isImplementedByTechnology should be used."@en ;
    schema:domainIncludes dpv:RightExerciseActivity ;
    schema:rangeIncludes dpv:Entity .

dpv:isImplementedUsingTechnology a rdf:Property,
        owl:ObjectProperty ;
    dcam:rangeIncludes dpv:Technology ;
    dct:contributor "Beatriz Esteves, Harshvardhan J. Pandit, Paul Ryan, Julian Flake" ;
    dct:created "2022-01-26"^^xsd:date ;
    dct:modified "2022-06-15"^^xsd:date ;
    sw:term_status "accepted"@en ;
    skos:definition "Indicates implementation details such as technologies or processes"@en ;
    skos:prefLabel "is implemented using technology"@en ;
    skos:scopeNote "The term 'technology' is inclusive of technologies, processes, and methods."@en ;
    schema:rangeIncludes dpv:Technology .

dpv:isIndicatedAtTime a rdf:Property,
        owl:ObjectProperty ;
    dct:contributor "Georg P Krog, Harshvardhan J. Pandit, Paul Ryan, Julian Flake" ;
    dct:created "2022-06-21"^^xsd:date ;
    sw:term_status "accepted"@en ;
    skos:definition "Specifies the temporal information for when the entity has indicated the specific context"@en ;
    skos:prefLabel "is indicated at time"@en .

dpv:isIndicatedBy a rdf:Property,
        owl:ObjectProperty ;
    dcam:rangeIncludes dpv:Entity ;
    dct:contributor "Georg P Krog, Harshvardhan J. Pandit, Paul Ryan, Julian Flake" ;
    dct:created "2022-06-21"^^xsd:date ;
    sw:term_status "accepted"@en ;
    skos:definition "Specifies entity who indicates the specific context"@en ;
    skos:prefLabel "is indicated by"@en ;
    schema:rangeIncludes dpv:Entity .

dpv:isPolicyFor a rdf:Property,
        owl:ObjectProperty ;
    dcam:domainIncludes dpv:Policy ;
    dct:contributor "Harshvardhan J. Pandit" ;
    dct:created "2022-01-26"^^xsd:date ;
    sw:term_status "accepted"@en ;
    skos:definition "Indicates the context or application of policy"@en ;
    skos:prefLabel "is policy for"@en ;
    schema:domainIncludes dpv:Policy .

dpv:isResidualRiskOf a rdf:Property,
        owl:ObjectProperty ;
    dcam:domainIncludes dpv:Risk ;
    dcam:rangeIncludes dpv:Risk ;
    dct:contributor "Harshvardhan J. Pandit, Georg P Krog, Paul Ryan, Julian Flake" ;
    dct:created "2022-07-20"^^xsd:date ;
    sw:term_status "accepted"@en ;
    skos:definition "Indicates this risk is the remaining or residual risk from applying mitigation measures or treatments to specified risk"@en ;
    skos:prefLabel "is residual risk of"@en ;
    schema:domainIncludes dpv:Risk ;
    schema:rangeIncludes dpv:Risk .

dpv:mitigatesRisk a rdf:Property,
        owl:ObjectProperty ;
    dcam:domainIncludes dpv:RiskMitigationMeasure ;
    dcam:rangeIncludes dpv:Risk ;
    dct:contributor "Harshvardhan J. Pandit" ;
    dct:created "2020-11-04"^^xsd:date ;
    sw:term_status "accepted"@en ;
    skos:definition "Indicates risks mitigated by this concept"@en ;
    skos:prefLabel "mitigates risk"@en ;
    schema:domainIncludes dpv:RiskMitigationMeasure ;
    schema:rangeIncludes dpv:Risk .

dpv:hasActivityStatus a rdf:Property,
        owl:ObjectProperty ;
    dcam:rangeIncludes dpv:ActivityStatus ;
    dct:contributor "Harshvardhan J. Pandit" ;
    dct:created "2022-05-18"^^xsd:date ;
    rdfs:subClassOf dpv:hasStatus ;
    rdfs:subPropertyOf dpv:hasStatus ;
    sw:term_status "accepted"@en ;
    skos:definition "Indicates the status of activity of specified concept"@en ;
    skos:prefLabel "has activity status"@en ;
    schema:rangeIncludes dpv:ActivityStatus .

dpv:hasAuditStatus a rdf:Property,
        owl:ObjectProperty ;
    dcam:rangeIncludes dpv:AuditStatus ;
    dct:contributor "Harshvardhan J. Pandit" ;
    dct:created "2022-06-22"^^xsd:date ;
    rdfs:subClassOf dpv:hasStatus ;
    rdfs:subPropertyOf dpv:hasStatus ;
    sw:term_status "accepted"@en ;
    skos:definition "Indicates the status of audit associated with specified concept"@en ;
    skos:prefLabel "has audit status"@en ;
    schema:rangeIncludes dpv:AuditStatus .

dpv:hasDataExporter a rdf:Property,
        owl:ObjectProperty ;
    dcam:rangeIncludes dpv:DataExporter ;
    dct:contributor "Paul Ryan, Georg P. Krog, Harshvardhan J. Pandit" ;
    dct:created "2022-02-09"^^xsd:date ;
    rdfs:subClassOf dpv:hasEntity ;
    rdfs:subPropertyOf dpv:hasEntity ;
    sw:term_status "accepted"@en ;
    skos:definition "Indiciates inclusion or applicability of a LegalEntity in the role of Data Exporter"@en ;
    skos:prefLabel "has data exporter"@en ;
    schema:rangeIncludes dpv:DataExporter .

dpv:hasDataImporter a rdf:Property,
        owl:ObjectProperty ;
    dcam:rangeIncludes dpv:DataImporter ;
    dct:contributor "Paul Ryan, Georg P. Krog, Harshvardhan J. Pandit" ;
    dct:created "2022-02-09"^^xsd:date ;
    rdfs:subClassOf dpv:hasRecipient ;
    rdfs:subPropertyOf dpv:hasRecipient ;
    sw:term_status "accepted"@en ;
    skos:definition "Indiciates inclusion or applicability of a LegalEntity in the role of Data Importer"@en ;
    skos:prefLabel "has data importer"@en ;
    schema:rangeIncludes dpv:DataImporter .

dpv:hasDataProcessor a rdf:Property,
        owl:ObjectProperty ;
    dcam:rangeIncludes dpv:DataProcessor ;
    dct:contributor "Paul Ryan, Georg P. Krog, Harshvardhan J. Pandit" ;
    dct:created "2022-02-09"^^xsd:date ;
    rdfs:subClassOf dpv:hasRecipient ;
    rdfs:subPropertyOf dpv:hasRecipient ;
    sw:term_status "accepted"@en ;
    skos:definition "Indiciates inclusion or applicability of a Data Processor"@en ;
    skos:prefLabel "has data processor"@en ;
    schema:rangeIncludes dpv:DataProcessor .

dpv:hasDataProtectionOfficer a rdf:Property,
        owl:ObjectProperty ;
    dcam:rangeIncludes dpv:DataProtectionOfficer ;
    dct:contributor "Paul Ryan, Rob Brennan" ;
    dct:created "2022-03-02"^^xsd:date ;
    rdfs:subClassOf dpv:hasRepresentative ;
    rdfs:subPropertyOf dpv:hasRepresentative ;
    sw:term_status "accepted"@en ;
    skos:definition "Specifices an associated data protection officer"@en ;
    skos:prefLabel "has data protection officer"@en ;
    schema:rangeIncludes dpv:DataProtectionOfficer .

dpv:hasDataSubject a rdf:Property,
        owl:ObjectProperty ;
    dcam:rangeIncludes dpv:DataSubject ;
    dct:contributor "Axel Polleres, Javier Fernández, Harshvardhan J. Pandit, Mark Lizar, Bud Bruegger" ;
    dct:created "2019-04-04"^^xsd:date ;
    dct:modified "2020-11-04"^^xsd:date ;
    rdfs:subClassOf dpv:hasEntity ;
    rdfs:subPropertyOf dpv:hasEntity ;
    sw:term_status "accepted"@en ;
    skos:definition "Indicates association with Data Subject"@en ;
    skos:prefLabel "has data subject"@en ;
    schema:rangeIncludes dpv:DataSubject .

dpv:hasDataSubjectScale a rdf:Property,
        owl:ObjectProperty ;
    dcam:rangeIncludes dpv:DataSubjectScale ;
    dct:contributor "Harshvardhan J. Pandit" ;
    dct:created "2022-06-22"^^xsd:date ;
    rdfs:subClassOf dpv:hasScale ;
    rdfs:subPropertyOf dpv:hasScale ;
    sw:term_status "accepted"@en ;
    skos:definition "Indicates the scale of data subjects"@en ;
    skos:prefLabel "has data subject scale"@en ;
    schema:rangeIncludes dpv:DataSubjectScale .

dpv:hasDataVolume a rdf:Property,
        owl:ObjectProperty ;
    dcam:rangeIncludes dpv:DataVolume ;
    dct:contributor "Harshvardhan J. Pandit" ;
    dct:created "2022-06-22"^^xsd:date ;
    rdfs:subClassOf dpv:hasScale ;
    rdfs:subPropertyOf dpv:hasScale ;
    sw:term_status "accepted"@en ;
    skos:definition "Indicates the volume of data"@en ;
    skos:prefLabel "has data volume"@en ;
    schema:rangeIncludes dpv:DataVolume .

dpv:hasGeographicCoverage a rdf:Property,
        owl:ObjectProperty ;
    dcam:rangeIncludes dpv:GeographicCoverage ;
    dct:contributor "Harshvardhan J. Pandit" ;
    dct:created "2022-06-22"^^xsd:date ;
    rdfs:subClassOf dpv:hasScale ;
    rdfs:subPropertyOf dpv:hasScale ;
    sw:term_status "accepted"@en ;
    skos:definition "Indicate the geographic coverage (of specified context)"@en ;
    skos:prefLabel "has geographic coverage"@en ;
    schema:rangeIncludes dpv:GeographicCoverage .

dpv:hasImpact a rdf:Property,
        owl:ObjectProperty ;
    dcam:rangeIncludes dpv:Impact ;
    dct:contributor "Harshvardhan J. Pandit, Julian Flake, Georg P Krog, Fajar Ekaputra, Beatriz Esteves" ;
    dct:created "2022-05-18"^^xsd:date ;
    rdfs:subClassOf dpv:hasConsequence ;
    rdfs:subPropertyOf dpv:hasConsequence ;
    sw:term_status "accepted"@en ;
    skos:definition "Indicates impact(s) possible or arising as consequences from specified concept"@en ;
    skos:prefLabel "has impact"@en ;
    schema:rangeIncludes dpv:Impact .

dpv:hasImpactOn a rdf:Property,
        owl:ObjectProperty ;
    dcam:domainIncludes dpv:Impact ;
    dct:contributor "Harshvardhan J. Pandit, Julian Flake, Georg P Krog, Fajar Ekaputra, Beatriz Esteves" ;
    dct:created "2022-05-18"^^xsd:date ;
    rdfs:subClassOf dpv:hasConsequenceOn ;
    rdfs:subPropertyOf dpv:hasConsequenceOn ;
    sw:term_status "accepted"@en ;
    skos:definition "Indicates the thing (e.g. plan, process, or entity) affected by an impact"@en ;
    skos:prefLabel "has impact on"@en ;
    schema:domainIncludes dpv:Impact .

dpv:hasJointDataControllers a rdf:Property,
        owl:ObjectProperty ;
    dcam:rangeIncludes dpv:JointDataControllers ;
    dct:contributor "Paul Ryan, Georg P. Krog, Harshvardhan J. Pandit" ;
    dct:created "2022-02-09"^^xsd:date ;
    rdfs:subClassOf dpv:hasDataController ;
    rdfs:subPropertyOf dpv:hasDataController ;
    sw:term_status "accepted"@en ;
    skos:definition "Indicates inclusion or applicability of a Joint Data Controller"@en ;
    skos:prefLabel "has joint data controllers"@en ;
    schema:rangeIncludes dpv:JointDataControllers .

dpv:hasLawfulness a rdf:Property,
        owl:ObjectProperty ;
    dcam:rangeIncludes dpv:Lawfulness ;
    dct:contributor "Harshvardhan J. Pandit" ;
    dct:created "2022-10-22"^^xsd:date ;
    rdfs:subClassOf dpv:hasComplianceStatus ;
    rdfs:subPropertyOf dpv:hasComplianceStatus ;
    sw:term_status "accepted"@en ;
    skos:definition "Indicates the status of being lawful or legally compliant"@en ;
    skos:prefLabel "has lawfulness"@en ;
    schema:rangeIncludes dpv:Lawfulness .

dpv:hasLegalMeasure a rdf:Property,
        owl:ObjectProperty ;
    dcam:rangeIncludes dpv:LegalMeasure ;
    dct:created "2023-12-10"^^xsd:date ;
    rdfs:subClassOf dpv:hasOrganisationalMeasure ;
    rdfs:subPropertyOf dpv:hasOrganisationalMeasure ;
    sw:term_status "accepted"@en ;
    skos:definition "Indicates use or applicability of Legal measure"@en ;
    skos:prefLabel "has legal measure"@en ;
    schema:rangeIncludes dpv:LegalMeasure .

dpv:hasNotice a rdf:Property,
        owl:ObjectProperty ;
    dcam:rangeIncludes dpv:Notice ;
    dct:contributor "Georg P Krog, Harshvardhan J. Pandit, Paul Ryan, Julian Flake" ;
    dct:created "2022-06-22"^^xsd:date ;
    rdfs:subClassOf dpv:hasOrganisationalMeasure ;
    rdfs:subPropertyOf dpv:hasOrganisationalMeasure ;
    sw:term_status "accepted"@en ;
    skos:definition "Indicates the use or applicability of a Notice for the specified context"@en ;
    skos:prefLabel "has notice"@en ;
    schema:rangeIncludes dpv:Notice .

dpv:hasObligation a rdf:Property,
        owl:ObjectProperty ;
    dcam:domainIncludes dpv:Context ;
    dcam:rangeIncludes dpv:Obligation ;
    dct:contributor "Harshvardhan J. Pandit, Georg P Krog, Beatriz Esteves, Paul Ryan" ;
    dct:created "2022-10-19"^^xsd:date ;
    rdfs:subClassOf dpv:hasRule ;
    rdfs:subPropertyOf dpv:hasRule ;
    sw:term_status "accepted"@en ;
    skos:definition "Specifying applicability or inclusion of an obligation rule within specified context"@en ;
    skos:prefLabel "has obligation"@en ;
    schema:domainIncludes dpv:Context ;
    schema:rangeIncludes dpv:Obligation .

dpv:hasPermission a rdf:Property,
        owl:ObjectProperty ;
    dcam:domainIncludes dpv:Context ;
    dcam:rangeIncludes dpv:Permission ;
    dct:contributor "Harshvardhan J. Pandit, Georg P Krog, Beatriz Esteves, Paul Ryan" ;
    dct:created "2022-10-19"^^xsd:date ;
    rdfs:subClassOf dpv:hasRule ;
    rdfs:subPropertyOf dpv:hasRule ;
    sw:term_status "accepted"@en ;
    skos:definition "Specifying applicability or inclusion of a permission rule within specified context"@en ;
    skos:prefLabel "has permission"@en ;
    schema:domainIncludes dpv:Context ;
    schema:rangeIncludes dpv:Permission .

dpv:hasPersonalData a rdf:Property,
        owl:ObjectProperty ;
    dcam:rangeIncludes dpv:PersonalData ;
    dct:contributor "Harshvardhan J. Pandit" ;
    dct:created "2022-01-19"^^xsd:date ;
    rdfs:subClassOf dpv:hasData ;
    rdfs:subPropertyOf dpv:hasData ;
    sw:term_status "accepted"@en ;
    skos:definition "Indicates association with Personal Data"@en ;
    skos:prefLabel "has personal data"@en ;
    schema:rangeIncludes dpv:PersonalData .

dpv:hasPhysicalMeasure a rdf:Property,
        owl:ObjectProperty ;
    dcam:rangeIncludes dpv:PhysicalMeasure ;
    dct:created "2023-12-10"^^xsd:date ;
    rdfs:subClassOf dpv:hasTechnicalOrganisationalMeasure ;
    rdfs:subPropertyOf dpv:hasTechnicalOrganisationalMeasure ;
    sw:term_status "accepted"@en ;
    skos:definition "Indicates use or applicability of Physical measure"@en ;
    skos:prefLabel "has physical measure"@en ;
    schema:rangeIncludes dpv:PhysicalMeasure .

dpv:hasPolicy a rdf:Property,
        owl:ObjectProperty ;
    dcam:rangeIncludes dpv:Policy ;
    dct:contributor "Harshvardhan J. Pandit" ;
    dct:created "2022-01-26"^^xsd:date ;
    rdfs:subClassOf dpv:hasTechnicalOrganisationalMeasure ;
    rdfs:subPropertyOf dpv:hasTechnicalOrganisationalMeasure ;
    sw:term_status "accepted"@en ;
    skos:definition "Indicates policy applicable or used"@en ;
    skos:prefLabel "has policy"@en ;
    schema:rangeIncludes dpv:Policy .

dpv:hasProhibition a rdf:Property,
        owl:ObjectProperty ;
    dcam:domainIncludes dpv:Context ;
    dcam:rangeIncludes dpv:Prohibition ;
    dct:contributor "Harshvardhan J. Pandit, Georg P Krog, Beatriz Esteves, Paul Ryan" ;
    dct:created "2022-10-19"^^xsd:date ;
    rdfs:subClassOf dpv:hasRule ;
    rdfs:subPropertyOf dpv:hasRule ;
    sw:term_status "accepted"@en ;
    skos:definition "Specifying applicability or inclusion of a prohibition rule within specified context"@en ;
    skos:prefLabel "has prohibition"@en ;
    schema:domainIncludes dpv:Context ;
    schema:rangeIncludes dpv:Prohibition .

dpv:hasRecipientDataController a rdf:Property,
        owl:ObjectProperty ;
    dcam:rangeIncludes dpv:DataController ;
    dct:contributor "Paul Ryan, Georg P. Krog, Harshvardhan J. Pandit" ;
    dct:created "2022-02-09"^^xsd:date ;
    rdfs:subClassOf dpv:hasRecipient ;
    rdfs:subPropertyOf dpv:hasRecipient ;
    sw:term_status "accepted"@en ;
    skos:definition "Indiciates inclusion or applicability of a Data Controller as a Recipient of persona data"@en ;
    skos:prefLabel "has recipient data controller"@en ;
    schema:rangeIncludes dpv:DataController .

dpv:hasRecipientThirdParty a rdf:Property,
        owl:ObjectProperty ;
    dcam:rangeIncludes dpv:ThirdParty ;
    dct:contributor "Paul Ryan, Georg P. Krog, Harshvardhan J. Pandit" ;
    dct:created "2022-02-09"^^xsd:date ;
    rdfs:subClassOf dpv:hasRecipient ;
    rdfs:subPropertyOf dpv:hasRecipient ;
    sw:term_status "accepted"@en ;
    skos:definition "Indiciates inclusion or applicability of a Third Party as a Recipient of persona data"@en ;
    skos:prefLabel "has recipient third party"@en ;
    schema:rangeIncludes dpv:ThirdParty .

dpv:hasRelationWithDataSubject a rdf:Property,
        owl:ObjectProperty ;
    dcam:domainIncludes dpv:Entity ;
    dct:contributor "Georg P Krog, Harshvardhan J. Pandit, Paul Ryan, Julian Flake" ;
    dct:created "2022-06-21"^^xsd:date ;
    rdfs:subClassOf dpv:hasEntity ;
    rdfs:subPropertyOf dpv:hasEntity ;
    sw:term_status "accepted"@en ;
    skos:definition "Indicates the relation between specified Entity and Data Subject"@en ;
    skos:prefLabel "has relation with data subject"@en ;
    schema:domainIncludes dpv:Entity .

dpv:hasResponsibleEntity a rdf:Property,
        owl:ObjectProperty ;
    dcam:rangeIncludes dpv:Entity ;
    dct:contributor "Harshvardhan J. Pandit" ;
    dct:created "2022-03-02"^^xsd:date ;
    rdfs:subClassOf dpv:hasEntity ;
    rdfs:subPropertyOf dpv:hasEntity ;
    sw:term_status "accepted"@en ;
    skos:definition "Specifies the indicated entity is responsible within some context"@en ;
    skos:prefLabel "has responsible entity"@en ;
    schema:rangeIncludes dpv:Entity .

dpv:hasTechnicalMeasure a rdf:Property,
        owl:ObjectProperty ;
    dcam:rangeIncludes dpv:TechnicalMeasure ;
    dct:contributor "Harshvardhan J. Pandit" ;
    dct:created "2022-02-09"^^xsd:date ;
    rdfs:subClassOf dpv:hasTechnicalOrganisationalMeasure ;
    rdfs:subPropertyOf dpv:hasTechnicalOrganisationalMeasure ;
    sw:term_status "accepted"@en ;
    skos:definition "Indicates use or applicability of Technical measure"@en ;
    skos:prefLabel "has technical measure"@en ;
    schema:rangeIncludes dpv:TechnicalMeasure .

dpv:hasThirdCountry a rdf:Property,
        owl:ObjectProperty ;
    dcam:rangeIncludes dpv:ThirdCountry ;
    dct:contributor "Harshvardhan J. Pandit, Georg P Krog" ;
    dct:created "2022-02-09"^^xsd:date ;
    rdfs:subClassOf dpv:hasCountry ;
    rdfs:subPropertyOf dpv:hasCountry ;
    sw:term_status "accepted"@en ;
    skos:definition "Indicates applicability or relevance of a 'third country'"@en ;
    skos:prefLabel "has third country"@en ;
    schema:rangeIncludes dpv:ThirdCountry .

dpv:isMitigatedByMeasure a rdf:Property,
        owl:ObjectProperty ;
    dcam:domainIncludes dpv:Risk ;
    dcam:rangeIncludes dpv:RiskMitigationMeasure ;
    dct:contributor "Harshvardhan J. Pandit" ;
    dct:created "2022-02-09"^^xsd:date ;
    rdfs:subClassOf dpv:hasTechnicalOrganisationalMeasure ;
    rdfs:subPropertyOf dpv:hasTechnicalOrganisationalMeasure ;
    sw:term_status "accepted"@en ;
    skos:definition "Indicate a risk is mitigated by specified measure"@en ;
    skos:prefLabel "is mitigated by measure"@en ;
    schema:domainIncludes dpv:Risk ;
    schema:rangeIncludes dpv:RiskMitigationMeasure .

dpv:isRepresentativeFor a rdf:Property,
        owl:ObjectProperty ;
    dcam:domainIncludes dpv:Representative ;
    dcam:rangeIncludes dpv:Entity ;
    dct:contributor "Harshvardhan J. Pandit" ;
    dct:created "2022-11-09"^^xsd:date ;
    rdfs:subClassOf dpv:hasEntity ;
    rdfs:subPropertyOf dpv:hasEntity ;
    sw:term_status "accepted"@en ;
    skos:definition "Indicates the entity is a representative for specified entity"@en ;
    skos:prefLabel "is representative for"@en ;
    schema:domainIncludes dpv:Representative ;
    schema:rangeIncludes dpv:Entity .

dpv:hasConsequence a rdf:Property,
        owl:ObjectProperty ;
    dcam:rangeIncludes dpv:Consequence ;
    dct:contributor "Harshvardhan J. Pandit, Julian Flake, Georg P Krog, Fajar Ekaputra, Beatriz Esteves" ;
    dct:created "2020-11-04"^^xsd:date ;
    dct:modified "2021-09-21"^^xsd:date ;
    rdfs:superPropertyOf dpv:hasImpact ;
    sw:term_status "accepted"@en ;
    skos:definition "Indicates consenquence(s) possible or arising from specified concept"@en ;
    skos:prefLabel "has consequence"@en ;
    skos:scopeNote "Removed plural suffix for consistency"@en ;
    schema:rangeIncludes dpv:Consequence .

dpv:hasConsequenceOn a rdf:Property,
        owl:ObjectProperty ;
    dcam:domainIncludes dpv:Consequence ;
    dct:contributor "Harshvardhan J. Pandit, Georg P Krog" ;
    dct:created "2022-11-24"^^xsd:date ;
    rdfs:superPropertyOf dpv:hasImpactOn ;
    sw:term_status "accepted"@en ;
    skos:definition "Indicates the thing (e.g. plan, process, or entity) affected by a consequence"@en ;
    skos:prefLabel "has consequence on"@en ;
    schema:domainIncludes dpv:Consequence .

dpv:hasData a rdf:Property,
        owl:ObjectProperty ;
    dcam:rangeIncludes dpv:Data ;
    dct:contributor "Harshvardhan J. Pandit" ;
    dct:created "2022-08-18"^^xsd:date ;
    rdfs:superPropertyOf dpv:hasPersonalData ;
    sw:term_status "accepted"@en ;
    skos:definition "Indicates associated with Data (may or may not be personal)"@en ;
    skos:prefLabel "has data"@en ;
    schema:rangeIncludes dpv:Data .

dpv:hasLocation a rdf:Property,
        owl:ObjectProperty ;
    dcam:rangeIncludes dpv:Location ;
    dct:contributor "Axel Polleres, Rob Brennan, Harshvardhan J. Pandit, Mark Lizar" ;
    dct:created "2019-04-05"^^xsd:date ;
    dct:source "(SPECIAL Project,https://specialprivacy.ercim.eu/)"@en ;
    rdfs:superPropertyOf dpv:hasCountry ;
    sw:term_status "accepted"@en ;
    skos:definition "Indicates information about location"@en ;
    skos:prefLabel "has location"@en ;
    schema:rangeIncludes dpv:Location .

dpv:hasComplianceStatus a rdf:Property,
        owl:ObjectProperty ;
    dcam:rangeIncludes dpv:ComplianceStatus ;
    dct:contributor "Harshvardhan J. Pandit" ;
    dct:created "2022-05-18"^^xsd:date ;
    rdfs:subClassOf dpv:hasStatus ;
    rdfs:subPropertyOf dpv:hasStatus ;
    rdfs:superPropertyOf dpv:hasLawfulness ;
    sw:term_status "accepted"@en ;
    skos:definition "Indicates the status of compliance of specified concept"@en ;
    skos:prefLabel "has compliance status"@en ;
    schema:rangeIncludes dpv:ComplianceStatus .

dpv:hasCountry a rdf:Property,
        owl:ObjectProperty ;
    dcam:rangeIncludes dpv:Country ;
    dct:contributor "Harshvardhan J. Pandit, Georg P Krog" ;
    dct:created "2022-01-19"^^xsd:date ;
    rdfs:subClassOf dpv:hasLocation ;
    rdfs:subPropertyOf dpv:hasLocation ;
    rdfs:superPropertyOf dpv:hasThirdCountry ;
    sw:term_status "accepted"@en ;
    skos:definition "Indicates applicability of specified country"@en ;
    skos:prefLabel "has country"@en ;
    schema:rangeIncludes dpv:Country .

dpv:hasDataController a rdf:Property,
        owl:ObjectProperty ;
    dcam:rangeIncludes dpv:DataController ;
    dct:contributor "Axel Polleres, Javier Fernández, Harshvardhan J. Pandit, Mark Lizar, Bud Bruegger" ;
    dct:created "2019-04-04"^^xsd:date ;
    dct:modified "2020-11-04"^^xsd:date ;
    rdfs:subClassOf dpv:hasEntity ;
    rdfs:subPropertyOf dpv:hasEntity ;
    rdfs:superPropertyOf dpv:hasJointDataControllers ;
    sw:term_status "accepted"@en ;
    skos:definition "Indicates association with Data Controller"@en ;
    skos:prefLabel "has data controller"@en ;
    schema:rangeIncludes dpv:DataController .

dpv:hasRepresentative a rdf:Property,
        owl:ObjectProperty ;
    dcam:domainIncludes dpv:Entity ;
    dcam:rangeIncludes dpv:Representative ;
    dct:contributor "Harshvardhan J.Pandit, Georg P Krog, Paul Ryan, Beatriz Esteves" ;
    dct:created "2020-11-04"^^xsd:date ;
    rdfs:subClassOf dpv:hasEntity ;
    rdfs:subPropertyOf dpv:hasEntity ;
    rdfs:superPropertyOf dpv:hasDataProtectionOfficer ;
    sw:term_status "accepted"@en ;
    skos:definition "Specifies representative of the legal entity"@en ;
    skos:prefLabel "has representative"@en ;
    schema:domainIncludes dpv:Entity ;
    schema:rangeIncludes dpv:Representative .

dpv:hasOrganisationalMeasure a rdf:Property,
        owl:ObjectProperty ;
    dcam:rangeIncludes dpv:OrganisationalMeasure ;
    dct:contributor "Harshvardhan J. Pandit" ;
    dct:created "2022-02-09"^^xsd:date ;
    rdfs:subClassOf dpv:hasTechnicalOrganisationalMeasure ;
    rdfs:subPropertyOf dpv:hasTechnicalOrganisationalMeasure ;
    rdfs:superPropertyOf dpv:hasLegalMeasure,
        dpv:hasNotice ;
    sw:term_status "accepted"@en ;
    skos:definition "Indicates use or applicability of Organisational measure"@en ;
    skos:prefLabel "has organisational measure"@en ;
    schema:rangeIncludes dpv:OrganisationalMeasure .

dpv:hasRule a rdf:Property,
        owl:ObjectProperty ;
    dcam:domainIncludes dpv:Context ;
    dcam:rangeIncludes dpv:Rule ;
    dct:contributor "Harshvardhan J. Pandit, Georg P Krog, Beatriz Esteves, Paul Ryan" ;
    dct:created "2022-10-19"^^xsd:date ;
    rdfs:superPropertyOf dpv:hasObligation,
        dpv:hasPermission,
        dpv:hasProhibition ;
    sw:term_status "accepted"@en ;
    skos:definition "Specifying applicability or inclusion of a rule within specified context"@en ;
    skos:prefLabel "has rule"@en ;
    schema:domainIncludes dpv:Context ;
    schema:rangeIncludes dpv:Rule .

dpv:hasScale a rdf:Property,
        owl:ObjectProperty ;
    dcam:rangeIncludes dpv:Scale ;
    dct:contributor "Harshvardhan J. Pandit" ;
    dct:created "2022-06-15"^^xsd:date ;
    rdfs:superPropertyOf dpv:hasDataSubjectScale,
        dpv:hasDataVolume,
        dpv:hasGeographicCoverage ;
    sw:term_status "accepted"@en ;
    skos:definition "Indicates the scale of specified concept"@en ;
    skos:prefLabel "has scale"@en ;
    schema:rangeIncludes dpv:Scale .

dpv:hasStatus a rdf:Property,
        owl:ObjectProperty ;
    dcam:domainIncludes dpv:RightExerciseActivity ;
    dcam:rangeIncludes dpv:Status ;
    dct:contributor "Harshvardhan J. Pandit" ;
    dct:created "2022-05-18"^^xsd:date ;
    rdfs:superPropertyOf dpv:hasActivityStatus,
        dpv:hasAuditStatus,
        dpv:hasComplianceStatus ;
    sw:term_status "accepted"@en ;
    skos:definition "Indicates the status of specified concept"@en ;
    skos:prefLabel "has status"@en ;
    skos:scopeNote "Indicates the status of a Right Exercise Activity"@en ;
    schema:domainIncludes dpv:RightExerciseActivity ;
    schema:rangeIncludes dpv:Status .

dpv:hasRecipient a rdf:Property,
        owl:ObjectProperty ;
    dcam:domainIncludes dpv:RightExerciseActivity ;
    dcam:rangeIncludes dpv:Recipient ;
    dct:contributor "Axel Polleres, Javier Fernández, Harshvardhan J. Pandit, Mark Lizar, Bud Bruegger" ;
    dct:created "2019-04-04"^^xsd:date ;
    dct:modified "2020-11-04"^^xsd:date ;
    dct:source "(SPECIAL Project,https://specialprivacy.ercim.eu/)"@en ;
    rdfs:subClassOf dpv:hasEntity ;
    rdfs:subPropertyOf dpv:hasEntity ;
    rdfs:superPropertyOf dpv:hasDataImporter,
        dpv:hasDataProcessor,
        dpv:hasRecipientDataController,
        dpv:hasRecipientThirdParty ;
    sw:term_status "accepted"@en ;
    skos:definition "Indicates Recipient of Data"@en ;
    skos:prefLabel "has recipient"@en ;
    skos:scopeNote "Indicates the Recipient of a Right Exercise Activity"@en ;
    schema:domainIncludes dpv:RightExerciseActivity ;
    schema:rangeIncludes dpv:Recipient .

dpv:hasTechnicalOrganisationalMeasure a rdf:Property,
        owl:ObjectProperty ;
    dcam:rangeIncludes dpv:TechnicalOrganisationalMeasure ;
    dct:contributor "Axel Polleres, Javier Fernández, Harshvardhan J. Pandit, Mark Lizar, Bud Bruegger" ;
    dct:created "2019-04-04"^^xsd:date ;
    dct:modified "2020-11-04"^^xsd:date ;
    rdfs:superPropertyOf dpv:hasOrganisationalMeasure,
        dpv:hasPhysicalMeasure,
        dpv:hasPolicy,
        dpv:hasTechnicalMeasure,
        dpv:isMitigatedByMeasure ;
    sw:term_status "accepted"@en ;
    skos:definition "Indicates use or applicability of Technical or Organisational measure"@en ;
    skos:prefLabel "has technical and organisational measure"@en ;
    schema:rangeIncludes dpv:TechnicalOrganisationalMeasure .

dpv:hasEntity a rdf:Property,
        owl:ObjectProperty ;
    dcam:rangeIncludes dpv:Entity ;
    dct:contributor "Harshvardhan J. Pandit" ;
    dct:created "2022-02-09"^^xsd:date ;
    rdfs:superPropertyOf dpv:hasDataController,
        dpv:hasDataExporter,
        dpv:hasDataSubject,
        dpv:hasRecipient,
        dpv:hasRelationWithDataSubject,
        dpv:hasRepresentative,
        dpv:hasResponsibleEntity,
        dpv:isRepresentativeFor ;
    sw:term_status "accepted"@en ;
    skos:definition "Indicates inclusion or applicability of an entity to some concept"@en ;
    skos:prefLabel "has entity"@en ;
    skos:scopeNote "parent property for controller, processor, data subject, authority, etc.?"@en ;
    schema:rangeIncludes dpv:Entity .

rdfs:Class rdfs:superClassOf dpv:Law,
        dpv:Location,
        dpv:LocationFixture .

